@prefix co:          <https://data.omgeving.vlaanderen.be/id/concept/observatieprocedure/> .
@prefix compound:    <https://pubchem.ncbi.nlm.nih.gov/compound/> .
@prefix cosc:        <https://data.omgeving.vlaanderen.be/id/collection/chemische_stof/> .
@prefix csc:         <https://data.omgeving.vlaanderen.be/id/concept/chemische_stof/> .
@prefix cscl:        <https://data.omgeving.vlaanderen.be/id/classificationlevel/chemische_stof/> .
@prefix dbo:         <http://dbpedia.org/ontology/> .
@prefix dbp:         <http://dbpedia.org/property/> .
@prefix dc:          <http://purl.org/dc/elements/1.1/> .
@prefix dct:         <http://purl.org/dc/terms/> .
@prefix list:        <https://data.omgeving.vlaanderen.be/id/list/chemische_stof/> .
@prefix omg_dataset: <https://data.omgeving.vlaanderen.be/id/dataset/> .
@prefix rdf:         <http://www.w3.org/1999/02/22-rdf-syntax-ns#> .
@prefix rdfs:        <http://www.w3.org/2000/01/rdf-schema#> .
@prefix skos:        <http://www.w3.org/2004/02/skos/core#> .
@prefix tax_nodes:   <http://classyfire.wishartlab.com/tax_nodes/> .
@prefix vcs:         <https://data.vlaanderen.be/ns/chemische_stof#> .
@prefix vlcs:        <https://data.omgeving.vlaanderen.be/id/conceptscheme/> .
@prefix wise:        <http://dd.eionet.europa.eu/vocabulary/wise/ObservedProperty/> .
@prefix wk:          <https://data.omgeving.vlaanderen.be/ns/wk#> .
@prefix xkos:        <http://rdf-vocabulary.ddialliance.org/xkos#> .
@prefix xsd:         <http://www.w3.org/2001/XMLSchema#> .

csc:CHEMONTID_0000265
        rdf:type         skos:Concept;
        rdfs:seeAlso     tax_nodes:C0000265;
        skos:definition  "Compounds containing a carboxylic acid group with the formula -C(=O)OH or a derivative thereof."@en;
        skos:inScheme    vlcs:chemische_stof;
        skos:notation    "CHEMONTID:0000265";
        skos:prefLabel   "Carboxylic acids and derivatives"@en .

csc:CHEMONTID_0000476
        rdf:type         skos:Concept;
        rdfs:seeAlso     tax_nodes:C0000476;
        skos:definition  "Organic aromatic compounds containing a benzene and a carboxylic acid group (or a derivative thereof) forming 3-phenylprop-2-enoic acid."@en;
        skos:inScheme    vlcs:chemische_stof;
        skos:notation    "CHEMONTID:0000476";
        skos:prefLabel   "Cinnamic acids and derivatives"@en .

csc:CHEMONTID_0002955
        rdf:type         skos:Concept;
        rdfs:seeAlso     tax_nodes:C0002955;
        skos:definition  "Tetrahydrogenated isoquinoline derivatives."@en;
        skos:inScheme    vlcs:chemische_stof;
        skos:notation    "CHEMONTID:0002955";
        skos:prefLabel   "Tetrahydroisoquinolines"@en .

csc:CHEMONTID_0004776
        rdf:type         skos:Concept;
        rdfs:seeAlso     tax_nodes:C0004776;
        skos:definition  "Organic compounds having the nitroso group, -NO, attached to carbon, or to another element, most commonly nitrogen or oxygen."@en;
        skos:inScheme    vlcs:chemische_stof;
        skos:notation    "CHEMONTID:0004776";
        skos:prefLabel   "Organic nitroso compounds"@en .

csc:CHEMONTID_0000295
        rdf:type         skos:Concept;
        rdfs:seeAlso     tax_nodes:C0000295;
        skos:definition  "Organic compounds containing a benzene ring fused to either isomers of diazepine(unsaturated seven-member heterocycle with two nitrogen atoms replacing two carbon atoms)."@en;
        skos:inScheme    vlcs:chemische_stof;
        skos:notation    "CHEMONTID:0000295";
        skos:prefLabel   "Benzodiazepines"@en .

csc:CHEMONTID_0000012
        rdf:type         skos:Concept;
        rdfs:seeAlso     tax_nodes:C0000012;
        skos:definition  "Fatty acids and their derivatives, and substances related biosynthetically or functionally to these compounds."@en;
        skos:inScheme    vlcs:chemische_stof;
        skos:notation    "CHEMONTID:0000012";
        skos:prefLabel   "Lipids and lipid-like molecules"@en .

csc:CHEMONTID_0000138
        rdf:type         skos:Concept;
        rdfs:seeAlso     tax_nodes:C0000138;
        skos:definition  "Organic compounds containing a methoxybenzene or a derivative thereof."@en;
        skos:inScheme    vlcs:chemische_stof;
        skos:notation    "CHEMONTID:0000138";
        skos:prefLabel   "Anisoles"@en .

csc:CHEMONTID_0002044
        rdf:type         skos:Concept;
        rdfs:seeAlso     tax_nodes:C0002044;
        skos:definition  "Compounds containing a phenylnaphthalene skeleton, which consists of a naphthalene bound to a phenyl group."@en;
        skos:inScheme    vlcs:chemische_stof;
        skos:notation    "CHEMONTID:0002044";
        skos:prefLabel   "Phenylnaphthalenes"@en .

csc:CHEMONTID_0000434
        rdf:type         skos:Concept;
        rdfs:seeAlso     tax_nodes:C0000434;
        skos:definition  "Inorganic non-metallic compounds in which the largest atom belongs to the class of 'other nonmetals'."@en;
        skos:inScheme    vlcs:chemische_stof;
        skos:notation    "CHEMONTID:0000434";
        skos:prefLabel   "Homogeneous other non-metal compounds"@en .

csc:CHEMONTID_0000253
        rdf:type         skos:Concept;
        rdfs:seeAlso     tax_nodes:C0000253;
        skos:definition  "Organic compounds containing a 1,2-diphenylethylene moiety. Stilbenes (C6-C2-C6 ) are derived from the common phenylpropene (C6-C3) skeleton building block. The introduction of one or more hydroxyl groups  to a phenyl ring lead to stilbenoids."@en;
        skos:inScheme    vlcs:chemische_stof;
        skos:notation    "CHEMONTID:0000253";
        skos:prefLabel   "Stilbenes"@en .

csc:CHEMONTID_0002340
        rdf:type         skos:Concept;
        rdfs:seeAlso     tax_nodes:C0002340;
        skos:definition  "Steroid derivatives in which one carbon atom in the steroidal skeleton has been substituted with a nitrogen atom."@en;
        skos:inScheme    vlcs:chemische_stof;
        skos:notation    "CHEMONTID:0002340";
        skos:prefLabel   "Azasteroids and derivatives"@en .

csc:CHEMONTID_0002858
        rdf:type         skos:Concept;
        rdfs:seeAlso     tax_nodes:C0002858;
        skos:definition  "Oxazaphospholanes containing the isofamide skeleton. Isofamide is a heterocyclic compound made up of a 1,3,2-oxazaphospholane, where the phosphorus atom is part of a phosphodiamide group, and the oxazaphospholane is substituted by two haloalkyl chains."@en;
        skos:inScheme    vlcs:chemische_stof;
        skos:notation    "CHEMONTID:0002858";
        skos:prefLabel   "Isofamides"@en .

csc:CHEMONTID_0001857
        rdf:type         skos:Concept;
        rdfs:seeAlso     tax_nodes:C0001857;
        skos:definition  "Compounds containing a naphthyridine moiety, a naphthalene in which a carbon atom has been replaced by a nitrogen in each of the two rings. The naphthyridine skeleton can also be described as an assembly two fused pyridine rings, which do not share their nitrogen atom."@en;
        skos:inScheme    vlcs:chemische_stof;
        skos:notation    "CHEMONTID:0001857";
        skos:prefLabel   "Naphthyridines"@en .

csc:CHEMONTID_0001465
        rdf:type         skos:Concept;
        rdfs:seeAlso     tax_nodes:C0001465;
        skos:definition  "Organic compounds containing or derived from anatoxin, homoanatoxin or other analogues. Anatoxins constitute a class of potent neurotoxic alkaloids."@en;
        skos:inScheme    vlcs:chemische_stof;
        skos:notation    "CHEMONTID:0001465";
        skos:prefLabel   "Anatoxins"@en .

csc:CHEMONTID_0001073
        rdf:type         skos:Concept;
        rdfs:seeAlso     tax_nodes:C0001073;
        skos:definition  "Inorganic non-metallic compoundscontaining a phosphate as its largest oxoanion."@en;
        skos:inScheme    vlcs:chemische_stof;
        skos:notation    "CHEMONTID:0001073";
        skos:prefLabel   "Non-metal phosphates"@en .

csc:CHEMONTID_0000072
        rdf:type         skos:Concept;
        rdfs:seeAlso     tax_nodes:C0000072;
        skos:definition  "Compounds containing a dibenzodiazepine moiety, which consists of two benzene connected by diazepine ring."@en;
        skos:inScheme    vlcs:chemische_stof;
        skos:notation    "CHEMONTID:0000072";
        skos:prefLabel   "Dibenzodiazepines"@en .

csc:CHEMONTID_0001550
        rdf:type         skos:Concept;
        rdfs:seeAlso     tax_nodes:C0001550;
        skos:definition  "Terpenes with three consecutive isoprene units."@en;
        skos:inScheme    vlcs:chemische_stof;
        skos:notation    "CHEMONTID:0001550";
        skos:prefLabel   "Sesquiterpenoids"@en .

csc:CHEMONTID_0002466
        rdf:type         skos:Concept;
        rdfs:seeAlso     tax_nodes:C0002466;
        skos:definition  "Organic heterocyclic compounds containing an oxazaphosphinane ring, which consists of three carbon atoms, one nitrogen atom, and one phosphorus atom."@en;
        skos:inScheme    vlcs:chemische_stof;
        skos:notation    "CHEMONTID:0002466";
        skos:prefLabel   "Oxazaphosphinanes"@en .

csc:CHEMONTID_0002285
        rdf:type         skos:Concept;
        rdfs:seeAlso     tax_nodes:C0002285;
        skos:definition  "Compounds containing a carboximidic group, with the general formula R-C(=NR1)OR2."@en;
        skos:inScheme    vlcs:chemische_stof;
        skos:notation    "CHEMONTID:0002285";
        skos:prefLabel   "Carboximidic acids and derivatives"@en .

csc:CHEMONTID_0002551
        rdf:type         skos:Concept;
        rdfs:seeAlso     tax_nodes:C0002551;
        skos:definition  "Compounds with a structure containing a benzene ring conjugated to a propanoic acid."@en;
        skos:inScheme    vlcs:chemische_stof;
        skos:notation    "CHEMONTID:0002551";
        skos:prefLabel   "Phenylpropanoic acids"@en .

csc:CHEMONTID_0003467
        rdf:type         skos:Concept;
        rdfs:seeAlso     tax_nodes:C0003467;
        skos:definition  "Organic compounds with a structure based on a C6-C3-C6 skeleton, where the two benzene rings are not linked together."@en;
        skos:inScheme    vlcs:chemische_stof;
        skos:notation    "CHEMONTID:0003467";
        skos:prefLabel   "Linear 1,3-diarylpropanoids"@en .

csc:CHEMONTID_0002496
        rdf:type         skos:Concept;
        rdfs:seeAlso     tax_nodes:C0002496;
        skos:definition  "Heterocyclic compounds containing a 2,3-dihydro-1H-iso-indole moiety."@en;
        skos:inScheme    vlcs:chemische_stof;
        skos:notation    "CHEMONTID:0002496";
        skos:prefLabel   "Isoindolines"@en .

csc:CHEMONTID_0000307
        rdf:type         skos:Concept;
        rdfs:seeAlso     tax_nodes:C0000307;
        skos:definition  "Organic compounds containing a saturated seven member heterocycle, with one nitrogen atom."@en;
        skos:inScheme    vlcs:chemische_stof;
        skos:notation    "CHEMONTID:0000307";
        skos:prefLabel   "Azepanes"@en .

csc:CHEMONTID_0002581
        rdf:type         skos:Concept;
        rdfs:seeAlso     tax_nodes:C0002581;
        skos:definition  "Neoflavonoids with a structure based on a 3,4-dihydro-4-aryl-2H-1-benzopyran skeleton."@en;
        skos:inScheme    vlcs:chemische_stof;
        skos:notation    "CHEMONTID:0002581";
        skos:prefLabel   "Neoflavans"@en .

csc:CHEMONTID_0000000
        rdf:type           skos:Concept;
        rdfs:seeAlso       tax_nodes:C0000000;
        skos:definition    "Compounds that contain at least one carbon atom, excluding isocyanide/cyanide and their non-hydrocarbyl derivatives, thiophosgene, carbon diselenide, carbon monosulfide, carbon disulfide, carbon subsulfide, carbon monoxide, carbon dioxide, Carbon suboxide, and dicarbon monoxide."@en;
        skos:inScheme      vlcs:chemische_stof;
        skos:notation      "CHEMONTID:0000000";
        skos:prefLabel     "Organic compounds"@en;
        skos:topConceptOf  vlcs:chemische_stof .

csc:CHEMONTID_0000518
        rdf:type         skos:Concept;
        rdfs:seeAlso     tax_nodes:C0000518;
        skos:definition  "Compounds containing a triphenylene moiety, which consists of four fused benzene rings forming a 9,10-benzo[l]phenanthrene."@en;
        skos:inScheme    vlcs:chemische_stof;
        skos:notation    "CHEMONTID:0000518";
        skos:prefLabel   "Triphenylenes"@en .

csc:CHEMONTID_0004794
        rdf:type         skos:Concept;
        rdfs:seeAlso     tax_nodes:C0004794;
        skos:definition  "Aromatic heterocyclic compounds containing a naphthalene moiety substituted at one or more positions by a chlorine atom."@en;
        skos:inScheme    vlcs:chemische_stof;
        skos:notation    "CHEMONTID:0004794";
        skos:prefLabel   "Chloronaphthalenes"@en .

csc:CHEMONTID_0001212
        rdf:type         skos:Concept;
        rdfs:seeAlso     tax_nodes:C0001212;
        skos:definition  "Organic compounds containing the thiol functional group linked to an alkyl chain."@en;
        skos:inScheme    vlcs:chemische_stof;
        skos:notation    "CHEMONTID:0001212";
        skos:prefLabel   "Alkylthiols"@en .

csc:CHEMONTID_0000211
        rdf:type         skos:Concept;
        rdfs:seeAlso     tax_nodes:C0000211;
        skos:definition  "Organic compounds containing an indole, which is a bicyclic ring system made up of a six-membered benzene ring fused to a five-membered nitrogen-containing pyrrole ring."@en;
        skos:inScheme    vlcs:chemische_stof;
        skos:notation    "CHEMONTID:0000211";
        skos:prefLabel   "Indoles and derivatives"@en .

csc:CHEMONTID_0000422
        rdf:type         skos:Concept;
        rdfs:seeAlso     tax_nodes:C0000422;
        skos:definition  "Inorganic compounds that contain only metal atoms."@en;
        skos:inScheme    vlcs:chemische_stof;
        skos:notation    "CHEMONTID:0000422";
        skos:prefLabel   "Homogeneous metal compounds"@en .

csc:CHEMONTID_0001549
        rdf:type         skos:Concept;
        rdfs:seeAlso     tax_nodes:C0001549;
        skos:definition  "Compounds containing a chain of two isoprene units."@en;
        skos:inScheme    vlcs:chemische_stof;
        skos:notation    "CHEMONTID:0001549";
        skos:prefLabel   "Monoterpenoids"@en .

csc:CHEMONTID_0001157
        rdf:type         skos:Concept;
        rdfs:seeAlso     tax_nodes:C0001157;
        skos:definition  "Compounds containing the sulfonyl group, with the general structure RS(=O)2R' ( R,R' must not be H)."@en;
        skos:inScheme    vlcs:chemische_stof;
        skos:notation    "CHEMONTID:0001157";
        skos:prefLabel   "Sulfonyls"@en .

csc:CHEMONTID_0000548
        rdf:type         skos:Concept;
        rdfs:seeAlso     tax_nodes:C0000548;
        skos:definition  "Inorganic compounds in which the heaviest atom bonded to a hydrogen atom is a halogen."@en;
        skos:inScheme    vlcs:chemische_stof;
        skos:notation    "CHEMONTID:0000548";
        skos:prefLabel   "Halogen hydrides"@en .

csc:CHEMONTID_0002901
        rdf:type         skos:Concept;
        rdfs:seeAlso     tax_nodes:C0002901;
        skos:definition  "Flavonoids with a structure based on the 3-phenylchromene skeleton, with a double bond between the C2 and C3 carbon atoms of the chromene moiety."@en;
        skos:inScheme    vlcs:chemische_stof;
        skos:notation    "CHEMONTID:0002901";
        skos:prefLabel   "Isoflav-2-enes"@en .

csc:CHEMONTID_0001368
        rdf:type         skos:Concept;
        rdfs:seeAlso     tax_nodes:C0001368;
        skos:definition  "Organic compounds containing a functional group with the general structure OC(=S)NR2 or SC(=O)NR2."@en;
        skos:inScheme    vlcs:chemische_stof;
        skos:notation    "CHEMONTID:0001368";
        skos:prefLabel   "Thiocarbamic acid derivatives"@en .

csc:CHEMONTID_0003455
        rdf:type         skos:Concept;
        rdfs:seeAlso     tax_nodes:C0003455;
        skos:definition  "Organic compounds containing a sulfate group that carries one or two O-ester groups."@en;
        skos:inScheme    vlcs:chemische_stof;
        skos:notation    "CHEMONTID:0003455";
        skos:prefLabel   "Sulfuric acid esters"@en .

csc:CHEMONTID_0004456
        rdf:type         skos:Concept;
        rdfs:seeAlso     tax_nodes:C0004456;
        skos:definition  "Organic compounds containing the selenite oxoanion, with the formula  [SO3]2-, or its conjugated base."@en;
        skos:inScheme    vlcs:chemische_stof;
        skos:notation    "CHEMONTID:0004456";
        skos:prefLabel   "Organic sulfites"@en .

csc:CHEMONTID_0001187
        rdf:type         skos:Concept;
        rdfs:seeAlso     tax_nodes:C0001187;
        skos:definition  "Organic compounds containing either the monothiacetal functional group (R2C(OR')(SR')) or the dithioacetal (R2C(SR')2) functional group ."@en;
        skos:inScheme    vlcs:chemische_stof;
        skos:notation    "CHEMONTID:0001187";
        skos:prefLabel   "Thioacetals"@en .

csc:CHEMONTID_0000186
        rdf:type         skos:Concept;
        rdfs:seeAlso     tax_nodes:C0000186;
        skos:definition  "Compounds containing a phenethylamine moiety, which consists of a phenyl group substituted at the second position by an ethan-1-amine."@en;
        skos:inScheme    vlcs:chemische_stof;
        skos:notation    "CHEMONTID:0000186";
        skos:prefLabel   "Phenethylamines"@en .

csc:CHEMONTID_0004752
        rdf:type         skos:Concept;
        rdfs:seeAlso     tax_nodes:C0004752;
        skos:definition  "Oxime ether derivatives with the general formula CC(R)=NOC(=O)N(R')R\\\", where R-R\\\" = H or organyl."@en;
        skos:inScheme    vlcs:chemische_stof;
        skos:notation    "CHEMONTID:0004752";
        skos:prefLabel   "Oxime carbamates"@en .

csc:CHEMONTID_0001272
        rdf:type         skos:Concept;
        rdfs:seeAlso     tax_nodes:C0001272;
        skos:definition  "Aromatic compounds containing a methoxyphenol moiety."@en;
        skos:inScheme    vlcs:chemische_stof;
        skos:notation    "CHEMONTID:0001272";
        skos:prefLabel   "Cresols"@en .

csc:CHEMONTID_0002484
        rdf:type         skos:Concept;
        rdfs:seeAlso     tax_nodes:C0002484;
        skos:definition  "Organic acids with the general formula RC(=N)-OH (R=H, organic group)."@en;
        skos:inScheme    vlcs:chemische_stof;
        skos:notation    "CHEMONTID:0002484";
        skos:prefLabel   "Carboximidic acids"@en .

csc:CHEMONTID_0001091
        rdf:type         skos:Concept;
        rdfs:seeAlso     tax_nodes:C0001091;
        skos:definition  "Compounds containing a benzene ring which bears a methane group."@en;
        skos:inScheme    vlcs:chemische_stof;
        skos:notation    "CHEMONTID:0001091";
        skos:prefLabel   "Toluenes"@en .

csc:CHEMONTID_0000090
        rdf:type         skos:Concept;
        rdfs:seeAlso     tax_nodes:C0000090;
        skos:definition  "Compounds containing a pyrrole ring, which is a five-member aromatic heterocycle with one nitrogen atom and four carbon atoms."@en;
        skos:inScheme    vlcs:chemische_stof;
        skos:notation    "CHEMONTID:0000090";
        skos:prefLabel   "Pyrroles"@en .

csc:CHEMONTID_0000029
        rdf:type         skos:Concept;
        rdfs:seeAlso     tax_nodes:C0000029;
        skos:definition  "Organic aromatic compounds containing a cinnamlaldehyde moiety, consisting of a benzene and an aldehyde group to form 3-phenylprop-2-enal."@en;
        skos:inScheme    vlcs:chemische_stof;
        skos:notation    "CHEMONTID:0000029";
        skos:prefLabel   "Cinnamaldehydes"@en .

csc:CHEMONTID_0004203
        rdf:type         skos:Concept;
        rdfs:seeAlso     tax_nodes:C0004203;
        skos:definition  "Aromatic compounds containing a methyl-3-methoxyacrylate moiety that carries a benzyl group at the C-alpha carbon."@en;
        skos:inScheme    vlcs:chemische_stof;
        skos:notation    "CHEMONTID:0004203";
        skos:prefLabel   "Phenyl-beta-methoxyacrylates"@en .

csc:CHEMONTID_0003413
        rdf:type         skos:Concept;
        rdfs:seeAlso     tax_nodes:C0003413;
        skos:definition  "Organic aromatic compounds that 1-benzothiopyran, a bicyclic compound made up of a benzene ring fused to a thiopyran, so that the sulfur atom is at the 1-position."@en;
        skos:inScheme    vlcs:chemische_stof;
        skos:notation    "CHEMONTID:0003413";
        skos:prefLabel   "1-benzothiopyrans"@en .

csc:CHEMONTID_0000410
        rdf:type         skos:Concept;
        rdfs:seeAlso     tax_nodes:C0000410;
        skos:definition  "Derivatives of diazene(diimide), HN=NH, wherein both hydrogens are substituted by hydrocarbyl groups, e.g. PhN=NPh azobenzene or diphenyldiazene."@en;
        skos:inScheme    vlcs:chemische_stof;
        skos:notation    "CHEMONTID:0000410";
        skos:prefLabel   "Azo compounds"@en .

csc:CHEMONTID_0004233
        rdf:type         skos:Concept;
        rdfs:seeAlso     tax_nodes:C0004233;
        skos:definition  "Aromatic compounds containing a benzenesulfonyl group, which consists of a monocyclic benzene moiety that carries a sulfonyl group."@en;
        skos:inScheme    vlcs:chemische_stof;
        skos:notation    "CHEMONTID:0004233";
        skos:prefLabel   "Benzenesulfonyl compounds"@en .

csc:CHEMONTID_0002749
        rdf:type         skos:Concept;
        rdfs:seeAlso     tax_nodes:C0002749;
        skos:definition  "Alkaloids having a core structure based on the strychnan, stemmadenine (seco-curan), or the akuammicine (curan) skeleton."@en;
        skos:inScheme    vlcs:chemische_stof;
        skos:notation    "CHEMONTID:0002749";
        skos:prefLabel   "Strychnos alkaloids"@en .

csc:CHEMONTID_0000355
        rdf:type         skos:Concept;
        rdfs:seeAlso     tax_nodes:C0000355;
        skos:definition  "Aromatic compounds containing a prop-2-ylbenzene moiety."@en;
        skos:inScheme    vlcs:chemische_stof;
        skos:notation    "CHEMONTID:0000355";
        skos:prefLabel   "Cumenes"@en .

csc:CHEMONTID_0002442
        rdf:type         skos:Concept;
        rdfs:seeAlso     tax_nodes:C0002442;
        skos:definition  "Piperidines with a nitroso functional group attached to the piperidine ring."@en;
        skos:inScheme    vlcs:chemische_stof;
        skos:notation    "CHEMONTID:0002442";
        skos:prefLabel   "Nitrosopiperidines"@en .

csc:CHEMONTID_0003569
        rdf:type         skos:Concept;
        rdfs:seeAlso     tax_nodes:C0003569;
        skos:definition  "Steroids with a structure based on the 21-carbon pregnane skeleton."@en;
        skos:inScheme    vlcs:chemische_stof;
        skos:notation    "CHEMONTID:0003569";
        skos:prefLabel   "Pregnane steroids"@en .

csc:CHEMONTID_0000089
        rdf:type         skos:Concept;
        rdfs:seeAlso     tax_nodes:C0000089;
        skos:definition  "Compounds containing a pyridine ring, which is a six-member aromatic heterocycle which consists of one nitrogen atom and five carbon atoms."@en;
        skos:inScheme    vlcs:chemische_stof;
        skos:notation    "CHEMONTID:0000089";
        skos:prefLabel   "Pyridines and derivatives"@en .

csc:CHEMONTID_0003865
        rdf:type         skos:Concept;
        rdfs:seeAlso     tax_nodes:C0003865;
        skos:definition  "Organic compounds consisting of an assembly of cations and anions."@en;
        skos:inScheme    vlcs:chemische_stof;
        skos:notation    "CHEMONTID:0003865";
        skos:prefLabel   "Organic salts"@en .

csc:CHEMONTID_0002864
        rdf:type         skos:Concept;
        rdfs:seeAlso     tax_nodes:C0002864;
        skos:definition  "Vinyl halides in which a bromine atom is bonded to an sp2-hybridised carbon atom."@en;
        skos:inScheme    vlcs:chemische_stof;
        skos:notation    "CHEMONTID:0002864";
        skos:prefLabel   "Vinyl bromides"@en .

csc:CHEMONTID_0004474
        rdf:type         skos:Concept;
        rdfs:seeAlso     tax_nodes:C0004474;
        skos:definition  "Hydrocarbons that contains only saturated carbon atoms, which are linked to one another through single bonds. These includes alkanes and cycloalkanes."@en;
        skos:inScheme    vlcs:chemische_stof;
        skos:notation    "CHEMONTID:0004474";
        skos:prefLabel   "Saturated hydrocarbons"@en .

csc:CHEMONTID_0001290
        rdf:type         skos:Concept;
        rdfs:seeAlso     tax_nodes:C0001290;
        skos:definition  "Compounds containing a carboxylic acid chain (of at least 2 carbon atoms) linked to an indole ring."@en;
        skos:inScheme    vlcs:chemische_stof;
        skos:notation    "CHEMONTID:0001290";
        skos:prefLabel   "Indolyl carboxylic acids and derivatives"@en .

csc:CHEMONTID_0001314
        rdf:type         skos:Concept;
        rdfs:seeAlso     tax_nodes:C0001314;
        skos:definition  "Organic compounds containing 1,3-dioxane, an aliphatic six-member ring with two oxygen atoms in ring positions 1 and 3."@en;
        skos:inScheme    vlcs:chemische_stof;
        skos:notation    "CHEMONTID:0001314";
        skos:prefLabel   "1,3-dioxanes"@en .

csc:CHEMONTID_0002049
        rdf:type         skos:Concept;
        rdfs:seeAlso     tax_nodes:C0002049;
        skos:definition  "Prenol lipids containing a carbohydrate moiety glycosidically bound to a terpene backbone."@en;
        skos:inScheme    vlcs:chemische_stof;
        skos:notation    "CHEMONTID:0002049";
        skos:prefLabel   "Terpene glycosides"@en .

csc:CHEMONTID_0000047
        rdf:type         skos:Concept;
        rdfs:seeAlso     tax_nodes:C0000047;
        skos:definition  "Tetralin lignans in which the benzene moiety of the tetralin skeleton is fused to a 1,3-dioxolane and the cyclohexane is fused to a butyrolactone (pyrrolidin-2-one)."@en;
        skos:inScheme    vlcs:chemische_stof;
        skos:notation    "CHEMONTID:0000047";
        skos:prefLabel   "Podophyllotoxins"@en .

csc:CHEMONTID_0000132
        rdf:type         skos:Concept;
        rdfs:seeAlso     tax_nodes:C0000132;
        skos:definition  "Compounds containing the enol functional group, with the structure HO(R)C=CR'. Ketones that have one or more alpha-hydrogen atoms undergo keto-enol tautomerization, the tautomer being an enol."@en;
        skos:inScheme    vlcs:chemische_stof;
        skos:notation    "CHEMONTID:0000132";
        skos:prefLabel   "Enols"@en .

csc:CHEMONTID_0000258
        rdf:type         skos:Concept;
        rdfs:seeAlso     tax_nodes:C0000258;
        skos:definition  "Compounds based on the cyclopenta[a]phenanthrene carbon skeleton, partially or completely hydrogenated; there are usually methyl groups at C-10 and C-13, and often an alkyl group at C-17. By extension, one or more bond scissions, ring expansions and/or ring contractions of the skeleton may have occurred."@en;
        skos:inScheme    vlcs:chemische_stof;
        skos:notation    "CHEMONTID:0000258";
        skos:prefLabel   "Steroids and steroid derivatives"@en .

csc:CHEMONTID_0000554
        rdf:type         skos:Concept;
        rdfs:seeAlso     tax_nodes:C0000554;
        skos:definition  "Inorganic compounds containing an oxygen atom of an oxidation state of -2, in which the heaviest atom bonded to the oxygen belongs to the class of 'other non-metals'."@en;
        skos:inScheme    vlcs:chemische_stof;
        skos:notation    "CHEMONTID:0000554";
        skos:prefLabel   "Other non-metal oxides"@en .

csc:CHEMONTID_0000162
        rdf:type         skos:Concept;
        rdfs:seeAlso     tax_nodes:C0000162;
        skos:definition  "Organic compounds containing a four-member lactam (a cyclic amide)."@en;
        skos:inScheme    vlcs:chemische_stof;
        skos:notation    "CHEMONTID:0000162";
        skos:prefLabel   "Beta lactams"@en .

csc:CHEMONTID_0001851
        rdf:type         skos:Concept;
        rdfs:seeAlso     tax_nodes:C0001851;
        skos:definition  "Compounds containing a pyrene moiety, which consists four fused benzene rings, resulting in a flat aromatic system."@en;
        skos:inScheme    vlcs:chemische_stof;
        skos:notation    "CHEMONTID:0001851";
        skos:prefLabel   "Pyrenes"@en .

csc:CHEMONTID_0000584
        rdf:type         skos:Concept;
        rdfs:seeAlso     tax_nodes:C0000584;
        skos:definition  "Inorganic compounds in which the largest halogen atom is fluorine, and the heaviest metal atom is a metalloid."@en;
        skos:inScheme    vlcs:chemische_stof;
        skos:notation    "CHEMONTID:0000584";
        skos:prefLabel   "Metalloid fluorides"@en .

csc:CHEMONTID_0002490
        rdf:type         skos:Concept;
        rdfs:seeAlso     tax_nodes:C0002490;
        skos:definition  "Azole derivatives obtained by conversion of one double bond of the azole ring to a single bond."@en;
        skos:inScheme    vlcs:chemische_stof;
        skos:notation    "CHEMONTID:0002490";
        skos:prefLabel   "Azolines"@en .

csc:CHEMONTID_0001302
        rdf:type         skos:Concept;
        rdfs:seeAlso     tax_nodes:C0001302;
        skos:definition  "Organic compounds containing phosphonic acid."@en;
        skos:inScheme    vlcs:chemische_stof;
        skos:notation    "CHEMONTID:0001302";
        skos:prefLabel   "Organic phosphonic acids"@en .

csc:CHEMONTID_0000301
        rdf:type         skos:Concept;
        rdfs:seeAlso     tax_nodes:C0000301;
        skos:definition  "Organic compounds containing a benzene ring fused to a furan. Furan is a five-membered aromatic ring with four carbon atoms and one oxygen atom."@en;
        skos:inScheme    vlcs:chemische_stof;
        skos:notation    "CHEMONTID:0000301";
        skos:prefLabel   "Benzofurans"@en .

csc:CHEMONTID_0000427
        rdf:type         skos:Concept;
        rdfs:seeAlso     tax_nodes:C0000427;
        skos:definition  "Inorganic compounds containing only metal atoms,with the largest atom being a post-transition metal atom."@en;
        skos:inScheme    vlcs:chemische_stof;
        skos:notation    "CHEMONTID:0000427";
        skos:prefLabel   "Homogeneous post-transition metal compounds"@en .

csc:CHEMONTID_0000035
        rdf:type         skos:Concept;
        rdfs:seeAlso     tax_nodes:C0000035;
        skos:definition  "Aromatic compounds containing a halogen atom linked to a benzene ring."@en;
        skos:inScheme    vlcs:chemische_stof;
        skos:notation    "CHEMONTID:0000035";
        skos:prefLabel   "Halobenzenes"@en .

csc:CHEMONTID_0000120
        rdf:type         skos:Concept;
        rdfs:seeAlso     tax_nodes:C0000120;
        skos:definition  "Organic compounds containing a ketone attached to two phenyl groups."@en;
        skos:inScheme    vlcs:chemische_stof;
        skos:notation    "CHEMONTID:0000120";
        skos:prefLabel   "Benzophenones"@en .

csc:CHEMONTID_0004812
        rdf:type         skos:Concept;
        rdfs:seeAlso     tax_nodes:C0004812;
        skos:definition  "Aromatic polycyclic compounds containing an acenaphthylene moiety. Acenaphthylene is a carbotricyclic compound, consisting of a naphthalene with positions C1 and C8 connected by an ethylene bridge."@en;
        skos:inScheme    vlcs:chemische_stof;
        skos:notation    "CHEMONTID:0004812";
        skos:prefLabel   "Acenaphthylenes"@en .

csc:CHEMONTID_0000331
        rdf:type         skos:Concept;
        rdfs:seeAlso     tax_nodes:C0000331;
        skos:definition  "Carboxylic acid amide derivatives of fatty acids, that are formed from a fatty acid and an amine."@en;
        skos:inScheme    vlcs:chemische_stof;
        skos:notation    "CHEMONTID:0000331";
        skos:prefLabel   "Fatty amides"@en .

csc:CHEMONTID_0000457
        rdf:type         skos:Concept;
        rdfs:seeAlso     tax_nodes:C0000457;
        skos:definition  "Inorganic compounds belonging either to the alkaline earth metal hydrides, the alkaline earth metal nitrides, the alkaline earth metal oxides, or the alkaline earth metal sulfides."@en;
        skos:inScheme    vlcs:chemische_stof;
        skos:notation    "CHEMONTID:0000457";
        skos:prefLabel   "Alkaline earth metal organides"@en .

csc:CHEMONTID_0001935
        rdf:type         skos:Concept;
        rdfs:seeAlso     tax_nodes:C0001935;
        skos:definition  "Compounds containing a N-phenylurea moiety, which is structurally characterized by a phenyl group linked to one nitrogen atom of a urea group."@en;
        skos:inScheme    vlcs:chemische_stof;
        skos:notation    "CHEMONTID:0001935";
        skos:prefLabel   "N-phenylureas"@en .

csc:CHEMONTID_0004631
        rdf:type         skos:Concept;
        rdfs:seeAlso     tax_nodes:C0004631;
        skos:definition  "Organosulfur compounds containing a thioether group that is substituted by an aryl group."@en;
        skos:inScheme    vlcs:chemische_stof;
        skos:notation    "CHEMONTID:0004631";
        skos:prefLabel   "Aryl thioethers"@en .

csc:CHEMONTID_0001151
        rdf:type         skos:Concept;
        rdfs:seeAlso     tax_nodes:C0001151;
        skos:definition  "Compounds containing an indane ring bearing a ketone group."@en;
        skos:inScheme    vlcs:chemische_stof;
        skos:notation    "CHEMONTID:0001151";
        skos:prefLabel   "Indanones"@en .

csc:CHEMONTID_0000542
        rdf:type         skos:Concept;
        rdfs:seeAlso     tax_nodes:C0000542;
        skos:definition  "Inorganic compounds containing an oxygen atom of an oxidation state of -2, in which the heaviest atom bonded to the oxygen is a lanthanide."@en;
        skos:inScheme    vlcs:chemische_stof;
        skos:notation    "CHEMONTID:0000542";
        skos:prefLabel   "Lanthanide oxides"@en .

csc:CHEMONTID_0003630
        rdf:type         skos:Concept;
        rdfs:seeAlso     tax_nodes:C0003630;
        skos:definition  "Electrically neutral organic molecules carrying a positive and a negative charge in one of their major canonical descriptions. In most dipolar compounds the charges are delocalized; however the term is also applied to species where this is not the case. The term 1,3-dipolar compounds is used for those in which a significant canonical resonance form can be represented by a separation of charge over three atoms (in connection with 1,3-dipolar cycloadditions)."@en;
        skos:inScheme    vlcs:chemische_stof;
        skos:notation    "CHEMONTID:0003630";
        skos:prefLabel   "Organic 1,3-dipolar compounds"@en .

csc:CHEMONTID_0002363
        rdf:type         skos:Concept;
        rdfs:seeAlso     tax_nodes:C0002363;
        skos:definition  "Amide derivatives of phenylacetic acids."@en;
        skos:inScheme    vlcs:chemische_stof;
        skos:notation    "CHEMONTID:0002363";
        skos:prefLabel   "Phenylacetamides"@en .

csc:CHEMONTID_0004450
        rdf:type         skos:Concept;
        rdfs:seeAlso     tax_nodes:C0004450;
        skos:definition  "Organic compounds containing acrylic acid CH2=CHCO2H or a derivative thereof."@en;
        skos:inScheme    vlcs:chemische_stof;
        skos:notation    "CHEMONTID:0004450";
        skos:prefLabel   "Acrylic acids and derivatives"@en .

csc:CHEMONTID_0002966
        rdf:type         skos:Concept;
        rdfs:seeAlso     tax_nodes:C0002966;
        skos:definition  "Carboxylic acids containing exactly four carboxyl groups."@en;
        skos:inScheme    vlcs:chemische_stof;
        skos:notation    "CHEMONTID:0002966";
        skos:prefLabel   "Tetracarboxylic acids and derivatives"@en .

csc:CHEMONTID_0000095
        rdf:type         skos:Concept;
        rdfs:seeAlso     tax_nodes:C0000095;
        skos:definition  "Heterocyclic compounds containing a five-member aromatic ring made up of one sulfur atom, one nitrogen, and three carbon atoms."@en;
        skos:inScheme    vlcs:chemische_stof;
        skos:notation    "CHEMONTID:0000095";
        skos:prefLabel   "Thiazoles"@en .

csc:CHEMONTID_0004208
        rdf:type         skos:Concept;
        rdfs:seeAlso     tax_nodes:C0004208;
        skos:definition  "Aromatic compounds that contain a xylene moiety, which is a monocyclic benzene carrying exactly two methyl groups."@en;
        skos:inScheme    vlcs:chemische_stof;
        skos:notation    "CHEMONTID:0004208";
        skos:prefLabel   "Xylenes"@en .

csc:CHEMONTID_0001205
        rdf:type         skos:Concept;
        rdfs:seeAlso     tax_nodes:C0001205;
        skos:definition  "Compounds containing a carboxylic acid group with the formula -C(=O)OH."@en;
        skos:inScheme    vlcs:chemische_stof;
        skos:notation    "CHEMONTID:0001205";
        skos:prefLabel   "Carboxylic acids"@en .

csc:CHEMONTID_0001392
        rdf:type         skos:Concept;
        rdfs:seeAlso     tax_nodes:C0001392;
        skos:definition  "Plant products of low molecular weight formed primarily from oxidative coupling of two p-propylphenol moieties. They can also be described as micromolecules with two phenylpropanoid units coupled together. They can be attached in various manners, like C5-C5', C8-C8'. Most known natural lignans are oxidized at C9 and C9´ and, based upon the way in which oxygen is incorporated into the skeleton and on the cyclization patterns, a wide range of lignans of very different structural types can be formed."@en;
        skos:inScheme    vlcs:chemische_stof;
        skos:notation    "CHEMONTID:0001392";
        skos:prefLabel   "Lignans, neolignans and related compounds"@en .

csc:CHEMONTID_0004504
        rdf:type         skos:Concept;
        rdfs:seeAlso     tax_nodes:C0004504;
        skos:definition  "Organic nitrogen compounds that contain the cyano (C#N) group. The group can be present either in the anionic or covalently bond form."@en;
        skos:inScheme    vlcs:chemische_stof;
        skos:notation    "CHEMONTID:0004504";
        skos:prefLabel   "Organic cyanides"@en .

csc:CHEMONTID_0004112
        rdf:type         skos:Concept;
        rdfs:seeAlso     tax_nodes:C0004112;
        skos:definition  "Organic compounds containing two benzoyl groups O-linked to each other via a peroxide group. Their skeleton has the general formula [C6H5C(O)]2O2."@en;
        skos:inScheme    vlcs:chemische_stof;
        skos:notation    "CHEMONTID:0004112";
        skos:prefLabel   "Benzoyl peroxides"@en .

csc:CHEMONTID_0000023
        rdf:type         skos:Concept;
        rdfs:seeAlso     tax_nodes:C0000023;
        skos:definition  "Compounds containing a naphthalene moiety, which consists of two fused benzene rings."@en;
        skos:inScheme    vlcs:chemische_stof;
        skos:notation    "CHEMONTID:0000023";
        skos:prefLabel   "Naphthalenes"@en .

csc:CHEMONTID_0000445
        rdf:type         skos:Concept;
        rdfs:seeAlso     tax_nodes:C0000445;
        skos:definition  "Inorganic oxoanionic compounds in which the heaviest atom not in an oxoanion is an alkali metal."@en;
        skos:inScheme    vlcs:chemische_stof;
        skos:notation    "CHEMONTID:0000445";
        skos:prefLabel   "Alkali metal oxoanionic compounds"@en .

csc:CHEMONTID_0000053
        rdf:type         skos:Concept;
        rdfs:seeAlso     tax_nodes:C0000053;
        skos:definition  "Organic compounds containing an amino group attached to a quinoline ring system."@en;
        skos:inScheme    vlcs:chemische_stof;
        skos:notation    "CHEMONTID:0000053";
        skos:prefLabel   "Aminoquinolines and derivatives"@en .

csc:CHEMONTID_0000530
        rdf:type         skos:Concept;
        rdfs:seeAlso     tax_nodes:C0000530;
        skos:definition  "Inorganic compounds containing an oxygen atom of an oxidation state of -2, in which the heaviest atom bonded to the oxygen is a post-transition metal."@en;
        skos:inScheme    vlcs:chemische_stof;
        skos:notation    "CHEMONTID:0000530";
        skos:prefLabel   "Post-transition metal oxides"@en .

csc:CHEMONTID_0000264
        rdf:type         skos:Concept;
        rdfs:seeAlso     tax_nodes:C0000264;
        skos:definition  "Compounds an organic acid or a derivative thereof."@en;
        skos:inScheme    vlcs:chemische_stof;
        skos:notation    "CHEMONTID:0000264";
        skos:prefLabel   "Organic acids and derivatives"@en .

list:subclass  rdf:type  rdf:List;
        rdf:first       cscl:subclass;
        rdf:rest        ();
        skos:prefLabel  "Niveau subklasse"@nl .

csc:CHEMONTID_0001295
        rdf:type         skos:Concept;
        rdfs:seeAlso     tax_nodes:C0001295;
        skos:definition  "Compounds containing an steroid backbone, with at least one hydrogen substituted by a hydroxyl group."@en;
        skos:inScheme    vlcs:chemische_stof;
        skos:notation    "CHEMONTID:0001295";
        skos:prefLabel   "Hydroxysteroids"@en .

csc:CHEMONTID_0000107
        rdf:type         skos:Concept;
        rdfs:seeAlso     tax_nodes:C0000107;
        skos:definition  "Compounds containing an oxazinane moiety, which consists of a saturated aliphatic six-member ring with one oxygen atom, a nitrogen atom, and four carbon atoms. Isomers  of oxaphospholane include 1,2-oxazinane, 1,3-oxazinane, and 1,4-oxazinane."@en;
        skos:inScheme    vlcs:chemische_stof;
        skos:notation    "CHEMONTID:0000107";
        skos:prefLabel   "Oxazinanes"@en .

csc:CHEMONTID_0000294
        rdf:type         skos:Concept;
        rdfs:seeAlso     tax_nodes:C0000294;
        skos:definition  "Organic compounds containing a benzene ring fused to an imidazole ring (five member ring containing a nitrogen atom, 4 carbon atoms, and two double bonds)."@en;
        skos:inScheme    vlcs:chemische_stof;
        skos:notation    "CHEMONTID:0000294";
        skos:prefLabel   "Benzimidazoles"@en .

csc:CHEMONTID_0001983
        rdf:type         skos:Concept;
        rdfs:seeAlso     tax_nodes:C0001983;
        skos:definition  "Compounds containing a dihydrofuran moiety, which is a furan derivative with only one double bond."@en;
        skos:inScheme    vlcs:chemische_stof;
        skos:notation    "CHEMONTID:0001983";
        skos:prefLabel   "Dihydrofurans"@en .

csc:CHEMONTID_0000403
        rdf:type         skos:Concept;
        rdfs:seeAlso     tax_nodes:C0000403;
        skos:definition  "Organic compounds containing the sulfuric acid or a derivative thereof."@en;
        skos:inScheme    vlcs:chemische_stof;
        skos:notation    "CHEMONTID:0000403";
        skos:prefLabel   "Organic sulfuric acids and derivatives"@en .

csc:CHEMONTID_0000011
        rdf:type         skos:Concept;
        rdfs:seeAlso     tax_nodes:C0000011;
        skos:definition  "Monosaccharides, disaccharides, oligosaccharides, polysaccharides, and their derivatives."@en;
        skos:inScheme    vlcs:chemische_stof;
        skos:notation    "CHEMONTID:0000011";
        skos:prefLabel   "Carbohydrates and carbohydrate conjugates"@en .

csc:CHEMONTID_0000433
        rdf:type         skos:Concept;
        rdfs:seeAlso     tax_nodes:C0000433;
        skos:definition  "Inorganic non-metallic compounds in which the largest atom is a halogen atom."@en;
        skos:inScheme    vlcs:chemische_stof;
        skos:notation    "CHEMONTID:0000433";
        skos:prefLabel   "Homogeneous noble gases"@en .

csc:CHEMONTID_0000041
        rdf:type         skos:Concept;
        rdfs:seeAlso     tax_nodes:C0000041;
        skos:definition  "Organic compounds containing to benzene rings linked together by a C-C bond."@en;
        skos:inScheme    vlcs:chemische_stof;
        skos:notation    "CHEMONTID:0000041";
        skos:prefLabel   "Biphenyls and derivatives"@en .

csc:CHEMONTID_0001168
        rdf:type         skos:Concept;
        rdfs:seeAlso     tax_nodes:C0001168;
        skos:definition  "Organic compounds comprising the ketene acetal functional group, with the general structure XC(Y)=C(R3)R4 (R1,R2=H, alkyl, aryl; X,Y=any hetero atom)."@en;
        skos:inScheme    vlcs:chemische_stof;
        skos:notation    "CHEMONTID:0001168";
        skos:prefLabel   "Ketene acetals"@en .

csc:CHEMONTID_0001253
        rdf:type         skos:Concept;
        rdfs:seeAlso     tax_nodes:C0001253;
        skos:definition  "Compounds containing a quinoline moiety, which consists of a benzene ring fused to a pyrimidine ring to form benzo[b]azabenzene."@en;
        skos:inScheme    vlcs:chemische_stof;
        skos:notation    "CHEMONTID:0001253";
        skos:prefLabel   "Quinolines and derivatives"@en .

csc:CHEMONTID_0001379
        rdf:type         skos:Concept;
        rdfs:seeAlso     tax_nodes:C0001379;
        skos:definition  "Organic compounds containing a benzene ring fused to a 1,4-dioxin ring."@en;
        skos:inScheme    vlcs:chemische_stof;
        skos:notation    "CHEMONTID:0001379";
        skos:prefLabel   "Benzo-p-dioxins"@en .

cscl:kingdom  rdf:type   xkos:ClassificationLevel;
        xkos:depth       "1"^^xsd:positiveInteger;
        skos:definition  "The top level (Kingdom) partitions chemicals into two dis-joint categories: organic compounds versus inorganic compounds. "@en;
        skos:inScheme    vlcs:chemische_stof;
        skos:member      csc:CHEMONTID_0000001 , csc:CHEMONTID_0000000;
        skos:prefLabel   "Rijk"@nl .

csc:CHEMONTID_0000463
        rdf:type         skos:Concept;
        rdfs:seeAlso     tax_nodes:C0000463;
        skos:definition  "Organic compounds containing an oxoanion."@en;
        skos:inScheme    vlcs:chemische_stof;
        skos:notation    "CHEMONTID:0000463";
        skos:prefLabel   "Organic oxoanionic compounds"@en .

csc:CHEMONTID_0001198
        rdf:type         skos:Concept;
        rdfs:seeAlso     tax_nodes:C0001198;
        skos:definition  "Organic compounds containing a functional group with the general structure R1C(=S)R2 (R1, R2=H, alkyl, aryl)."@en;
        skos:inScheme    vlcs:chemische_stof;
        skos:notation    "CHEMONTID:0001198";
        skos:prefLabel   "Thiocarbonyl compounds"@en .

csc:CHEMONTID_0003370
        rdf:type         skos:Concept;
        rdfs:seeAlso     tax_nodes:C0003370;
        skos:definition  "Organonitrogen aromatic compounds that contain a central azo group, where each nitrogen atom is conjugated to a benzene ring."@en;
        skos:inScheme    vlcs:chemische_stof;
        skos:notation    "CHEMONTID:0003370";
        skos:prefLabel   "Azobenzenes"@en .

csc:CHEMONTID_0001518
        rdf:type         skos:Concept;
        rdfs:seeAlso     tax_nodes:C0001518;
        skos:definition  "Compounds containing a chemical bond between a carbon atom and an iodine atom."@en;
        skos:inScheme    vlcs:chemische_stof;
        skos:notation    "CHEMONTID:0001518";
        skos:prefLabel   "Organoiodides"@en .

csc:CHEMONTID_0000517
        rdf:type         skos:Concept;
        rdfs:seeAlso     tax_nodes:C0000517;
        skos:definition  "Compounds containing two amine groups joined by a carbonyl (C=O) functional group."@en;
        skos:inScheme    vlcs:chemische_stof;
        skos:notation    "CHEMONTID:0000517";
        skos:prefLabel   "Ureas"@en .

csc:CHEMONTID_0000210
        rdf:type         skos:Concept;
        rdfs:seeAlso     tax_nodes:C0000210;
        skos:definition  "Compounds containing a three ring system containing a pyrrole ring fused on either side to a benzene ring."@en;
        skos:inScheme    vlcs:chemische_stof;
        skos:notation    "CHEMONTID:0000210";
        skos:prefLabel   "Carbazoles"@en .

csc:CHEMONTID_0001729
        rdf:type         skos:Concept;
        rdfs:seeAlso     tax_nodes:C0001729;
        skos:definition  "Compounds containing an oxepane ring, which is a seven-member saturated aliphatic heterocycle with one oxygen and six carbon atoms."@en;
        skos:inScheme    vlcs:chemische_stof;
        skos:notation    "CHEMONTID:0001729";
        skos:prefLabel   "Oxepanes"@en .

csc:CHEMONTID_0002338
        rdf:type         skos:Concept;
        rdfs:seeAlso     tax_nodes:C0002338;
        skos:definition  "Polycyclic compounds containing a thiophene ring fused to a 7 member carbocyclic moiety. Thiophene is 5-membered ring consisting of four carbon atoms and one sulfur atom."@en;
        skos:inScheme    vlcs:chemische_stof;
        skos:notation    "CHEMONTID:0002338";
        skos:prefLabel   "Cycloheptathiophenes"@en .

csc:CHEMONTID_0001814
        rdf:type         skos:Concept;
        rdfs:seeAlso     tax_nodes:C0001814;
        skos:definition  "Compounds containing a phenylphosphine, which consists of phosphine substituent bound to a phenyl group."@en;
        skos:inScheme    vlcs:chemische_stof;
        skos:notation    "CHEMONTID:0001814";
        skos:prefLabel   "Phenylphosphines and derivatives"@en .

csc:CHEMONTID_0002031
        rdf:type         skos:Concept;
        rdfs:seeAlso     tax_nodes:C0002031;
        skos:definition  "Sterol lipids with a structure based on the stigmastane skeleton, which consists of a cholestane moiety bearing an ethyl group at the carbon atom C24."@en;
        skos:inScheme    vlcs:chemische_stof;
        skos:notation    "CHEMONTID:0002031";
        skos:prefLabel   "Stigmastanes and derivatives"@en .

csc:CHEMONTID_0001030
        rdf:type         skos:Concept;
        rdfs:seeAlso     tax_nodes:C0001030;
        skos:definition  "Organic compounds containing the acyl chloride functional group."@en;
        skos:inScheme    vlcs:chemische_stof;
        skos:notation    "CHEMONTID:0001030";
        skos:prefLabel   "Aryl chlorides"@en .

csc:CHEMONTID_0001548
        rdf:type         skos:Concept;
        rdfs:seeAlso     tax_nodes:C0001548;
        skos:definition  "Carboxylic acids (or derivative thereof) containing a halogen atom bonded to the alpha carbon atom."@en;
        skos:inScheme    vlcs:chemische_stof;
        skos:notation    "CHEMONTID:0001548";
        skos:prefLabel   "Alpha-halocarboxylic acids and derivatives"@en .

csc:CHEMONTID_0001633
        rdf:type         skos:Concept;
        rdfs:seeAlso     tax_nodes:C0001633;
        skos:definition  "Homoisoflavonoids with a structure based on the chromone system. Chromone is a bicyclic compound consisting of a 1-benzopyran, which bears a ketone group at the 4-position."@en;
        skos:inScheme    vlcs:chemische_stof;
        skos:notation    "CHEMONTID:0001633";
        skos:prefLabel   "Homoisoflavones"@en .

csc:CHEMONTID_0004189
        rdf:type         skos:Concept;
        rdfs:seeAlso     tax_nodes:C0004189;
        skos:definition  "Compounds containing the coumaran skeleton, which consists of a benzene ring fused to a 2,3-dihydrofuran ring."@en;
        skos:inScheme    vlcs:chemische_stof;
        skos:notation    "CHEMONTID:0004189";
        skos:prefLabel   "Coumarans"@en .

csc:CHEMONTID_0001578
        rdf:type         skos:Concept;
        rdfs:seeAlso     tax_nodes:C0001578;
        skos:definition  "Organic compounds containing a benzene ring fused to a furanone."@en;
        skos:inScheme    vlcs:chemische_stof;
        skos:notation    "CHEMONTID:0001578";
        skos:prefLabel   "Benzofuranones"@en .

csc:CHEMONTID_0000185
        rdf:type         skos:Concept;
        rdfs:seeAlso     tax_nodes:C0000185;
        skos:definition  "Compounds containing a phenylmethtylamine moiety, which consists of a phenyl group substituted by an methanamine."@en;
        skos:inScheme    vlcs:chemische_stof;
        skos:notation    "CHEMONTID:0000185";
        skos:prefLabel   "Phenylmethylamines"@en .

csc:CHEMONTID_0000270
        rdf:type         skos:Concept;
        rdfs:seeAlso     tax_nodes:C0000270;
        skos:definition  "Compounds containing a sulfonic acid or derivative, with the general structure RS(=O)2X (R=alkyl, aryl; X=any heteroatom)."@en;
        skos:inScheme    vlcs:chemische_stof;
        skos:notation    "CHEMONTID:0000270";
        skos:prefLabel   "Organosulfonic acids and derivatives"@en .

csc:CHEMONTID_0004485
        rdf:type         skos:Concept;
        rdfs:seeAlso     tax_nodes:C0004485;
        skos:definition  "Organohalogen compounds containing a monocyclic cyclohexane moiety that is substituted at one or more positions by an halogen atom."@en;
        skos:inScheme    vlcs:chemische_stof;
        skos:notation    "CHEMONTID:0004485";
        skos:prefLabel   "Cyclohexyl halides"@en .

csc:CHEMONTID_0002507
        rdf:type         skos:Concept;
        rdfs:seeAlso     tax_nodes:C0002507;
        skos:definition  "Naturally occurring oxygen heterocycles with a structure based on a 16-carbon skeleton including a chromanone, chromone or chromane system with a benzyl group at position C-3."@en;
        skos:inScheme    vlcs:chemische_stof;
        skos:notation    "CHEMONTID:0002507";
        skos:prefLabel   "Homoisoflavonoids"@en .

csc:CHEMONTID_0001506
        rdf:type         skos:Concept;
        rdfs:seeAlso     tax_nodes:C0001506;
        skos:definition  "Nucleotides with a purine base attached to the ribosyl moiety."@en;
        skos:inScheme    vlcs:chemische_stof;
        skos:notation    "CHEMONTID:0001506";
        skos:prefLabel   "Purine nucleotides"@en .

csc:CHEMONTID_0001114
        rdf:type         skos:Concept;
        rdfs:seeAlso     tax_nodes:C0001114;
        skos:definition  "Organic compounds containing an aldehyde substituted with a keto group on the C3 carbon atom."@en;
        skos:inScheme    vlcs:chemische_stof;
        skos:notation    "CHEMONTID:0001114";
        skos:prefLabel   "Beta-keto acids and derivatives"@en .

csc:CHEMONTID_0000113
        rdf:type         skos:Concept;
        rdfs:seeAlso     tax_nodes:C0000113;
        skos:definition  "Compounds containing a phenylhydrazide moiety, which consists of a hydrazide substituent attached to a phenyl group."@en;
        skos:inScheme    vlcs:chemische_stof;
        skos:notation    "CHEMONTID:0000113";
        skos:prefLabel   "Phenylhydrazines"@en .

csc:CHEMONTID_0000505
        rdf:type         skos:Concept;
        rdfs:seeAlso     tax_nodes:C0000505;
        skos:definition  "Compounds containing a sulfonyl group( which as the general structure RS(=O)2R' (R,R' =alkyl, aryl)) attached to two carbon atoms."@en;
        skos:inScheme    vlcs:chemische_stof;
        skos:notation    "CHEMONTID:0000505";
        skos:prefLabel   "Sulfones"@en .

csc:CHEMONTID_0001693
        rdf:type         skos:Concept;
        rdfs:seeAlso     tax_nodes:C0001693;
        skos:definition  "Organic compounds containing an amino group attached to a triazine ring."@en;
        skos:inScheme    vlcs:chemische_stof;
        skos:notation    "CHEMONTID:0001693";
        skos:prefLabel   "Aminotriazines"@en .

csc:CHEMONTID_0000716
        rdf:type         skos:Concept;
        rdfs:seeAlso     tax_nodes:C0000716;
        skos:definition  "Large heterocyclic aromatic ring systems consisting, at the core, of three pyrroles and one pyrroline coupled through four methine linkages."@en;
        skos:inScheme    vlcs:chemische_stof;
        skos:notation    "CHEMONTID:0000716";
        skos:prefLabel   "Chlorins"@en .

csc:CHEMONTID_0000324
        rdf:type         skos:Concept;
        rdfs:seeAlso     tax_nodes:C0000324;
        skos:definition  "Carboxylic ester derivatives of a fatty acid."@en;
        skos:inScheme    vlcs:chemische_stof;
        skos:notation    "CHEMONTID:0000324";
        skos:prefLabel   "Fatty acid esters"@en .

csc:CHEMONTID_0003412
        rdf:type         skos:Concept;
        rdfs:seeAlso     tax_nodes:C0003412;
        skos:definition  "Organic heterocyclic compounds containing a benzene ring fused to a pyran ring. Pyran a six-membered heterocyclic, non-aromatic ring, made up of five carbon atoms and one oxygen atom and containing two double bonds."@en;
        skos:inScheme    vlcs:chemische_stof;
        skos:notation    "CHEMONTID:0003412";
        skos:prefLabel   "Benzothiopyrans"@en .

csc:CHEMONTID_0000058
        rdf:type         skos:Concept;
        rdfs:seeAlso     tax_nodes:C0000058;
        skos:definition  "Polycyclic compounds with a four-ring skeleton with three condensed six-member rings forming a partially hydrogenated phenanthrene moiety, one of which is aromatic while the two others are alicyclic."@en;
        skos:inScheme    vlcs:chemische_stof;
        skos:notation    "CHEMONTID:0000058";
        skos:prefLabel   "Morphinans"@en .

cscl:subclass  rdf:type  xkos:ClassificationLevel;
        xkos:depth       "4"^^xsd:positiveInteger;
        skos:definition  "SubClasses, which typically consist of >10,000 known compounds. There are 1729 SubClasses in the current taxonomy. Additionally, there are 2296 addi-tional categories below the SubClass level covering taxo-nomic levels 5–11."@en;
        skos:inScheme    vlcs:chemische_stof;
        skos:member      csc:CHEMONTID_0000410 , csc:CHEMONTID_0002858 , csc:CHEMONTID_0000229 , csc:CHEMONTID_0004113 , csc:CHEMONTID_0001527 , csc:CHEMONTID_0000099 , csc:CHEMONTID_0000138 , csc:CHEMONTID_0004681 , csc:CHEMONTID_0000245 , csc:CHEMONTID_0001142 , csc:CHEMONTID_0001578 , csc:CHEMONTID_0002031 , csc:CHEMONTID_0000553 , csc:CHEMONTID_0000365 , csc:CHEMONTID_0001295 , csc:CHEMONTID_0000284 , csc:CHEMONTID_0000129 , csc:CHEMONTID_0000555 , csc:CHEMONTID_0000525 , csc:CHEMONTID_0001973 , csc:CHEMONTID_0001093 , csc:CHEMONTID_0000045 , csc:CHEMONTID_0001152 , csc:CHEMONTID_0000033 , csc:CHEMONTID_0004677 , csc:CHEMONTID_0001022 , csc:CHEMONTID_0004201 , csc:CHEMONTID_0004112 , csc:CHEMONTID_0003936 , csc:CHEMONTID_0000538 , csc:CHEMONTID_0004551 , csc:CHEMONTID_0002542 , csc:CHEMONTID_0002275 , csc:CHEMONTID_0001359 , csc:CHEMONTID_0002496 , csc:CHEMONTID_0003688 , csc:CHEMONTID_0001753 , csc:CHEMONTID_0000552 , csc:CHEMONTID_0000075 , csc:CHEMONTID_0004387 , csc:CHEMONTID_0001982 , csc:CHEMONTID_0001710 , csc:CHEMONTID_0000895 , csc:CHEMONTID_0001243 , csc:CHEMONTID_0004450 , csc:CHEMONTID_0001935 , csc:CHEMONTID_0000270 , csc:CHEMONTID_0004622 , csc:CHEMONTID_0001986 , csc:CHEMONTID_0000176 , csc:CHEMONTID_0002484 , csc:CHEMONTID_0003970 , csc:CHEMONTID_0000320 , csc:CHEMONTID_0000549 , csc:CHEMONTID_0001633 , csc:CHEMONTID_0000921 , csc:CHEMONTID_0001804 , csc:CHEMONTID_0003455 , csc:CHEMONTID_0001279 , csc:CHEMONTID_0000189 , csc:CHEMONTID_0002340 , csc:CHEMONTID_0002132 , csc:CHEMONTID_0002442 , csc:CHEMONTID_0000014 , csc:CHEMONTID_0004640 , csc:CHEMONTID_0002180 , csc:CHEMONTID_0002861 , csc:CHEMONTID_0003194 , csc:CHEMONTID_0002838 , csc:CHEMONTID_0001530 , csc:CHEMONTID_0001057 , csc:CHEMONTID_0003953 , csc:CHEMONTID_0000151 , csc:CHEMONTID_0003413 , csc:CHEMONTID_0004711 , csc:CHEMONTID_0002441 , csc:CHEMONTID_0000346 , csc:CHEMONTID_0004164 , csc:CHEMONTID_0000162 , csc:CHEMONTID_0000583 , csc:CHEMONTID_0001180 , csc:CHEMONTID_0000132 , csc:CHEMONTID_0001764 , csc:CHEMONTID_0001062 , csc:CHEMONTID_0001572 , csc:CHEMONTID_0000032 , csc:CHEMONTID_0004676 , csc:CHEMONTID_0001158 , csc:CHEMONTID_0002017 , csc:CHEMONTID_0001212 , csc:CHEMONTID_0000250 , csc:CHEMONTID_0000405 , csc:CHEMONTID_0004752 , csc:CHEMONTID_0002680 , csc:CHEMONTID_0000303 , csc:CHEMONTID_0001073 , csc:CHEMONTID_0000013 , csc:CHEMONTID_0000375 , csc:CHEMONTID_0000395 , csc:CHEMONTID_0000363 , csc:CHEMONTID_0001722 , csc:CHEMONTID_0000113 , csc:CHEMONTID_0001544 , csc:CHEMONTID_0000074 , csc:CHEMONTID_0001691 , csc:CHEMONTID_0002257 , csc:CHEMONTID_0004152 , csc:CHEMONTID_0004794 , csc:CHEMONTID_0000316 , csc:CHEMONTID_0004504 , csc:CHEMONTID_0004089 , csc:CHEMONTID_0004485 , csc:CHEMONTID_0001437 , csc:CHEMONTID_0002044 , csc:CHEMONTID_0000517 , csc:CHEMONTID_0001091 , csc:CHEMONTID_0000031 , csc:CHEMONTID_0000163 , csc:CHEMONTID_0000548 , csc:CHEMONTID_0000226 , csc:CHEMONTID_0004632 , csc:CHEMONTID_0001272 , csc:CHEMONTID_0000186 , csc:CHEMONTID_0000056 , csc:CHEMONTID_0004097 , csc:CHEMONTID_0001313 , csc:CHEMONTID_0000112 , csc:CHEMONTID_0000411 , csc:CHEMONTID_0001322 , csc:CHEMONTID_0004776 , csc:CHEMONTID_0000505 , csc:CHEMONTID_0000327 , csc:CHEMONTID_0001549 , csc:CHEMONTID_0001715 , csc:CHEMONTID_0001097 , csc:CHEMONTID_0003567 , csc:CHEMONTID_0001026 , csc:CHEMONTID_0000640 , csc:CHEMONTID_0000554 , csc:CHEMONTID_0000095 , csc:CHEMONTID_0004443 , csc:CHEMONTID_0003569 , csc:CHEMONTID_0001861 , csc:CHEMONTID_0000518 , csc:CHEMONTID_0001151 , csc:CHEMONTID_0000072 , csc:CHEMONTID_0003815 , csc:CHEMONTID_0000417 , csc:CHEMONTID_0000067 , csc:CHEMONTID_0000055 , csc:CHEMONTID_0004456 , csc:CHEMONTID_0002363 , csc:CHEMONTID_0003981 , csc:CHEMONTID_0004647 , csc:CHEMONTID_0001888 , csc:CHEMONTID_0000190 , csc:CHEMONTID_0001055 , csc:CHEMONTID_0002500 , csc:CHEMONTID_0003411 , csc:CHEMONTID_0004162 , csc:CHEMONTID_0000331 , csc:CHEMONTID_0000308 , csc:CHEMONTID_0000299 , csc:CHEMONTID_0002552 , csc:CHEMONTID_0002320 , csc:CHEMONTID_0001460 , csc:CHEMONTID_0003808 , csc:CHEMONTID_0002863 , csc:CHEMONTID_0002902 , csc:CHEMONTID_0002995 , csc:CHEMONTID_0004646 , csc:CHEMONTID_0004157 , csc:CHEMONTID_0000310 , csc:CHEMONTID_0000011 , csc:CHEMONTID_0002348 , csc:CHEMONTID_0002049 , csc:CHEMONTID_0002445 , csc:CHEMONTID_0000081 , csc:CHEMONTID_0004631 , csc:CHEMONTID_0000079 , csc:CHEMONTID_0001114 , csc:CHEMONTID_0000504 , csc:CHEMONTID_0003893 , csc:CHEMONTID_0000326 , csc:CHEMONTID_0000015 , csc:CHEMONTID_0000036 , csc:CHEMONTID_0002317 , csc:CHEMONTID_0000254 , csc:CHEMONTID_0004105 , csc:CHEMONTID_0001334 , csc:CHEMONTID_0001205 , csc:CHEMONTID_0002449 , csc:CHEMONTID_0001466 , csc:CHEMONTID_0002042 , csc:CHEMONTID_0000330 , csc:CHEMONTID_0000041 , csc:CHEMONTID_0000038 , csc:CHEMONTID_0004107 , csc:CHEMONTID_0002336 , csc:CHEMONTID_0003566 , csc:CHEMONTID_0000399 , csc:CHEMONTID_0004628 , csc:CHEMONTID_0002901 , csc:CHEMONTID_0003597 , csc:CHEMONTID_0000522 , csc:CHEMONTID_0000355 , csc:CHEMONTID_0003809 , csc:CHEMONTID_0001524 , csc:CHEMONTID_0002651 , csc:CHEMONTID_0000392 , csc:CHEMONTID_0001016 , csc:CHEMONTID_0000139 , csc:CHEMONTID_0001920 , csc:CHEMONTID_0001168 , csc:CHEMONTID_0001961 , csc:CHEMONTID_0004208 , csc:CHEMONTID_0000262 , csc:CHEMONTID_0000503 , csc:CHEMONTID_0001857 , csc:CHEMONTID_0000047 , csc:CHEMONTID_0000035 , csc:CHEMONTID_0001368 , csc:CHEMONTID_0000285 , csc:CHEMONTID_0001891 , csc:CHEMONTID_0002010 , csc:CHEMONTID_0000093 , csc:CHEMONTID_0001871 , csc:CHEMONTID_0001553 , csc:CHEMONTID_0000398 , csc:CHEMONTID_0001814 , csc:CHEMONTID_0004789 , csc:CHEMONTID_0000298 , csc:CHEMONTID_0000542 , csc:CHEMONTID_0000530 , csc:CHEMONTID_0004233 , csc:CHEMONTID_0000053 , csc:CHEMONTID_0000901 , csc:CHEMONTID_0001245 , csc:CHEMONTID_0000185 , csc:CHEMONTID_0001030 , csc:CHEMONTID_0001077 , csc:CHEMONTID_0001379 , csc:CHEMONTID_0000546 , csc:CHEMONTID_0000534 , csc:CHEMONTID_0001548 , csc:CHEMONTID_0000078 , csc:CHEMONTID_0003862 , csc:CHEMONTID_0000550 , csc:CHEMONTID_0000372 , csc:CHEMONTID_0000369 , csc:CHEMONTID_0003568 , csc:CHEMONTID_0001987 , csc:CHEMONTID_0001607 , csc:CHEMONTID_0001027 , csc:CHEMONTID_0001975 , csc:CHEMONTID_0001065 , csc:CHEMONTID_0004766 , csc:CHEMONTID_0004203 , csc:CHEMONTID_0000408 , csc:CHEMONTID_0001831 , csc:CHEMONTID_0004155 , csc:CHEMONTID_0000210 , csc:CHEMONTID_0000324 , csc:CHEMONTID_0001534 , csc:CHEMONTID_0004660 , csc:CHEMONTID_0000120 , csc:CHEMONTID_0003410 , csc:CHEMONTID_0001286 , csc:CHEMONTID_0001550 , csc:CHEMONTID_0000490 , csc:CHEMONTID_0003449 , csc:CHEMONTID_0003480 , csc:CHEMONTID_0000584 , csc:CHEMONTID_0002966 , csc:CHEMONTID_0000087 , csc:CHEMONTID_0001204 , csc:CHEMONTID_0002581 , csc:CHEMONTID_0001183 , csc:CHEMONTID_0001314 , csc:CHEMONTID_0004758 , csc:CHEMONTID_0001693 , csc:CHEMONTID_0004742 , csc:CHEMONTID_0002497 , csc:CHEMONTID_0004024 , csc:CHEMONTID_0000321 , csc:CHEMONTID_0001244 , csc:CHEMONTID_0001908 , csc:CHEMONTID_0002864 , csc:CHEMONTID_0001470 , csc:CHEMONTID_0000501 , csc:CHEMONTID_0001290 , csc:CHEMONTID_0004670 , csc:CHEMONTID_0000194 , csc:CHEMONTID_0002811 , csc:CHEMONTID_0004714 , csc:CHEMONTID_0004665 , csc:CHEMONTID_0000153 , csc:CHEMONTID_0001302 , csc:CHEMONTID_0000141 , csc:CHEMONTID_0004785 , csc:CHEMONTID_0000526 , csc:CHEMONTID_0001581 , csc:CHEMONTID_0001551 , csc:CHEMONTID_0000049 , csc:CHEMONTID_0000037 , csc:CHEMONTID_0002798 , csc:CHEMONTID_0001194 , csc:CHEMONTID_0001974 , csc:CHEMONTID_0004476 , csc:CHEMONTID_0000716 , csc:CHEMONTID_0002608;
        skos:prefLabel   "Subklasse"@nl .

csc:CHEMONTID_0004443
        rdf:type         skos:Concept;
        rdfs:seeAlso     tax_nodes:C0004443;
        skos:definition  "Metal alkyls, where the alkyl group is attached to a transition metal atom."@en;
        skos:inScheme    vlcs:chemische_stof;
        skos:notation    "CHEMONTID:0004443";
        skos:prefLabel   "Transition metal alkyls"@en .

csc:CHEMONTID_0002441
        rdf:type         skos:Concept;
        rdfs:seeAlso     tax_nodes:C0002441;
        skos:definition  "Naphthalene derivatives carrying one or more hydroxyl (-OH) groups at any ring position."@en;
        skos:inScheme    vlcs:chemische_stof;
        skos:notation    "CHEMONTID:0002441";
        skos:prefLabel   "Naphthols and derivatives"@en .

csc:CHEMONTID_0003568
        rdf:type         skos:Concept;
        rdfs:seeAlso     tax_nodes:C0003568;
        skos:definition  "Steroids with a structure based on the 19-carbon androstane skeleton."@en;
        skos:inScheme    vlcs:chemische_stof;
        skos:notation    "CHEMONTID:0003568";
        skos:prefLabel   "Androstane steroids"@en .

csc:CHEMONTID_0000299
        rdf:type         skos:Concept;
        rdfs:seeAlso     tax_nodes:C0000299;
        skos:definition  "Hydroxy acids with a 6 to 12 carbon atoms long side chain."@en;
        skos:inScheme    vlcs:chemische_stof;
        skos:notation    "CHEMONTID:0000299";
        skos:prefLabel   "Medium-chain hydroxy acids and derivatives"@en .

csc:CHEMONTID_0002863
        rdf:type         skos:Concept;
        rdfs:seeAlso     tax_nodes:C0002863;
        skos:definition  "Vinyl halides in which a chlorine atom is bonded to an sp2-hybridised carbon atom."@en;
        skos:inScheme    vlcs:chemische_stof;
        skos:notation    "CHEMONTID:0002863";
        skos:prefLabel   "Vinyl chlorides"@en .

csc:CHEMONTID_0001862
        rdf:type         skos:Concept;
        rdfs:seeAlso     tax_nodes:C0001862;
        skos:definition  "Organic compounds containing a six-member aliphatic saturated heterocycle made up of three sulfur atoms and three carbon atoms."@en;
        skos:inScheme    vlcs:chemische_stof;
        skos:notation    "CHEMONTID:0001862";
        skos:prefLabel   "Trithianes"@en .

csc:CHEMONTID_0001470
        rdf:type         skos:Concept;
        rdfs:seeAlso     tax_nodes:C0001470;
        skos:definition  "Inorganic compounds containing a metallic oxoanion to which either no atom or a non metal atom is bonded."@en;
        skos:inScheme    vlcs:chemische_stof;
        skos:notation    "CHEMONTID:0001470";
        skos:prefLabel   "Miscellaneous metallic oxoanionic compounds"@en .

csc:CHEMONTID_0000408
        rdf:type         skos:Concept;
        rdfs:seeAlso     tax_nodes:C0000408;
        skos:definition  "Organic compounds containing phosphoric acid ester functional group, with the general structure R1P(=O)(R2)OR3. R1,R2 = O,N,  or halogen atom; R3 = organyl group."@en;
        skos:inScheme    vlcs:chemische_stof;
        skos:notation    "CHEMONTID:0000408";
        skos:prefLabel   "Phosphate esters"@en .

cscl:superclass  rdf:type  xkos:ClassificationLevel;
        xkos:depth       "2"^^xsd:positiveInteger;
        skos:definition  "SuperClasses (which includes 26 organic and 5 inorganic categories) consist of generic categories of compounds with general structural identifiers (e.g. organic acids and derivatives, phenylpropanoids and polyketides, organometallic com-pounds, homogeneous metal compounds), each of which covers millions of known compounds. "@en;
        skos:inScheme    vlcs:chemische_stof;
        skos:member      csc:CHEMONTID_0000400 , csc:CHEMONTID_0003865 , csc:CHEMONTID_0000422 , csc:CHEMONTID_0000267 , csc:CHEMONTID_0000289 , csc:CHEMONTID_0000012 , csc:CHEMONTID_0004707 , csc:CHEMONTID_0000423 , csc:CHEMONTID_0000004 , csc:CHEMONTID_0004603 , csc:CHEMONTID_0000462 , csc:CHEMONTID_0004150 , csc:CHEMONTID_0000279 , csc:CHEMONTID_0002448 , csc:CHEMONTID_0003630 , csc:CHEMONTID_0001392 , csc:CHEMONTID_0002837 , csc:CHEMONTID_0000261 , csc:CHEMONTID_0000002 , csc:CHEMONTID_0000424 , csc:CHEMONTID_0000264 , csc:CHEMONTID_0004478;
        skos:prefLabel   "Superklasse"@nl .

csc:CHEMONTID_0004105
        rdf:type         skos:Concept;
        rdfs:seeAlso     tax_nodes:C0004105;
        skos:definition  "Compounds containing a triazine ring, which is a heterocyclic ring, similar to the six-member benzene ring but with three carbons replaced by nitrogen atoms, at ring positions 1, 3, and 5."@en;
        skos:inScheme    vlcs:chemische_stof;
        skos:notation    "CHEMONTID:0004105";
        skos:prefLabel   "1,3,5-triazines"@en .

csc:CHEMONTID_0001313
        rdf:type         skos:Concept;
        rdfs:seeAlso     tax_nodes:C0001313;
        skos:definition  "Organic compounds containing 1,4-dioxane, an aliphatic six-member ring with two oxygen atoms in ring positions 1 and 4."@en;
        skos:inScheme    vlcs:chemische_stof;
        skos:notation    "CHEMONTID:0001313";
        skos:prefLabel   "1,4-dioxanes"@en .

csc:CHEMONTID_0001524
        rdf:type         skos:Concept;
        rdfs:seeAlso     tax_nodes:C0001524;
        skos:definition  "Compounds containing bond between a carbon atom and a tin atom."@en;
        skos:inScheme    vlcs:chemische_stof;
        skos:notation    "CHEMONTID:0001524";
        skos:prefLabel   "Organotin compounds"@en .

csc:CHEMONTID_0001077
        rdf:type         skos:Concept;
        rdfs:seeAlso     tax_nodes:C0001077;
        skos:definition  "Inorganic non-metallic compoundscontaining a sulfate as its largest oxoanion."@en;
        skos:inScheme    vlcs:chemische_stof;
        skos:notation    "CHEMONTID:0001077";
        skos:prefLabel   "Non-metal sulfates"@en .

csc:CHEMONTID_0000076
        rdf:type         skos:Concept;
        rdfs:seeAlso     tax_nodes:C0000076;
        skos:definition  "Compounds containing a furan ring, which is a five-member aromatic ring with one oxygen atom, four carbon atoms."@en;
        skos:inScheme    vlcs:chemische_stof;
        skos:notation    "CHEMONTID:0000076";
        skos:prefLabel   "Furans"@en .

csc:CHEMONTID_0000553
        rdf:type         skos:Concept;
        rdfs:seeAlso     tax_nodes:C0000553;
        skos:definition  "Inorganic compounds of nitrogen where nitrogen has a formal oxidation state of −3, and the heaviest atom bonded to it belongs to the class of 'other non-metals'."@en;
        skos:inScheme    vlcs:chemische_stof;
        skos:notation    "CHEMONTID:0000553";
        skos:prefLabel   "Other non-metal nitrides"@en .

csc:CHEMONTID_0000372
        rdf:type         skos:Concept;
        rdfs:seeAlso     tax_nodes:C0000372;
        skos:definition  "Compounds containing the fentanyl moiety or a derivative, which is based on a N-(1-(2-phenylethyl)-4-piperidinyl)-N-phenylpropanamide skeleton."@en;
        skos:inScheme    vlcs:chemische_stof;
        skos:notation    "CHEMONTID:0000372";
        skos:prefLabel   "Fentanyls"@en .

csc:CHEMONTID_0001850
        rdf:type         skos:Concept;
        rdfs:seeAlso     tax_nodes:C0001850;
        skos:definition  "Compounds containing a thiophenol ring, which a phenol derivative obtained by replacing the oxygen atom from the hydroxyl group (attached to the benzene) by a sulfur atom."@en;
        skos:inScheme    vlcs:chemische_stof;
        skos:notation    "CHEMONTID:0001850";
        skos:prefLabel   "Thiophenols"@en .

csc:CHEMONTID_0003194
        rdf:type         skos:Concept;
        rdfs:seeAlso     tax_nodes:C0003194;
        skos:definition  "Organic compounds containing a C[Si] bond."@en;
        skos:inScheme    vlcs:chemische_stof;
        skos:notation    "CHEMONTID:0003194";
        skos:prefLabel   "Organosilicon compounds"@en .

csc:CHEMONTID_0000583
        rdf:type         skos:Concept;
        rdfs:seeAlso     tax_nodes:C0000583;
        skos:definition  "Inorganic compounds in which the largest halogen atom is Chlorine, and the heaviest metal atom is a metalloid."@en;
        skos:inScheme    vlcs:chemische_stof;
        skos:notation    "CHEMONTID:0000583";
        skos:prefLabel   "Metalloid chlorides"@en .

csc:CHEMONTID_0000004
        rdf:type         skos:Concept;
        rdfs:seeAlso     tax_nodes:C0000004;
        skos:definition  "Organic compounds containing a carbon-sulfur bond."@en;
        skos:inScheme    vlcs:chemische_stof;
        skos:notation    "CHEMONTID:0000004";
        skos:prefLabel   "Organosulfur compounds"@en .

csc:CHEMONTID_0001819
        rdf:type         skos:Concept;
        rdfs:seeAlso     tax_nodes:C0001819;
        skos:definition  "Polycyclic compounds containing an isoindole moiety, which is structurally characterized by a cyclohexadiene fused to a pyrrole ring."@en;
        skos:inScheme    vlcs:chemische_stof;
        skos:notation    "CHEMONTID:0001819";
        skos:prefLabel   "Isoindoles and derivatives"@en .

csc:CHEMONTID_0000426
        rdf:type         skos:Concept;
        rdfs:seeAlso     tax_nodes:C0000426;
        skos:definition  "Inorganic compounds containing only metal atoms,with the largest atom being a transition metal atom."@en;
        skos:inScheme    vlcs:chemische_stof;
        skos:notation    "CHEMONTID:0000426";
        skos:prefLabel   "Homogeneous transition metal compounds"@en .

csc:CHEMONTID_0000245
        rdf:type         skos:Concept;
        rdfs:seeAlso     tax_nodes:C0000245;
        skos:definition  "Aromatic heterocyclic compounds containing a purine moiety, which is formed a pyrimidine-ring ring fused to an imidazole ring."@en;
        skos:inScheme    vlcs:chemische_stof;
        skos:notation    "CHEMONTID:0000245";
        skos:prefLabel   "Purines and purine derivatives"@en .

csc:CHEMONTID_0000330
        rdf:type         skos:Concept;
        rdfs:seeAlso     tax_nodes:C0000330;
        skos:definition  "Compounds containing a phenylbenzimidazole skeleton, which consists of a benzimidazole moiety where its imidazole ring is attached to a phenyl group."@en;
        skos:inScheme    vlcs:chemische_stof;
        skos:notation    "CHEMONTID:0000330";
        skos:prefLabel   "Phenylbenzimidazoles"@en .

csc:CHEMONTID_0003936
        rdf:type         skos:Concept;
        rdfs:seeAlso     tax_nodes:C0003936;
        skos:definition  "Organosulfur compounds with the general formula R3SC(=S)N(R1)R2; R1-R2 =  H or organyl group, R3 = organyl."@en;
        skos:inScheme    vlcs:chemische_stof;
        skos:notation    "CHEMONTID:0003936";
        skos:prefLabel   "Dithiocarbamic acid esters"@en .

csc:CHEMONTID_0001065
        rdf:type         skos:Concept;
        rdfs:seeAlso     tax_nodes:C0001065;
        skos:definition  "Inorganic non-metallic compoundscontaining a perchlorate as its largest oxoanion."@en;
        skos:inScheme    vlcs:chemische_stof;
        skos:notation    "CHEMONTID:0001065";
        skos:prefLabel   "Non-metal perchlorates"@en .

csc:CHEMONTID_0000064
        rdf:type         skos:Concept;
        rdfs:seeAlso     tax_nodes:C0000064;
        skos:definition  "Cyclic amides of amino carboxylic acids, having a 1-azacycloalkan-2-one structure, or analogues having unsaturation or heteroatoms replacing one or more carbon atoms of the ring.  They are nitrogen analogues (the a nitrogen atom replacing the o atom of the cyclic carboxylic acid group ) of the naturally occurring macrolides."@en;
        skos:inScheme    vlcs:chemische_stof;
        skos:notation    "CHEMONTID:0000064";
        skos:prefLabel   "Macrolactams"@en .

csc:CHEMONTID_0000456
        rdf:type         skos:Concept;
        rdfs:seeAlso     tax_nodes:C0000456;
        skos:definition  "Inorganic compounds belonging either to the alkali metal hydrides, the alkali metal nitrides, the alkali metal oxides, or the alkali metal sulfides."@en;
        skos:inScheme    vlcs:chemische_stof;
        skos:notation    "CHEMONTID:0000456";
        skos:prefLabel   "Alkali metal organides"@en .

vlcs:chemische_stof  rdf:type  skos:ConceptScheme;
        xkos:levels         list:kingdom;
        skos:hasTopConcept  csc:CHEMONTID_0000001 , csc:CHEMONTID_0000000 .

csc:CHEMONTID_0002754
        rdf:type         skos:Concept;
        rdfs:seeAlso     tax_nodes:C0002754;
        skos:definition  "Aromatic alcohols containing a 3-phenylprop-2-en-1-ol moiety."@en;
        skos:inScheme    vlcs:chemische_stof;
        skos:notation    "CHEMONTID:0002754";
        skos:prefLabel   "Cinnamyl alcohols"@en .

csc:CHEMONTID_0001753
        rdf:type         skos:Concept;
        rdfs:seeAlso     tax_nodes:C0001753;
        skos:definition  "Organic compounds containing an indole attached to a benzoyl moiety through the acyl group."@en;
        skos:inScheme    vlcs:chemische_stof;
        skos:notation    "CHEMONTID:0001753";
        skos:prefLabel   "Benzoylindoles"@en .

csc:CHEMONTID_0001572
        rdf:type         skos:Concept;
        rdfs:seeAlso     tax_nodes:C0001572;
        skos:definition  "Organic compounds containing the thiophosphoric acid functional group or a derivative thereof, with the general structure ROP(OR')(OR'')=S, where at least one R-group is an organyl group."@en;
        skos:inScheme    vlcs:chemische_stof;
        skos:notation    "CHEMONTID:0001572";
        skos:prefLabel   "Thiophosphoric acid esters"@en .

csc:CHEMONTID_0001180
        rdf:type         skos:Concept;
        rdfs:seeAlso     tax_nodes:C0001180;
        skos:definition  "Organic compounds containing the sulfuric acid functional group, with the generic structure HOS(=O)(=O)OH."@en;
        skos:inScheme    vlcs:chemische_stof;
        skos:notation    "CHEMONTID:0001180";
        skos:prefLabel   "Organic sulfuric acids"@en .

csc:CHEMONTID_0004660
        rdf:type         skos:Concept;
        rdfs:seeAlso     tax_nodes:C0004660;
        skos:definition  "Aromatic compounds containing a benzo-1,2,3-triazine, which is substituted by an organothiophosphate group at the 3-position. Their general structure is R-CSP(=S)(OR')OR'', where R=benzo-1,2,3-triazine, R',R\\\" = any atom."@en;
        skos:inScheme    vlcs:chemische_stof;
        skos:notation    "CHEMONTID:0004660";
        skos:prefLabel   "Benzotriazine organothiophosphates"@en .

csc:CHEMONTID_0001204
        rdf:type         skos:Concept;
        rdfs:seeAlso     tax_nodes:C0001204;
        skos:definition  "Organic compounds containing the phosphoric acid amide functional group."@en;
        skos:inScheme    vlcs:chemische_stof;
        skos:notation    "CHEMONTID:0001204";
        skos:prefLabel   "Organic phosphoramides"@en .

csc:CHEMONTID_0003809
        rdf:type         skos:Concept;
        rdfs:seeAlso     tax_nodes:C0003809;
        skos:definition  "Glycerolipids that carry exactly two acyl chains attached to the glycerol moiety."@en;
        skos:inScheme    vlcs:chemische_stof;
        skos:notation    "CHEMONTID:0003809";
        skos:prefLabel   "Diradylglycerols"@en .

csc:CHEMONTID_0002995
        rdf:type         skos:Concept;
        rdfs:seeAlso     tax_nodes:C0002995;
        skos:definition  "Carboxylic acids containing exactly five carboxyl groups."@en;
        skos:inScheme    vlcs:chemische_stof;
        skos:notation    "CHEMONTID:0002995";
        skos:prefLabel   "Pentacarboxylic acids and derivatives"@en .

csc:CHEMONTID_0004714
        rdf:type         skos:Concept;
        rdfs:seeAlso     tax_nodes:C0004714;
        skos:definition  "Ester derivatives of phenylcarbamic acids."@en;
        skos:inScheme    vlcs:chemische_stof;
        skos:notation    "CHEMONTID:0004714";
        skos:prefLabel   "Phenylcarbamic acid esters"@en .

csc:CHEMONTID_0001234
        rdf:type         skos:Concept;
        rdfs:seeAlso     tax_nodes:C0001234;
        skos:definition  "Organic compounds containing the isothiocyanate group, an isocyanate analogue with the general formula RN=C=S."@en;
        skos:inScheme    vlcs:chemische_stof;
        skos:notation    "CHEMONTID:0001234";
        skos:prefLabel   "Isothiocyanates"@en .

csc:CHEMONTID_0000233
        rdf:type         skos:Concept;
        rdfs:seeAlso     tax_nodes:C0000233;
        skos:definition  "Organic compounds containing thiolane, a five-member saturated ring containing four carbon atoms and a sulfur atom."@en;
        skos:inScheme    vlcs:chemische_stof;
        skos:notation    "CHEMONTID:0000233";
        skos:prefLabel   "Thiolanes"@en .

csc:CHEMONTID_0002320
        rdf:type         skos:Concept;
        rdfs:seeAlso     tax_nodes:C0002320;
        skos:definition  "Aromatic compounds containing benzene substituted by a hydroxyl group and a halogen atom."@en;
        skos:inScheme    vlcs:chemische_stof;
        skos:notation    "CHEMONTID:0002320";
        skos:prefLabel   "Halophenols"@en .

csc:CHEMONTID_0002838
        rdf:type         skos:Concept;
        rdfs:seeAlso     tax_nodes:C0002838;
        skos:definition  "Acyclic and cyclic hydrocarbons having one or more carbon-carbon double bonds, apart from the formal ones in aromatic compounds. The class of olefins subsumes alkenes and cycloalkenes and the corresponding polyenes."@en;
        skos:inScheme    vlcs:chemische_stof;
        skos:notation    "CHEMONTID:0002838";
        skos:prefLabel   "Olefins"@en .

csc:CHEMONTID_0000444
        rdf:type         skos:Concept;
        rdfs:seeAlso     tax_nodes:C0000444;
        skos:definition  "Inorganic halogenic compounds in which the heaviest metal atom is a post-transition metal."@en;
        skos:inScheme    vlcs:chemische_stof;
        skos:notation    "CHEMONTID:0000444";
        skos:prefLabel   "Post-transition metal salts"@en .

csc:CHEMONTID_0004659
        rdf:type         skos:Concept;
        rdfs:seeAlso     tax_nodes:C0004659;
        skos:definition  "Organic compounds containing a 1,2,3-triazine ring fused to a benzene ring."@en;
        skos:inScheme    vlcs:chemische_stof;
        skos:notation    "CHEMONTID:0004659";
        skos:prefLabel   "Benzo-1,2,3-triazines"@en .

csc:CHEMONTID_0001530
        rdf:type         skos:Concept;
        rdfs:seeAlso     tax_nodes:C0001530;
        skos:definition  "Organic compounds containing a benzene bearing a nitrile substituent."@en;
        skos:inScheme    vlcs:chemische_stof;
        skos:notation    "CHEMONTID:0001530";
        skos:prefLabel   "Benzonitriles"@en .

csc:CHEMONTID_0000921
        rdf:type         skos:Concept;
        rdfs:seeAlso     tax_nodes:C0000921;
        skos:definition  "Inorganic compounds in which the largest oxoanion is silicate, and in which the heaviest atom not in an oxoanion is an alkaline earth metal."@en;
        skos:inScheme    vlcs:chemische_stof;
        skos:notation    "CHEMONTID:0000921";
        skos:prefLabel   "Alkaline earth metal silicates"@en .

csc:CHEMONTID_0004478
        rdf:type         skos:Concept;
        rdfs:seeAlso     tax_nodes:C0004478;
        skos:definition  "Compounds arising by replacement of one or both hydrogen atoms of acetylene (ethyne) by a metal or other cationic group. E.g. NaC#CH monosodium acetylide. By extension, analogous compounds derived from terminal acetylenes, RC#CH. The class is limited here to derivatives of acetylene where the hydrogen atom is replaced with an element with similar or lower electronegativity that carbon."@en;
        skos:inScheme    vlcs:chemische_stof;
        skos:notation    "CHEMONTID:0004478";
        skos:prefLabel   "Acetylides"@en .

csc:CHEMONTID_0000389
        rdf:type         skos:Concept;
        rdfs:seeAlso     tax_nodes:C0000389;
        skos:definition  "Organic compounds containing a ketone group and a carboxylic acid group."@en;
        skos:inScheme    vlcs:chemische_stof;
        skos:notation    "CHEMONTID:0000389";
        skos:prefLabel   "Keto acids and derivatives"@en .

csc:CHEMONTID_0002868
        rdf:type         skos:Concept;
        rdfs:seeAlso     tax_nodes:C0002868;
        skos:definition  "Organic compounds in which the halogen atom is bonded to an sp2-hybridised carbon atom of a carbon-carbon double bond (C=C)."@en;
        skos:inScheme    vlcs:chemische_stof;
        skos:notation    "CHEMONTID:0002868";
        skos:prefLabel   "Vinyl halides"@en .

csc:CHEMONTID_0003688
        rdf:type         skos:Concept;
        rdfs:seeAlso     tax_nodes:C0003688;
        skos:definition  "Organic compounds having the divalent diazo group, =N+=N-, attached to a carbon atom."@en;
        skos:inScheme    vlcs:chemische_stof;
        skos:notation    "CHEMONTID:0003688";
        skos:prefLabel   "Diazo compounds"@en .

csc:CHEMONTID_0000293
        rdf:type         skos:Concept;
        rdfs:seeAlso     tax_nodes:C0000293;
        skos:definition  "Organic compounds containing a benzene ring fused to an azepine ring (unsaturated seven-membered heterocycle with one nitrogen atom replacing a carbon atom)."@en;
        skos:inScheme    vlcs:chemische_stof;
        skos:notation    "CHEMONTID:0000293";
        skos:prefLabel   "Benzazepines"@en .

csc:CHEMONTID_0000106
        rdf:type         skos:Concept;
        rdfs:seeAlso     tax_nodes:C0000106;
        skos:definition  "Compounds containing an oxathiolane moiety, which consists of a saturated aliphatic five-member ring with one oxygen atom, a sulfur atom, and three carbon atoms. Isomers  of oxaphospholane include meta-oxathiolane, and ortho-oxathiolane."@en;
        skos:inScheme    vlcs:chemische_stof;
        skos:notation    "CHEMONTID:0000106";
        skos:prefLabel   "Oxathiolanes"@en .

csc:CHEMONTID_0002319
        rdf:type         skos:Concept;
        rdfs:seeAlso     tax_nodes:C0002319;
        skos:definition  "Aromatic compounds containing a benzene ring substituted by a hydroxyl group and an ester group."@en;
        skos:inScheme    vlcs:chemische_stof;
        skos:notation    "CHEMONTID:0002319";
        skos:prefLabel   "Phenol esters"@en .

csc:CHEMONTID_0000317
        rdf:type         skos:Concept;
        rdfs:seeAlso     tax_nodes:C0000317;
        skos:definition  "Organic compounds containing a benzene fused to a thiazepine ring (a seven-membered ring with a nitrogen atom and a sulfur atom replacing two carbon atoms)."@en;
        skos:inScheme    vlcs:chemische_stof;
        skos:notation    "CHEMONTID:0000317";
        skos:prefLabel   "Benzothiazepines"@en .

csc:CHEMONTID_0001982
        rdf:type         skos:Concept;
        rdfs:seeAlso     tax_nodes:C0001982;
        skos:definition  "Compounds containing a furan ring bearing a ketone group."@en;
        skos:inScheme    vlcs:chemische_stof;
        skos:notation    "CHEMONTID:0001982";
        skos:prefLabel   "Furanones"@en .

csc:CHEMONTID_0002012
        rdf:type         skos:Concept;
        rdfs:seeAlso     tax_nodes:C0002012;
        skos:definition  "Compounds containing an oxane (tetrahydropyran) ring, which is a six-member saturated aliphatic heterocycle with one oxygen atom and five carbon atoms."@en;
        skos:inScheme    vlcs:chemische_stof;
        skos:notation    "CHEMONTID:0002012";
        skos:prefLabel   "Oxanes"@en .

csc:CHEMONTID_0000402
        rdf:type         skos:Concept;
        rdfs:seeAlso     tax_nodes:C0000402;
        skos:definition  "Organic compounds containing phosphoric acid or a derivative thereof."@en;
        skos:inScheme    vlcs:chemische_stof;
        skos:notation    "CHEMONTID:0000402";
        skos:prefLabel   "Organic phosphoric acids and derivatives"@en .

csc:CHEMONTID_0001614
        rdf:type         skos:Concept;
        rdfs:seeAlso     tax_nodes:C0001614;
        skos:definition  "Compounds with a structure based on the 4-phenylchromene backbone."@en;
        skos:inScheme    vlcs:chemische_stof;
        skos:notation    "CHEMONTID:0001614";
        skos:prefLabel   "Neoflavonoids"@en .

csc:CHEMONTID_0004436
        rdf:type         skos:Concept;
        rdfs:seeAlso     tax_nodes:C0004436;
        skos:definition  "Organometallic compounds hat containing a metal atom substituted by on or more alkyl groups."@en;
        skos:inScheme    vlcs:chemische_stof;
        skos:notation    "CHEMONTID:0004436";
        skos:prefLabel   "Metal alkyls"@en .

csc:CHEMONTID_0002042
        rdf:type         skos:Concept;
        rdfs:seeAlso     tax_nodes:C0002042;
        skos:definition  "Polycyclic aromatic compounds containing a terphenyl skeleton, which consists of a benzene ring substituted with two phenyl groups. Isomers of terphenyl include m-terphenyls (1,3-diphenylbenzenes),  o-terphenyls (1,2-diphenylbenzenes),  p-terphenyls (1,4-diphenylbenzenes)."@en;
        skos:inScheme    vlcs:chemische_stof;
        skos:notation    "CHEMONTID:0002042";
        skos:prefLabel   "Terphenyls"@en .

csc:CHEMONTID_0000432
        rdf:type         skos:Concept;
        rdfs:seeAlso     tax_nodes:C0000432;
        skos:definition  "Inorganic non-metallic compounds in which the largest atom is a nobel gas."@en;
        skos:inScheme    vlcs:chemische_stof;
        skos:notation    "CHEMONTID:0000432";
        skos:prefLabel   "Homogeneous halogens"@en .

csc:CHEMONTID_0004647
        rdf:type         skos:Concept;
        rdfs:seeAlso     tax_nodes:C0004647;
        skos:definition  "Phenols that are unsubstituted at the 4-position."@en;
        skos:inScheme    vlcs:chemische_stof;
        skos:notation    "CHEMONTID:0004647";
        skos:prefLabel   "1-hydroxy-4-unsubstituted benzenoids"@en .

csc:CHEMONTID_0004551
        rdf:type         skos:Concept;
        rdfs:seeAlso     tax_nodes:C0004551;
        skos:definition  "Organofluorine compounds that contain a benzene ring substituted with one or more trifluoromethyl groups."@en;
        skos:inScheme    vlcs:chemische_stof;
        skos:notation    "CHEMONTID:0004551";
        skos:prefLabel   "Trifluoromethylbenzenes"@en .

csc:CHEMONTID_0000462
        rdf:type         skos:Concept;
        rdfs:seeAlso     tax_nodes:C0000462;
        skos:definition  "Organic compounds containing a bond between a carbon atom and metal atom."@en;
        skos:inScheme    vlcs:chemische_stof;
        skos:notation    "CHEMONTID:0000462";
        skos:prefLabel   "Organometallic compounds"@en .

csc:CHEMONTID_0004677
        rdf:type         skos:Concept;
        rdfs:seeAlso     tax_nodes:C0004677;
        skos:definition  "Aromatic compounds hat contain a phenol ether attached to the C2-atom of a phenylpropionic acid ester."@en;
        skos:inScheme    vlcs:chemische_stof;
        skos:notation    "CHEMONTID:0004677";
        skos:prefLabel   "2-phenoxypropionic acid esters"@en .

csc:CHEMONTID_0000305
        rdf:type         skos:Concept;
        rdfs:seeAlso     tax_nodes:C0000305;
        skos:definition  "Compounds containing a pyrazolopyrimidine skeleton, which consists of a pyrazole fused to a pyrimidine. Pyrazole is 5-membered ring consisting of three carbon atoms and two adjacent nitrogen centers. Pyrimidine is 6-membered ring consisting of four carbon atoms and two adjacent nitrogen atoms at the 1- and 3- ring position."@en;
        skos:inScheme    vlcs:chemische_stof;
        skos:notation    "CHEMONTID:0000305";
        skos:prefLabel   "Pyrazolopyrimidines"@en .

csc:CHEMONTID_0000039
        rdf:type         skos:Concept;
        rdfs:seeAlso     tax_nodes:C0000039;
        skos:definition  "Organic compounds containing a sulfamic acid moiety or a derivative, with the general structure R1N(R2)S(=O)2OR3  (R1,R2,R3=H, alkyl, aryl)."@en;
        skos:inScheme    vlcs:chemische_stof;
        skos:notation    "CHEMONTID:0000039";
        skos:prefLabel   "Sulfamic acid derivatives"@en .

csc:CHEMONTID_0001517
        rdf:type         skos:Concept;
        rdfs:seeAlso     tax_nodes:C0001517;
        skos:definition  "Compounds containing a chemical bond between a carbon atom and a fluorine atom."@en;
        skos:inScheme    vlcs:chemische_stof;
        skos:notation    "CHEMONTID:0001517";
        skos:prefLabel   "Organofluorides"@en .

csc:CHEMONTID_0003815
        rdf:type         skos:Concept;
        rdfs:seeAlso     tax_nodes:C0003815;
        skos:definition  "Glycerolipids that carry exactly three acyl chains attached to the glycerol moiety."@en;
        skos:inScheme    vlcs:chemische_stof;
        skos:notation    "CHEMONTID:0003815";
        skos:prefLabel   "Triradylcglycerols"@en .

csc:CHEMONTID_0001813
        rdf:type         skos:Concept;
        rdfs:seeAlso     tax_nodes:C0001813;
        skos:definition  "Compounds containing non-peptidic structural elements that is capable of mimicking or antagonizing the biological action(s) of a natural parent peptide."@en;
        skos:inScheme    vlcs:chemische_stof;
        skos:notation    "CHEMONTID:0001813";
        skos:prefLabel   "Peptidomimetics"@en .

csc:CHEMONTID_0000546
        rdf:type         skos:Concept;
        rdfs:seeAlso     tax_nodes:C0000546;
        skos:definition  "Inorganic compounds containing an oxygen atom of an oxidation state of -2, in which the heaviest atom bonded to the oxygen is an alkaline earth metal."@en;
        skos:inScheme    vlcs:chemische_stof;
        skos:notation    "CHEMONTID:0000546";
        skos:prefLabel   "Alkaline earth metal oxides"@en .

csc:CHEMONTID_0000365
        rdf:type         skos:Concept;
        rdfs:seeAlso     tax_nodes:C0000365;
        skos:definition  "Compounds containing a cyclohexylsulfamic acid moiety."@en;
        skos:inScheme    vlcs:chemische_stof;
        skos:notation    "CHEMONTID:0000365";
        skos:prefLabel   "Cyclamates"@en .

csc:CHEMONTID_0000099
        rdf:type         skos:Concept;
        rdfs:seeAlso     tax_nodes:C0000099;
        skos:definition  "Compounds containing  a five-member aromatic ring of two carbon atoms and three nitrogen atoms."@en;
        skos:inScheme    vlcs:chemische_stof;
        skos:notation    "CHEMONTID:0000099";
        skos:prefLabel   "Triazoles"@en .

csc:CHEMONTID_0004665
        rdf:type         skos:Concept;
        rdfs:seeAlso     tax_nodes:C0004665;
        skos:definition  "Organooxygen compounds containing a O,S-diester derivative of phosphoroamidothioic acid. They have the general structure RSP(=O)(OR')(NH2), where R,R' are organyl groups."@en;
        skos:inScheme    vlcs:chemische_stof;
        skos:notation    "CHEMONTID:0004665";
        skos:prefLabel   "Phosphoramidothioic-acid-O,S-diesters"@en .

list:superclass  rdf:type  rdf:List;
        rdf:first       cscl:superclass;
        rdf:rest        list:class;
        skos:prefLabel  "Niveau superklasse"@nl .

csc:CHEMONTID_0001270
        rdf:type         skos:Concept;
        rdfs:seeAlso     tax_nodes:C0001270;
        skos:definition  "Inorganic compounds containing non-metal as well as metal atoms but not belonging to afore mentioned classes."@en;
        skos:inScheme    vlcs:chemische_stof;
        skos:notation    "CHEMONTID:0001270";
        skos:prefLabel   "Miscellaneous mixed metal/non-metals"@en .

csc:CHEMONTID_0001209
        rdf:type         skos:Concept;
        rdfs:seeAlso     tax_nodes:C0001209;
        skos:definition  "Organic compounds containing the thiourea functional group, a derivative of urea with the general structure (R1(N)R2C(=S)(R3)R4, R1-R4=H, alkyl, aryl), obtained by replacing the carbonyl group of urea with a thiocarbonyl group."@en;
        skos:inScheme    vlcs:chemische_stof;
        skos:notation    "CHEMONTID:0001209";
        skos:prefLabel   "Thioureas"@en .

csc:CHEMONTID_0000395
        rdf:type         skos:Concept;
        rdfs:seeAlso     tax_nodes:C0000395;
        skos:definition  "Organic compounds containing the nitrate oxoanion, with the formula NO3-."@en;
        skos:inScheme    vlcs:chemische_stof;
        skos:notation    "CHEMONTID:0000395";
        skos:prefLabel   "Organic nitrates"@en .

csc:CHEMONTID_0001396
        rdf:type         skos:Concept;
        rdfs:seeAlso     tax_nodes:C0001396;
        skos:definition  "Organic compounds containing a benzene fused to an oxazine ring (a six-membered aliphatic ring with four carbon atoms, one oxygen atom, and one nitrogen atom)."@en;
        skos:inScheme    vlcs:chemische_stof;
        skos:notation    "CHEMONTID:0001396";
        skos:prefLabel   "Benzoxazines"@en .

csc:CHEMONTID_0004484
        rdf:type         skos:Concept;
        rdfs:seeAlso     tax_nodes:C0004484;
        skos:definition  "Organic compounds containing a phosphorous acid, which is tri-esterified with alkyl groups."@en;
        skos:inScheme    vlcs:chemische_stof;
        skos:notation    "CHEMONTID:0004484";
        skos:prefLabel   "Trialkylphosphites"@en .

csc:CHEMONTID_0000480
        rdf:type         skos:Concept;
        rdfs:seeAlso     tax_nodes:C0000480;
        skos:definition  "Compounds comprising a pyrimidine base attached to a ribosyl or deoxyribosyl moiety."@en;
        skos:inScheme    vlcs:chemische_stof;
        skos:notation    "CHEMONTID:0000480";
        skos:prefLabel   "Pyrimidine nucleosides"@en .

csc:CHEMONTID_0000419
        rdf:type         skos:Concept;
        rdfs:seeAlso     tax_nodes:C0000419;
        skos:definition  "Organic compounds containing phosphonic acid or a derivative thereof."@en;
        skos:inScheme    vlcs:chemische_stof;
        skos:notation    "CHEMONTID:0000419";
        skos:prefLabel   "Organic phosphonic acids and derivatives"@en .

csc:CHEMONTID_0000027
        rdf:type         skos:Concept;
        rdfs:seeAlso     tax_nodes:C0000027;
        skos:definition  "Compounds containing an indane moiety, which consists of a cyclopentane fused to a benzene ring."@en;
        skos:inScheme    vlcs:chemische_stof;
        skos:notation    "CHEMONTID:0000027";
        skos:prefLabel   "Indanes"@en .

csc:CHEMONTID_0002506
        rdf:type         skos:Concept;
        rdfs:seeAlso     tax_nodes:C0002506;
        skos:definition  "Natural products derived from 3-phenylchromen-4-one."@en;
        skos:inScheme    vlcs:chemische_stof;
        skos:notation    "CHEMONTID:0002506";
        skos:prefLabel   "Isoflavonoids"@en .

csc:CHEMONTID_0000504
        rdf:type         skos:Concept;
        rdfs:seeAlso     tax_nodes:C0000504;
        skos:definition  "Derivatives of lineolic acid. Lineolic acid is a polyunsaturated omega-6 18 carbon long fatty acid, with two CC double bonds at the 9- and 12-positions."@en;
        skos:inScheme    vlcs:chemische_stof;
        skos:notation    "CHEMONTID:0000504";
        skos:prefLabel   "Lineolic acids and derivatives"@en .

csc:CHEMONTID_0000112
        rdf:type         skos:Concept;
        rdfs:seeAlso     tax_nodes:C0000112;
        skos:definition  "Compounds comprising the hydrazine functional group, with the general formula R1R2NNR3R4."@en;
        skos:inScheme    vlcs:chemische_stof;
        skos:notation    "CHEMONTID:0000112";
        skos:prefLabel   "Hydrazines and derivatives"@en .

csc:CHEMONTID_0002693
        rdf:type         skos:Concept;
        rdfs:seeAlso     tax_nodes:C0002693;
        skos:definition  "Compounds containing a triazinane ring, which is a six-membered saturated heterocycle with  three nitrogen ring atoms and three ring carbon atoms."@en;
        skos:inScheme    vlcs:chemische_stof;
        skos:notation    "CHEMONTID:0002693";
        skos:prefLabel   "Triazinanes"@en .

csc:CHEMONTID_0000238
        rdf:type         skos:Concept;
        rdfs:seeAlso     tax_nodes:C0000238;
        skos:definition  "Naturally occurring polyphenols which be categorized into four main classes: hydrolyzable tannin (based on ellagic acid or gallic acid), condensed tannins (made of oligomeric or polymeric proanthocyanidins), complex tannins (made of a catechin bound to a gallotannin or elagitannin), and phlorotannins (oligomers of phloroglucinol)."@en;
        skos:inScheme    vlcs:chemische_stof;
        skos:notation    "CHEMONTID:0000238";
        skos:prefLabel   "Tannins"@en .

csc:CHEMONTID_0004201
        rdf:type         skos:Concept;
        rdfs:seeAlso     tax_nodes:C0004201;
        skos:definition  "Compound containing a triazole ring fused to the benzene or the thiazole moiety of the benzothiazole ring system."@en;
        skos:inScheme    vlcs:chemische_stof;
        skos:notation    "CHEMONTID:0004201";
        skos:prefLabel   "Triazolobenzothiazoles"@en .

csc:CHEMONTID_0000323
        rdf:type         skos:Concept;
        rdfs:seeAlso     tax_nodes:C0000323;
        skos:definition  "Organic compounds containing a bond between a carbon atom and an oxygen atom."@en;
        skos:inScheme    vlcs:chemische_stof;
        skos:notation    "CHEMONTID:0000323";
        skos:prefLabel   "Organooxygen compounds"@en .

csc:CHEMONTID_0003411
        rdf:type         skos:Concept;
        rdfs:seeAlso     tax_nodes:C0003411;
        skos:definition  "Organic aromatic compounds that 1-benzopyran, a bicyclic compound made up of a benzene ring fused to a pyran, so that the oxygen atom is at the 2-position."@en;
        skos:inScheme    vlcs:chemische_stof;
        skos:notation    "CHEMONTID:0003411";
        skos:prefLabel   "2-benzopyrans"@en .

csc:CHEMONTID_0000534
        rdf:type         skos:Concept;
        rdfs:seeAlso     tax_nodes:C0000534;
        skos:definition  "Inorganic compounds containing an oxygen atom of an oxidation state of -2, in which the heaviest atom bonded to the oxygen is a metalloid."@en;
        skos:inScheme    vlcs:chemische_stof;
        skos:notation    "CHEMONTID:0000534";
        skos:prefLabel   "Metalloid oxides"@en .

csc:CHEMONTID_0001831
        rdf:type         skos:Concept;
        rdfs:seeAlso     tax_nodes:C0001831;
        skos:definition  "Organic compounds containing a carbonyl group, with the general structure RC(=O)R', where R=organyl, R'=H, N, O, organyl group or halide group."@en;
        skos:inScheme    vlcs:chemische_stof;
        skos:notation    "CHEMONTID:0001831";
        skos:prefLabel   "Carbonyl compounds"@en .

csc:CHEMONTID_0003567
        rdf:type         skos:Concept;
        rdfs:seeAlso     tax_nodes:C0003567;
        skos:definition  "Steroids with a structure based on the ergostane skeleton, which arises from the methylation of cholestane at the 24-position."@en;
        skos:inScheme    vlcs:chemische_stof;
        skos:notation    "CHEMONTID:0003567";
        skos:prefLabel   "Ergostane steroids"@en .

csc:CHEMONTID_0000087
        rdf:type         skos:Concept;
        rdfs:seeAlso     tax_nodes:C0000087;
        skos:definition  "Compounds containing a pyrazole ring, which is a five-member aromatic ring with two nitrogen atoms (at positions 1 and 2) and three carbon atoms."@en;
        skos:inScheme    vlcs:chemische_stof;
        skos:notation    "CHEMONTID:0000087";
        skos:prefLabel   "Pyrazoles"@en .

csc:CHEMONTID_0002566
        rdf:type         skos:Concept;
        rdfs:seeAlso     tax_nodes:C0002566;
        skos:definition  "Aromatic polycyclic compounds containing an isoquinoline moiety, which consists of a benzene ring fused to a pyridine ring and forming benzo[c]pyridine."@en;
        skos:inScheme    vlcs:chemische_stof;
        skos:notation    "CHEMONTID:0002566";
        skos:prefLabel   "Isoquinolines and derivatives"@en .

csc:CHEMONTID_0002651
        rdf:type         skos:Concept;
        rdfs:seeAlso     tax_nodes:C0002651;
        skos:definition  "Diarylheptanoids with an open heptane chain. The two aromatic rings are linked only by the heptane chain."@en;
        skos:inScheme    vlcs:chemische_stof;
        skos:notation    "CHEMONTID:0002651";
        skos:prefLabel   "Linear diarylheptanoids"@en .

csc:CHEMONTID_0003260
        rdf:type         skos:Concept;
        rdfs:seeAlso     tax_nodes:C0003260;
        skos:definition  "Organosulfur compounds a sulfenyl group with the general formula RS (R = organyl)."@en;
        skos:inScheme    vlcs:chemische_stof;
        skos:notation    "CHEMONTID:0003260";
        skos:prefLabel   "Sulfenyl compounds"@en .

csc:CHEMONTID_0000298
        rdf:type         skos:Concept;
        rdfs:seeAlso     tax_nodes:C0000298;
        skos:definition  "Long chain aldehydes with a chain of at least 12 carbon atoms."@en;
        skos:inScheme    vlcs:chemische_stof;
        skos:notation    "CHEMONTID:0000298";
        skos:prefLabel   "Fatty aldehydes"@en .

csc:CHEMONTID_0004387
        rdf:type         skos:Concept;
        rdfs:seeAlso     tax_nodes:C0004387;
        skos:definition  "Aromatic heterocyclic compounds containing a pyrazolo[3,4-d]pyrimidine ring system, which consists of a pyrazole ring fused to but and not sharing a nitrogen atom with a pyrimidine ring."@en;
        skos:inScheme    vlcs:chemische_stof;
        skos:notation    "CHEMONTID:0004387";
        skos:prefLabel   "Pyrazolo[3,4-d]pyrimidines"@en .

csc:CHEMONTID_0001861
        rdf:type         skos:Concept;
        rdfs:seeAlso     tax_nodes:C0001861;
        skos:definition  "Heterocyclic compounds containing a pyridine ring substituted by one or more sulfonamide groups."@en;
        skos:inScheme    vlcs:chemische_stof;
        skos:notation    "CHEMONTID:0001861";
        skos:prefLabel   "Pyridinesulfonamides"@en .

csc:CHEMONTID_0003597
        rdf:type         skos:Concept;
        rdfs:seeAlso     tax_nodes:C0003597;
        skos:definition  "Organic aromatic compounds that contain a naphthalene moiety that carries a sulfonic acid group (or a derivative thereof) at one or more positions. Naphthalene is a bicyclic compound that is made up of two fused benzene ring."@en;
        skos:inScheme    vlcs:chemische_stof;
        skos:notation    "CHEMONTID:0003597";
        skos:prefLabel   "Naphthalene sulfonic acids and derivatives"@en .

csc:CHEMONTID_0001987
        rdf:type         skos:Concept;
        rdfs:seeAlso     tax_nodes:C0001987;
        skos:definition  "Organic polycyclic compounds containing an isosorbide(1,4-Dianhydrosorbitol) moiety, which consists of two -oxolan-3-ol rings."@en;
        skos:inScheme    vlcs:chemische_stof;
        skos:notation    "CHEMONTID:0001987";
        skos:prefLabel   "Isosorbides"@en .

csc:CHEMONTID_0002017
        rdf:type         skos:Concept;
        rdfs:seeAlso     tax_nodes:C0002017;
        skos:definition  "Compounds containing a thiophene ring which bears a carboxylic acid group (or a salt/ester thereof)."@en;
        skos:inScheme    vlcs:chemische_stof;
        skos:notation    "CHEMONTID:0002017";
        skos:prefLabel   "Thiophene carboxylic acids and derivatives"@en .

csc:CHEMONTID_0001016
        rdf:type         skos:Concept;
        rdfs:seeAlso     tax_nodes:C0001016;
        skos:definition  "Saturated monocyclic hydrocarbons (with or without side chains)."@en;
        skos:inScheme    vlcs:chemische_stof;
        skos:notation    "CHEMONTID:0001016";
        skos:prefLabel   "Cycloalkanes"@en .

csc:CHEMONTID_0000015
        rdf:type         skos:Concept;
        rdfs:seeAlso     tax_nodes:C0000015;
        skos:definition  "Compounds containing a dibenzofuran moiety, which consists of two benzene rings fused to a central furan ring."@en;
        skos:inScheme    vlcs:chemische_stof;
        skos:notation    "CHEMONTID:0000015";
        skos:prefLabel   "Dibenzofurans"@en .

csc:CHEMONTID_0004707
        rdf:type         skos:Concept;
        rdfs:seeAlso     tax_nodes:C0004707;
        skos:definition  "Organic compounds containing a nitrogen atom."@en;
        skos:inScheme    vlcs:chemische_stof;
        skos:notation    "CHEMONTID:0004707";
        skos:prefLabel   "Organic nitrogen compounds"@en .

csc:CHEMONTID_0003893
        rdf:type         skos:Concept;
        rdfs:seeAlso     tax_nodes:C0003893;
        skos:definition  "Organophosphorus compounds containing a diester derivative of phosphonic acid, with the general structure ROP(=O)OR' (R,R' = organyl group)."@en;
        skos:inScheme    vlcs:chemische_stof;
        skos:notation    "CHEMONTID:0003893";
        skos:prefLabel   "Phosphonic acid diesters"@en .

csc:CHEMONTID_0000226
        rdf:type         skos:Concept;
        rdfs:seeAlso     tax_nodes:C0000226;
        skos:definition  "Heterocyclic compounds containing a five-member saturated aliphatic ring with one nitrogen atom, one sulfur atom, three carbon atoms."@en;
        skos:inScheme    vlcs:chemische_stof;
        skos:notation    "CHEMONTID:0000226";
        skos:prefLabel   "Thiazolidines"@en .

csc:CHEMONTID_0001891
        rdf:type         skos:Concept;
        rdfs:seeAlso     tax_nodes:C0001891;
        skos:definition  "Polycyclic aromatic compounds containing a sulfinyl group attached at the position 2 of a benzimidazole moiety."@en;
        skos:inScheme    vlcs:chemische_stof;
        skos:notation    "CHEMONTID:0001891";
        skos:prefLabel   "Sulfinylbenzimidazoles"@en .

csc:CHEMONTID_0000311
        rdf:type         skos:Concept;
        rdfs:seeAlso     tax_nodes:C0000311;
        skos:definition  "Organic compounds containing a benzene fused to a thiazole ring (a five-membered ring with four carbon atoms, one nitrogen atom and one sulfur atom)."@en;
        skos:inScheme    vlcs:chemische_stof;
        skos:notation    "CHEMONTID:0000311";
        skos:prefLabel   "Benzothiazoles"@en .

csc:CHEMONTID_0001438
        rdf:type         skos:Concept;
        rdfs:seeAlso     tax_nodes:C0001438;
        skos:definition  "Organic derivatives of thiophosphonic acid, thiophosphoric acid, dithiophosphoric acid, or phosphorotrithioic acid, or derivatives thereof. Thiophosphonic acid, dithiophosphoric acid, thiophosphoric acid, and phosphorotrithioic acid are thiophosphorus compounds with the formula OP(O)(=S), OP(S)(=S)O, OP(O)(=S)O, and OP(=S)(S)S, respectively."@en;
        skos:inScheme    vlcs:chemische_stof;
        skos:notation    "CHEMONTID:0001438";
        skos:prefLabel   "Organothiophosphorus compounds"@en .

csc:CHEMONTID_0000437
        rdf:type         skos:Concept;
        rdfs:seeAlso     tax_nodes:C0000437;
        skos:definition  "Inorganic compounds containing 'other non-metals' and halogen."@en;
        skos:inScheme    vlcs:chemische_stof;
        skos:notation    "CHEMONTID:0000437";
        skos:prefLabel   "Other non-metal halides"@en .

csc:CHEMONTID_0000045
        rdf:type         skos:Concept;
        rdfs:seeAlso     tax_nodes:C0000045;
        skos:definition  "Compounds containing a phenylpropene moiety, which consists of a propene substituent bound to a phenyl group."@en;
        skos:inScheme    vlcs:chemische_stof;
        skos:notation    "CHEMONTID:0000045";
        skos:prefLabel   "Phenylpropenes"@en .

csc:CHEMONTID_0001523
        rdf:type         skos:Concept;
        rdfs:seeAlso     tax_nodes:C0001523;
        skos:definition  "Organic compounds containing a post-transition metal atom."@en;
        skos:inScheme    vlcs:chemische_stof;
        skos:notation    "CHEMONTID:0001523";
        skos:prefLabel   "Organo-post-transition metal compounds"@en .

csc:CHEMONTID_0000522
        rdf:type         skos:Concept;
        rdfs:seeAlso     tax_nodes:C0000522;
        skos:definition  "Inorganic compounds containing an oxygen atom of an oxidation state of -2, in which the heaviest atom bonded to the oxygen is an actinide."@en;
        skos:inScheme    vlcs:chemische_stof;
        skos:notation    "CHEMONTID:0000522";
        skos:prefLabel   "Actinide oxides"@en .

csc:CHEMONTID_0000130
        rdf:type         skos:Concept;
        rdfs:seeAlso     tax_nodes:C0000130;
        skos:definition  "Organic compounds containing a spirodecane moiety with at least one nitrogen atom."@en;
        skos:inScheme    vlcs:chemische_stof;
        skos:notation    "CHEMONTID:0000130";
        skos:prefLabel   "Azaspirodecane derivatives"@en .

csc:CHEMONTID_0002132
        rdf:type         skos:Concept;
        rdfs:seeAlso     tax_nodes:C0002132;
        skos:definition  "Compounds containing a dithioacetal functional group with the general structure R2C(SR')2."@en;
        skos:inScheme    vlcs:chemische_stof;
        skos:notation    "CHEMONTID:0002132";
        skos:prefLabel   "Dithioacetals"@en .

csc:CHEMONTID_0004164
        rdf:type         skos:Concept;
        rdfs:seeAlso     tax_nodes:C0004164;
        skos:definition  "O-ester derivatives of dithiophosphates, with the general structure RSP(O)(O)=S (R = organyl group)."@en;
        skos:inScheme    vlcs:chemische_stof;
        skos:notation    "CHEMONTID:0004164";
        skos:prefLabel   "Dithiophosphate O-esters"@en .

csc:CHEMONTID_0000075
        rdf:type         skos:Concept;
        rdfs:seeAlso     tax_nodes:C0000075;
        skos:definition  "Compounds containing a pyrimidne ring, which is a six-member aromatic heterocycle which consists of two nitrogen atoms (at positions 1 and 3) and four carbon atoms."@en;
        skos:inScheme    vlcs:chemische_stof;
        skos:notation    "CHEMONTID:0000075";
        skos:prefLabel   "Pyrimidines and pyrimidine derivatives"@en .

csc:CHEMONTID_0001553
        rdf:type         skos:Concept;
        rdfs:seeAlso     tax_nodes:C0001553;
        skos:definition  "Terpene molecules containing six isoprene units."@en;
        skos:inScheme    vlcs:chemische_stof;
        skos:notation    "CHEMONTID:0001553";
        skos:prefLabel   "Triterpenoids"@en .

csc:CHEMONTID_0000552
        rdf:type         skos:Concept;
        rdfs:seeAlso     tax_nodes:C0000552;
        skos:definition  "Inorganic compounds in which the heaviest atom bonded to a hydrogen atom is belongs to the class of 'other non-metals'."@en;
        skos:inScheme    vlcs:chemische_stof;
        skos:notation    "CHEMONTID:0000552";
        skos:prefLabel   "Other non-metal hydrides"@en .

csc:CHEMONTID_0000160
        rdf:type         skos:Concept;
        rdfs:seeAlso     tax_nodes:C0000160;
        skos:definition  "Compounds containing a lactam ring, which is a cyclic amide of amino carboxylic acids, having a 1-azacycloalkan-2-one structure (or an analogue having unsaturation or heteroatoms replacing one or more carbon atoms of the ring)."@en;
        skos:inScheme    vlcs:chemische_stof;
        skos:notation    "CHEMONTID:0000160";
        skos:prefLabel   "Lactams"@en .

csc:CHEMONTID_0001764
        rdf:type         skos:Concept;
        rdfs:seeAlso     tax_nodes:C0001764;
        skos:definition  "Compounds containing a pyridinium ring, which is the cationic form of pyridine."@en;
        skos:inScheme    vlcs:chemische_stof;
        skos:notation    "CHEMONTID:0001764";
        skos:prefLabel   "Pyridinium derivatives"@en .

csc:CHEMONTID_0001975
        rdf:type         skos:Concept;
        rdfs:seeAlso     tax_nodes:C0001975;
        skos:definition  "Compounds containing a pyrrolidinylpyridine ring system, which consists of a pyrrolidine ring linked to a pyridine ring."@en;
        skos:inScheme    vlcs:chemische_stof;
        skos:notation    "CHEMONTID:0001975";
        skos:prefLabel   "Pyrrolidinylpyridines"@en .

csc:CHEMONTID_0000190
        rdf:type         skos:Concept;
        rdfs:seeAlso     tax_nodes:C0000190;
        skos:definition  "Compounds containing a methoxy group attached to the benzene ring of a phenol moiety."@en;
        skos:inScheme    vlcs:chemische_stof;
        skos:notation    "CHEMONTID:0000190";
        skos:prefLabel   "Methoxyphenols"@en .

csc:CHEMONTID_0000129
        rdf:type         skos:Concept;
        rdfs:seeAlso     tax_nodes:C0000129;
        skos:definition  "Organic compounds in which at least one hydroxyl functional group (-OH) is bound to a carbon atom, usually connected to other carbon or hydrogen atoms."@en;
        skos:inScheme    vlcs:chemische_stof;
        skos:notation    "CHEMONTID:0000129";
        skos:prefLabel   "Alcohols and polyols"@en .

csc:CHEMONTID_0001607
        rdf:type         skos:Concept;
        rdfs:seeAlso     tax_nodes:C0001607;
        skos:definition  "Phenolic compounds containing a cis-fused tetrahydrochromeno[3,4-b]chromene nucleus. Many rotenoids contain an additional ring, e.g. rotenone. They are isoflavonoids characterized by the presence of an extra carbon atom in an additional heterocyclic ring."@en;
        skos:inScheme    vlcs:chemische_stof;
        skos:notation    "CHEMONTID:0001607";
        skos:prefLabel   "Rotenoids"@en .

csc:CHEMONTID_0002608
        rdf:type         skos:Concept;
        rdfs:seeAlso     tax_nodes:C0002608;
        skos:definition  "Alcohols substituted by a chlorine atom at a saturated carbon atom otherwise bearing only hydrogen or hydrocarbyl groups."@en;
        skos:inScheme    vlcs:chemische_stof;
        skos:notation    "CHEMONTID:0002608";
        skos:prefLabel   "Chlorohydrins"@en .

csc:CHEMONTID_0000425
        rdf:type         skos:Concept;
        rdfs:seeAlso     tax_nodes:C0000425;
        skos:definition  "Inorganic compounds containing only metal atoms,with the largest atom being a alkali metal atom."@en;
        skos:inScheme    vlcs:chemische_stof;
        skos:notation    "CHEMONTID:0000425";
        skos:prefLabel   "Homogeneous alkali metal compounds"@en .

csc:CHEMONTID_0000033
        rdf:type         skos:Concept;
        rdfs:seeAlso     tax_nodes:C0000033;
        skos:definition  "Organic compounds containing the phenylmethanol substructure."@en;
        skos:inScheme    vlcs:chemische_stof;
        skos:notation    "CHEMONTID:0000033";
        skos:prefLabel   "Benzyl alcohols"@en .

csc:CHEMONTID_0000159
        rdf:type         skos:Concept;
        rdfs:seeAlso     tax_nodes:C0000159;
        skos:definition  "Compounds containing a cyclic ether with three ring atoms(one oxygen and two carbon atoms)."@en;
        skos:inScheme    vlcs:chemische_stof;
        skos:notation    "CHEMONTID:0000159";
        skos:prefLabel   "Epoxides"@en .

csc:CHEMONTID_0000510
        rdf:type         skos:Concept;
        rdfs:seeAlso     tax_nodes:C0000510;
        skos:definition  "Organic compounds containing the functional group with the general structure R-CS-NR'R, where R, R', and R are organic groups."@en;
        skos:inScheme    vlcs:chemische_stof;
        skos:notation    "CHEMONTID:0000510";
        skos:prefLabel   "Thioamides"@en .

csc:CHEMONTID_0001245
        rdf:type         skos:Concept;
        rdfs:seeAlso     tax_nodes:C0001245;
        skos:definition  "Compounds containing a gamma butyrolactone moiety, which consists of an aliphatic five-member ring with four carbon atoms, one oxygen atom, and bears a ketone group on the carbon adjacent to the oxygen atom."@en;
        skos:inScheme    vlcs:chemische_stof;
        skos:notation    "CHEMONTID:0001245";
        skos:prefLabel   "Gamma butyrolactones"@en .

csc:CHEMONTID_0001722
        rdf:type         skos:Concept;
        rdfs:seeAlso     tax_nodes:C0001722;
        skos:definition  "Ester derivatives of a fatty alcohol."@en;
        skos:inScheme    vlcs:chemische_stof;
        skos:notation    "CHEMONTID:0001722";
        skos:prefLabel   "Fatty alcohol esters"@en .

csc:CHEMONTID_0000455
        rdf:type         skos:Concept;
        rdfs:seeAlso     tax_nodes:C0000455;
        skos:definition  "Organic compounds belonging to either the actinide hydrides, actinide nitrides, actinide oxides, or actinide sulfides."@en;
        skos:inScheme    vlcs:chemische_stof;
        skos:notation    "CHEMONTID:0000455";
        skos:prefLabel   "Actinide organides"@en .

csc:CHEMONTID_0002542
        rdf:type         skos:Concept;
        rdfs:seeAlso     tax_nodes:C0002542;
        skos:definition  "Aromatic ethers with the general formula ROCR' (R = alkyl, aryl; R'=benzene)."@en;
        skos:inScheme    vlcs:chemische_stof;
        skos:notation    "CHEMONTID:0002542";
        skos:prefLabel   "Benzylethers"@en .

csc:CHEMONTID_0004152
        rdf:type         skos:Concept;
        rdfs:seeAlso     tax_nodes:C0004152;
        skos:definition  "Organic compounds containing a pyridine ring substituted at one or more positions by a methyl group."@en;
        skos:inScheme    vlcs:chemische_stof;
        skos:notation    "CHEMONTID:0004152";
        skos:prefLabel   "Methylpyridines"@en .

csc:CHEMONTID_0000189
        rdf:type         skos:Concept;
        rdfs:seeAlso     tax_nodes:C0000189;
        skos:definition  "Compounds containing a piperazine ring, which is a saturated aliphatic six-member heterocyclic with two nitrogen atoms at positions 1 and 4, as well as four carbon atoms."@en;
        skos:inScheme    vlcs:chemische_stof;
        skos:notation    "CHEMONTID:0000189";
        skos:prefLabel   "Piperazines"@en .

csc:CHEMONTID_0004097
        rdf:type         skos:Concept;
        rdfs:seeAlso     tax_nodes:C0004097;
        skos:definition  "Organic compounds containing a benzene ring fused to a 1,4-azepine."@en;
        skos:inScheme    vlcs:chemische_stof;
        skos:notation    "CHEMONTID:0004097";
        skos:prefLabel   "1,4-benzodiazepines"@en .

csc:CHEMONTID_0000093
        rdf:type         skos:Concept;
        rdfs:seeAlso     tax_nodes:C0000093;
        skos:definition  "Cyclic organic compounds containing a thiadiazole ring, which is a five-membered aromatic heterocycle made up of one sulfur atom and two nitrogen atoms."@en;
        skos:inScheme    vlcs:chemische_stof;
        skos:notation    "CHEMONTID:0000093";
        skos:prefLabel   "Thiadiazoles"@en .

csc:CHEMONTID_0002180
        rdf:type         skos:Concept;
        rdfs:seeAlso     tax_nodes:C0002180;
        skos:definition  "Compounds consisting of a pyrimidine linked to a ribose which lacks a hydroxyl group at position 2."@en;
        skos:inScheme    vlcs:chemische_stof;
        skos:notation    "CHEMONTID:0002180";
        skos:prefLabel   "Pyrimidine 2'-deoxyribonucleosides"@en .

csc:CHEMONTID_0004785
        rdf:type         skos:Concept;
        rdfs:seeAlso     tax_nodes:C0004785;
        skos:definition  "Stilbenes that carry a sulfone group at one or more positions of either benzene rings."@en;
        skos:inScheme    vlcs:chemische_stof;
        skos:notation    "CHEMONTID:0004785";
        skos:prefLabel   "Sulfonated stilbenes"@en .

csc:CHEMONTID_0003808
        rdf:type         skos:Concept;
        rdfs:seeAlso     tax_nodes:C0003808;
        skos:definition  "Glycerolipids that carry exactly one acyl chain attached to the glycerol moiety."@en;
        skos:inScheme    vlcs:chemische_stof;
        skos:notation    "CHEMONTID:0003808";
        skos:prefLabel   "Monoradylglycerols"@en .

csc:CHEMONTID_0004502
        rdf:type         skos:Concept;
        rdfs:seeAlso     tax_nodes:C0004502;
        skos:definition  "Nucleosides in which the oxygen atom at the 5'position of the ribose moiety has been replaced by another atom. The nucleobases here are limited to purine, pyrimidine, and pyridine derivatives."@en;
        skos:inScheme    vlcs:chemische_stof;
        skos:notation    "CHEMONTID:0004502";
        skos:prefLabel   "5'-deoxyribonucleosides"@en .

csc:CHEMONTID_0001022
        rdf:type         skos:Concept;
        rdfs:seeAlso     tax_nodes:C0001022;
        skos:definition  "Organic compounds containing the functional group -CO-Cl."@en;
        skos:inScheme    vlcs:chemische_stof;
        skos:notation    "CHEMONTID:0001022";
        skos:prefLabel   "Acyl chlorides"@en .

csc:CHEMONTID_0000021
        rdf:type         skos:Concept;
        rdfs:seeAlso     tax_nodes:C0000021;
        skos:definition  "Compounds containing an indene moiety(which consists of a cyclopentadiene fused to a benzene ring), or a isoindene moiety (which consists of a cyclopentadiene fused to cyclohexadiene ring)."@en;
        skos:inScheme    vlcs:chemische_stof;
        skos:notation    "CHEMONTID:0000021";
        skos:prefLabel   "Indenes and isoindenes"@en .

csc:CHEMONTID_0002500
        rdf:type         skos:Concept;
        rdfs:seeAlso     tax_nodes:C0002500;
        skos:definition  "Acyclic branched or unbranched hydrocarbons having the general formula CnH2n+2 , and therefore consisting entirely of hydrogen atoms and saturated carbon atoms."@en;
        skos:inScheme    vlcs:chemische_stof;
        skos:notation    "CHEMONTID:0002500";
        skos:prefLabel   "Alkanes"@en .

csc:CHEMONTID_0000147
        rdf:type         skos:Concept;
        rdfs:seeAlso     tax_nodes:C0000147;
        skos:definition  "Organic compounds containing a lactone ring of at least twelve members."@en;
        skos:inScheme    vlcs:chemische_stof;
        skos:notation    "CHEMONTID:0000147";
        skos:prefLabel   "Macrolides and analogues"@en .

csc:CHEMONTID_0004628
        rdf:type         skos:Concept;
        rdfs:seeAlso     tax_nodes:C0004628;
        skos:definition  "Phenols that carry an alkoxy group at the 4-position of the benzene ring."@en;
        skos:inScheme    vlcs:chemische_stof;
        skos:notation    "CHEMONTID:0004628";
        skos:prefLabel   "4-alkoxyphenols"@en .

csc:CHEMONTID_0001359
        rdf:type         skos:Concept;
        rdfs:seeAlso     tax_nodes:C0001359;
        skos:definition  "Organic compounds containing a carboxylic acid substituted with a hydroxyl group on the adjacent carbon."@en;
        skos:inScheme    vlcs:chemische_stof;
        skos:notation    "CHEMONTID:0001359";
        skos:prefLabel   "Alpha hydroxy acids and derivatives"@en .

csc:CHEMONTID_0001710
        rdf:type         skos:Concept;
        rdfs:seeAlso     tax_nodes:C0001710;
        skos:definition  "Tannins with a structure characterized by either of the following models. In model 1, the structure contains galloyl units (in some cases, shikimic acid units) are linked to diverse polyol carbohydrate-, catechin-, or triterpenoid units. In model 2, contains at least two galloyl units C-C coupled to each other, and do not contain a glycosidically linked catechin unit."@en;
        skos:inScheme    vlcs:chemische_stof;
        skos:notation    "CHEMONTID:0001710";
        skos:prefLabel   "Hydrolyzable tannins"@en .

csc:CHEMONTID_0002445
        rdf:type         skos:Concept;
        rdfs:seeAlso     tax_nodes:C0002445;
        skos:definition  "Organic acids with the general formula OOC(R)=O (R = H, organyl group)."@en;
        skos:inScheme    vlcs:chemische_stof;
        skos:notation    "CHEMONTID:0002445";
        skos:prefLabel   "Peroxycarboxylic acids and derivatives"@en .

csc:CHEMONTID_0002837
        rdf:type         skos:Concept;
        rdfs:seeAlso     tax_nodes:C0002837;
        skos:definition  "Organic compounds made up only of carbon and hydrogen atoms."@en;
        skos:inScheme    vlcs:chemische_stof;
        skos:notation    "CHEMONTID:0002837";
        skos:prefLabel   "Hydrocarbons"@en .

csc:CHEMONTID_0000262
        rdf:type         skos:Concept;
        rdfs:seeAlso     tax_nodes:C0000262;
        skos:definition  "Aliphatic monocarboxylic acids with a saturated or unsaturated aliphatic tail (with at least 4 Carbon atoms)."@en;
        skos:inScheme    vlcs:chemische_stof;
        skos:notation    "CHEMONTID:0000262";
        skos:prefLabel   "Fatty acids and conjugates"@en .

csc:CHEMONTID_0004477
        rdf:type         skos:Concept;
        rdfs:seeAlso     tax_nodes:C0004477;
        skos:definition  "Aromatic compounds that are made up of carbon and hydrogen atoms only."@en;
        skos:inScheme    vlcs:chemische_stof;
        skos:notation    "CHEMONTID:0004477";
        skos:prefLabel   "Aromatic hydrocarbons"@en .

csc:CHEMONTID_0002867
        rdf:type         skos:Concept;
        rdfs:seeAlso     tax_nodes:C0002867;
        skos:definition  "Organic compounds containing a linear aliphatic chain (or ring system) carrying a C-X bond, where X is a halogen atom."@en;
        skos:inScheme    vlcs:chemische_stof;
        skos:notation    "CHEMONTID:0002867";
        skos:prefLabel   "Alkyl halides"@en .

csc:CHEMONTID_0003953
        rdf:type         skos:Concept;
        rdfs:seeAlso     tax_nodes:C0003953;
        skos:definition  "Compounds containing a quinoline moiety, which carries a hydroxy group at the 8-position. Quinoline consists of a benzene ring fused to a pyrimidine ring to form benzo[b]azabenzene."@en;
        skos:inScheme    vlcs:chemische_stof;
        skos:notation    "CHEMONTID:0003953";
        skos:prefLabel   "8-hydroxyquinolines"@en .

csc:CHEMONTID_0000081
        rdf:type         skos:Concept;
        rdfs:seeAlso     tax_nodes:C0000081;
        skos:definition  "Heterocyclic organic compounds containing an isoxazole moiety, with a structure characterized by a five-member aromatic ring with one oxygen atom and one nitrogen atom at ring positions 1 and 2, respectively."@en;
        skos:inScheme    vlcs:chemische_stof;
        skos:notation    "CHEMONTID:0000081";
        skos:prefLabel   "Isoxazoles"@en .

csc:CHEMONTID_0000895
        rdf:type         skos:Concept;
        rdfs:seeAlso     tax_nodes:C0000895;
        skos:definition  "Inorganic compounds in which the largest oxoanion is borate, and in which the heaviest atom not in an oxoanion is an alkali metal."@en;
        skos:inScheme    vlcs:chemische_stof;
        skos:notation    "CHEMONTID:0000895";
        skos:prefLabel   "Alkali metal borates"@en .

csc:CHEMONTID_0000316
        rdf:type         skos:Concept;
        rdfs:seeAlso     tax_nodes:C0000316;
        skos:definition  "Organic compounds containing a benzene fused to a pyrene(benzo[def]phenanthrene) ring system."@en;
        skos:inScheme    vlcs:chemische_stof;
        skos:notation    "CHEMONTID:0000316";
        skos:prefLabel   "Benzopyrenes"@en .

csc:CHEMONTID_0002348
        rdf:type         skos:Concept;
        rdfs:seeAlso     tax_nodes:C0002348;
        skos:definition  "Heterocyclic compounds containing a quinoline moiety substituted with a phenyl group."@en;
        skos:inScheme    vlcs:chemische_stof;
        skos:notation    "CHEMONTID:0002348";
        skos:prefLabel   "Phenylquinolines"@en .

csc:CHEMONTID_0000346
        rdf:type         skos:Concept;
        rdfs:seeAlso     tax_nodes:C0000346;
        skos:definition  "Organic compounds containing exactly two carboxylic acid groups."@en;
        skos:inScheme    vlcs:chemische_stof;
        skos:notation    "CHEMONTID:0000346";
        skos:prefLabel   "Dicarboxylic acids and derivatives"@en .

csc:CHEMONTID_0000431
        rdf:type         skos:Concept;
        rdfs:seeAlso     tax_nodes:C0000431;
        skos:definition  "Inorganic compounds containing only metal atoms,with the largest atom being a metalloid atom."@en;
        skos:inScheme    vlcs:chemische_stof;
        skos:notation    "CHEMONTID:0000431";
        skos:prefLabel   "Homogeneous metalloid compounds"@en .

csc:CHEMONTID_0004646
        rdf:type         skos:Concept;
        rdfs:seeAlso     tax_nodes:C0004646;
        skos:definition  "Phenols that a unsubstituted at the 2-position."@en;
        skos:inScheme    vlcs:chemische_stof;
        skos:notation    "CHEMONTID:0004646";
        skos:prefLabel   "1-hydroxy-2-unsubstituted benzenoids"@en .

csc:CHEMONTID_0000250
        rdf:type         skos:Concept;
        rdfs:seeAlso     tax_nodes:C0000250;
        skos:definition  "Organic compounds containing an imidazolidine ring, which is a saturated ring (derived from imidazole) with two nitrogen atoms at positions 1 and 3 respectively, and containing only single bonds."@en;
        skos:inScheme    vlcs:chemische_stof;
        skos:notation    "CHEMONTID:0000250";
        skos:prefLabel   "Imidazolidines"@en .

csc:CHEMONTID_0000461
        rdf:type         skos:Concept;
        rdfs:seeAlso     tax_nodes:C0000461;
        skos:definition  "Inorganic compounds belonging to either the alkaline earth metal hydrides, alkaline earth metal nitrides, alkaline earth metal oxides, alkaline earth metal sulfides."@en;
        skos:inScheme    vlcs:chemische_stof;
        skos:notation    "CHEMONTID:0000461";
        skos:prefLabel   "Transition metal organides"@en .

csc:CHEMONTID_0004676
        rdf:type         skos:Concept;
        rdfs:seeAlso     tax_nodes:C0004676;
        skos:definition  "Aromatic compounds hat contain a phenol ether attached to the C2-atom of a phenylpropionic acid."@en;
        skos:inScheme    vlcs:chemische_stof;
        skos:notation    "CHEMONTID:0004676";
        skos:prefLabel   "2-phenoxypropionic acids"@en .

csc:CHEMONTID_0000195
        rdf:type         skos:Concept;
        rdfs:seeAlso     tax_nodes:C0000195;
        skos:definition  "Compounds containing a piperidine ring, which is a saturated aliphatic six-member ring with one nitrogen atom and five carbon atoms."@en;
        skos:inScheme    vlcs:chemische_stof;
        skos:notation    "CHEMONTID:0000195";
        skos:prefLabel   "Piperidines"@en .

csc:CHEMONTID_0003886
        rdf:type         skos:Concept;
        rdfs:seeAlso     tax_nodes:C0003886;
        skos:definition  "Cyclic organooxygen compounds containing the structure RC(=N)N where the central carbon atom and one of the linked nitrogen atoms are part of the same ring( R here is an organyl group). They can also be viewed as analogs of lactams where the oxygen atom is replaced by a nitrogen atom."@en;
        skos:inScheme    vlcs:chemische_stof;
        skos:notation    "CHEMONTID:0003886";
        skos:prefLabel   "Imidolactams"@en .

csc:CHEMONTID_0000491
        rdf:type         skos:Concept;
        rdfs:seeAlso     tax_nodes:C0000491;
        skos:definition  "Compounds containing a sulfoxide functional group, with the structure RS(=O)R' (R,R' not H)."@en;
        skos:inScheme    vlcs:chemische_stof;
        skos:notation    "CHEMONTID:0000491";
        skos:prefLabel   "Sulfoxides"@en .

csc:CHEMONTID_0000038
        rdf:type         skos:Concept;
        rdfs:seeAlso     tax_nodes:C0000038;
        skos:definition  "Organic aromatic compounds containing a sulfanilide moiety, with the general structure RS(=O)(=O)NC1=CC=CC=C1."@en;
        skos:inScheme    vlcs:chemische_stof;
        skos:notation    "CHEMONTID:0000038";
        skos:prefLabel   "Sulfanilides"@en .

csc:CHEMONTID_0001516
        rdf:type         skos:Concept;
        rdfs:seeAlso     tax_nodes:C0001516;
        skos:definition  "Compounds containing a chemical bond between a carbon atom and a chlorine atom."@en;
        skos:inScheme    vlcs:chemische_stof;
        skos:notation    "CHEMONTID:0001516";
        skos:prefLabel   "Organochlorides"@en .

csc:CHEMONTID_0001908
        rdf:type         skos:Concept;
        rdfs:seeAlso     tax_nodes:C0001908;
        skos:definition  "Organic compounds containing a benzene fused to a quinoline ring system."@en;
        skos:inScheme    vlcs:chemische_stof;
        skos:notation    "CHEMONTID:0001908";
        skos:prefLabel   "Benzoquinolines"@en .

csc:CHEMONTID_0000123
        rdf:type         skos:Concept;
        rdfs:seeAlso     tax_nodes:C0000123;
        skos:definition  "Organic compounds containing a benzene ring fused to a pyran ring. Pyran a six-membered heterocyclic, non-aromatic ring, made up of five carbon atoms and one oxygen atom and containing two double bonds."@en;
        skos:inScheme    vlcs:chemische_stof;
        skos:notation    "CHEMONTID:0000123";
        skos:prefLabel   "Benzopyrans"@en .

csc:CHEMONTID_0002336
        rdf:type         skos:Concept;
        rdfs:seeAlso     tax_nodes:C0002336;
        skos:definition  "Polycyclic aromatic compounds containing a benzene ring linked to a pyrrolidine ring through a CC or CN bond. Pyrrolidine is a five-membered saturated aliphatic heterocycle with one nitrogen atom and four carbon atoms."@en;
        skos:inScheme    vlcs:chemische_stof;
        skos:notation    "CHEMONTID:0002336";
        skos:prefLabel   "Phenylpyrrolidines"@en .

csc:CHEMONTID_0004157
        rdf:type         skos:Concept;
        rdfs:seeAlso     tax_nodes:C0004157;
        skos:definition  "Organic compounds in which at least one of the four hydrogen atoms of methane (CH4) are replaced by halogen atoms."@en;
        skos:inScheme    vlcs:chemische_stof;
        skos:notation    "CHEMONTID:0004157";
        skos:prefLabel   "Halomethanes"@en .

csc:CHEMONTID_0003633
        rdf:type         skos:Concept;
        rdfs:seeAlso     tax_nodes:C0003633;
        skos:definition  "Organic 1,3-dipolar compounds with the general structure  X#N+-Z- <-> X-=N+=Z <-> X-=N-Z+ <-> X-N=Z (X = C or O, Z = C, N, or O)."@en;
        skos:inScheme    vlcs:chemische_stof;
        skos:notation    "CHEMONTID:0003633";
        skos:prefLabel   "Propargyl-type 1,3-dipolar organic compounds"@en .

csc:CHEMONTID_0000153
        rdf:type         skos:Concept;
        rdfs:seeAlso     tax_nodes:C0000153;
        skos:definition  "Compounds containing a naphthohydroquinone moiety, which consists of a benzene ring linearly fused to a bezene-1,4-dione (quinone)."@en;
        skos:inScheme    vlcs:chemische_stof;
        skos:notation    "CHEMONTID:0000153";
        skos:prefLabel   "Naphthoquinones"@en .

csc:CHEMONTID_0000279
        rdf:type         skos:Concept;
        rdfs:seeAlso     tax_nodes:C0000279;
        skos:definition  "Naturally occurring chemical compounds that contain mostly basic nitrogen atoms. This group also includes some related compounds with neutral and even weakly acidic properties. Also some synthetic compounds of similar structure are attributed to alkaloids. In addition to carbon, hydrogen and nitrogen, alkaloids may also contain oxygen, sulfur and more rarely other elements such as chlorine, bromine, and phosphorus."@en;
        skos:inScheme    vlcs:chemische_stof;
        skos:notation    "CHEMONTID:0000279";
        skos:prefLabel   "Alkaloids and derivatives"@en .

csc:CHEMONTID_0000756
        rdf:type         skos:Concept;
        rdfs:seeAlso     tax_nodes:C0000756;
        skos:definition  "Organic polycyclic compounds containing an imidazole ring fused to a thiazole ring. Imidazole is 5-membered ring consisting of three carbon atoms, and two nitrogen centers at the 1- and 3-positions. Thiazole is a 6-membered ring that contains both sulfur and nitrogen."@en;
        skos:inScheme    vlcs:chemische_stof;
        skos:notation    "CHEMONTID:0000756";
        skos:prefLabel   "Imidazothiazoles"@en .

csc:CHEMONTID_0000364
        rdf:type         skos:Concept;
        rdfs:seeAlso     tax_nodes:C0000364;
        skos:definition  "Compounds comprising the organic carbonic acid or a derivative thereof."@en;
        skos:inScheme    vlcs:chemische_stof;
        skos:notation    "CHEMONTID:0000364";
        skos:prefLabel   "Organic carbonic acids and derivatives"@en .

csc:CHEMONTID_0000098
        rdf:type         skos:Concept;
        rdfs:seeAlso     tax_nodes:C0000098;
        skos:definition  "Compounds containing a triazine ring, which is a heterocyclic ring, similar to the six-member benzene ring but with three carbons replaced by nitrogen atoms."@en;
        skos:inScheme    vlcs:chemische_stof;
        skos:notation    "CHEMONTID:0000098";
        skos:prefLabel   "Triazines"@en .

csc:CHEMONTID_0001027
        rdf:type         skos:Concept;
        rdfs:seeAlso     tax_nodes:C0001027;
        skos:definition  "Organic compounds containing the alkyl fluoride functional group with formula R-F , where R is an alkyl group."@en;
        skos:inScheme    vlcs:chemische_stof;
        skos:notation    "CHEMONTID:0001027";
        skos:prefLabel   "Alkyl fluorides"@en .

csc:CHEMONTID_0001691
        rdf:type         skos:Concept;
        rdfs:seeAlso     tax_nodes:C0001691;
        skos:definition  "Compounds containing a steroid moiety which bears a carboxylic acid ester group."@en;
        skos:inScheme    vlcs:chemische_stof;
        skos:notation    "CHEMONTID:0001691";
        skos:prefLabel   "Steroid esters"@en .

csc:CHEMONTID_0000503
        rdf:type         skos:Concept;
        rdfs:seeAlso     tax_nodes:C0000503;
        skos:definition  "Compounds containing positively charged polyatomic ion of the structure NR4+, R being an alkyl group or an aryl group."@en;
        skos:inScheme    vlcs:chemische_stof;
        skos:notation    "CHEMONTID:0000503";
        skos:prefLabel   "Quaternary ammonium salts"@en .

csc:CHEMONTID_0001715
        rdf:type         skos:Concept;
        rdfs:seeAlso     tax_nodes:C0001715;
        skos:definition  "Derivatives of  quinoline in which in which at least one double bond in the quinoline moiety are reduced by adding two hydrogen atoms."@en;
        skos:inScheme    vlcs:chemische_stof;
        skos:notation    "CHEMONTID:0001715";
        skos:prefLabel   "Hydroquinolines"@en .

csc:CHEMONTID_0003410
        rdf:type         skos:Concept;
        rdfs:seeAlso     tax_nodes:C0003410;
        skos:definition  "Organic aromatic compounds that 1-benzopyran, a bicyclic compound made up of a benzene ring fused to a pyran, so that the oxygen atom is at the 1-position."@en;
        skos:inScheme    vlcs:chemische_stof;
        skos:notation    "CHEMONTID:0003410";
        skos:prefLabel   "1-benzopyrans"@en .

csc:CHEMONTID_0001057
        rdf:type         skos:Concept;
        rdfs:seeAlso     tax_nodes:C0001057;
        skos:definition  "Inorganic non-metallic compounds containing a hypochlorite as its largest oxoanion."@en;
        skos:inScheme    vlcs:chemische_stof;
        skos:notation    "CHEMONTID:0001057";
        skos:prefLabel   "Non-metal hypochlorites"@en .

csc:CHEMONTID_0000056
        rdf:type         skos:Concept;
        rdfs:seeAlso     tax_nodes:C0000056;
        skos:definition  "Compounds containing a quinoline moiety which bears a ketone group."@en;
        skos:inScheme    vlcs:chemische_stof;
        skos:notation    "CHEMONTID:0000056";
        skos:prefLabel   "Quinolones and derivatives"@en .

csc:CHEMONTID_0001534
        rdf:type         skos:Concept;
        rdfs:seeAlso     tax_nodes:C0001534;
        skos:definition  "Lipids structurally characterized by the presence of a quinone or hydroquinone moiety."@en;
        skos:inScheme    vlcs:chemische_stof;
        skos:notation    "CHEMONTID:0001534";
        skos:prefLabel   "Quinone and hydroquinone lipids"@en .

csc:CHEMONTID_0001142
        rdf:type         skos:Concept;
        rdfs:seeAlso     tax_nodes:C0001142;
        skos:definition  "Compounds containing the polyaromatic chrysene moiety, which consists of a benzene ring fused to a phenanthrene ring system to form Benzo[a]phenanthrene."@en;
        skos:inScheme    vlcs:chemische_stof;
        skos:notation    "CHEMONTID:0001142";
        skos:prefLabel   "Chrysenes"@en .

csc:CHEMONTID_0000141
        rdf:type         skos:Concept;
        rdfs:seeAlso     tax_nodes:C0000141;
        skos:definition  "Compounds containing a nitrophenol moiety, which consists of a benzene ring bearing both a hydroxyl group and a nitro group on two different ring carbon atoms."@en;
        skos:inScheme    vlcs:chemische_stof;
        skos:notation    "CHEMONTID:0000141";
        skos:prefLabel   "Nitrophenols"@en .

csc:CHEMONTID_0004622
        rdf:type         skos:Concept;
        rdfs:seeAlso     tax_nodes:C0004622;
        skos:definition  "Hydrocarbons that contains one or more unsaturated carbon atoms, and an aliphatic branch."@en;
        skos:inScheme    vlcs:chemische_stof;
        skos:notation    "CHEMONTID:0004622";
        skos:prefLabel   "Branched unsaturated hydrocarbons"@en .

csc:CHEMONTID_0000267
        rdf:type         skos:Concept;
        rdfs:seeAlso     tax_nodes:C0000267;
        skos:definition  "Organic compounds containing a bond between a carbon atom and a halogen atom (At, F, Cl, Br, I)."@en;
        skos:inScheme    vlcs:chemische_stof;
        skos:notation    "CHEMONTID:0000267";
        skos:prefLabel   "Organohalogen compounds"@en .

csc:CHEMONTID_0004441
        rdf:type         skos:Concept;
        rdfs:seeAlso     tax_nodes:C0004441;
        skos:definition  "Organometallic compounds containing an allylic group attached to the metal atom."@en;
        skos:inScheme    vlcs:chemische_stof;
        skos:notation    "CHEMONTID:0004441";
        skos:prefLabel   "Metal allyls"@en .

csc:CHEMONTID_0003566
        rdf:type         skos:Concept;
        rdfs:seeAlso     tax_nodes:C0003566;
        skos:definition  "Steroids with a structure containing the 27-carbon cholestane skeleton."@en;
        skos:inScheme    vlcs:chemische_stof;
        skos:notation    "CHEMONTID:0003566";
        skos:prefLabel   "Cholestane steroids"@en .

csc:CHEMONTID_0002650
        rdf:type         skos:Concept;
        rdfs:seeAlso     tax_nodes:C0002650;
        skos:definition  "Phenylpropanoids with a structure containing two  aromatic rings joined by a seven carbons (a 1,7-diphenylheptane skeleton) and may have various substituents."@en;
        skos:inScheme    vlcs:chemische_stof;
        skos:notation    "CHEMONTID:0002650";
        skos:prefLabel   "Diarylheptanoids"@en .

csc:CHEMONTID_0003385
        rdf:type         skos:Concept;
        rdfs:seeAlso     tax_nodes:C0003385;
        skos:definition  "Organic compounds that contain dithiophosphoric acid or a derivative thereof, with the general formula ROP(S)(=S)OR', (R,R'=H, or organyl group)."@en;
        skos:inScheme    vlcs:chemische_stof;
        skos:notation    "CHEMONTID:0003385";
        skos:prefLabel   "Organic dithiophosphoric acids and derivatives"@en .

csc:CHEMONTID_0003862
        rdf:type         skos:Concept;
        rdfs:seeAlso     tax_nodes:C0003862;
        skos:definition  "Organosulfur compounds containing a thioether group that is substituted by two alkyl groups."@en;
        skos:inScheme    vlcs:chemische_stof;
        skos:notation    "CHEMONTID:0003862";
        skos:prefLabel   "Dialkylthioethers"@en .

csc:CHEMONTID_0002861
        rdf:type         skos:Concept;
        rdfs:seeAlso     tax_nodes:C0002861;
        skos:definition  "Vinyl halides in which a fluorine atom is bonded to an sp2-hybridised carbon atom."@en;
        skos:inScheme    vlcs:chemische_stof;
        skos:notation    "CHEMONTID:0002861";
        skos:prefLabel   "Vinyl fluorides"@en .

csc:CHEMONTID_0001986
        rdf:type         skos:Concept;
        rdfs:seeAlso     tax_nodes:C0001986;
        skos:definition  "Carboxylic acids containing exactly three carboxyl groups."@en;
        skos:inScheme    vlcs:chemische_stof;
        skos:notation    "CHEMONTID:0001986";
        skos:prefLabel   "Tricarboxylic acids and derivatives"@en .

csc:CHEMONTID_0000014
        rdf:type         skos:Concept;
        rdfs:seeAlso     tax_nodes:C0000014;
        skos:definition  "Compounds containing a phenylbutylamine moiety, which consists of a phenyl group substituted at the fourth carbon by an butan-1-amine."@en;
        skos:inScheme    vlcs:chemische_stof;
        skos:notation    "CHEMONTID:0000014";
        skos:prefLabel   "Phenylbutylamines"@en .

csc:CHEMONTID_0002680
        rdf:type         skos:Concept;
        rdfs:seeAlso     tax_nodes:C0002680;
        skos:definition  "Alkaloids with a structure based on the lysergic acid skeleton."@en;
        skos:inScheme    vlcs:chemische_stof;
        skos:notation    "CHEMONTID:0002680";
        skos:prefLabel   "Lysergic acids and derivatives"@en .

csc:CHEMONTID_0000310
        rdf:type         skos:Concept;
        rdfs:seeAlso     tax_nodes:C0000310;
        skos:definition  "Polycyclic aromatic compounds containing a phenothiazine moiety, which is a linear tricyclic system that consists of a two benzene rings joined by a para-thiazine ring."@en;
        skos:inScheme    vlcs:chemische_stof;
        skos:notation    "CHEMONTID:0000310";
        skos:prefLabel   "Phenothiazines"@en .

csc:CHEMONTID_0001437
        rdf:type         skos:Concept;
        rdfs:seeAlso     tax_nodes:C0001437;
        skos:definition  "Organic compounds containing a benzene fused to an oxazine ring (a six-member aliphatic ring with four carbon atoms, one oxygen atom, and one nitrogen atom) bearing a ketone group."@en;
        skos:inScheme    vlcs:chemische_stof;
        skos:notation    "CHEMONTID:0001437";
        skos:prefLabel   "Benzoxazinones"@en .

csc:CHEMONTID_0000436
        rdf:type         skos:Concept;
        rdfs:seeAlso     tax_nodes:C0000436;
        skos:definition  "Organic compounds comprising a five-member nitrogen heterocyclic ring containing at least one other non-carbon atom of either nitrogen, sulfur, or oxygen."@en;
        skos:inScheme    vlcs:chemische_stof;
        skos:notation    "CHEMONTID:0000436";
        skos:prefLabel   "Azoles"@en .

csc:CHEMONTID_0002257
        rdf:type         skos:Concept;
        rdfs:seeAlso     tax_nodes:C0002257;
        skos:definition  "Heterocyclic compounds containing a pyrrole ring substituted at one or more positions."@en;
        skos:inScheme    vlcs:chemische_stof;
        skos:notation    "CHEMONTID:0002257";
        skos:prefLabel   "Substituted pyrroles"@en .

csc:CHEMONTID_0001859
        rdf:type         skos:Concept;
        rdfs:seeAlso     tax_nodes:C0001859;
        skos:definition  "Compounds containing a pyridopyrimidine, which consists of a pyridine fused to a pyrimidine. Pyridine is 6-membered ring consisting of five carbon atoms and a nitrogen atom. Pyrimidine is a 6-membered ring consisting of four carbon atoms and two nitrogen centers at the 1- and 3- ring positions."@en;
        skos:inScheme    vlcs:chemische_stof;
        skos:notation    "CHEMONTID:0001859";
        skos:prefLabel   "Pyridopyrimidines"@en .

csc:CHEMONTID_0000074
        rdf:type         skos:Concept;
        rdfs:seeAlso     tax_nodes:C0000074;
        skos:definition  "Compounds containing a pyridazine ring, which is a six-member aromatic ring containing two nitrogen atoms at positions 1 and 2, and four carbon atoms."@en;
        skos:inScheme    vlcs:chemische_stof;
        skos:notation    "CHEMONTID:0000074";
        skos:prefLabel   "Pyridazines and derivatives"@en .

csc:CHEMONTID_0004640
        rdf:type         skos:Concept;
        rdfs:seeAlso     tax_nodes:C0004640;
        skos:definition  "Aromatic compounds containing a methylcarbamic acid esterified with a phenyl group."@en;
        skos:inScheme    vlcs:chemische_stof;
        skos:notation    "CHEMONTID:0004640";
        skos:prefLabel   "Phenyl methylcarbamates"@en .

csc:CHEMONTID_0002679
        rdf:type         skos:Concept;
        rdfs:seeAlso     tax_nodes:C0002679;
        skos:definition  "Compounds containing an ergoline moiety, which is structurally characterized by he presence of a 4,6,6a,7,8,9,10,10a-octahydroindolo[4,3-fg] quinoline."@en;
        skos:inScheme    vlcs:chemische_stof;
        skos:notation    "CHEMONTID:0002679";
        skos:prefLabel   "Ergoline and derivatives"@en .

csc:CHEMONTID_0004766
        rdf:type         skos:Concept;
        rdfs:seeAlso     tax_nodes:C0004766;
        skos:definition  "Aromatic compound contaning a phosphonothioate, which is C-substituted with a phenyl group."@en;
        skos:inScheme    vlcs:chemische_stof;
        skos:notation    "CHEMONTID:0004766";
        skos:prefLabel   "Phenylphosphonothioates"@en .

csc:CHEMONTID_0001286
        rdf:type         skos:Concept;
        rdfs:seeAlso     tax_nodes:C0001286;
        skos:definition  "Organic compounds containing two hydroxyl groups attached to a benzene ring."@en;
        skos:inScheme    vlcs:chemische_stof;
        skos:notation    "CHEMONTID:0001286";
        skos:prefLabel   "Benzenediols"@en .

csc:CHEMONTID_0000285
        rdf:type         skos:Concept;
        rdfs:seeAlso     tax_nodes:C0000285;
        skos:definition  "Organic heterocyclic compounds derived from oxoacids RkE(=O)l(OH)m (l not 0) by replacing an OH group by the NHPh group or derivative formed by ring substitution."@en;
        skos:inScheme    vlcs:chemische_stof;
        skos:notation    "CHEMONTID:0000285";
        skos:prefLabel   "Anilides"@en .

csc:CHEMONTID_0000309
        rdf:type         skos:Concept;
        rdfs:seeAlso     tax_nodes:C0000309;
        skos:definition  "Organic compounds containing a benzene fused to a thiazine ring (a six-membered ring with four carbon atoms, one nitrogen atom and one sulfur atom)."@en;
        skos:inScheme    vlcs:chemische_stof;
        skos:notation    "CHEMONTID:0000309";
        skos:prefLabel   "Benzothiazines"@en .

csc:CHEMONTID_0001974
        rdf:type         skos:Concept;
        rdfs:seeAlso     tax_nodes:C0001974;
        skos:definition  "Compounds containing a piperidine ring which bears a carboxylic acid group (or a derivative thereof)."@en;
        skos:inScheme    vlcs:chemische_stof;
        skos:notation    "CHEMONTID:0001974";
        skos:prefLabel   "Piperidinecarboxylic acids and derivatives"@en .

csc:CHEMONTID_0004670
        rdf:type         skos:Concept;
        rdfs:seeAlso     tax_nodes:C0004670;
        skos:definition  "Aromatic compounds that contain a phenol ether, which carries an amine group on the benzene ring."@en;
        skos:inScheme    vlcs:chemische_stof;
        skos:notation    "CHEMONTID:0004670";
        skos:prefLabel   "Aminophenyl ethers"@en .

csc:CHEMONTID_0000002
        rdf:type         skos:Concept;
        rdfs:seeAlso     tax_nodes:C0000002;
        skos:definition  "Compounds containing a ring with least one carbon atom and one non-carbon atom."@en;
        skos:inScheme    vlcs:chemische_stof;
        skos:notation    "CHEMONTID:0000002";
        skos:prefLabel   "Organoheterocyclic compounds"@en .

csc:CHEMONTID_0000424
        rdf:type         skos:Concept;
        rdfs:seeAlso     tax_nodes:C0000424;
        skos:definition  "Compounds that contains both metal and non metal atoms."@en;
        skos:inScheme    vlcs:chemische_stof;
        skos:notation    "CHEMONTID:0000424";
        skos:prefLabel   "Mixed metal/non-metal compounds"@en .

csc:CHEMONTID_0000032
        rdf:type         skos:Concept;
        rdfs:seeAlso     tax_nodes:C0000032;
        skos:definition  "Organic compounds containing a sulfonic acid or a derivative thereof that is linked to a benzene ring."@en;
        skos:inScheme    vlcs:chemische_stof;
        skos:notation    "CHEMONTID:0000032";
        skos:prefLabel   "Benzenesulfonic acids and derivatives"@en .

csc:CHEMONTID_0001510
        rdf:type         skos:Concept;
        rdfs:seeAlso     tax_nodes:C0001510;
        skos:definition  "Lignans that contain a lactone moiety. They include 1-aryltetralin lactones, dibenzylbutyrolactone lignans, and podophyllotoxins, among others."@en;
        skos:inScheme    vlcs:chemische_stof;
        skos:notation    "CHEMONTID:0001510";
        skos:prefLabel   "Lignan lactones"@en .

csc:CHEMONTID_0000901
        rdf:type         skos:Concept;
        rdfs:seeAlso     tax_nodes:C0000901;
        skos:definition  "Inorganic compounds in which the largest oxoanion is silicate, and in which the heaviest atom not in an oxoanion is an alkali metal."@en;
        skos:inScheme    vlcs:chemische_stof;
        skos:notation    "CHEMONTID:0000901";
        skos:prefLabel   "Alkali metal silicates"@en .

csc:CHEMONTID_0001244
        rdf:type         skos:Concept;
        rdfs:seeAlso     tax_nodes:C0001244;
        skos:definition  "Cyclic organic compounds containing an oxan-2- one moiety."@en;
        skos:inScheme    vlcs:chemische_stof;
        skos:notation    "CHEMONTID:0001244";
        skos:prefLabel   "Delta valerolactones"@en .

csc:CHEMONTID_0000369
        rdf:type         skos:Concept;
        rdfs:seeAlso     tax_nodes:C0000369;
        skos:definition  "Compounds containing a diphenylmethane moiety, which consists of a methane wherein two hydrogen atoms are replaced by two phenyl groups."@en;
        skos:inScheme    vlcs:chemische_stof;
        skos:notation    "CHEMONTID:0000369";
        skos:prefLabel   "Diphenylmethanes"@en .

csc:CHEMONTID_0001455
        rdf:type         skos:Concept;
        rdfs:seeAlso     tax_nodes:C0001455;
        skos:definition  "Polycyclic aromatic compounds containing four pyrrole rings joined by one-carbon units linking position 2 of one pyrrole ring to position 5 of the next."@en;
        skos:inScheme    vlcs:chemische_stof;
        skos:notation    "CHEMONTID:0001455";
        skos:prefLabel   "Tetrapyrroles and derivatives"@en .

csc:CHEMONTID_0000454
        rdf:type         skos:Concept;
        rdfs:seeAlso     tax_nodes:C0000454;
        skos:definition  "Inorganic compounds belonging to either the halogen hydrides, halogen nitrides, halogen oxides, or halogen sulfides."@en;
        skos:inScheme    vlcs:chemische_stof;
        skos:notation    "CHEMONTID:0000454";
        skos:prefLabel   "Halogen organides"@en .

csc:CHEMONTID_0003934
        rdf:type         skos:Concept;
        rdfs:seeAlso     tax_nodes:C0003934;
        skos:definition  "Organosulfur compounds with the general formula SC(=S)N(R1)R2; R1-R2 =  H or organyl group."@en;
        skos:inScheme    vlcs:chemische_stof;
        skos:notation    "CHEMONTID:0003934";
        skos:prefLabel   "Dithiocarbamic acids and derivatives"@en .

csc:CHEMONTID_0002275
        rdf:type         skos:Concept;
        rdfs:seeAlso     tax_nodes:C0002275;
        skos:definition  "Polycyclic aromatic compounds containing a naphthalene moiety substituted by one or more nitro groups."@en;
        skos:inScheme    vlcs:chemische_stof;
        skos:notation    "CHEMONTID:0002275";
        skos:prefLabel   "Nitronaphthalenes"@en .

csc:CHEMONTID_0000399
        rdf:type         skos:Concept;
        rdfs:seeAlso     tax_nodes:C0000399;
        skos:definition  "Compounds containing a phenylazide moiety, which consists of a linear azide substituent attached to a phenyl group."@en;
        skos:inScheme    vlcs:chemische_stof;
        skos:notation    "CHEMONTID:0000399";
        skos:prefLabel   "Phenylazides"@en .

csc:CHEMONTID_0001093
        rdf:type         skos:Concept;
        rdfs:seeAlso     tax_nodes:C0001093;
        skos:definition  "Derivatives of carboxylic acid."@en;
        skos:inScheme    vlcs:chemische_stof;
        skos:notation    "CHEMONTID:0001093";
        skos:prefLabel   "Carboxylic acid derivatives"@en .

csc:CHEMONTID_0002118
        rdf:type         skos:Concept;
        rdfs:seeAlso     tax_nodes:C0002118;
        skos:definition  "Polycyclic compounds containing an oxazole ring fused to a pyridine ring."@en;
        skos:inScheme    vlcs:chemische_stof;
        skos:notation    "CHEMONTID:0002118";
        skos:prefLabel   "Oxazolopyridines"@en .

csc:CHEMONTID_0001202
        rdf:type         skos:Concept;
        rdfs:seeAlso     tax_nodes:C0001202;
        skos:definition  "Compounds containing the ester derivative of thiocarboxylic acid, with the general structure R-S-R' (R,R'=alkyl, aryl)."@en;
        skos:inScheme    vlcs:chemische_stof;
        skos:notation    "CHEMONTID:0001202";
        skos:prefLabel   "Thioethers"@en .

csc:CHEMONTID_0000327
        rdf:type         skos:Concept;
        rdfs:seeAlso     tax_nodes:C0000327;
        skos:definition  "Organic compounds containing two phosphonate groups linked together through a carbon atoms."@en;
        skos:inScheme    vlcs:chemische_stof;
        skos:notation    "CHEMONTID:0000327";
        skos:prefLabel   "Bisphosphonates"@en .

csc:CHEMONTID_0004024
        rdf:type         skos:Concept;
        rdfs:seeAlso     tax_nodes:C0004024;
        skos:definition  "Compounds containing bond between a carbon atom and a lead atom."@en;
        skos:inScheme    vlcs:chemische_stof;
        skos:notation    "CHEMONTID:0004024";
        skos:prefLabel   "Organolead compounds"@en .

csc:CHEMONTID_0000020
        rdf:type         skos:Concept;
        rdfs:seeAlso     tax_nodes:C0000020;
        skos:definition  "Compounds containing a fluorene moiety, which consists of two benzene rings connected through either a cyclopentane, cyclopentene, or cyclopenta-1,3-diene."@en;
        skos:inScheme    vlcs:chemische_stof;
        skos:notation    "CHEMONTID:0000020";
        skos:prefLabel   "Fluorenes"@en .

csc:CHEMONTID_0000538
        rdf:type         skos:Concept;
        rdfs:seeAlso     tax_nodes:C0000538;
        skos:definition  "Inorganic compounds containing an oxygen atom of an oxidation state of -2, in which the heaviest atom bonded to the oxygen is a transition metal."@en;
        skos:inScheme    vlcs:chemische_stof;
        skos:notation    "CHEMONTID:0000538";
        skos:prefLabel   "Transition metal oxides"@en .

csc:CHEMONTID_0001443
        rdf:type         skos:Concept;
        rdfs:seeAlso     tax_nodes:C0001443;
        skos:definition  "Polycyclic aromatic compounds containing triazole ring fused to a pyrimidine ring. Triazole is a five-membered ring consisting of two carbon atoms and three nitrogen atoms. Pyrimidine is a 6-membered ring consisting of four carbon atoms and two nitrogen centers at the 1- and 3- ring positions."@en;
        skos:inScheme    vlcs:chemische_stof;
        skos:notation    "CHEMONTID:0001443";
        skos:prefLabel   "Triazolopyrimidines"@en .

csc:CHEMONTID_0000442
        rdf:type         skos:Concept;
        rdfs:seeAlso     tax_nodes:C0000442;
        skos:definition  "Inorganic halogenic compounds in which the heaviest metal atom is a metalloid."@en;
        skos:inScheme    vlcs:chemische_stof;
        skos:notation    "CHEMONTID:0000442";
        skos:prefLabel   "Metalloid salts"@en .

csc:CHEMONTID_0000050
        rdf:type         skos:Concept;
        rdfs:seeAlso     tax_nodes:C0000050;
        skos:definition  "Cyclic esters of hydroxy carboxylic acids, containing a 1-oxacycloalkan-2-one structure, or analogues having unsaturation or heteroatoms replacing one or more carbon atoms of the ring."@en;
        skos:inScheme    vlcs:chemische_stof;
        skos:notation    "CHEMONTID:0000050";
        skos:prefLabel   "Lactones"@en .

csc:CHEMONTID_0001920
        rdf:type         skos:Concept;
        rdfs:seeAlso     tax_nodes:C0001920;
        skos:definition  "Compounds containing a triazine ring which bears a ketone group a carbon atom."@en;
        skos:inScheme    vlcs:chemische_stof;
        skos:notation    "CHEMONTID:0001920";
        skos:prefLabel   "Triazinones"@en .

csc:CHEMONTID_0000176
        rdf:type         skos:Concept;
        rdfs:seeAlso     tax_nodes:C0000176;
        skos:definition  "Organic compounds containing a carboxylic acid substituent attached to a benzene ring."@en;
        skos:inScheme    vlcs:chemische_stof;
        skos:notation    "CHEMONTID:0000176";
        skos:prefLabel   "Benzoic acids and derivatives"@en .

csc:CHEMONTID_0004742
        rdf:type         skos:Concept;
        rdfs:seeAlso     tax_nodes:C0004742;
        skos:definition  "Aromatic compounds contaning a phenoxy group."@en;
        skos:inScheme    vlcs:chemische_stof;
        skos:notation    "CHEMONTID:0004742";
        skos:prefLabel   "Phenoxy compounds"@en .

csc:CHEMONTID_0000261
        rdf:type         skos:Concept;
        rdfs:seeAlso     tax_nodes:C0000261;
        skos:definition  "Organic compounds that are synthesized either from the amino acid phenylalanine (phenylpropanoids) or the decarboxylative condensation of malonyl-CoA (polyketides). Phenylpropanoids are aromatic compounds based on the phenylpropane skeleton. Polyketides usually consist of alternating carbonyl and methylene groups (beta-polyketones), biogenetically derived from repeated condensation of acetyl coenzyme A (via malonyl coenzyme A), and usually the compounds derived from them by further condensations."@en;
        skos:inScheme    vlcs:chemische_stof;
        skos:notation    "CHEMONTID:0000261";
        skos:prefLabel   "Phenylpropanoids and polyketides"@en .

csc:CHEMONTID_0002389
        rdf:type         skos:Concept;
        rdfs:seeAlso     tax_nodes:C0002389;
        skos:definition  "Organic compounds containing diazinane, a six-membered saturated heterocycle containing four carbon atoms and two nitrogen atoms."@en;
        skos:inScheme    vlcs:chemische_stof;
        skos:notation    "CHEMONTID:0002389";
        skos:prefLabel   "Diazinanes"@en .

csc:CHEMONTID_0002866
        rdf:type         skos:Concept;
        rdfs:seeAlso     tax_nodes:C0002866;
        skos:definition  "Organic compounds containing an aromatic ring (or ring system) carrying a C-X bond."@en;
        skos:inScheme    vlcs:chemische_stof;
        skos:notation    "CHEMONTID:0002866";
        skos:prefLabel   "Aryl halides"@en .

csc:CHEMONTID_0004476
        rdf:type         skos:Concept;
        rdfs:seeAlso     tax_nodes:C0004476;
        skos:definition  "Aliphatic Hydrocarbons that contains one or more unsaturated carbon atoms. These compounds contain one or more double or triple bonds."@en;
        skos:inScheme    vlcs:chemische_stof;
        skos:notation    "CHEMONTID:0004476";
        skos:prefLabel   "Unsaturated aliphatic hydrocarbons"@en .

csc:CHEMONTID_0000472
        rdf:type         skos:Concept;
        rdfs:seeAlso     tax_nodes:C0000472;
        skos:definition  "Compounds comprising one or more hydroxy acid groups."@en;
        skos:inScheme    vlcs:chemische_stof;
        skos:notation    "CHEMONTID:0000472";
        skos:prefLabel   "Hydroxy acids and derivatives"@en .

csc:CHEMONTID_0000019
        rdf:type         skos:Concept;
        rdfs:seeAlso     tax_nodes:C0000019;
        skos:definition  "Compounds containing a dibenzocycloheptene moiety, which consists of two benzene rings connected by a cycloheptene ring."@en;
        skos:inScheme    vlcs:chemische_stof;
        skos:notation    "CHEMONTID:0000019";
        skos:prefLabel   "Dibenzocycloheptenes"@en .

csc:CHEMONTID_0002106
        rdf:type         skos:Concept;
        rdfs:seeAlso     tax_nodes:C0002106;
        skos:definition  "Polyketides containing a tetracenequinone ring structure with a sugar attached by glycosidic linkage."@en;
        skos:inScheme    vlcs:chemische_stof;
        skos:notation    "CHEMONTID:0002106";
        skos:prefLabel   "Anthracyclines"@en .

csc:CHEMONTID_0002317
        rdf:type         skos:Concept;
        rdfs:seeAlso     tax_nodes:C0002317;
        skos:definition  "Polycyclic aromatic compounds containing a benzene ring linked to a pyridine ring through a CC or CN bond."@en;
        skos:inScheme    vlcs:chemische_stof;
        skos:notation    "CHEMONTID:0002317";
        skos:prefLabel   "Phenylpyridines"@en .

csc:CHEMONTID_0000315
        rdf:type         skos:Concept;
        rdfs:seeAlso     tax_nodes:C0000315;
        skos:definition  "Organic compounds containing a benzene fused to a triazole ring (a five-membered ring with two carbon atoms and three nitrogen atoms)."@en;
        skos:inScheme    vlcs:chemische_stof;
        skos:notation    "CHEMONTID:0000315";
        skos:prefLabel   "Benzotriazoles"@en .

csc:CHEMONTID_0002010
        rdf:type         skos:Concept;
        rdfs:seeAlso     tax_nodes:C0002010;
        skos:definition  "Compounds containing at least two different types of amino acids (alpha, beta, gamma, delta) linked to each other through a peptide bond."@en;
        skos:inScheme    vlcs:chemische_stof;
        skos:notation    "CHEMONTID:0002010";
        skos:prefLabel   "Hybrid peptides"@en .

csc:CHEMONTID_0000049
        rdf:type         skos:Concept;
        rdfs:seeAlso     tax_nodes:C0000049;
        skos:definition  "Compounds containing a tametraline moiety, which consists of a tetrahydronaphthalene linked to a phenyl group to form N-methyl-4-phenyl-1,2,3,4-tetrahydronaphthalen-1-amine skeleton."@en;
        skos:inScheme    vlcs:chemische_stof;
        skos:notation    "CHEMONTID:0000049";
        skos:prefLabel   "Tametralines"@en .

csc:CHEMONTID_0001527
        rdf:type         skos:Concept;
        rdfs:seeAlso     tax_nodes:C0001527;
        skos:definition  "Cyclic aromatic compounds containing a diphenylacetonitrile moiety, which consists of a diphenylmethane linked to and acetonitrile to form 2,2-diphenylacetonitrile."@en;
        skos:inScheme    vlcs:chemische_stof;
        skos:notation    "CHEMONTID:0001527";
        skos:prefLabel   "Diphenylacetonitriles"@en .

csc:CHEMONTID_0000526
        rdf:type         skos:Concept;
        rdfs:seeAlso     tax_nodes:C0000526;
        skos:definition  "Inorganic compounds containing an oxygen atom of an oxidation state of -2, in which the heaviest atom bonded to the oxygen is an alkali metal."@en;
        skos:inScheme    vlcs:chemische_stof;
        skos:notation    "CHEMONTID:0000526";
        skos:prefLabel   "Alkali metal oxides"@en .

csc:CHEMONTID_0000134
        rdf:type         skos:Concept;
        rdfs:seeAlso     tax_nodes:C0000134;
        skos:definition  "Compounds containing a phenol moiety, which is a benzene bearing a hydroxyl group."@en;
        skos:inScheme    vlcs:chemische_stof;
        skos:notation    "CHEMONTID:0000134";
        skos:prefLabel   "Phenols"@en .

csc:CHEMONTID_0000400
        rdf:type         skos:Concept;
        rdfs:seeAlso     tax_nodes:C0000400;
        skos:definition  "Organic compounds containing the phosphorus atom."@en;
        skos:inScheme    vlcs:chemische_stof;
        skos:notation    "CHEMONTID:0000400";
        skos:prefLabel   "Organophosphorus compounds"@en .

csc:CHEMONTID_0002528
        rdf:type         skos:Concept;
        rdfs:seeAlso     tax_nodes:C0002528;
        skos:definition  "Alcohols substituted by a halogen atom at a saturated carbon atom otherwise bearing only hydrogen or hydrocarbyl groups (usually used to mean beta-halo alcohols)."@en;
        skos:inScheme    vlcs:chemische_stof;
        skos:notation    "CHEMONTID:0002528";
        skos:prefLabel   "Halohydrins"@en .

csc:CHEMONTID_0001346
        rdf:type         skos:Concept;
        rdfs:seeAlso     tax_nodes:C0001346;
        skos:definition  "Organic compounds containing a five-member heterocyclic compound with five nitrogen atoms, and two nitrogen atoms at positions 1 and 2 (Pyridazines), 1 and 3 (Pyrimidines), or 1 and 4 (Pyrazines)."@en;
        skos:inScheme    vlcs:chemische_stof;
        skos:notation    "CHEMONTID:0001346";
        skos:prefLabel   "Diazines"@en .

csc:CHEMONTID_0004434
        rdf:type         skos:Concept;
        rdfs:seeAlso     tax_nodes:C0004434;
        skos:definition  "Compounds containing a sulfonic acid or derivative, with the general structure RS(=O)2X (R= H or organyl group, X=any heteroatom)."@en;
        skos:inScheme    vlcs:chemische_stof;
        skos:notation    "CHEMONTID:0004434";
        skos:prefLabel   "Organic sulfonic acids and derivatives"@en .

csc:CHEMONTID_0000430
        rdf:type         skos:Concept;
        rdfs:seeAlso     tax_nodes:C0000430;
        skos:definition  "Inorganic compounds containing only metal atoms,with the largest atom being a transition metal atom."@en;
        skos:inScheme    vlcs:chemische_stof;
        skos:notation    "CHEMONTID:0000430";
        skos:prefLabel   "Homogeneous actinide compounds"@en .

csc:CHEMONTID_0000079
        rdf:type         skos:Concept;
        rdfs:seeAlso     tax_nodes:C0000079;
        skos:definition  "Organic compounds containing an imidazoline ring, which is an unsaturated ring (derived from imidazole) with two nitrogen atoms at positions 1 and 3 respectively, and containing only one CN double bond."@en;
        skos:inScheme    vlcs:chemische_stof;
        skos:notation    "CHEMONTID:0000079";
        skos:prefLabel   "Imidazolines"@en .

csc:CHEMONTID_0000375
        rdf:type         skos:Concept;
        rdfs:seeAlso     tax_nodes:C0000375;
        skos:definition  "Compounds containing a guanidine moiety, with the general structure (R1R2N)(R3R4N)C=N-R5."@en;
        skos:inScheme    vlcs:chemische_stof;
        skos:notation    "CHEMONTID:0000375";
        skos:prefLabel   "Guanidines"@en .

csc:CHEMONTID_0001853
        rdf:type         skos:Concept;
        rdfs:seeAlso     tax_nodes:C0001853;
        skos:definition  "Compounds containing a six-member aliphatic saturated heterocycle made up of three oxygen atoms and three carbon atoms."@en;
        skos:inScheme    vlcs:chemische_stof;
        skos:notation    "CHEMONTID:0001853";
        skos:prefLabel   "Trioxanes"@en .

csc:CHEMONTID_0003940
        rdf:type         skos:Concept;
        rdfs:seeAlso     tax_nodes:C0003940;
        skos:definition  "Organic compounds containing an oxide group."@en;
        skos:inScheme    vlcs:chemische_stof;
        skos:notation    "CHEMONTID:0003940";
        skos:prefLabel   "Organic oxides"@en .

csc:CHEMONTID_0000460
        rdf:type         skos:Concept;
        rdfs:seeAlso     tax_nodes:C0000460;
        skos:definition  "Inorganic compounds belonging to either of the metalloid hydrides, metalloid nitrides, metalloid oxides, metalloid sulfides."@en;
        skos:inScheme    vlcs:chemische_stof;
        skos:notation    "CHEMONTID:0000460";
        skos:prefLabel   "Metalloid organides"@en .

csc:CHEMONTID_0000194
        rdf:type         skos:Concept;
        rdfs:seeAlso     tax_nodes:C0000194;
        skos:definition  "Compounds containing a furan ring which bears a nitro group."@en;
        skos:inScheme    vlcs:chemische_stof;
        skos:notation    "CHEMONTID:0000194";
        skos:prefLabel   "Nitrofurans"@en .

csc:CHEMONTID_0002799
        rdf:type         skos:Concept;
        rdfs:seeAlso     tax_nodes:C0002799;
        skos:definition  "Organosulfur compounds with the general formula RSSSR' (R,R'=alkyl, aryl)."@en;
        skos:inScheme    vlcs:chemische_stof;
        skos:notation    "CHEMONTID:0002799";
        skos:prefLabel   "Organic trisulfides"@en .

csc:CHEMONTID_0000218
        rdf:type         skos:Concept;
        rdfs:seeAlso     tax_nodes:C0000218;
        skos:definition  "Compounds containing a pyrrolidine ring, which is a five-membered saturated aliphatic heterocycle with one nitrogen atom and four carbon atoms."@en;
        skos:inScheme    vlcs:chemische_stof;
        skos:notation    "CHEMONTID:0000218";
        skos:prefLabel   "Pyrrolidines"@en .

csc:CHEMONTID_0003970
        rdf:type         skos:Concept;
        rdfs:seeAlso     tax_nodes:C0003970;
        skos:definition  "Organic compounds containing a pyridine ring substituted at one or more positions by a halogen atom."@en;
        skos:inScheme    vlcs:chemische_stof;
        skos:notation    "CHEMONTID:0003970";
        skos:prefLabel   "Halopyridines"@en .

csc:CHEMONTID_0000490
        rdf:type         skos:Concept;
        rdfs:seeAlso     tax_nodes:C0000490;
        skos:definition  "Organic compounds containing a sulfonyl group with the structure R-S(=O)2-R', where R' is an urea."@en;
        skos:inScheme    vlcs:chemische_stof;
        skos:notation    "CHEMONTID:0000490";
        skos:prefLabel   "Sulfonylureas"@en .

csc:CHEMONTID_0000303
        rdf:type         skos:Concept;
        rdfs:seeAlso     tax_nodes:C0000303;
        skos:definition  "Compounds containing a phenylpiperidine skeleton, which consists of a piperidine bound to a phenyl group."@en;
        skos:inScheme    vlcs:chemische_stof;
        skos:notation    "CHEMONTID:0000303";
        skos:prefLabel   "Phenylpiperidines"@en .

csc:CHEMONTID_0000429
        rdf:type         skos:Concept;
        rdfs:seeAlso     tax_nodes:C0000429;
        skos:definition  "Inorganic compounds containing only metal atoms, with the largest atom being a lanthanide atom."@en;
        skos:inScheme    vlcs:chemische_stof;
        skos:notation    "CHEMONTID:0000429";
        skos:prefLabel   "Homogeneous lanthanide compounds"@en .

csc:CHEMONTID_0000037
        rdf:type         skos:Concept;
        rdfs:seeAlso     tax_nodes:C0000037;
        skos:definition  "Organic compounds containing an ethenylbenzene moiety."@en;
        skos:inScheme    vlcs:chemische_stof;
        skos:notation    "CHEMONTID:0000037";
        skos:prefLabel   "Styrenes"@en .

csc:CHEMONTID_0001515
        rdf:type         skos:Concept;
        rdfs:seeAlso     tax_nodes:C0001515;
        skos:definition  "Compounds containing a chemical bond between a carbon atom and a bromine atom."@en;
        skos:inScheme    vlcs:chemische_stof;
        skos:notation    "CHEMONTID:0001515";
        skos:prefLabel   "Organobromides"@en .

csc:CHEMONTID_0003909
        rdf:type         skos:Concept;
        rdfs:seeAlso     tax_nodes:C0003909;
        skos:definition  "Organic molecules synthesized by chain elongation of an acetyl-CoA primer with malonyl-CoA (or methylmalonyl-CoA) groups that might contain a cyclic functionality and/or are substituted with heteroatoms."@en;
        skos:inScheme    vlcs:chemische_stof;
        skos:notation    "CHEMONTID:0003909";
        skos:prefLabel   "Fatty Acyls"@en .

csc:CHEMONTID_0004603
        rdf:type         skos:Concept;
        rdfs:seeAlso     tax_nodes:C0004603;
        skos:definition  "Organic compounds that contain one or more oxygen atoms."@en;
        skos:inScheme    vlcs:chemische_stof;
        skos:notation    "CHEMONTID:0004603";
        skos:prefLabel   "Organic oxygen compounds"@en .

csc:CHEMONTID_0001334
        rdf:type         skos:Concept;
        rdfs:seeAlso     tax_nodes:C0001334;
        skos:definition  "Aliphatic alcohols consisting of a chain of a least six carbon atoms."@en;
        skos:inScheme    vlcs:chemische_stof;
        skos:notation    "CHEMONTID:0001334";
        skos:prefLabel   "Fatty alcohols"@en .

csc:CHEMONTID_0000459
        rdf:type         skos:Concept;
        rdfs:seeAlso     tax_nodes:C0000459;
        skos:definition  "Inorganic compounds belonging to either the lanthanide hydrides, lanthanide nitrides, lanthanide oxides, lanthanide sulfides."@en;
        skos:inScheme    vlcs:chemische_stof;
        skos:notation    "CHEMONTID:0000459";
        skos:prefLabel   "Lanthanide organides"@en .

csc:CHEMONTID_0000067
        rdf:type         skos:Concept;
        rdfs:seeAlso     tax_nodes:C0000067;
        skos:definition  "Compounds containing a pyrazine ring, which is a six-member aromatic heterocycle, that consists of two nitrogen atoms (at positions 1 and 4) and four carbon atoms."@en;
        skos:inScheme    vlcs:chemische_stof;
        skos:notation    "CHEMONTID:0000067";
        skos:prefLabel   "Pyrazines"@en .

csc:CHEMONTID_0001279
        rdf:type         skos:Concept;
        rdfs:seeAlso     tax_nodes:C0001279;
        skos:definition  "Compounds containing having two beta-haloalkyl groups bound to a sulfur atom."@en;
        skos:inScheme    vlcs:chemische_stof;
        skos:notation    "CHEMONTID:0001279";
        skos:prefLabel   "Sulfur mustard compounds"@en .

csc:CHEMONTID_0000278
        rdf:type         skos:Concept;
        rdfs:seeAlso     tax_nodes:C0000278;
        skos:definition  "Organic compounds containing a nitrogen atom."@en;
        skos:inScheme    vlcs:chemische_stof;
        skos:notation    "CHEMONTID:0000278";
        skos:prefLabel   "Organonitrogen compounds"@en .

csc:CHEMONTID_0000363
        rdf:type         skos:Concept;
        rdfs:seeAlso     tax_nodes:C0000363;
        skos:definition  "Organic compounds containing the cyanate functional group with the formula [OCN]-."@en;
        skos:inScheme    vlcs:chemische_stof;
        skos:notation    "CHEMONTID:0000363";
        skos:prefLabel   "Cyanates"@en .

csc:CHEMONTID_0000097
        rdf:type         skos:Concept;
        rdfs:seeAlso     tax_nodes:C0000097;
        skos:definition  "Compounds containing a five-membered aromatic moiety made up of one sulfur atom and four carbon atoms."@en;
        skos:inScheme    vlcs:chemische_stof;
        skos:notation    "CHEMONTID:0000097";
        skos:prefLabel   "Thiophenes"@en .

csc:CHEMONTID_0001183
        rdf:type         skos:Concept;
        rdfs:seeAlso     tax_nodes:C0001183;
        skos:definition  "Organic compounds containing the sulfuric acid diamide functional group, with the generic structure R1N(R2)S(=O)(=O)ON(R3)R4 (R1-R4 = H or organyl."@en;
        skos:inScheme    vlcs:chemische_stof;
        skos:notation    "CHEMONTID:0001183";
        skos:prefLabel   "Sulfuric acid diamides"@en .

csc:CHEMONTID_0004789
        rdf:type         skos:Concept;
        rdfs:seeAlso     tax_nodes:C0004789;
        skos:definition  "Aromatic heterocyclic compounds containing a benzene ring fused to a diazine ring. The diazine ring is an analogue of benzene, where two carbon atoms are replaced by nitrogen atoms."@en;
        skos:inScheme    vlcs:chemische_stof;
        skos:notation    "CHEMONTID:0004789";
        skos:prefLabel   "Benzodiazines"@en .

csc:CHEMONTID_0001871
        rdf:type         skos:Concept;
        rdfs:seeAlso     tax_nodes:C0001871;
        skos:definition  "Compounds containing a naphthalene moiety, which bears a carboxylic acid group or a derivative at one or more positions. Naphthalene is a bicyclic compound that is made up of two fused benzene ring."@en;
        skos:inScheme    vlcs:chemische_stof;
        skos:notation    "CHEMONTID:0001871";
        skos:prefLabel   "Naphthalenecarboxylic acids and derivatives"@en .

csc:CHEMONTID_0001026
        rdf:type         skos:Concept;
        rdfs:seeAlso     tax_nodes:C0001026;
        skos:definition  "Organic compounds containing the alkyl chloride functional group with formula R-Cl , where R is an alkyl group."@en;
        skos:inScheme    vlcs:chemische_stof;
        skos:notation    "CHEMONTID:0001026";
        skos:prefLabel   "Alkyl chlorides"@en .

csc:CHEMONTID_0000025
        rdf:type         skos:Concept;
        rdfs:seeAlso     tax_nodes:C0000025;
        skos:definition  "Polycyclic compounds containing a phenanthrene moiety, which is a tricyclic aromatic compound with three non-linearly fused benzene."@en;
        skos:inScheme    vlcs:chemische_stof;
        skos:notation    "CHEMONTID:0000025";
        skos:prefLabel   "Phenanthrenes and derivatives"@en .

csc:CHEMONTID_0000417
        rdf:type         skos:Concept;
        rdfs:seeAlso     tax_nodes:C0000417;
        skos:definition  "Compounds containing an anisole where the methane group is linked to an acetic acid or a derivative."@en;
        skos:inScheme    vlcs:chemische_stof;
        skos:notation    "CHEMONTID:0000417";
        skos:prefLabel   "Phenoxyacetic acid derivatives"@en .

csc:CHEMONTID_0002323
        rdf:type         skos:Concept;
        rdfs:seeAlso     tax_nodes:C0002323;
        skos:definition  "Heterocyclic aromatic compounds containing a benzene ring fused to a thiadiazole ring. Thiadiazole is a five-membered aromatic heterocycle made up of one sulfur atom and two nitrogen atoms."@en;
        skos:inScheme    vlcs:chemische_stof;
        skos:notation    "CHEMONTID:0002323";
        skos:prefLabel   "Benzothiadiazoles"@en .

csc:CHEMONTID_0001322
        rdf:type         skos:Concept;
        rdfs:seeAlso     tax_nodes:C0001322;
        skos:definition  "Compounds containing a pyridine ring bearing a carboxylic acid group or a derivative thereof."@en;
        skos:inScheme    vlcs:chemische_stof;
        skos:notation    "CHEMONTID:0001322";
        skos:prefLabel   "Pyridinecarboxylic acids and derivatives"@en .

csc:CHEMONTID_0000321
        rdf:type         skos:Concept;
        rdfs:seeAlso     tax_nodes:C0000321;
        skos:definition  "Organic compounds containing an acyl moiety of benzoic acid with the formula (C6H5CO-)."@en;
        skos:inScheme    vlcs:chemische_stof;
        skos:notation    "CHEMONTID:0000321";
        skos:prefLabel   "Benzoyl derivatives"@en .

csc:CHEMONTID_0002449
        rdf:type         skos:Concept;
        rdfs:seeAlso     tax_nodes:C0002449;
        skos:definition  "Compounds formally derived from ammonia by replacing one, two or three hydrogen atoms by hydrocarbyl groups, and having the general structures RNH2 (primary amines), R2NH (secondary amines), R3N (tertiary amines)."@en;
        skos:inScheme    vlcs:chemische_stof;
        skos:notation    "CHEMONTID:0002449";
        skos:prefLabel   "Amines"@en .

csc:CHEMONTID_0002800
        rdf:type         skos:Concept;
        rdfs:seeAlso     tax_nodes:C0002800;
        skos:definition  "Organosulfur compounds with the general formula RSSR' (R,R' = alkyl, aryl)."@en;
        skos:inScheme    vlcs:chemische_stof;
        skos:notation    "CHEMONTID:0002800";
        skos:prefLabel   "Organic disulfides"@en .

csc:CHEMONTID_0000055
        rdf:type         skos:Concept;
        rdfs:seeAlso     tax_nodes:C0000055;
        skos:definition  "Compounds containing a dibenzothiazepine moiety, which consists of two benzene connected by a thiazepine ring."@en;
        skos:inScheme    vlcs:chemische_stof;
        skos:notation    "CHEMONTID:0000055";
        skos:prefLabel   "Dibenzothiazepines"@en .

csc:CHEMONTID_0004144
        rdf:type         skos:Concept;
        rdfs:seeAlso     tax_nodes:C0004144;
        skos:definition  "Compounds containing an aromatic ring where a carbon atom is linked to an hetero atom."@en;
        skos:inScheme    vlcs:chemische_stof;
        skos:notation    "CHEMONTID:0004144";
        skos:prefLabel   "Heteroaromatic compounds"@en .

csc:CHEMONTID_0004089
        rdf:type         skos:Concept;
        rdfs:seeAlso     tax_nodes:C0004089;
        skos:definition  "Organic compounds containing a disulfide group R-SS-R' where R and R' are both alkyl groups."@en;
        skos:inScheme    vlcs:chemische_stof;
        skos:notation    "CHEMONTID:0004089";
        skos:prefLabel   "Dialkyldisulfides"@en .

csc:CHEMONTID_0000296
        rdf:type         skos:Concept;
        rdfs:seeAlso     tax_nodes:C0000296;
        skos:definition  "Organic compounds containing a benzene ring fused to either isomers of dioxole. Dioxole is a five-membered unsaturated ring of two oxygen atoms and three carbon atoms."@en;
        skos:inScheme    vlcs:chemische_stof;
        skos:notation    "CHEMONTID:0000296";
        skos:prefLabel   "Benzodioxoles"@en .

csc:CHEMONTID_0004681
        rdf:type         skos:Concept;
        rdfs:seeAlso     tax_nodes:C0004681;
        skos:definition  "Polycyclic aromatic compounds containing a 1,2,4-triazolo[1,5-a]pyrimidine ring system, which is substituted with a sulfonamide at the 2-position."@en;
        skos:inScheme    vlcs:chemische_stof;
        skos:notation    "CHEMONTID:0004681";
        skos:prefLabel   "1,2,4-triazolopyrimidine-2-sulfonamides"@en .

csc:CHEMONTID_0000405
        rdf:type         skos:Concept;
        rdfs:seeAlso     tax_nodes:C0000405;
        skos:definition  "Compounds containing bond between a carbon atom and an arsenic atom."@en;
        skos:inScheme    vlcs:chemische_stof;
        skos:notation    "CHEMONTID:0000405";
        skos:prefLabel   "Organoarsenic compounds"@en .

csc:CHEMONTID_0000013
        rdf:type         skos:Concept;
        rdfs:seeAlso     tax_nodes:C0000013;
        skos:definition  "Organic compounds containing an amino acid or a peptide backbone, or derivatives thereof."@en;
        skos:inScheme    vlcs:chemische_stof;
        skos:notation    "CHEMONTID:0000013";
        skos:prefLabel   "Amino acids, peptides, and analogues"@en .

csc:CHEMONTID_0002100
        rdf:type         skos:Concept;
        rdfs:seeAlso     tax_nodes:C0002100;
        skos:definition  "Organic compounds containing a benzene ring fused to a dioxin ring. Dioxin a six-membered unsaturated ring of two oxygen atoms and four carbon atoms."@en;
        skos:inScheme    vlcs:chemische_stof;
        skos:notation    "CHEMONTID:0002100";
        skos:prefLabel   "Benzodioxins"@en .

csc:CHEMONTID_0000139
        rdf:type         skos:Concept;
        rdfs:seeAlso     tax_nodes:C0000139;
        skos:definition  "Compounds containing a hydroxyethyl group attached to the C4 carbon of a phenol group."@en;
        skos:inScheme    vlcs:chemische_stof;
        skos:notation    "CHEMONTID:0000139";
        skos:prefLabel   "Tyrosols and derivatives"@en .

csc:CHEMONTID_0000224
        rdf:type         skos:Concept;
        rdfs:seeAlso     tax_nodes:C0000224;
        skos:definition  "Cyclic organic compounds containing a thiadiazine ring, which is a six-member unsaturated heterocycle made up of one sulfur atom and two nitrogen atoms."@en;
        skos:inScheme    vlcs:chemische_stof;
        skos:notation    "CHEMONTID:0000224";
        skos:prefLabel   "Thiadiazines"@en .

csc:CHEMONTID_0004524
        rdf:type         skos:Concept;
        rdfs:seeAlso     tax_nodes:C0004524;
        skos:definition  "Aromatic compounds containing a triphenyl moiety."@en;
        skos:inScheme    vlcs:chemische_stof;
        skos:notation    "CHEMONTID:0004524";
        skos:prefLabel   "Triphenyl compounds"@en .

csc:CHEMONTID_0000435
        rdf:type         skos:Concept;
        rdfs:seeAlso     tax_nodes:C0000435;
        skos:definition  "Inorganic non-metallic compounds containing an oxoanion."@en;
        skos:inScheme    vlcs:chemische_stof;
        skos:notation    "CHEMONTID:0000435";
        skos:prefLabel   "Non-metal oxoanionic compounds"@en .

list:kingdom  rdf:type  rdf:List;
        rdf:first       cscl:kingdom;
        rdf:rest        list:superclass;
        skos:prefLabel  "Niveau rijk"@nl .

csc:CHEMONTID_0002648
        rdf:type         skos:Concept;
        rdfs:seeAlso     tax_nodes:C0002648;
        skos:definition  "Heterocyclic compounds containing a saturated, aliphatic, five-membered ring where a carbon is replaced by an oxygen."@en;
        skos:inScheme    vlcs:chemische_stof;
        skos:notation    "CHEMONTID:0002648";
        skos:prefLabel   "Tetrahydrofurans"@en .

csc:CHEMONTID_0000254
        rdf:type         skos:Concept;
        rdfs:seeAlso     tax_nodes:C0000254;
        skos:definition  "Compounds bearing an ether group with the formula Compounds ROR (R not H)."@en;
        skos:inScheme    vlcs:chemische_stof;
        skos:notation    "CHEMONTID:0000254";
        skos:prefLabel   "Ethers"@en .

csc:CHEMONTID_0002341
        rdf:type         skos:Concept;
        rdfs:seeAlso     tax_nodes:C0002341;
        skos:definition  "Aromatic compounds containing an ether group substituted with a benzene ring."@en;
        skos:inScheme    vlcs:chemische_stof;
        skos:notation    "CHEMONTID:0002341";
        skos:prefLabel   "Phenol ethers"@en .

csc:CHEMONTID_0001466
        rdf:type         skos:Concept;
        rdfs:seeAlso     tax_nodes:C0001466;
        skos:definition  "Steroids with a structure based on the estrane skeleton."@en;
        skos:inScheme    vlcs:chemische_stof;
        skos:notation    "CHEMONTID:0001466";
        skos:prefLabel   "Estrane steroids"@en .

csc:CHEMONTID_0004162
        rdf:type         skos:Concept;
        rdfs:seeAlso     tax_nodes:C0004162;
        skos:definition  "Organic compounds containing an indole moiety that carries a hydroxyl group."@en;
        skos:inScheme    vlcs:chemische_stof;
        skos:notation    "CHEMONTID:0004162";
        skos:prefLabel   "Hydroxyindoles"@en .

csc:CHEMONTID_0002552
        rdf:type         skos:Concept;
        rdfs:seeAlso     tax_nodes:C0002552;
        skos:definition  "Quinolines in which the quinoline ring system is substituted by a carboxyl group at one or more positions."@en;
        skos:inScheme    vlcs:chemische_stof;
        skos:notation    "CHEMONTID:0002552";
        skos:prefLabel   "Quinoline carboxylic acids"@en .

csc:CHEMONTID_0001551
        rdf:type         skos:Concept;
        rdfs:seeAlso     tax_nodes:C0001551;
        skos:definition  "Terpene compounds formed by four isoprene units."@en;
        skos:inScheme    vlcs:chemische_stof;
        skos:notation    "CHEMONTID:0001551";
        skos:prefLabel   "Diterpenoids"@en .

csc:CHEMONTID_0000550
        rdf:type         skos:Concept;
        rdfs:seeAlso     tax_nodes:C0000550;
        skos:definition  "Inorganic compounds containing an oxygen atom of an oxidation state of -2, in which the heaviest atom bonded to the oxygen is a halogen."@en;
        skos:inScheme    vlcs:chemische_stof;
        skos:notation    "CHEMONTID:0000550";
        skos:prefLabel   "Halogen oxides"@en .

csc:CHEMONTID_0000284
        rdf:type         skos:Concept;
        rdfs:seeAlso     tax_nodes:C0000284;
        skos:definition  "Organic compounds containing an aminobenzene moiety."@en;
        skos:inScheme    vlcs:chemische_stof;
        skos:notation    "CHEMONTID:0000284";
        skos:prefLabel   "Aniline and substituted anilines"@en .

csc:CHEMONTID_0001370
        rdf:type         skos:Concept;
        rdfs:seeAlso     tax_nodes:C0001370;
        skos:definition  "Organic compounds containing a metalloid atom."@en;
        skos:inScheme    vlcs:chemische_stof;
        skos:notation    "CHEMONTID:0001370";
        skos:prefLabel   "Organometalloid compounds"@en .

csc:CHEMONTID_0001888
        rdf:type         skos:Concept;
        rdfs:seeAlso     tax_nodes:C0001888;
        skos:definition  "Organic compounds containing a gamma-sultone, a Intramolecular cyclic ester of hydroxy sulfonic acid, with a SO ring bond, and three ring carbon atoms."@en;
        skos:inScheme    vlcs:chemische_stof;
        skos:notation    "CHEMONTID:0001888";
        skos:prefLabel   "Gamma sultones"@en .

csc:CHEMONTID_0002497
        rdf:type         skos:Concept;
        rdfs:seeAlso     tax_nodes:C0002497;
        skos:definition  "Compounds containing an indole moiety, which consists of pyrrole ring fused to benzene  to form 2,3-benzopyrrole."@en;
        skos:inScheme    vlcs:chemische_stof;
        skos:notation    "CHEMONTID:0002497";
        skos:prefLabel   "Indoles"@en .

csc:CHEMONTID_0000308
        rdf:type         skos:Concept;
        rdfs:seeAlso     tax_nodes:C0000308;
        skos:definition  "Organic compounds containing a benzene fused to a thiadiazine ring (a six-member ring with two nitrogen atoms and a sulfur atom)."@en;
        skos:inScheme    vlcs:chemische_stof;
        skos:notation    "CHEMONTID:0000308";
        skos:prefLabel   "Benzothiadiazines"@en .

csc:CHEMONTID_0001973
        rdf:type         skos:Concept;
        rdfs:seeAlso     tax_nodes:C0001973;
        skos:definition  "Organic compounds containing a benzene fused to an oxazole ring (a five-member aliphatic ring with three carbon atoms, one oxygen atom, and one nitrogen atom) bearing a ketone group."@en;
        skos:inScheme    vlcs:chemische_stof;
        skos:notation    "CHEMONTID:0001973";
        skos:prefLabel   "Benzoxazolones"@en .

csc:CHEMONTID_0001581
        rdf:type         skos:Concept;
        rdfs:seeAlso     tax_nodes:C0001581;
        skos:definition  "Compounds containing a piperidine ring which bears a ketone."@en;
        skos:inScheme    vlcs:chemische_stof;
        skos:notation    "CHEMONTID:0001581";
        skos:prefLabel   "Piperidinones"@en .

csc:CHEMONTID_0000001
        rdf:type           skos:Concept;
        rdfs:seeAlso       tax_nodes:C0000001;
        skos:definition    "Compounds that do not contain a C atom. Exceptions are made for isocyanide/cyanide and their non-hydrocarbyl derivatives, thiophosgene, carbon diselenide, carbon monosulfide, carbon disulfide, carbon subsulfide, carbon monoxide, carbon trioxide, carbon suboxide, and dicarbon monoxide."@en;
        skos:inScheme      vlcs:chemische_stof;
        skos:notation      "CHEMONTID:0000001";
        skos:prefLabel     "Inorganic compounds"@en;
        skos:topConceptOf  vlcs:chemische_stof .

cscl:class  rdf:type     xkos:ClassificationLevel;
        xkos:depth       "3"^^xsd:positiveInteger;
        skos:definition  "Classes typically consist of more spe-cific chemical categories with more specific and recogniz-able structural features (pyrimidine nucleosides, flavanols, benzazepines, actinide salts). Chemical Classes usually contain >100,000 known compounds. "@en;
        skos:inScheme    vlcs:chemische_stof;
        skos:member      csc:CHEMONTID_0000258 , csc:CHEMONTID_0002955 , csc:CHEMONTID_0000160 , csc:CHEMONTID_0000460 , csc:CHEMONTID_0000195 , csc:CHEMONTID_0001517 , csc:CHEMONTID_0002679 , csc:CHEMONTID_0003467 , csc:CHEMONTID_0001443 , csc:CHEMONTID_0003886 , csc:CHEMONTID_0000403 , csc:CHEMONTID_0000457 , csc:CHEMONTID_0000307 , csc:CHEMONTID_0000123 , csc:CHEMONTID_0000218 , csc:CHEMONTID_0004477 , csc:CHEMONTID_0000434 , csc:CHEMONTID_0000756 , csc:CHEMONTID_0001518 , csc:CHEMONTID_0000098 , csc:CHEMONTID_0000317 , csc:CHEMONTID_0001813 , csc:CHEMONTID_0003934 , csc:CHEMONTID_0000159 , csc:CHEMONTID_0000431 , csc:CHEMONTID_0000472 , csc:CHEMONTID_0001851 , csc:CHEMONTID_0000211 , csc:CHEMONTID_0000323 , csc:CHEMONTID_0001455 , csc:CHEMONTID_0000311 , csc:CHEMONTID_0000435 , csc:CHEMONTID_0000147 , csc:CHEMONTID_0000253 , csc:CHEMONTID_0002551 , csc:CHEMONTID_0000476 , csc:CHEMONTID_0002800 , csc:CHEMONTID_0000039 , csc:CHEMONTID_0001303 , csc:CHEMONTID_0001438 , csc:CHEMONTID_0000432 , csc:CHEMONTID_0002338 , csc:CHEMONTID_0001187 , csc:CHEMONTID_0002012 , csc:CHEMONTID_0001202 , csc:CHEMONTID_0000309 , csc:CHEMONTID_0001819 , csc:CHEMONTID_0001729 , csc:CHEMONTID_0004434 , csc:CHEMONTID_0002341 , csc:CHEMONTID_0000181 , csc:CHEMONTID_0002106 , csc:CHEMONTID_0001797 , csc:CHEMONTID_0001614 , csc:CHEMONTID_0001465 , csc:CHEMONTID_0002323 , csc:CHEMONTID_0004502 , csc:CHEMONTID_0000145 , csc:CHEMONTID_0000064 , csc:CHEMONTID_0001816 , csc:CHEMONTID_0002485 , csc:CHEMONTID_0002507 , csc:CHEMONTID_0000433 , csc:CHEMONTID_0000456 , csc:CHEMONTID_0002866 , csc:CHEMONTID_0000463 , csc:CHEMONTID_0001853 , csc:CHEMONTID_0002799 , csc:CHEMONTID_0002491 , csc:CHEMONTID_0000296 , csc:CHEMONTID_0001270 , csc:CHEMONTID_0000402 , csc:CHEMONTID_0000023 , csc:CHEMONTID_0000302 , csc:CHEMONTID_0000437 , csc:CHEMONTID_0000278 , csc:CHEMONTID_0000419 , csc:CHEMONTID_0000444 , csc:CHEMONTID_0001850 , csc:CHEMONTID_0003370 , csc:CHEMONTID_0001234 , csc:CHEMONTID_0002754 , csc:CHEMONTID_0000389 , csc:CHEMONTID_0000097 , csc:CHEMONTID_0000027 , csc:CHEMONTID_0000293 , csc:CHEMONTID_0003909 , csc:CHEMONTID_0001396 , csc:CHEMONTID_0000076 , csc:CHEMONTID_0000454 , csc:CHEMONTID_0000445 , csc:CHEMONTID_0001859 , csc:CHEMONTID_0000427 , csc:CHEMONTID_0004149 , csc:CHEMONTID_0003412 , csc:CHEMONTID_0004474 , csc:CHEMONTID_0000294 , csc:CHEMONTID_0000442 , csc:CHEMONTID_0001370 , csc:CHEMONTID_0000265 , csc:CHEMONTID_0001862 , csc:CHEMONTID_0001253 , csc:CHEMONTID_0003260 , csc:CHEMONTID_0000050 , csc:CHEMONTID_0002749 , csc:CHEMONTID_0002528 , csc:CHEMONTID_0004524 , csc:CHEMONTID_0000480 , csc:CHEMONTID_0000364 , csc:CHEMONTID_0001983 , csc:CHEMONTID_0004812 , csc:CHEMONTID_0000021 , csc:CHEMONTID_0002466 , csc:CHEMONTID_0003940 , csc:CHEMONTID_0000455 , csc:CHEMONTID_0001209 , csc:CHEMONTID_0003633 , csc:CHEMONTID_0000048 , csc:CHEMONTID_0004484 , csc:CHEMONTID_0000368 , csc:CHEMONTID_0000224 , csc:CHEMONTID_0001516 , csc:CHEMONTID_0000459 , csc:CHEMONTID_0002319 , csc:CHEMONTID_0000175 , csc:CHEMONTID_0000491 , csc:CHEMONTID_0000019 , csc:CHEMONTID_0000510 , csc:CHEMONTID_0000130 , csc:CHEMONTID_0002279 , csc:CHEMONTID_0000425 , csc:CHEMONTID_0000103 , csc:CHEMONTID_0004189 , csc:CHEMONTID_0000018 , csc:CHEMONTID_0000259 , csc:CHEMONTID_0004144 , csc:CHEMONTID_0000430 , csc:CHEMONTID_0004436 , csc:CHEMONTID_0003631 , csc:CHEMONTID_0000238 , csc:CHEMONTID_0000106 , csc:CHEMONTID_0002650 , csc:CHEMONTID_0000461 , csc:CHEMONTID_0001510 , csc:CHEMONTID_0000090 , csc:CHEMONTID_0003094 , csc:CHEMONTID_0002867 , csc:CHEMONTID_0000426 , csc:CHEMONTID_0004788 , csc:CHEMONTID_0000233 , csc:CHEMONTID_0000020 , csc:CHEMONTID_0000458 , csc:CHEMONTID_0002100 , csc:CHEMONTID_0002389 , csc:CHEMONTID_0003385 , csc:CHEMONTID_0001346 , csc:CHEMONTID_0001523 , csc:CHEMONTID_0000025 , csc:CHEMONTID_0002285 , csc:CHEMONTID_0002118 , csc:CHEMONTID_0000107 , csc:CHEMONTID_0000058 , csc:CHEMONTID_0004441 , csc:CHEMONTID_0000446 , csc:CHEMONTID_0001198 , csc:CHEMONTID_0000453 , csc:CHEMONTID_0001157 , csc:CHEMONTID_0000428 , csc:CHEMONTID_0000029 , csc:CHEMONTID_0004475 , csc:CHEMONTID_0000295 , csc:CHEMONTID_0002648 , csc:CHEMONTID_0000089 , csc:CHEMONTID_0004659 , csc:CHEMONTID_0002868 , csc:CHEMONTID_0002506 , csc:CHEMONTID_0000301 , csc:CHEMONTID_0000315 , csc:CHEMONTID_0002566 , csc:CHEMONTID_0002865 , csc:CHEMONTID_0001515 , csc:CHEMONTID_0000134 , csc:CHEMONTID_0002490 , csc:CHEMONTID_0000436 , csc:CHEMONTID_0000429 , csc:CHEMONTID_0002693 , csc:CHEMONTID_0001506 , csc:CHEMONTID_0000305;
        skos:prefLabel   "Klasse"@nl .

csc:CHEMONTID_0001816
        rdf:type         skos:Concept;
        rdfs:seeAlso     tax_nodes:C0001816;
        skos:definition  "Organic compounds containing a two furan rings fused to each other. Furan is a five-membered aromatic ring with four carbon atoms and one oxygen atom."@en;
        skos:inScheme    vlcs:chemische_stof;
        skos:notation    "CHEMONTID:0001816";
        skos:prefLabel   "Furofurans"@en .

csc:CHEMONTID_0000423
        rdf:type         skos:Concept;
        rdfs:seeAlso     tax_nodes:C0000423;
        skos:definition  "Inorganic compounds that contain only metal elements."@en;
        skos:inScheme    vlcs:chemische_stof;
        skos:notation    "CHEMONTID:0000423";
        skos:prefLabel   "Homogeneous non-metal compounds"@en .

csc:CHEMONTID_0000031
        rdf:type         skos:Concept;
        rdfs:seeAlso     tax_nodes:C0000031;
        skos:definition  "Organic compounds containing a sulfonamide group that is S-linked to a benzene ring."@en;
        skos:inScheme    vlcs:chemische_stof;
        skos:notation    "CHEMONTID:0000031";
        skos:prefLabel   "Benzenesulfonamides"@en .

csc:CHEMONTID_0001158
        rdf:type         skos:Concept;
        rdfs:seeAlso     tax_nodes:C0001158;
        skos:definition  "Compounds containing a pyrrolidine ring which bears a C=O group."@en;
        skos:inScheme    vlcs:chemische_stof;
        skos:notation    "CHEMONTID:0001158";
        skos:prefLabel   "Pyrrolidones"@en .

csc:CHEMONTID_0000549
        rdf:type         skos:Concept;
        rdfs:seeAlso     tax_nodes:C0000549;
        skos:definition  "Inorganic compounds of nitrogen where nitrogen has a formal oxidation state of -3, and the heaviest atom bonded to it is a halogen."@en;
        skos:inScheme    vlcs:chemische_stof;
        skos:notation    "CHEMONTID:0000549";
        skos:prefLabel   "Halogen nitrides"@en .

csc:CHEMONTID_0002902
        rdf:type         skos:Concept;
        rdfs:seeAlso     tax_nodes:C0002902;
        skos:definition  "A group of macrolides with a structure containing a 16-membered lactone ring fused to a 1,7-dioxaspiroundecane ring system and to either a benzofuran (or hydrogenated derivative thereof). In some cases (e.g. Milbemycin E), the tetrahydrofuranyl ring is missing. Milbemycins can be o-glycosylated at C13 to form Avermectins. Milbemycins are produced by Streptomyces species."@en;
        skos:inScheme    vlcs:chemische_stof;
        skos:notation    "CHEMONTID:0002902";
        skos:prefLabel   "Milbemycins"@en .

csc:CHEMONTID_0001243
        rdf:type         skos:Concept;
        rdfs:seeAlso     tax_nodes:C0001243;
        skos:definition  "Organic compounds containing a four-member lactone (a cyclic ester)."@en;
        skos:inScheme    vlcs:chemische_stof;
        skos:notation    "CHEMONTID:0001243";
        skos:prefLabel   "Beta propiolactones"@en .

csc:CHEMONTID_0000368
        rdf:type         skos:Concept;
        rdfs:seeAlso     tax_nodes:C0000368;
        skos:definition  "Compounds containing a dioxane ring, which is a six-membered saturated ring of two oxygen atoms and four carbon atoms. The dioxanes are divided in 1,2-dioxanes, 1,3-dioxanes, and 1,4-dioxanes."@en;
        skos:inScheme    vlcs:chemische_stof;
        skos:notation    "CHEMONTID:0000368";
        skos:prefLabel   "Dioxanes"@en .

list:class  rdf:type    rdf:List;
        rdf:first       cscl:class;
        rdf:rest        list:subclass;
        skos:prefLabel  "Niveau klasse"@nl .

csc:CHEMONTID_0001062
        rdf:type         skos:Concept;
        rdfs:seeAlso     tax_nodes:C0001062;
        skos:definition  "Inorganic non-metallic compoundscontaining a nitrate as its largest oxoanion."@en;
        skos:inScheme    vlcs:chemische_stof;
        skos:notation    "CHEMONTID:0001062";
        skos:prefLabel   "Non-metal nitrates"@en .

csc:CHEMONTID_0000453
        rdf:type         skos:Concept;
        rdfs:seeAlso     tax_nodes:C0000453;
        skos:definition  "Inorganic compounds belonging to either of the other non-metal Hydrides, other non-metal nitrides, other non-metal oxides, or the other non-metal sulfides."@en;
        skos:inScheme    vlcs:chemische_stof;
        skos:notation    "CHEMONTID:0000453";
        skos:prefLabel   "Other non-metal organides"@en .

csc:CHEMONTID_0004150
        rdf:type         skos:Concept;
        rdfs:seeAlso     tax_nodes:C0004150;
        skos:definition  "Derivatives of hydrocarbons obtained by substituting one or more carbon atoms by an heteroatom. They contain at least one carbon atom and heteroatom."@en;
        skos:inScheme    vlcs:chemische_stof;
        skos:notation    "CHEMONTID:0004150";
        skos:prefLabel   "Hydrocarbon derivatives"@en .

csc:CHEMONTID_0000398
        rdf:type         skos:Concept;
        rdfs:seeAlso     tax_nodes:C0000398;
        skos:definition  "Compounds having two beta-haloalkyl groups bound to a nitrogen atom."@en;
        skos:inScheme    vlcs:chemische_stof;
        skos:notation    "CHEMONTID:0000398";
        skos:prefLabel   "Nitrogen mustard compounds"@en .

csc:CHEMONTID_0002485
        rdf:type         skos:Concept;
        rdfs:seeAlso     tax_nodes:C0002485;
        skos:definition  "Organic compounds containing a functional group with the structure RSH (R = organyl)."@en;
        skos:inScheme    vlcs:chemische_stof;
        skos:notation    "CHEMONTID:0002485";
        skos:prefLabel   "Thiols"@en .

csc:CHEMONTID_0003094
        rdf:type         skos:Concept;
        rdfs:seeAlso     tax_nodes:C0003094;
        skos:definition  "Organic heterocyclic compounds containing a six-membered saturated heterocycle with two nitrogen, one sulfur, and three carbon atoms."@en;
        skos:inScheme    vlcs:chemische_stof;
        skos:notation    "CHEMONTID:0003094";
        skos:prefLabel   "Thiadiazinanes"@en .

csc:CHEMONTID_0001961
        rdf:type         skos:Concept;
        rdfs:seeAlso     tax_nodes:C0001961;
        skos:definition  "Natural or synthetic compounds having sequences of amino and hydroxy carboxylic acid residues (usually α-amino and α-hydroxy acids), commonly but not necessarily regularly alternating."@en;
        skos:inScheme    vlcs:chemische_stof;
        skos:notation    "CHEMONTID:0001961";
        skos:prefLabel   "Depsipeptides"@en .

csc:CHEMONTID_0000326
        rdf:type         skos:Concept;
        rdfs:seeAlso     tax_nodes:C0000326;
        skos:definition  "Organic compounds containing two pyridine rings linked to each other."@en;
        skos:inScheme    vlcs:chemische_stof;
        skos:notation    "CHEMONTID:0000326";
        skos:prefLabel   "Bipyridines and oligopyridines"@en .

csc:CHEMONTID_0001804
        rdf:type         skos:Concept;
        rdfs:seeAlso     tax_nodes:C0001804;
        skos:definition  "Organic compounds containing the pyrophosphate oxoanion, with the structure OP([O-])(=O)OP(O)([O-])=O."@en;
        skos:inScheme    vlcs:chemische_stof;
        skos:notation    "CHEMONTID:0001804";
        skos:prefLabel   "Organic pyrophosphates"@en .

csc:CHEMONTID_0004149
        rdf:type         skos:Concept;
        rdfs:seeAlso     tax_nodes:C0004149;
        skos:definition  "Polycyclic organic compounds made up only of carbon and hydrogen atoms."@en;
        skos:inScheme    vlcs:chemische_stof;
        skos:notation    "CHEMONTID:0004149";
        skos:prefLabel   "Polycyclic hydrocarbons"@en .

csc:CHEMONTID_0000411
        rdf:type         skos:Concept;
        rdfs:seeAlso     tax_nodes:C0000411;
        skos:definition  "Compounds containing the oxime functional group, with the general structure R1(R2)C=NOH."@en;
        skos:inScheme    vlcs:chemische_stof;
        skos:notation    "CHEMONTID:0000411";
        skos:prefLabel   "Oximes"@en .

csc:CHEMONTID_0000145
        rdf:type         skos:Concept;
        rdfs:seeAlso     tax_nodes:C0000145;
        skos:definition  "Polycyclic aromatic compounds containing a 1-benzopyran moiety with a ketone group at the C2 carbon atom (1-benzopyran-2-one)."@en;
        skos:inScheme    vlcs:chemische_stof;
        skos:notation    "CHEMONTID:0000145";
        skos:prefLabel   "Coumarins and derivatives"@en .

csc:CHEMONTID_0004711
        rdf:type         skos:Concept;
        rdfs:seeAlso     tax_nodes:C0004711;
        skos:definition  "Aromatic heteropolycyclic compounds that contain a carbamic acid ester group, which is N-linked to the C2-atom of a benzimidazole moiety."@en;
        skos:inScheme    vlcs:chemische_stof;
        skos:notation    "CHEMONTID:0004711";
        skos:prefLabel   "2-benzimidazolylcarbamic acid esters"@en .

csc:CHEMONTID_0000175
        rdf:type         skos:Concept;
        rdfs:seeAlso     tax_nodes:C0000175;
        skos:definition  "Lipids formed by joining fatty acids to glycerol by ester bonds."@en;
        skos:inScheme    vlcs:chemische_stof;
        skos:notation    "CHEMONTID:0000175";
        skos:prefLabel   "Glycerolipids"@en .

csc:CHEMONTID_0004475
        rdf:type         skos:Concept;
        rdfs:seeAlso     tax_nodes:C0004475;
        skos:definition  "Hydrocarbons that contains one or more unsaturated carbon atoms. These compounds contain one or more double, triple, or aromatic bonds."@en;
        skos:inScheme    vlcs:chemische_stof;
        skos:notation    "CHEMONTID:0004475";
        skos:prefLabel   "Unsaturated hydrocarbons"@en .

csc:CHEMONTID_0002865
        rdf:type         skos:Concept;
        rdfs:seeAlso     tax_nodes:C0002865;
        skos:definition  "Organic compounds with the general structure RC(=O)X, where X is a halogen atom."@en;
        skos:inScheme    vlcs:chemische_stof;
        skos:notation    "CHEMONTID:0002865";
        skos:prefLabel   "Acyl halides"@en .

csc:CHEMONTID_0004107
        rdf:type         skos:Concept;
        rdfs:seeAlso     tax_nodes:C0004107;
        skos:definition  "Compounds containing a triazine ring, which is a heterocyclic ring, similar to the six-member benzene ring but with three carbons replaced by nitrogen atoms, at ring positions 1, 2, and 4."@en;
        skos:inScheme    vlcs:chemische_stof;
        skos:notation    "CHEMONTID:0004107";
        skos:prefLabel   "1,2,4-triazines"@en .

csc:CHEMONTID_0000018
        rdf:type         skos:Concept;
        rdfs:seeAlso     tax_nodes:C0000018;
        skos:definition  "Organic compounds containing a system of three linearly fused benzene rings."@en;
        skos:inScheme    vlcs:chemische_stof;
        skos:notation    "CHEMONTID:0000018";
        skos:prefLabel   "Anthracenes"@en .

csc:CHEMONTID_0000103
        rdf:type         skos:Concept;
        rdfs:seeAlso     tax_nodes:C0000103;
        skos:definition  "Organic compounds containing a saturated three-member heterocycle with one amino group and two methylene groups."@en;
        skos:inScheme    vlcs:chemische_stof;
        skos:notation    "CHEMONTID:0000103";
        skos:prefLabel   "Aziridines"@en .

csc:CHEMONTID_0000229
        rdf:type         skos:Concept;
        rdfs:seeAlso     tax_nodes:C0000229;
        skos:definition  "Heterocyclic compounds containing a five-member unsaturated aliphatic ring with one nitrogen atom, one sulfur atom, three carbon atoms."@en;
        skos:inScheme    vlcs:chemische_stof;
        skos:notation    "CHEMONTID:0000229";
        skos:prefLabel   "Thiazolines"@en .

csc:CHEMONTID_0003981
        rdf:type         skos:Concept;
        rdfs:seeAlso     tax_nodes:C0003981;
        skos:definition  "Organic compounds containing  a benzene skeleton substituted with a halomethyl group."@en;
        skos:inScheme    vlcs:chemische_stof;
        skos:notation    "CHEMONTID:0003981";
        skos:prefLabel   "Benzyl halides"@en .

csc:CHEMONTID_0000048
        rdf:type         skos:Concept;
        rdfs:seeAlso     tax_nodes:C0000048;
        skos:definition  "Polycyclic aromatic compounds containing a tetralin moiety, which consists of a benzene fused to a cyclohexane."@en;
        skos:inScheme    vlcs:chemische_stof;
        skos:notation    "CHEMONTID:0000048";
        skos:prefLabel   "Tetralins"@en .

csc:CHEMONTID_0000525
        rdf:type         skos:Concept;
        rdfs:seeAlso     tax_nodes:C0000525;
        skos:definition  "Inorganic compounds of nitrogen where nitrogen has a formal oxidation state of -3, and the heaviest metal atom is an alkali metal."@en;
        skos:inScheme    vlcs:chemische_stof;
        skos:notation    "CHEMONTID:0000525";
        skos:prefLabel   "Alkali metal nitrides"@en .

csc:CHEMONTID_0000259
        rdf:type         skos:Concept;
        rdfs:seeAlso     tax_nodes:C0000259;
        skos:definition  "Lipids synthesized from the five-carbon-unit precursors isopentenyl diphosphate and dimethylallyl diphosphate."@en;
        skos:inScheme    vlcs:chemische_stof;
        skos:notation    "CHEMONTID:0000259";
        skos:prefLabel   "Prenol lipids"@en .

csc:CHEMONTID_0000078
        rdf:type         skos:Concept;
        rdfs:seeAlso     tax_nodes:C0000078;
        skos:definition  "Compounds containing an imidazole ring, which is an aromatic five-member ring with two nitrogen atoms at positions 1 and 3, and three carbon atoms."@en;
        skos:inScheme    vlcs:chemische_stof;
        skos:notation    "CHEMONTID:0000078";
        skos:prefLabel   "Imidazoles"@en .

csc:CHEMONTID_0000555
        rdf:type         skos:Concept;
        rdfs:seeAlso     tax_nodes:C0000555;
        skos:definition  "Inorganic compounds containing a sulfur atom of an oxidation state of -2, in which the heaviest atom bonded to the oxygen belongs to the class of other non-metals."@en;
        skos:inScheme    vlcs:chemische_stof;
        skos:notation    "CHEMONTID:0000555";
        skos:prefLabel   "Other non-metal sulfides"@en .

csc:CHEMONTID_0000163
        rdf:type         skos:Concept;
        rdfs:seeAlso     tax_nodes:C0000163;
        skos:definition  "Cyclic amides of caproic acid. Caproic acid is the carboxylic acid derived from hexane with the general formula C5H11COOH."@en;
        skos:inScheme    vlcs:chemische_stof;
        skos:notation    "CHEMONTID:0000163";
        skos:prefLabel   "Caprolactams"@en .

csc:CHEMONTID_0000640
        rdf:type         skos:Concept;
        rdfs:seeAlso     tax_nodes:C0000640;
        skos:definition  "Inorganic compounds in which the largest oxoanion is hypochlorite, and in which the heaviest atom not in an oxoanion is an alkali metal."@en;
        skos:inScheme    vlcs:chemische_stof;
        skos:notation    "CHEMONTID:0000640";
        skos:prefLabel   "Alkali metal hypochlorites"@en .

csc:CHEMONTID_0000289
        rdf:type         skos:Concept;
        rdfs:seeAlso     tax_nodes:C0000289;
        skos:definition  "Compounds containing a nucleobase linked to a ribose or deoxyribose sugar via a beta-glycosidic linkage. The ribose or deoxyribose moiety bears at least a phosphate group in case of nucleotides."@en;
        skos:inScheme    vlcs:chemische_stof;
        skos:notation    "CHEMONTID:0000289";
        skos:prefLabel   "Nucleosides, nucleotides, and analogues"@en .

csc:CHEMONTID_0001460
        rdf:type         skos:Concept;
        rdfs:seeAlso     tax_nodes:C0001460;
        skos:definition  "Compounds containing a secosteroid backbone, usually secoergostane or secocholestane."@en;
        skos:inScheme    vlcs:chemische_stof;
        skos:notation    "CHEMONTID:0001460";
        skos:prefLabel   "Vitamin D and derivatives"@en .

csc:CHEMONTID_0001194
        rdf:type         skos:Concept;
        rdfs:seeAlso     tax_nodes:C0001194;
        skos:definition  "Steroid derivatives carrying a C=O group attached to steroid skeleton."@en;
        skos:inScheme    vlcs:chemische_stof;
        skos:notation    "CHEMONTID:0001194";
        skos:prefLabel   "Oxosteroids"@en .

csc:CHEMONTID_0002798
        rdf:type         skos:Concept;
        rdfs:seeAlso     tax_nodes:C0002798;
        skos:definition  "Triazinanes having three nitrogen ring atoms at the 1-, 3-, and 5- positions."@en;
        skos:inScheme    vlcs:chemische_stof;
        skos:notation    "CHEMONTID:0002798";
        skos:prefLabel   "1,3,5-triazinanes"@en .

csc:CHEMONTID_0001797
        rdf:type         skos:Concept;
        rdfs:seeAlso     tax_nodes:C0001797;
        skos:definition  "Organic polycyclic compounds containing an imidazole ring fused to a pyrimidine ring. Imidazole is 5-membered ring consisting of three carbon atoms, and two nitrogen centers at the 1- and 3-positions. Pyrimidine is a 6-membered ring consisting of four carbon atoms and two nitrogen centers at the 1- and 3- ring positions."@en;
        skos:inScheme    vlcs:chemische_stof;
        skos:notation    "CHEMONTID:0001797";
        skos:prefLabel   "Imidazopyrimidines"@en .

csc:CHEMONTID_0002491
        rdf:type         skos:Concept;
        rdfs:seeAlso     tax_nodes:C0002491;
        skos:definition  "Azole derivatives obtained by conversion of both double bonds of the azole ring to single bonds, yielding a saturated ring."@en;
        skos:inScheme    vlcs:chemische_stof;
        skos:notation    "CHEMONTID:0002491";
        skos:prefLabel   "Azolidines"@en .

csc:CHEMONTID_0001303
        rdf:type         skos:Concept;
        rdfs:seeAlso     tax_nodes:C0001303;
        skos:definition  "Organic compounds containing the thiophosphoric acid functional group or a derivative thereof, with the general structure RP(R')(R'')=S, where R,R',R'' = O,N, halogen residue."@en;
        skos:inScheme    vlcs:chemische_stof;
        skos:notation    "CHEMONTID:0001303";
        skos:prefLabel   "Organic thiophosphoric acids and derivatives"@en .

csc:CHEMONTID_0000302
        rdf:type         skos:Concept;
        rdfs:seeAlso     tax_nodes:C0000302;
        skos:definition  "Organic compounds containing a benzene fused to an oxazole ring Oxazole is five-membered aromatic ring with a nitrogen and an oxygen atoms at the 1- and 3-position, respectively."@en;
        skos:inScheme    vlcs:chemische_stof;
        skos:notation    "CHEMONTID:0000302";
        skos:prefLabel   "Benzoxazoles"@en .

csc:CHEMONTID_0000428
        rdf:type         skos:Concept;
        rdfs:seeAlso     tax_nodes:C0000428;
        skos:definition  "Inorganic compounds containing only metal atoms,with the largest atom being a alkaline earth metal atom."@en;
        skos:inScheme    vlcs:chemische_stof;
        skos:notation    "CHEMONTID:0000428";
        skos:prefLabel   "Homogeneous alkaline earth metal compounds"@en .

csc:CHEMONTID_0000036
        rdf:type         skos:Concept;
        rdfs:seeAlso     tax_nodes:C0000036;
        skos:definition  "Compounds containing a nitrobenzene moiety, which consists of a benzene ring with a carbon bearing a nitro group."@en;
        skos:inScheme    vlcs:chemische_stof;
        skos:notation    "CHEMONTID:0000036";
        skos:prefLabel   "Nitrobenzenes"@en .

csc:CHEMONTID_0002811
        rdf:type         skos:Concept;
        rdfs:seeAlso     tax_nodes:C0002811;
        skos:definition  "Organic compounds containing a phenylpropane moiety."@en;
        skos:inScheme    vlcs:chemische_stof;
        skos:notation    "CHEMONTID:0002811";
        skos:prefLabel   "Phenylpropanes"@en .

csc:CHEMONTID_0000458
        rdf:type         skos:Concept;
        rdfs:seeAlso     tax_nodes:C0000458;
        skos:definition  "Inorganic compounds belonging either to the post-transition metal hydrides, post-transition metal nitrides, post-transition metal oxides, or the post-transition metal sulfides."@en;
        skos:inScheme    vlcs:chemische_stof;
        skos:notation    "CHEMONTID:0000458";
        skos:prefLabel   "Post-transition metal organides"@en .

csc:CHEMONTID_0004155
        rdf:type         skos:Concept;
        rdfs:seeAlso     tax_nodes:C0004155;
        skos:definition  "Aromatic compounds containing two benzene rings linked to each other through an ether group."@en;
        skos:inScheme    vlcs:chemische_stof;
        skos:notation    "CHEMONTID:0004155";
        skos:prefLabel   "Diphenylethers"@en .

csc:CHEMONTID_0001544
        rdf:type         skos:Concept;
        rdfs:seeAlso     tax_nodes:C0001544;
        skos:definition  "Nucleotides consisting of a purine base linked to a ribose to which at least one phosphate group is attached."@en;
        skos:inScheme    vlcs:chemische_stof;
        skos:notation    "CHEMONTID:0001544";
        skos:prefLabel   "Purine ribonucleotides"@en .

csc:CHEMONTID_0001152
        rdf:type         skos:Concept;
        rdfs:seeAlso     tax_nodes:C0001152;
        skos:definition  "Compounds having the nitro group, -NO2 (free valence on nitrogen), which may be attached to carbon, nitrogen (as in nitramines), or oxygen (as in nitrates), among other elements (in the absence of specification, C-nitro compounds are usually implied)."@en;
        skos:inScheme    vlcs:chemische_stof;
        skos:notation    "CHEMONTID:0001152";
        skos:prefLabel   "Organic nitro compounds"@en .

csc:CHEMONTID_0000151
        rdf:type         skos:Concept;
        rdfs:seeAlso     tax_nodes:C0000151;
        skos:definition  "Organic compounds containing either anthracene-9,10-quinone, 1,4-anthraquinone, or 1,2-anthraquinone."@en;
        skos:inScheme    vlcs:chemische_stof;
        skos:notation    "CHEMONTID:0000151";
        skos:prefLabel   "Anthraquinones"@en .

csc:CHEMONTID_0002279
        rdf:type         skos:Concept;
        rdfs:seeAlso     tax_nodes:C0002279;
        skos:definition  "Aromatic compounds containing one monocyclic ring system consisting of benzene."@en;
        skos:inScheme    vlcs:chemische_stof;
        skos:notation    "CHEMONTID:0002279";
        skos:prefLabel   "Benzene and substituted derivatives"@en .

csc:CHEMONTID_0003631
        rdf:type         skos:Concept;
        rdfs:seeAlso     tax_nodes:C0003631;
        skos:definition  "Organic 1,3-dipolar compounds with the general structure  X=Y+-Z- <-> X--Y+=Z<-> X+-Y-Z-<-> X-=Y-Z+ (X, Z = C, N, or O; Y = N or O)."@en;
        skos:inScheme    vlcs:chemische_stof;
        skos:notation    "CHEMONTID:0003631";
        skos:prefLabel   "Allyl-type 1,3-dipolar organic compounds"@en .

csc:CHEMONTID_0004632
        rdf:type         skos:Concept;
        rdfs:seeAlso     tax_nodes:C0004632;
        skos:definition  "Organosulfur compounds containing a sulfoxide group substituted with a phenyl group."@en;
        skos:inScheme    vlcs:chemische_stof;
        skos:notation    "CHEMONTID:0004632";
        skos:prefLabel   "Phenyl sulfoxides"@en .

csc:CHEMONTID_0004758
        rdf:type         skos:Concept;
        rdfs:seeAlso     tax_nodes:C0004758;
        skos:definition  "Aromatic heterocyclic compounds containing a furan ring, which carries a carboxyl group or a derivative thereof."@en;
        skos:inScheme    vlcs:chemische_stof;
        skos:notation    "CHEMONTID:0004758";
        skos:prefLabel   "Furoic acid and derivatives"@en .

csc:CHEMONTID_0001097
        rdf:type         skos:Concept;
        rdfs:seeAlso     tax_nodes:C0001097;
        skos:definition  "Organic compounds containing a carbonyl group substituted with a benzyloxyl group."@en;
        skos:inScheme    vlcs:chemische_stof;
        skos:notation    "CHEMONTID:0001097";
        skos:prefLabel   "Benzyloxycarbonyls"@en .

csc:CHEMONTID_0000181
        rdf:type         skos:Concept;
        rdfs:seeAlso     tax_nodes:C0000181;
        skos:definition  "Polyketides having an octahydrotetracene-2-carboxamide skeleton, substituted with many hydroxy and other groups."@en;
        skos:inScheme    vlcs:chemische_stof;
        skos:notation    "CHEMONTID:0000181";
        skos:prefLabel   "Tetracyclines"@en .

csc:CHEMONTID_0004788
        rdf:type         skos:Concept;
        rdfs:seeAlso     tax_nodes:C0004788;
        skos:definition  "Aromatic heterocyclic chemical compounds containing a naphthalene derivative, where two carbon atoms are replaced by nitrogen atoms. They are subdivided in benzodiazines and naphthyridines."@en;
        skos:inScheme    vlcs:chemische_stof;
        skos:notation    "CHEMONTID:0004788";
        skos:prefLabel   "Diazanaphthalenes"@en .

csc:CHEMONTID_0000392
        rdf:type         skos:Concept;
        rdfs:seeAlso     tax_nodes:C0000392;
        skos:definition  "Organic compounds containing a morpholine moiety, which consists of a six-member aliphatic saturated ring with the formula C4H9NO, where the oxygen and nitrogen atoms lie at positions 1 and 4, respectively."@en;
        skos:inScheme    vlcs:chemische_stof;
        skos:notation    "CHEMONTID:0000392";
        skos:prefLabel   "Morpholines"@en .

csc:CHEMONTID_0003480
        rdf:type         skos:Concept;
        rdfs:seeAlso     tax_nodes:C0003480;
        skos:definition  "Compound containing an ester derivative of cinnamic acid."@en;
        skos:inScheme    vlcs:chemische_stof;
        skos:notation    "CHEMONTID:0003480";
        skos:prefLabel   "Cinnamic acid esters"@en .

csc:CHEMONTID_0004113
        rdf:type         skos:Concept;
        rdfs:seeAlso     tax_nodes:C0004113;
        skos:definition  "Organic aromatic compounds containing a monocyclic benzene moiety carrying exactly or one more methoxy groups."@en;
        skos:inScheme    vlcs:chemische_stof;
        skos:notation    "CHEMONTID:0004113";
        skos:prefLabel   "Methoxybenzenes"@en .

csc:CHEMONTID_0000501
        rdf:type         skos:Concept;
        rdfs:seeAlso     tax_nodes:C0000501;
        skos:definition  "Organic compounds containing the isocyanic acid tautomer, HN=C=O, of cyanic acid, HOC#N or its hydrocarbyl derivatives RN=C=O."@en;
        skos:inScheme    vlcs:chemische_stof;
        skos:notation    "CHEMONTID:0000501";
        skos:prefLabel   "Isocyanates"@en .

csc:CHEMONTID_0003449
        rdf:type         skos:Concept;
        rdfs:seeAlso     tax_nodes:C0003449;
        skos:definition  "Compounds containing a pyrrolidine moiety that is substituted at the N1-position with an alkyl group. Pyrrolidine is a five-membered saturated aliphatic heterocycle with one nitrogen atom and four carbon atoms."@en;
        skos:inScheme    vlcs:chemische_stof;
        skos:notation    "CHEMONTID:0003449";
        skos:prefLabel   "N-alkylpyrrolidines"@en .

csc:CHEMONTID_0000320
        rdf:type         skos:Concept;
        rdfs:seeAlso     tax_nodes:C0000320;
        skos:definition  "Compounds with two benzene rings connected by an azepine ring. Azepine is an unsaturated seven-member heterocycle with one nitrogen atom replacing a carbon atom."@en;
        skos:inScheme    vlcs:chemische_stof;
        skos:notation    "CHEMONTID:0000320";
        skos:prefLabel   "Dibenzazepines"@en .

csc:CHEMONTID_0002448
        rdf:type         skos:Concept;
        rdfs:seeAlso     tax_nodes:C0002448;
        skos:definition  "Aromatic compounds containing one or more benzene rings."@en;
        skos:inScheme    vlcs:chemische_stof;
        skos:notation    "CHEMONTID:0002448";
        skos:prefLabel   "Benzenoids"@en .

csc:CHEMONTID_0001055
        rdf:type         skos:Concept;
        rdfs:seeAlso     tax_nodes:C0001055;
        skos:definition  "Inorganic non-metallic compounds containing the hydroxide group as its largest oxoanion."@en;
        skos:inScheme    vlcs:chemische_stof;
        skos:notation    "CHEMONTID:0001055";
        skos:prefLabel   "Non-metal hydroxides"@en .

csc:CHEMONTID_0000446
        rdf:type         skos:Concept;
        rdfs:seeAlso     tax_nodes:C0000446;
        skos:definition  "Inorganic oxoanionic compounds in which the heaviest atom not in an oxoanion is an alkaline earth metal."@en;
        skos:inScheme    vlcs:chemische_stof;
        skos:notation    "CHEMONTID:0000446";
        skos:prefLabel   "Alkaline earth metal oxoanionic compounds"@en .
