@prefix :      <https://data.omgeving.vlaanderen.be/id/concept/chemische_stof/ChemOnt.owl#> .
@prefix tax_nodes: <http://classyfire.wishartlab.com/tax_nodes/> .
@prefix owl:   <http://www.w3.org/2002/07/owl#> .
@prefix xsd:   <http://www.w3.org/2001/XMLSchema#> .
@prefix skos:  <http://www.w3.org/2004/02/skos/core#> .
@prefix rdfs:  <http://www.w3.org/2000/01/rdf-schema#> .
@prefix omg_dataset: <https://data.omgeving.vlaanderen.be/id/dataset/> .
@prefix vlcs:  <https://data.omgeving.vlaanderen.be/id/conceptscheme/> .
@prefix cosc:  <https://data.omgeving.vlaanderen.be/id/collection/chemische_stof/> .
@prefix wise:  <http://dd.eionet.europa.eu/vocabulary/wise/ObservedProperty/> .
@prefix dct:   <http://purl.org/dc/terms/> .
@prefix wk:    <https://data.omgeving.vlaanderen.be/ns/wk#> .
@prefix xml:   <http://www.w3.org/XML/1998/namespace> .
@prefix vcs:   <https://data.vlaanderen.be/ns/chemische_stof#> .
@prefix list:  <https://data.omgeving.vlaanderen.be/id/list/chemische_stof/> .
@prefix co:    <https://data.omgeving.vlaanderen.be/id/concept/observatieprocedure/> .
@prefix compound: <https://pubchem.ncbi.nlm.nih.gov/compound/> .
@prefix xkos:  <http://rdf-vocabulary.ddialliance.org/xkos#> .
@prefix dbo:   <http://dbpedia.org/ontology/> .
@prefix cs:    <https://data.vlaanderen.be/ns/chemische_stof#> .
@prefix csc:   <https://data.omgeving.vlaanderen.be/id/concept/chemische_stof/> .
@prefix dbp:   <http://dbpedia.org/property/> .
@prefix rdf:   <http://www.w3.org/1999/02/22-rdf-syntax-ns#> .
@prefix cscl:  <https://data.omgeving.vlaanderen.be/id/classificationlevel/chemische_stof/> .
@prefix dc:    <http://purl.org/dc/elements/1.1/> .

csc:CHEMONTID_0000274
        a                skos:Concept ;
        skos:altLabel    "acridines"@en ;
        skos:broader     csc:CHEMONTID_0001908 ;
        skos:definition  "Organic compounds containing the acridine moiety, a linear tricyclic heterocycle which consists of two benzene rings joined by a pyridine ring."@en ;
        skos:inScheme    vlcs:chemische_stof ;
        skos:notation    "CHEMONTID:0000274" ;
        skos:prefLabel   "Acridines"@en .

csc:CHEMONTID_0000021
        a                skos:Concept ;
        rdfs:seeAlso     tax_nodes:C0000021 ;
        skos:altLabel    "indene"@en ;
        skos:broader     csc:CHEMONTID_0002448 ;
        skos:definition  "Compounds containing an indene moiety(which consists of a cyclopentadiene fused to a benzene ring), or a isoindene moiety (which consists of a cyclopentadiene fused to cyclohexadiene ring)."@en ;
        skos:inScheme    vlcs:chemische_stof ;
        skos:notation    "CHEMONTID:0000021" ;
        skos:prefLabel   "Indenes and isoindenes"@en .

csc:CHEMONTID_0004066
        a                skos:Concept ;
        skos:broader     csc:CHEMONTID_0001524 ;
        skos:definition  "Compounds containing a tin compound bonded to exactly three carbon atoms."@en ;
        skos:inScheme    vlcs:chemische_stof ;
        skos:notation    "CHEMONTID:0004066" ;
        skos:prefLabel   "Triorganotin compounds"@en .

csc:CHEMONTID_0004785
        a                skos:Concept ;
        rdfs:seeAlso     tax_nodes:C0004785 ;
        skos:broader     csc:CHEMONTID_0000253 ;
        skos:definition  "Stilbenes that carry a sulfone group at one or more positions of either benzene rings."@en ;
        skos:inScheme    vlcs:chemische_stof ;
        skos:notation    "CHEMONTID:0004785" ;
        skos:prefLabel   "Sulfonated stilbenes"@en .

csc:CHEMONTID_0001179
        a                skos:Concept ;
        skos:altLabel    "organosulfonic acid"@en , "sulfonic acids"@en , "Sulfonic Acids"@en ;
        skos:broader     csc:CHEMONTID_0000270 ;
        skos:definition  "Compounds containing the sulfonic acid group, which has the general structure RS(=O)2OH (R is not a hydrogen atom)."@en ;
        skos:inScheme    vlcs:chemische_stof ;
        skos:notation    "CHEMONTID:0001179" ;
        skos:prefLabel   "Organosulfonic acids"@en .

csc:CHEMONTID_0004532
        a                skos:Concept ;
        skos:broader     csc:CHEMONTID_0003970 ;
        skos:definition  "Organic compounds containing a pyridine ring substituted at the 2-position by a halogen atom."@en ;
        skos:inScheme    vlcs:chemische_stof ;
        skos:notation    "CHEMONTID:0004532" ;
        skos:prefLabel   "2-halopyridines"@en .

csc:CHEMONTID_0001470
        a                skos:Concept ;
        rdfs:seeAlso     tax_nodes:C0001470 ;
        skos:broader     csc:CHEMONTID_0001270 ;
        skos:definition  "Inorganic compounds containing a metallic oxoanion to which either no atom or a non metal atom is bonded."@en ;
        skos:inScheme    vlcs:chemische_stof ;
        skos:notation    "CHEMONTID:0001470" ;
        skos:prefLabel   "Miscellaneous metallic oxoanionic compounds"@en .

csc:CHEMONTID_0004707
        a                skos:Concept ;
        rdfs:seeAlso     tax_nodes:C0004707 ;
        skos:broader     csc:CHEMONTID_0000000 ;
        skos:definition  "Organic compounds containing a nitrogen atom."@en ;
        skos:inScheme    vlcs:chemische_stof ;
        skos:notation    "CHEMONTID:0004707" ;
        skos:prefLabel   "Organic nitrogen compounds"@en .

csc:CHEMONTID_0000242
        a                skos:Concept ;
        skos:altLabel    "a nitroimidazole"@en ;
        skos:broader     csc:CHEMONTID_0002310 ;
        skos:definition  "Compounds containing an imidazole ring which bears a nitro group."@en ;
        skos:inScheme    vlcs:chemische_stof ;
        skos:notation    "CHEMONTID:0000242" ;
        skos:prefLabel   "Nitroimidazoles"@en .

csc:CHEMONTID_0000417
        a                skos:Concept ;
        rdfs:seeAlso     tax_nodes:C0000417 ;
        skos:broader     csc:CHEMONTID_0002279 ;
        skos:definition  "Compounds containing an anisole where the methane group is linked to an acetic acid or a derivative."@en ;
        skos:inScheme    vlcs:chemische_stof ;
        skos:notation    "CHEMONTID:0000417" ;
        skos:prefLabel   "Phenoxyacetic acid derivatives"@en .

csc:CHEMONTID_0004209
        a                skos:Concept ;
        skos:broader     csc:CHEMONTID_0004208 ;
        skos:definition  "Aromatic compounds that contain a m-xylene moiety, which is a monocyclic benzene carrying exactly two methyl groups at the 1- and 3-positions."@en ;
        skos:inScheme    vlcs:chemische_stof ;
        skos:notation    "CHEMONTID:0004209" ;
        skos:prefLabel   "m-Xylenes"@en .

csc:CHEMONTID_0001691
        a                skos:Concept ;
        rdfs:seeAlso     tax_nodes:C0001691 ;
        skos:altLabel    "A steryl ester"@en , "Steryl esters"@en , "steroid ester"@en , "a sterol ester"@en ;
        skos:broader     csc:CHEMONTID_0000258 ;
        skos:definition  "Compounds containing a steroid moiety which bears a carboxylic acid ester group."@en ;
        skos:inScheme    vlcs:chemische_stof ;
        skos:notation    "CHEMONTID:0001691" ;
        skos:prefLabel   "Steroid esters"@en .

csc:CHEMONTID_0000463
        a                skos:Concept ;
        rdfs:seeAlso     tax_nodes:C0000463 ;
        skos:broader     csc:CHEMONTID_0004603 ;
        skos:definition  "Organic compounds containing an oxoanion."@en ;
        skos:inScheme    vlcs:chemische_stof ;
        skos:notation    "CHEMONTID:0000463" ;
        skos:prefLabel   "Organic oxoanionic compounds"@en .

csc:CHEMONTID_0000210
        a                skos:Concept ;
        rdfs:seeAlso     tax_nodes:C0000210 ;
        skos:altLabel    "Carbazoles"@en ;
        skos:broader     csc:CHEMONTID_0000211 ;
        skos:definition  "Compounds containing a three ring system containing a pyrrole ring fused on either side to a benzene ring."@en ;
        skos:inScheme    vlcs:chemische_stof ;
        skos:notation    "CHEMONTID:0000210" ;
        skos:prefLabel   "Carbazoles"@en .

csc:CHEMONTID_0001368
        a                skos:Concept ;
        rdfs:seeAlso     tax_nodes:C0001368 ;
        skos:altLabel    "thiocarbonyl compound"@en ;
        skos:broader     csc:CHEMONTID_0001198 ;
        skos:definition  "Organic compounds containing a functional group with the general structure OC(=S)NR2 or SC(=O)NR2."@en ;
        skos:inScheme    vlcs:chemische_stof ;
        skos:notation    "CHEMONTID:0001368" ;
        skos:prefLabel   "Thiocarbamic acid derivatives"@en .

csc:CHEMONTID_0004721
        a                skos:Concept ;
        skos:broader     csc:CHEMONTID_0004639 ;
        skos:definition  "Aromatic compounds containing a 1,3,5-triazine ring that is substituted at the 2-position with a chlorine atom."@en ;
        skos:inScheme    vlcs:chemische_stof ;
        skos:notation    "CHEMONTID:0004721" ;
        skos:prefLabel   "Chloro-s-triazines"@en .

csc:CHEMONTID_0000431
        a                skos:Concept ;
        rdfs:seeAlso     tax_nodes:C0000431 ;
        skos:broader     csc:CHEMONTID_0000422 ;
        skos:definition  "Inorganic compounds containing only metal atoms,with the largest atom being a metalloid atom."@en ;
        skos:inScheme    vlcs:chemische_stof ;
        skos:notation    "CHEMONTID:0000431" ;
        skos:prefLabel   "Homogeneous metalloid compounds"@en .

csc:CHEMONTID_0004476
        a                skos:Concept ;
        rdfs:seeAlso     tax_nodes:C0004476 ;
        skos:broader     csc:CHEMONTID_0004475 ;
        skos:definition  "Aliphatic Hydrocarbons that contains one or more unsaturated carbon atoms. These compounds contain one or more double or triple bonds."@en ;
        skos:inScheme    vlcs:chemische_stof ;
        skos:notation    "CHEMONTID:0004476" ;
        skos:prefLabel   "Unsaturated aliphatic hydrocarbons"@en .

csc:CHEMONTID_0004223
        a                skos:Concept ;
        skos:broader     csc:CHEMONTID_0004220 ;
        skos:definition  "Aromatic that contain a m-toluamide, where the carboxamide group is N- substituted with two alkyl chains."@en ;
        skos:inScheme    vlcs:chemische_stof ;
        skos:notation    "CHEMONTID:0004223" ;
        skos:prefLabel   "N,N-dialkyl-m-toluamides"@en .

csc:CHEMONTID_0000186
        a                skos:Concept ;
        rdfs:seeAlso     tax_nodes:C0000186 ;
        skos:altLabel    "Phenethylamines"@en , "primary amine"@en ;
        skos:broader     csc:CHEMONTID_0002279 ;
        skos:definition  "Compounds containing a phenethylamine moiety, which consists of a phenyl group substituted at the second position by an ethan-1-amine."@en ;
        skos:inScheme    vlcs:chemische_stof ;
        skos:notation    "CHEMONTID:0000186" ;
        skos:prefLabel   "Phenethylamines"@en .

csc:CHEMONTID_0002564
        a                skos:Concept ;
        skos:altLabel    "dichlorobenzene"@en ;
        skos:broader     csc:CHEMONTID_0001099 ;
        skos:definition  "Compounds containing a benzene with exactly two chlorine atoms attached to it."@en ;
        skos:inScheme    vlcs:chemische_stof ;
        skos:notation    "CHEMONTID:0002564" ;
        skos:prefLabel   "Dichlorobenzenes"@en .

csc:CHEMONTID_0003967
        a                skos:Concept ;
        skos:altLabel    "fluorotelomer alcohol"@en ;
        skos:broader     csc:CHEMONTID_0001027 ;
        skos:definition  "Fluorocarbon-based oligomers linked to an alcohol chain."@en ;
        skos:inScheme    vlcs:chemische_stof ;
        skos:notation    "CHEMONTID:0003967" ;
        skos:prefLabel   "Fluorotelomer alcohols"@en .

csc:CHEMONTID_0001880
        a                skos:Concept ;
        skos:broader     csc:CHEMONTID_0000347 ;
        skos:definition  "Amino acids having a (-NH2) group attached to the gamma carbon atom."@en ;
        skos:inScheme    vlcs:chemische_stof ;
        skos:notation    "CHEMONTID:0001880" ;
        skos:prefLabel   "Gamma amino acids and derivatives"@en .

csc:CHEMONTID_0004619
        a                skos:Concept ;
        skos:broader     csc:CHEMONTID_0004616 ;
        skos:definition  "Aryl phosphates in which the phosphate is esterified at exactly three positions."@en ;
        skos:inScheme    vlcs:chemische_stof ;
        skos:notation    "CHEMONTID:0004619" ;
        skos:prefLabel   "Aryl phosphotriesters"@en .

csc:CHEMONTID_0004665
        a                skos:Concept ;
        rdfs:seeAlso     tax_nodes:C0004665 ;
        skos:broader     csc:CHEMONTID_0001438 ;
        skos:definition  "Organooxygen compounds containing a O,S-diester derivative of phosphoroamidothioic acid. They have the general structure RSP(=O)(OR')(NH2), where R,R' are organyl groups."@en ;
        skos:inScheme    vlcs:chemische_stof ;
        skos:notation    "CHEMONTID:0004665" ;
        skos:prefLabel   "Phosphoramidothioic-acid-O,S-diesters"@en .

csc:CHEMONTID_0001350
        a                skos:Concept ;
        skos:altLabel    "benzoate ester"@en ;
        skos:broader     csc:CHEMONTID_0000176 ;
        skos:definition  "Ester derivatives of benzoic acid."@en ;
        skos:inScheme    vlcs:chemische_stof ;
        skos:notation    "CHEMONTID:0001350" ;
        skos:prefLabel   "Benzoic acid esters"@en .

csc:CHEMONTID_0003981
        a                skos:Concept ;
        rdfs:seeAlso     tax_nodes:C0003981 ;
        skos:altLabel    "benzyl halide"@en ;
        skos:broader     csc:CHEMONTID_0002279 ;
        skos:definition  "Organic compounds containing  a benzene skeleton substituted with a halomethyl group."@en ;
        skos:inScheme    vlcs:chemische_stof ;
        skos:notation    "CHEMONTID:0003981" ;
        skos:prefLabel   "Benzyl halides"@en .

csc:CHEMONTID_0000375
        a                skos:Concept ;
        rdfs:seeAlso     tax_nodes:C0000375 ;
        skos:altLabel    "Guanidines"@en , "guanidines"@en ;
        skos:broader     csc:CHEMONTID_0000278 ;
        skos:definition  "Compounds containing a guanidine moiety, with the general structure (R1R2N)(R3R4N)C=N-R5."@en ;
        skos:inScheme    vlcs:chemische_stof ;
        skos:notation    "CHEMONTID:0000375" ;
        skos:prefLabel   "Guanidines"@en .

csc:CHEMONTID_0002500
        a                skos:Concept ;
        rdfs:seeAlso     tax_nodes:C0002500 ;
        skos:altLabel    "alkane"@en ;
        skos:broader     csc:CHEMONTID_0004474 ;
        skos:definition  "Acyclic branched or unbranched hydrocarbons having the general formula CnH2n+2 , and therefore consisting entirely of hydrogen atoms and saturated carbon atoms."@en ;
        skos:inScheme    vlcs:chemische_stof ;
        skos:notation    "CHEMONTID:0002500" ;
        skos:prefLabel   "Alkanes"@en .

csc:CHEMONTID_0002002
        a                skos:Concept ;
        skos:altLabel    "diterpenoid"@en ;
        skos:broader     csc:CHEMONTID_0002930 ;
        skos:definition  "Tricyclic diterpenoids structurally characterized by the presence of a 1-oxo-decahydro-3a,9-propanocyclopenta[8]annulene skeleton."@en ;
        skos:inScheme    vlcs:chemische_stof ;
        skos:notation    "CHEMONTID:0002002" ;
        skos:prefLabel   "Mutilin derivatives"@en .

csc:CHEMONTID_0001027
        a                skos:Concept ;
        rdfs:seeAlso     tax_nodes:C0001027 ;
        skos:altLabel    "organofluorine compound"@en , "an alkyl fluoride"@en ;
        skos:broader     csc:CHEMONTID_0002867 ;
        skos:definition  "Organic compounds containing the alkyl fluoride functional group with formula R-F , where R is an alkyl group."@en ;
        skos:inScheme    vlcs:chemische_stof ;
        skos:notation    "CHEMONTID:0001027" ;
        skos:prefLabel   "Alkyl fluorides"@en .

csc:CHEMONTID_0004808
        a                skos:Concept ;
        skos:broader     csc:CHEMONTID_0000118 ;
        skos:definition  "Organic compounds contaning a halogen atom attached to the alpha carbon atom relative to C=O group."@en ;
        skos:inScheme    vlcs:chemische_stof ;
        skos:notation    "CHEMONTID:0004808" ;
        skos:prefLabel   "Alpha-haloketones"@en .

csc:CHEMONTID_0000518
        a                skos:Concept ;
        rdfs:seeAlso     tax_nodes:C0000518 ;
        skos:altLabel    "carbopolycyclic compound"@en ;
        skos:broader     csc:CHEMONTID_0000025 ;
        skos:definition  "Compounds containing a triphenylene moiety, which consists of four fused benzene rings forming a 9,10-benzo[l]phenanthrene."@en ;
        skos:inScheme    vlcs:chemische_stof ;
        skos:notation    "CHEMONTID:0000518" ;
        skos:prefLabel   "Triphenylenes"@en .

csc:CHEMONTID_0001073
        a                skos:Concept ;
        rdfs:seeAlso     tax_nodes:C0001073 ;
        skos:altLabel    "p-block molecular entity"@en ;
        skos:broader     csc:CHEMONTID_0000435 ;
        skos:definition  "Inorganic non-metallic compoundscontaining a phosphate as its largest oxoanion."@en , "Inorganic non-metallic compounds containing a phosphate as its largest oxoanion."@en ;
        skos:inScheme    vlcs:chemische_stof ;
        skos:notation    "CHEMONTID:0001073" ;
        skos:prefLabel   "Non-metal phosphates"@en .

csc:CHEMONTID_0000098
        a                skos:Concept ;
        rdfs:seeAlso     tax_nodes:C0000098 ;
        skos:altLabel    "triazines"@en ;
        skos:broader     csc:CHEMONTID_0000002 ;
        skos:definition  "Compounds containing a triazine ring, which is a heterocyclic ring, similar to the six-member benzene ring but with three carbons replaced by nitrogen atoms."@en ;
        skos:inScheme    vlcs:chemische_stof ;
        skos:notation    "CHEMONTID:0000098" ;
        skos:prefLabel   "Triazines"@en .

csc:CHEMONTID_0002223
        a                skos:Concept ;
        skos:altLabel    "butenolide"@en ;
        skos:broader     csc:CHEMONTID_0001982 ;
        skos:definition  "Dihydrofurans with a carbonyl group at the C2 carbon atom."@en ;
        skos:inScheme    vlcs:chemische_stof ;
        skos:notation    "CHEMONTID:0002223" ;
        skos:prefLabel   "Butenolides"@en .

csc:CHEMONTID_0001248
        a                skos:Concept ;
        skos:altLabel    "hydroxybenzoic acid"@en ;
        skos:broader     csc:CHEMONTID_0000176 ;
        skos:definition  "Compounds containing a hydroxybenzoic acid (or a derivative), which is a benzene ring bearing a carboxyl and a hydroxyl groups."@en ;
        skos:inScheme    vlcs:chemische_stof ;
        skos:notation    "CHEMONTID:0001248" ;
        skos:prefLabel   "Hydroxybenzoic acid derivatives"@en .

csc:CHEMONTID_0003626
        a                skos:Concept ;
        skos:altLabel    "enoate ester"@en ;
        skos:broader     csc:CHEMONTID_0003628 ;
        skos:definition  "An alpha,beta-unsaturated carboxylic ester of general formula R1C(R2)=C(R3)C(=O)OR4 (R4= organyl compound) in which the ester C=O function is conjugated to a C=C double bond at the alpha,beta position."@en ;
        skos:inScheme    vlcs:chemische_stof ;
        skos:notation    "CHEMONTID:0003626" ;
        skos:prefLabel   "Enoate esters"@en .

csc:CHEMONTID_0000311
        a                skos:Concept ;
        rdfs:seeAlso     tax_nodes:C0000311 ;
        skos:altLabel    "Benzothiazoles"@en ;
        skos:broader     csc:CHEMONTID_0000002 ;
        skos:definition  "Organic compounds containing a benzene fused to a thiazole ring (a five-membered ring with four carbon atoms, one nitrogen atom and one sulfur atom)."@en ;
        skos:inScheme    vlcs:chemische_stof ;
        skos:notation    "CHEMONTID:0000311" ;
        skos:prefLabel   "Benzothiazoles"@en .

csc:CHEMONTID_0003672
        a                skos:Concept ;
        skos:altLabel    "alpha,beta-unsaturated ketone"@en ;
        skos:broader     csc:CHEMONTID_0003131 ;
        skos:definition  "Ketones with the general structure R#CC(=O)R' or R=CC(=O)R', where R=organyl and R'= organyl group."@en ;
        skos:inScheme    vlcs:chemische_stof ;
        skos:notation    "CHEMONTID:0003672" ;
        skos:prefLabel   "Alpha,beta-unsaturated ketones"@en .

csc:CHEMONTID_0001469
        a                skos:Concept ;
        skos:altLabel    "cholestanoid"@en ;
        skos:broader     csc:CHEMONTID_0003566 ;
        skos:definition  "Compounds containing a 3-hydroxylated cholestane core."@en ;
        skos:inScheme    vlcs:chemische_stof ;
        skos:notation    "CHEMONTID:0001469" ;
        skos:prefLabel   "Cholesterols and derivatives"@en .

csc:CHEMONTID_0002444
        a                skos:Concept ;
        skos:altLabel    "N-nitrosoureas"@en ;
        skos:broader     csc:CHEMONTID_0001229 ;
        skos:definition  "Organonitrogen compounds with the general formula H3CN(N=O)R(N)=O (R = any atom)."@en ;
        skos:inScheme    vlcs:chemische_stof ;
        skos:notation    "CHEMONTID:0002444" ;
        skos:prefLabel   "N-methylnitrosoureas"@en .

csc:CHEMONTID_0001935
        a                skos:Concept ;
        rdfs:seeAlso     tax_nodes:C0001935 ;
        skos:altLabel    "ureas"@en , "Phenylcarbamides"@en ;
        skos:broader     csc:CHEMONTID_0002279 ;
        skos:definition  "Compounds containing a N-phenylurea moiety, which is structurally characterized by a phenyl group linked to one nitrogen atom of a urea group."@en ;
        skos:inScheme    vlcs:chemische_stof ;
        skos:notation    "CHEMONTID:0001935" ;
        skos:prefLabel   "N-phenylureas"@en .

csc:CHEMONTID_0004577
        a                skos:Concept ;
        skos:broader     csc:CHEMONTID_0004576 ;
        skos:definition  "O-acylated derivatives of salicylic acid."@en ;
        skos:inScheme    vlcs:chemische_stof ;
        skos:notation    "CHEMONTID:0004577" ;
        skos:prefLabel   "Acylsalicylic acids"@en .

csc:CHEMONTID_0002490
        a                skos:Concept ;
        rdfs:seeAlso     tax_nodes:C0002490 ;
        skos:altLabel    "organonitrogen heterocyclic compound"@en ;
        skos:broader     csc:CHEMONTID_0000002 ;
        skos:definition  "Azole derivatives obtained by conversion of one double bond of the azole ring to a single bond."@en ;
        skos:inScheme    vlcs:chemische_stof ;
        skos:notation    "CHEMONTID:0002490" ;
        skos:prefLabel   "Azolines"@en .

csc:CHEMONTID_0003893
        a                skos:Concept ;
        rdfs:seeAlso     tax_nodes:C0003893 ;
        skos:broader     csc:CHEMONTID_0000419 ;
        skos:definition  "Organophosphorus compounds containing a diester derivative of phosphonic acid, with the general structure ROP(=O)OR' (R,R' = organyl group)."@en ;
        skos:inScheme    vlcs:chemische_stof ;
        skos:notation    "CHEMONTID:0003893" ;
        skos:prefLabel   "Phosphonic acid diesters"@en .

csc:CHEMONTID_0001262
        a                skos:Concept ;
        skos:altLabel    "aminopyrimidine"@en ;
        skos:broader     csc:CHEMONTID_0000075 ;
        skos:definition  "Organic compounds containing an amino group attached to a pyrimidine ring. Pyrimidine is a 6-membered ring consisting of four carbon atoms and two nitrogen centers at the 1- and 3- ring positions."@en ;
        skos:inScheme    vlcs:chemische_stof ;
        skos:notation    "CHEMONTID:0001262" ;
        skos:prefLabel   "Aminopyrimidines and derivatives"@en .

csc:CHEMONTID_0001437
        a                skos:Concept ;
        rdfs:seeAlso     tax_nodes:C0001437 ;
        skos:altLabel    "benzoxazine"@en ;
        skos:broader     csc:CHEMONTID_0001396 ;
        skos:definition  "Organic compounds containing a benzene fused to an oxazine ring (a six-member aliphatic ring with four carbon atoms, one oxygen atom, and one nitrogen atom) bearing a ketone group."@en ;
        skos:inScheme    vlcs:chemische_stof ;
        skos:notation    "CHEMONTID:0001437" ;
        skos:prefLabel   "Benzoxazinones"@en .

csc:CHEMONTID_0003815
        a                skos:Concept ;
        rdfs:seeAlso     tax_nodes:C0003815 ;
        skos:altLabel    "glycerolipid"@en , "Triradylglycerols"@en ;
        skos:broader     csc:CHEMONTID_0000175 ;
        skos:definition  "Glycerolipids that carry exactly three acyl chains attached to the glycerol moiety."@en ;
        skos:inScheme    vlcs:chemische_stof ;
        skos:notation    "CHEMONTID:0003815" ;
        skos:prefLabel   "Triradylcglycerols"@en .

csc:CHEMONTID_0000209
        a                skos:Concept ;
        skos:broader     csc:CHEMONTID_0000207 ;
        skos:definition  "Compounds containing a phthalazine bearing a ketone group."@en ;
        skos:inScheme    vlcs:chemische_stof ;
        skos:notation    "CHEMONTID:0000209" ;
        skos:prefLabel   "Phthalazinones"@en .

csc:CHEMONTID_0000500
        a                skos:Concept ;
        skos:altLabel    "biphenyls"@en , "organochlorine compound"@en ;
        skos:broader     csc:CHEMONTID_0000041 ;
        skos:definition  "Organic compounds containing at least one chlorine atom attached to either benzene ring of the biphenyl moiety."@en ;
        skos:inScheme    vlcs:chemische_stof ;
        skos:notation    "CHEMONTID:0000500" ;
        skos:prefLabel   "Chlorinated biphenyls"@en .

csc:CHEMONTID_0001658
        a                skos:Concept ;
        skos:altLabel    "dicarboximide"@en ;
        skos:broader     csc:CHEMONTID_0001657 ;
        skos:definition  "Compounds comprising an N-substituted carboxylic acid imide group, with the general structure R1N(C(R2)=O)C(R3)=O (R2,R3=H, alkyl, aryl; R1=Anything but H)."@en ;
        skos:inScheme    vlcs:chemische_stof ;
        skos:notation    "CHEMONTID:0001658" ;
        skos:prefLabel   "N-substituted carboxylic acid imides"@en .

csc:CHEMONTID_0000002
        a                skos:Concept ;
        rdfs:seeAlso     tax_nodes:C0000002 ;
        skos:altLabel    "organic heterocyclic compound"@en ;
        skos:broader     csc:CHEMONTID_0000000 ;
        skos:definition  "Compounds containing a ring with least one carbon atom and one non-carbon atom."@en ;
        skos:inScheme    vlcs:chemische_stof ;
        skos:notation    "CHEMONTID:0000002" ;
        skos:prefLabel   "Organoheterocyclic compounds"@en .

csc:CHEMONTID_0004766
        a                skos:Concept ;
        rdfs:seeAlso     tax_nodes:C0004766 ;
        skos:broader     csc:CHEMONTID_0002279 ;
        skos:definition  "Aromatic compound contaning a phosphonothioate, which is C-substituted with a phenyl group."@en ;
        skos:inScheme    vlcs:chemische_stof ;
        skos:notation    "CHEMONTID:0004766" ;
        skos:prefLabel   "Phenylphosphonothioates"@en .

csc:CHEMONTID_0004513
        a                skos:Concept ;
        skos:broader     csc:CHEMONTID_0002982 ;
        skos:definition  "N-acyl-phenylureas that have the acyl group substituted by a phenyl group."@en ;
        skos:inScheme    vlcs:chemische_stof ;
        skos:notation    "CHEMONTID:0004513" ;
        skos:prefLabel   "N-benzoyl-N'-phenylureas"@en .

csc:CHEMONTID_0000476
        a                skos:Concept ;
        rdfs:seeAlso     tax_nodes:C0000476 ;
        skos:altLabel    "olefinic compound"@en ;
        skos:broader     csc:CHEMONTID_0000261 ;
        skos:definition  "Organic aromatic compounds containing a benzene and a carboxylic acid group (or a derivative thereof) forming 3-phenylprop-2-enoic acid."@en ;
        skos:inScheme    vlcs:chemische_stof ;
        skos:notation    "CHEMONTID:0000476" ;
        skos:prefLabel   "Cinnamic acids and derivatives"@en .

csc:CHEMONTID_0004734
        a                skos:Concept ;
        skos:altLabel    "diamino-1,3,5-triazine"@en ;
        skos:broader     csc:CHEMONTID_0001693 ;
        skos:definition  "Aromatic compounds containing a 1,3,5-triazine ring which is 2,4-disusbtituted wit amine groups."@en ;
        skos:inScheme    vlcs:chemische_stof ;
        skos:notation    "CHEMONTID:0004734" ;
        skos:prefLabel   "1,3,5-triazine-2,4-diamines"@en .

csc:CHEMONTID_0000444
        a                skos:Concept ;
        rdfs:seeAlso     tax_nodes:C0000444 ;
        skos:altLabel    "inorganic salt"@en , "salt"@en ;
        skos:broader     csc:CHEMONTID_0000424 ;
        skos:definition  "Inorganic halogenic compounds in which the heaviest metal atom is a post-transition metal."@en ;
        skos:inScheme    vlcs:chemische_stof ;
        skos:notation    "CHEMONTID:0000444" ;
        skos:prefLabel   "Post-transition metal salts"@en .

csc:CHEMONTID_0003086
        a                skos:Concept ;
        skos:altLabel    "medium-chain fatty acid"@en ;
        skos:broader     csc:CHEMONTID_0000262 ;
        skos:definition  "Fatty acids with an aliphatic tail that contains between 4 and 12 carbon atoms."@en ;
        skos:inScheme    vlcs:chemische_stof ;
        skos:notation    "CHEMONTID:0003086" ;
        skos:prefLabel   "Medium-chain fatty acids"@en .

csc:CHEMONTID_0000199
        a                skos:Concept ;
        skos:altLabel    "Thioxanthenes"@en ;
        skos:broader     csc:CHEMONTID_0003413 ;
        skos:definition  "Organic polycyclic compounds containing a thioxanthene moiety, which is an aromatic tricycle derived from xanthene by replacing the oxygen atom with a sulfur atom."@en ;
        skos:inScheme    vlcs:chemische_stof ;
        skos:notation    "CHEMONTID:0000199" ;
        skos:prefLabel   "Thioxanthenes"@en .

csc:CHEMONTID_0000490
        a                skos:Concept ;
        rdfs:seeAlso     tax_nodes:C0000490 ;
        skos:altLabel    "N-sulfonylurea"@en , "Sulfonylurea Compounds"@en ;
        skos:broader     csc:CHEMONTID_0000278 ;
        skos:definition  "Organic compounds containing a sulfonyl group with the structure R-S(=O)2-R', where R' is an urea."@en ;
        skos:inScheme    vlcs:chemische_stof ;
        skos:notation    "CHEMONTID:0000490" ;
        skos:prefLabel   "Sulfonylureas"@en .

csc:CHEMONTID_0001893
        a                skos:Concept ;
        skos:altLabel    "pyrimidines"@en , "organohalogen compound"@en ;
        skos:broader     csc:CHEMONTID_0000075 ;
        skos:definition  "Aromatic compounds containing a halogen atom linked to a pyrimidine ring. Pyrimidine is a 6-membered ring consisting of four carbon atoms and two nitrogen centers at the 1- and 3- ring positions."@en ;
        skos:inScheme    vlcs:chemische_stof ;
        skos:notation    "CHEMONTID:0001893" ;
        skos:prefLabel   "Halopyrimidines"@en .

csc:CHEMONTID_0004702
        a                skos:Concept ;
        skos:altLabel    "Alkyl 4-hydroxybenzoates"@en , "para-Hydroxybenzoic acid alkyl esters"@en ;
        skos:broader     csc:CHEMONTID_0004701 ;
        skos:definition  "Aromatic compounds containing a benzoic acid, which is esterified with an alkyl group and para-substituted with a hydroxyl group."@en ;
        skos:inScheme    vlcs:chemische_stof ;
        skos:notation    "CHEMONTID:0004702" ;
        skos:prefLabel   "p-Hydroxybenzoic acid alkyl esters"@en .

csc:CHEMONTID_0000167
        a                skos:Concept ;
        skos:altLabel    "Carbapenems"@en , "carbapenems"@en ;
        skos:broader     csc:CHEMONTID_0000162 ;
        skos:definition  "Beta-lactam derivatives in which the beta-lactam ring shares the nitrogen atom with a pyrrole-2-carboxylic acid."@en ;
        skos:inScheme    vlcs:chemische_stof ;
        skos:notation    "CHEMONTID:0000167" ;
        skos:prefLabel   "Carbapenems"@en .

csc:CHEMONTID_0002798
        a                skos:Concept ;
        rdfs:seeAlso     tax_nodes:C0002798 ;
        skos:altLabel    "1,3,5-triazinanes"@en , "sym-Triazinanes"@en ;
        skos:broader     csc:CHEMONTID_0002693 ;
        skos:definition  "Triazinanes having three nitrogen ring atoms at the 1-, 3-, and 5- positions."@en ;
        skos:inScheme    vlcs:chemische_stof ;
        skos:notation    "CHEMONTID:0002798" ;
        skos:prefLabel   "1,3,5-triazinanes"@en .

csc:CHEMONTID_0001142
        a                skos:Concept ;
        rdfs:seeAlso     tax_nodes:C0001142 ;
        skos:altLabel    "Chrysenes"@en , "1,2-Benzphenanthrenes"@en , "carbopolycyclic compound"@en ;
        skos:broader     csc:CHEMONTID_0000025 ;
        skos:definition  "Compounds containing the polyaromatic chrysene moiety, which consists of a benzene ring fused to a phenanthrene ring system to form Benzo[a]phenanthrene."@en ;
        skos:inScheme    vlcs:chemische_stof ;
        skos:notation    "CHEMONTID:0001142" ;
        skos:prefLabel   "Chrysenes"@en .

csc:CHEMONTID_0001861
        a                skos:Concept ;
        rdfs:seeAlso     tax_nodes:C0001861 ;
        skos:altLabel    "sulfonamide"@en , "pyridines"@en ;
        skos:broader     csc:CHEMONTID_0000089 ;
        skos:definition  "Heterocyclic compounds containing a pyridine ring substituted by one or more sulfonamide groups."@en ;
        skos:inScheme    vlcs:chemische_stof ;
        skos:notation    "CHEMONTID:0001861" ;
        skos:prefLabel   "Pyridinesulfonamides"@en .

csc:CHEMONTID_0001363
        a                skos:Concept ;
        skos:altLabel    "enone"@en ;
        skos:broader     csc:CHEMONTID_0003672 ;
        skos:definition  "Compounds containing the enone functional group, with the structure RC(=O)CR'."@en ;
        skos:inScheme    vlcs:chemische_stof ;
        skos:notation    "CHEMONTID:0001363" ;
        skos:prefLabel   "Enones"@en .

csc:CHEMONTID_0002766
        a                skos:Concept ;
        skos:altLabel    "chlorophenol"@en ;
        skos:broader     csc:CHEMONTID_0002320 ;
        skos:definition  "Halophenols carrying a chlorine on the benzene ring."@en ;
        skos:inScheme    vlcs:chemische_stof ;
        skos:notation    "CHEMONTID:0002766" ;
        skos:prefLabel   "Chlorophenols"@en .

csc:CHEMONTID_0000135
        a                skos:Concept ;
        skos:altLabel    "o-Dihydroxybenzenes"@en , "catechols"@en , "a catechol"@en , "Catechols"@en , "Ortho-Dihydroxybenzenes"@en , "a 1,2-benzenediol"@en , "1,2-Benzenediols"@en ;
        skos:broader     csc:CHEMONTID_0001286 ;
        skos:definition  "Compounds containing a 1,2-benzenediol moiety."@en ;
        skos:inScheme    vlcs:chemische_stof ;
        skos:notation    "CHEMONTID:0000135" ;
        skos:prefLabel   "Catechols"@en .

csc:CHEMONTID_0004646
        a                skos:Concept ;
        rdfs:seeAlso     tax_nodes:C0004646 ;
        skos:broader     csc:CHEMONTID_0000134 ;
        skos:definition  "Phenols that a unsubstituted at the 2-position."@en ;
        skos:inScheme    vlcs:chemische_stof ;
        skos:notation    "CHEMONTID:0004646" ;
        skos:prefLabel   "1-hydroxy-2-unsubstituted benzenoids"@en .

csc:CHEMONTID_0000181
        a                skos:Concept ;
        rdfs:seeAlso     tax_nodes:C0000181 ;
        skos:altLabel    "Tetracyclines"@en , "tetracyclines"@en ;
        skos:broader     csc:CHEMONTID_0000261 ;
        skos:definition  "Polyketides having an octahydrotetracene-2-carboxamide skeleton, substituted with many hydroxy and other groups."@en ;
        skos:inScheme    vlcs:chemische_stof ;
        skos:notation    "CHEMONTID:0000181" ;
        skos:prefLabel   "Tetracyclines"@en .

csc:CHEMONTID_0003962
        a                skos:Concept ;
        skos:altLabel    "organofluorine compound"@en , "organophosphorus compound"@en , "carbonyl compound"@en , "PFCAs"@en ;
        skos:broader     csc:CHEMONTID_0001027 ;
        skos:definition  "Organic compounds containing an alkyl chain attached to the C-alpha of a carboxylic acid group (or a derivative thereof), where all hydrogens of the alkyl chain are replaced by fluorine atoms."@en ;
        skos:inScheme    vlcs:chemische_stof ;
        skos:notation    "CHEMONTID:0003962" ;
        skos:prefLabel   "Perfluoroalkyl carboxylic acid and derivatives"@en .

csc:CHEMONTID_0002987
        a                skos:Concept ;
        skos:altLabel    "6-aminopurines"@en ;
        skos:broader     csc:CHEMONTID_0000245 ;
        skos:definition  "Purines that carry an amino group at position 6. Purine is a bicyclic aromatic compound made up of a pyrimidine ring fused to an imidazole ring."@en ;
        skos:inScheme    vlcs:chemische_stof ;
        skos:notation    "CHEMONTID:0002987" ;
        skos:prefLabel   "6-aminopurines"@en .

csc:CHEMONTID_0000356
        a                skos:Concept ;
        skos:altLabel    "diarylheptanoid"@en ;
        skos:broader     csc:CHEMONTID_0002651 ;
        skos:definition  "Aromatic compounds containing a curcumin moiety, which is composed of two aryl buten-2-one (feruloyl) chromophores joined by a methylene group."@en ;
        skos:inScheme    vlcs:chemische_stof ;
        skos:notation    "CHEMONTID:0000356" ;
        skos:prefLabel   "Curcuminoids"@en .

csc:CHEMONTID_0000103
        a                skos:Concept ;
        rdfs:seeAlso     tax_nodes:C0000103 ;
        skos:altLabel    "Aziridines"@en ;
        skos:broader     csc:CHEMONTID_0000002 ;
        skos:definition  "Organic compounds containing a saturated three-member heterocycle with one amino group and two methylene groups."@en ;
        skos:inScheme    vlcs:chemische_stof ;
        skos:notation    "CHEMONTID:0000103" ;
        skos:prefLabel   "Aziridines"@en .

csc:CHEMONTID_0001506
        a                skos:Concept ;
        rdfs:seeAlso     tax_nodes:C0001506 ;
        skos:altLabel    "purine nucleotide"@en ;
        skos:broader     csc:CHEMONTID_0000289 ;
        skos:definition  "Nucleotides with a purine base attached to the ribosyl moiety."@en ;
        skos:inScheme    vlcs:chemische_stof ;
        skos:notation    "CHEMONTID:0001506" ;
        skos:prefLabel   "Purine nucleotides"@en .

csc:CHEMONTID_0004148
        a                skos:Concept ;
        skos:altLabel    "N-acyl-L-alpha-amino acid"@en ;
        skos:broader     csc:CHEMONTID_0002402 ;
        skos:definition  "N-acylated alpha amino acids which have the L-configuration of the alpha-carbon atom."@en ;
        skos:inScheme    vlcs:chemische_stof ;
        skos:notation    "CHEMONTID:0004148" ;
        skos:prefLabel   "N-acyl-L-alpha-amino acids"@en .

csc:CHEMONTID_0002955
        a                skos:Concept ;
        rdfs:seeAlso     tax_nodes:C0002955 ;
        skos:altLabel    "isoquinolines"@en ;
        skos:broader     csc:CHEMONTID_0000002 ;
        skos:definition  "Tetrahydrogenated isoquinoline derivatives."@en ;
        skos:inScheme    vlcs:chemische_stof ;
        skos:notation    "CHEMONTID:0002955" ;
        skos:prefLabel   "Tetrahydroisoquinolines"@en .

csc:CHEMONTID_0000324
        a                skos:Concept ;
        rdfs:seeAlso     tax_nodes:C0000324 ;
        skos:altLabel    "Fatty esters"@en , "fatty acid ester"@en ;
        skos:broader     csc:CHEMONTID_0003909 ;
        skos:definition  "Carboxylic ester derivatives of a fatty acid."@en ;
        skos:inScheme    vlcs:chemische_stof ;
        skos:notation    "CHEMONTID:0000324" ;
        skos:prefLabel   "Fatty acid esters"@en .

csc:CHEMONTID_0002282
        a                skos:Concept ;
        skos:altLabel    "imidazolidine-2,4-dione"@en ;
        skos:broader     csc:CHEMONTID_0002273 ;
        skos:definition  "Heterocyclic aromatic compounds containing an imiazolidinedione moiety substituted by a phenyl group."@en ;
        skos:inScheme    vlcs:chemische_stof ;
        skos:notation    "CHEMONTID:0002282" ;
        skos:prefLabel   "Phenylhydantoins"@en .

csc:CHEMONTID_0004660
        a                skos:Concept ;
        rdfs:seeAlso     tax_nodes:C0004660 ;
        skos:broader     csc:CHEMONTID_0004659 ;
        skos:definition  "Aromatic compounds containing a benzo-1,2,3-triazine, which is substituted by an organothiophosphate group at the 3-position. Their general structure is R-CSP(=S)(OR')OR'', where R=benzo-1,2,3-triazine, R',R\\\" = any atom."@en , "Aromatic compounds containing a benzo-1,2,3-triazine, which is substituted by an organothiophosphate group at the 3-position. Their general structure is R-CSP(=S)(OR')OR'', where R=benzo-1,2,3-triazine, R',R\" = any atom."@en ;
        skos:inScheme    vlcs:chemische_stof ;
        skos:notation    "CHEMONTID:0004660" ;
        skos:prefLabel   "Benzotriazine organothiophosphates"@en .

csc:CHEMONTID_0000079
        a                skos:Concept ;
        rdfs:seeAlso     tax_nodes:C0000079 ;
        skos:altLabel    "dihydroimidazoles"@en , "Imidazolines"@en ;
        skos:broader     csc:CHEMONTID_0002490 ;
        skos:definition  "Organic compounds containing an imidazoline ring, which is an unsaturated ring (derived from imidazole) with two nitrogen atoms at positions 1 and 3 respectively, and containing only one CN double bond."@en ;
        skos:inScheme    vlcs:chemische_stof ;
        skos:notation    "CHEMONTID:0000079" ;
        skos:prefLabel   "Imidazolines"@en .

csc:CHEMONTID_0001229
        a                skos:Concept ;
        skos:altLabel    "N-nitrosoureas"@en , "Nitrosourea Compounds"@en ;
        skos:broader     csc:CHEMONTID_0000517 ;
        skos:definition  "Compounds containing a nitro group and an urea group N-N linked together, with the general structure R1N(R2)C(=O)N(R3)N=O."@en ;
        skos:inScheme    vlcs:chemische_stof ;
        skos:notation    "CHEMONTID:0001229" ;
        skos:prefLabel   "Nitrosoureas"@en .

csc:CHEMONTID_0002204
        a                skos:Concept ;
        skos:altLabel    "C-glycosyl compound"@en ;
        skos:broader     csc:CHEMONTID_0002105 ;
        skos:definition  "Glycoside in which a sugar group is bonded through one carbon to another group via a C-glycosidic bond."@en ;
        skos:inScheme    vlcs:chemische_stof ;
        skos:notation    "CHEMONTID:0002204" ;
        skos:prefLabel   "C-glycosyl compounds"@en .

csc:CHEMONTID_0004162
        a                skos:Concept ;
        rdfs:seeAlso     tax_nodes:C0004162 ;
        skos:altLabel    "hydroxyindoles"@en ;
        skos:broader     csc:CHEMONTID_0000211 ;
        skos:definition  "Organic compounds containing an indole moiety that carries a hydroxyl group."@en ;
        skos:inScheme    vlcs:chemische_stof ;
        skos:notation    "CHEMONTID:0004162" ;
        skos:prefLabel   "Hydroxyindoles"@en .

csc:CHEMONTID_0001275
        a                skos:Concept ;
        skos:altLabel    "p-Cresols"@en , "hydroxytoluene"@en , "a 1,4-cresol"@en , "1,4-Cresols"@en , "a p-cresol"@en ;
        skos:broader     csc:CHEMONTID_0001272 ;
        skos:definition  "Compounds containing a para cresol moiety, which consists of a benzene ring bearing one hydroxyl group at ring positions 1 and 4."@en ;
        skos:inScheme    vlcs:chemische_stof ;
        skos:notation    "CHEMONTID:0001275" ;
        skos:prefLabel   "Para cresols"@en .

csc:CHEMONTID_0000047
        a                skos:Concept ;
        rdfs:seeAlso     tax_nodes:C0000047 ;
        skos:broader     csc:CHEMONTID_0001510 ;
        skos:definition  "Tetralin lignans in which the benzene moiety of the tetralin skeleton is fused to a 1,3-dioxolane and the cyclohexane is fused to a butyrolactone (pyrrolidin-2-one)."@en ;
        skos:inScheme    vlcs:chemische_stof ;
        skos:notation    "CHEMONTID:0000047" ;
        skos:prefLabel   "Podophyllotoxins"@en .

csc:CHEMONTID_0001022
        a                skos:Concept ;
        rdfs:seeAlso     tax_nodes:C0001022 ;
        skos:altLabel    "acyl chloride"@en ;
        skos:broader     csc:CHEMONTID_0002865 ;
        skos:definition  "Organic compounds containing the functional group -CO-Cl."@en ;
        skos:inScheme    vlcs:chemische_stof ;
        skos:notation    "CHEMONTID:0001022" ;
        skos:prefLabel   "Acyl chlorides"@en .

csc:CHEMONTID_0001994
        a                skos:Concept ;
        skos:altLabel    "cyclodepsipeptide"@en ;
        skos:broader     csc:CHEMONTID_0001961 ;
        skos:definition  "Natural or synthetic compounds having sequences of amino and hydroxy carboxylic acid residues (usually α-amino and α-hydroxy acids) connected in a ring. The residues are commonly but not necessarily regularly alternating."@en ;
        skos:inScheme    vlcs:chemische_stof ;
        skos:notation    "CHEMONTID:0001994" ;
        skos:prefLabel   "Cyclic depsipeptides"@en .

csc:CHEMONTID_0000093
        a                skos:Concept ;
        rdfs:seeAlso     tax_nodes:C0000093 ;
        skos:altLabel    "Thiadiazoles"@en ;
        skos:broader     csc:CHEMONTID_0000436 ;
        skos:definition  "Cyclic organic compounds containing a thiadiazole ring, which is a five-membered aromatic heterocycle made up of one sulfur atom and two nitrogen atoms."@en ;
        skos:inScheme    vlcs:chemische_stof ;
        skos:notation    "CHEMONTID:0000093" ;
        skos:prefLabel   "Thiadiazoles"@en .

csc:CHEMONTID_0001243
        a                skos:Concept ;
        rdfs:seeAlso     tax_nodes:C0001243 ;
        skos:altLabel    "beta-lactone"@en ;
        skos:broader     csc:CHEMONTID_0000050 ;
        skos:definition  "Organic compounds containing a four-member lactone (a cyclic ester)."@en ;
        skos:inScheme    vlcs:chemische_stof ;
        skos:notation    "CHEMONTID:0001243" ;
        skos:prefLabel   "Beta propiolactones"@en .

csc:CHEMONTID_0000015
        a                skos:Concept ;
        rdfs:seeAlso     tax_nodes:C0000015 ;
        skos:altLabel    "dibenzofurans"@en ;
        skos:broader     csc:CHEMONTID_0000301 ;
        skos:definition  "Compounds containing a dibenzofuran moiety, which consists of two benzene rings fused to a central furan ring."@en ;
        skos:inScheme    vlcs:chemische_stof ;
        skos:notation    "CHEMONTID:0000015" ;
        skos:prefLabel   "Dibenzofurans"@en .

csc:CHEMONTID_0002867
        a                skos:Concept ;
        rdfs:seeAlso     tax_nodes:C0002867 ;
        skos:altLabel    "halogenoalkanes"@en , "haloalkane"@en ;
        skos:broader     csc:CHEMONTID_0000267 ;
        skos:definition  "Organic compounds containing a linear aliphatic chain (or ring system) carrying a C-X bond, where X is a halogen atom."@en ;
        skos:inScheme    vlcs:chemische_stof ;
        skos:notation    "CHEMONTID:0002867" ;
        skos:prefLabel   "Alkyl halides"@en .

csc:CHEMONTID_0003597
        a                skos:Concept ;
        rdfs:seeAlso     tax_nodes:C0003597 ;
        skos:altLabel    "sulfonic acid derivative"@en , "naphthalenes"@en ;
        skos:broader     csc:CHEMONTID_0000023 ;
        skos:definition  "Organic aromatic compounds that contain a naphthalene moiety that carries a sulfonic acid group (or a derivative thereof) at one or more positions. Naphthalene is a bicyclic compound that is made up of two fused benzene ring."@en ;
        skos:inScheme    vlcs:chemische_stof ;
        skos:notation    "CHEMONTID:0003597" ;
        skos:prefLabel   "Naphthalene sulfonic acids and derivatives"@en .

csc:CHEMONTID_0000282
        a                skos:Concept ;
        skos:altLabel    "aminoglycoside"@en ;
        skos:broader     csc:CHEMONTID_0003305 ;
        skos:definition  "Molecules or a portion of a molecule composed of amino-modified sugars."@en ;
        skos:inScheme    vlcs:chemische_stof ;
        skos:notation    "CHEMONTID:0000282" ;
        skos:prefLabel   "Aminoglycosides"@en .

csc:CHEMONTID_0000457
        a                skos:Concept ;
        rdfs:seeAlso     tax_nodes:C0000457 ;
        skos:broader     csc:CHEMONTID_0000424 ;
        skos:definition  "Inorganic compounds belonging either to the alkaline earth metal hydrides, the alkaline earth metal nitrides, the alkaline earth metal oxides, or the alkaline earth metal sulfides."@en ;
        skos:inScheme    vlcs:chemische_stof ;
        skos:notation    "CHEMONTID:0000457" ;
        skos:prefLabel   "Alkaline earth metal organides"@en .

csc:CHEMONTID_0003099
        a                skos:Concept ;
        skos:altLabel    "carbonyl compound"@en , "organohalogen compound"@en ;
        skos:broader     csc:CHEMONTID_0003096 ;
        skos:definition  "Benzoic acids or derivatives carrying a halogen atom at the 3-position of the benzene ring."@en ;
        skos:inScheme    vlcs:chemische_stof ;
        skos:notation    "CHEMONTID:0003099" ;
        skos:prefLabel   "3-halobenzoic acids and derivatives"@en .

csc:CHEMONTID_0001607
        a                skos:Concept ;
        rdfs:seeAlso     tax_nodes:C0001607 ;
        skos:altLabel    "Rotenoid flavonoids"@en , "rotenoid"@en , "a rotenoid"@en ;
        skos:broader     csc:CHEMONTID_0002506 ;
        skos:definition  "Phenolic compounds containing a cis-fused tetrahydrochromeno[3,4-b]chromene nucleus. Many rotenoids contain an additional ring, e.g. rotenone. They are isoflavonoids characterized by the presence of an extra carbon atom in an additional heterocyclic ring."@en ;
        skos:inScheme    vlcs:chemische_stof ;
        skos:notation    "CHEMONTID:0001607" ;
        skos:prefLabel   "Rotenoids"@en .

csc:CHEMONTID_0001187
        a                skos:Concept ;
        rdfs:seeAlso     tax_nodes:C0001187 ;
        skos:altLabel    "thioacetals"@en , "thioacetal"@en ;
        skos:broader     csc:CHEMONTID_0000004 ;
        skos:definition  "Organic compounds containing either the monothiacetal functional group (R2C(OR')(SR')) or the dithioacetal (R2C(SR')2) functional group ."@en ;
        skos:inScheme    vlcs:chemische_stof ;
        skos:notation    "CHEMONTID:0001187" ;
        skos:prefLabel   "Thioacetals"@en .

csc:CHEMONTID_0003565
        a                skos:Concept ;
        skos:altLabel    "Aristolane sesquiterpenoids"@en , "sesquiterpenoid"@en ;
        skos:broader     csc:CHEMONTID_0001550 ;
        skos:definition  "Sesquiterpenoids with a structure based on the aristolane skeleton. Aristolanes arise from the C6,C11 cyclization of the bicyclic eremophilane skeleton."@en ;
        skos:inScheme    vlcs:chemische_stof ;
        skos:notation    "CHEMONTID:0003565" ;
        skos:prefLabel   "Aristolane sesquiterpenoids"@en .

csc:CHEMONTID_0000250
        a                skos:Concept ;
        rdfs:seeAlso     tax_nodes:C0000250 ;
        skos:altLabel    "Imidazolidines"@en ;
        skos:broader     csc:CHEMONTID_0002491 ;
        skos:definition  "Organic compounds containing an imidazolidine ring, which is a saturated ring (derived from imidazole) with two nitrogen atoms at positions 1 and 3 respectively, and containing only single bonds."@en ;
        skos:inScheme    vlcs:chemische_stof ;
        skos:notation    "CHEMONTID:0000250" ;
        skos:prefLabel   "Imidazolidines"@en .

csc:CHEMONTID_0001109
        a                skos:Concept ;
        skos:altLabel    "2-benzofurans"@en , "cyclic dicarboxylic anhydride"@en ;
        skos:broader     csc:CHEMONTID_0001578 ;
        skos:definition  "Compounds containing a phthalic anhydride moiety (or a derivative thereof), which consists of a benzene fused to a furan-1,3-dione."@en ;
        skos:inScheme    vlcs:chemische_stof ;
        skos:notation    "CHEMONTID:0001109" ;
        skos:prefLabel   "Phthalic anhydrides"@en .

csc:CHEMONTID_0000425
        a                skos:Concept ;
        rdfs:seeAlso     tax_nodes:C0000425 ;
        skos:broader     csc:CHEMONTID_0000422 ;
        skos:definition  "Inorganic compounds containing only metal atoms,with the largest atom being a alkali metal atom."@en ;
        skos:inScheme    vlcs:chemische_stof ;
        skos:notation    "CHEMONTID:0000425" ;
        skos:prefLabel   "Homogeneous alkali metal compounds"@en .

csc:CHEMONTID_0004010
        a                skos:Concept ;
        skos:broader     csc:CHEMONTID_0004009 ;
        skos:definition  "Ester derivatives of m-phthalic acids, which are based on a benzene 1,3-dicarboxylic acid skeleton."@en ;
        skos:inScheme    vlcs:chemische_stof ;
        skos:notation    "CHEMONTID:0004010" ;
        skos:prefLabel   "m-Phthalate esters"@en .

csc:CHEMONTID_0004484
        a                skos:Concept ;
        rdfs:seeAlso     tax_nodes:C0004484 ;
        skos:broader     csc:CHEMONTID_0000400 ;
        skos:definition  "Organic compounds containing a phosphorous acid, which is tri-esterified with alkyl groups."@en ;
        skos:inScheme    vlcs:chemische_stof ;
        skos:notation    "CHEMONTID:0004484" ;
        skos:prefLabel   "Trialkylphosphites"@en .

csc:CHEMONTID_0004659
        a                skos:Concept ;
        rdfs:seeAlso     tax_nodes:C0004659 ;
        skos:broader     csc:CHEMONTID_0000002 ;
        skos:definition  "Organic compounds containing a 1,2,3-triazine ring fused to a benzene ring."@en ;
        skos:inScheme    vlcs:chemische_stof ;
        skos:notation    "CHEMONTID:0004659" ;
        skos:prefLabel   "Benzo-1,2,3-triazines"@en .

csc:CHEMONTID_0000194
        a                skos:Concept ;
        rdfs:seeAlso     tax_nodes:C0000194 ;
        skos:altLabel    "Nitrofurans"@en ;
        skos:broader     csc:CHEMONTID_0000076 ;
        skos:definition  "Compounds containing a furan ring which bears a nitro group."@en ;
        skos:inScheme    vlcs:chemische_stof ;
        skos:notation    "CHEMONTID:0000194" ;
        skos:prefLabel   "Nitrofurans"@en .

csc:CHEMONTID_0000369
        a                skos:Concept ;
        rdfs:seeAlso     tax_nodes:C0000369 ;
        skos:altLabel    "diarylmethane"@en ;
        skos:broader     csc:CHEMONTID_0002279 ;
        skos:definition  "Compounds containing a diphenylmethane moiety, which consists of a methane wherein two hydrogen atoms are replaced by two phenyl groups."@en ;
        skos:inScheme    vlcs:chemische_stof ;
        skos:notation    "CHEMONTID:0000369" ;
        skos:prefLabel   "Diphenylmethanes"@en .

csc:CHEMONTID_0002074
        a                skos:Concept ;
        skos:altLabel    "Organosulfites"@en , "sulfite ester"@en ;
        skos:broader     csc:CHEMONTID_0004456 ;
        skos:definition  "Organic compounds containing an organic group attached to the sulfite oxoanion, with the formula  R[SO3]2-."@en ;
        skos:inScheme    vlcs:chemische_stof ;
        skos:notation    "CHEMONTID:0002074" ;
        skos:prefLabel   "Sulfite esters"@en .

csc:CHEMONTID_0001099
        a                skos:Concept ;
        skos:altLabel    "organochlorine compound"@en ;
        skos:broader     csc:CHEMONTID_0000035 ;
        skos:definition  "Compounds containing one or more chlorine atoms attached to a benzene moiety."@en ;
        skos:inScheme    vlcs:chemische_stof ;
        skos:notation    "CHEMONTID:0001099" ;
        skos:prefLabel   "Chlorobenzenes"@en .

csc:CHEMONTID_0004452
        a                skos:Concept ;
        skos:altLabel    "Acrylates"@en ;
        skos:broader     csc:CHEMONTID_0004450 ;
        skos:definition  "Organic compounds containing and ester acrylic acid (CH2=CHC(=O)OH)."@en ;
        skos:inScheme    vlcs:chemische_stof ;
        skos:notation    "CHEMONTID:0004452" ;
        skos:prefLabel   "Acrylic acid esters"@en .

csc:CHEMONTID_0000162
        a                skos:Concept ;
        rdfs:seeAlso     tax_nodes:C0000162 ;
        skos:altLabel    "beta-Lactams"@en ;
        skos:broader     csc:CHEMONTID_0000160 ;
        skos:definition  "Organic compounds containing a four-member lactam (a cyclic amide)."@en ;
        skos:inScheme    vlcs:chemische_stof ;
        skos:notation    "CHEMONTID:0000162" ;
        skos:prefLabel   "Beta lactams"@en .

csc:CHEMONTID_0001565
        a                skos:Concept ;
        skos:altLabel    "Iridoid, 10-alkyliridoid and secoiridoid monoterpenoids"@en , "iridoid monoterpenoid"@en ;
        skos:broader     csc:CHEMONTID_0001549 ;
        skos:definition  "Monoterpenes containing a skeleton structurally characterized by the presence of a cylopentane fused to a pyran ( forming a 4,7-dimethylcyclopenta[c]pyran), or a derivative where the pentane moiety is open."@en ;
        skos:inScheme    vlcs:chemische_stof ;
        skos:notation    "CHEMONTID:0001565" ;
        skos:prefLabel   "Iridoids and derivatives"@en .

csc:CHEMONTID_0004673
        a                skos:Concept ;
        skos:broader     csc:CHEMONTID_0004298 ;
        skos:definition  "Alkyl-phenylketones where the alkyl group is a cyclohexane 1,3-dione."@en ;
        skos:inScheme    vlcs:chemische_stof ;
        skos:notation    "CHEMONTID:0004673" ;
        skos:prefLabel   "Benzoylcyclohexane-1,3-diones"@en .

csc:CHEMONTID_0002042
        a                skos:Concept ;
        rdfs:seeAlso     tax_nodes:C0002042 ;
        skos:altLabel    "a diphenylbenzene"@en , "ring assembly"@en , "Diphenylbenzenes"@en , "a terphenyl"@en ;
        skos:broader     csc:CHEMONTID_0002279 ;
        skos:definition  "Polycyclic aromatic compounds containing a terphenyl skeleton, which consists of a benzene ring substituted with two phenyl groups. Isomers of terphenyl include m-terphenyls (1,3-diphenylbenzenes),  o-terphenyls (1,2-diphenylbenzenes),  p-terphenyls (1,4-diphenylbenzenes)."@en ;
        skos:inScheme    vlcs:chemische_stof ;
        skos:notation    "CHEMONTID:0002042" ;
        skos:prefLabel   "Terphenyls"@en .

csc:CHEMONTID_0000130
        a                skos:Concept ;
        rdfs:seeAlso     tax_nodes:C0000130 ;
        skos:broader     csc:CHEMONTID_0000002 ;
        skos:definition  "Organic compounds containing a spirodecane moiety with at least one nitrogen atom."@en ;
        skos:inScheme    vlcs:chemische_stof ;
        skos:notation    "CHEMONTID:0000130" ;
        skos:prefLabel   "Azaspirodecane derivatives"@en .

csc:CHEMONTID_0000305
        a                skos:Concept ;
        rdfs:seeAlso     tax_nodes:C0000305 ;
        skos:altLabel    "pyrazolopyrimidine"@en ;
        skos:broader     csc:CHEMONTID_0000002 ;
        skos:definition  "Compounds containing a pyrazolopyrimidine skeleton, which consists of a pyrazole fused to a pyrimidine. Pyrazole is 5-membered ring consisting of three carbon atoms and two adjacent nitrogen centers. Pyrimidine is 6-membered ring consisting of four carbon atoms and two adjacent nitrogen atoms at the 1- and 3- ring position."@en ;
        skos:inScheme    vlcs:chemische_stof ;
        skos:notation    "CHEMONTID:0000305" ;
        skos:prefLabel   "Pyrazolopyrimidines"@en .

csc:CHEMONTID_0003413
        a                skos:Concept ;
        rdfs:seeAlso     tax_nodes:C0003413 ;
        skos:altLabel    "organosulfur heterocyclic compound"@en , "organic heterobicyclic compound"@en ;
        skos:broader     csc:CHEMONTID_0003412 ;
        skos:definition  "Organic aromatic compounds that 1-benzothiopyran, a bicyclic compound made up of a benzene ring fused to a thiopyran, so that the sulfur atom is at the 1-position."@en ;
        skos:inScheme    vlcs:chemische_stof ;
        skos:notation    "CHEMONTID:0003413" ;
        skos:prefLabel   "1-benzothiopyrans"@en .

csc:CHEMONTID_0002010
        a                skos:Concept ;
        rdfs:seeAlso     tax_nodes:C0002010 ;
        skos:altLabel    "peptide"@en ;
        skos:broader     csc:CHEMONTID_0001813 ;
        skos:definition  "Compounds containing at least two different types of amino acids (alpha, beta, gamma, delta) linked to each other through a peptide bond."@en ;
        skos:inScheme    vlcs:chemische_stof ;
        skos:notation    "CHEMONTID:0002010" ;
        skos:prefLabel   "Hybrid peptides"@en .

csc:CHEMONTID_0002982
        a                skos:Concept ;
        skos:broader     csc:CHEMONTID_0001935 ;
        skos:definition  "Urea derivatives where one nitrogen atom of the urea group is linked to a phenyl group and the other is acylated."@en ;
        skos:inScheme    vlcs:chemische_stof ;
        skos:notation    "CHEMONTID:0002982" ;
        skos:prefLabel   "N-acyl-phenylureas"@en .

csc:CHEMONTID_0000526
        a                skos:Concept ;
        rdfs:seeAlso     tax_nodes:C0000526 ;
        skos:altLabel    "inorganic oxide"@en , "alkali metal salt"@en ;
        skos:broader     csc:CHEMONTID_0000456 ;
        skos:definition  "Inorganic compounds containing an oxygen atom of an oxidation state of -2, in which the heaviest atom bonded to the oxygen is an alkali metal."@en ;
        skos:inScheme    vlcs:chemische_stof ;
        skos:notation    "CHEMONTID:0000526" ;
        skos:prefLabel   "Alkali metal oxides"@en .

csc:CHEMONTID_0002484
        a                skos:Concept ;
        rdfs:seeAlso     tax_nodes:C0002484 ;
        skos:altLabel    "carboximidic acid"@en ;
        skos:broader     csc:CHEMONTID_0002285 ;
        skos:definition  "Organic acids with the general formula RC(=N)-OH (R=H, organic group)."@en ;
        skos:inScheme    vlcs:chemische_stof ;
        skos:notation    "CHEMONTID:0002484" ;
        skos:prefLabel   "Carboximidic acids"@en .

csc:CHEMONTID_0001975
        a                skos:Concept ;
        rdfs:seeAlso     tax_nodes:C0001975 ;
        skos:altLabel    "pyrrolidines"@en , "pyridines"@en ;
        skos:broader     csc:CHEMONTID_0000089 ;
        skos:definition  "Compounds containing a pyrrolidinylpyridine ring system, which consists of a pyrrolidine ring linked to a pyridine ring."@en ;
        skos:inScheme    vlcs:chemische_stof ;
        skos:notation    "CHEMONTID:0001975" ;
        skos:prefLabel   "Pyrrolidinylpyridines"@en .

csc:CHEMONTID_0002950
        a                skos:Concept ;
        skos:altLabel    "very long-chain fatty acid"@en ;
        skos:broader     csc:CHEMONTID_0000262 ;
        skos:definition  "Fatty acids with an aliphatic tail that contains at least 22 carbon atoms."@en ;
        skos:inScheme    vlcs:chemische_stof ;
        skos:notation    "CHEMONTID:0002950" ;
        skos:prefLabel   "Very long-chain fatty acids"@en .

csc:CHEMONTID_0003809
        a                skos:Concept ;
        rdfs:seeAlso     tax_nodes:C0003809 ;
        skos:altLabel    "a diorganylglycerol"@en , "Diradylglycerols"@en , "disubstituted glycerol"@en , "Diorganylglycerols"@en ;
        skos:broader     csc:CHEMONTID_0000175 ;
        skos:definition  "Glycerolipids that carry exactly two acyl chains attached to the glycerol moiety."@en ;
        skos:inScheme    vlcs:chemische_stof ;
        skos:notation    "CHEMONTID:0003809" ;
        skos:prefLabel   "Diradylglycerols"@en .

csc:CHEMONTID_0001722
        a                skos:Concept ;
        rdfs:seeAlso     tax_nodes:C0001722 ;
        skos:altLabel    "carboxylic ester"@en ;
        skos:broader     csc:CHEMONTID_0003909 ;
        skos:definition  "Ester derivatives of a fatty alcohol."@en ;
        skos:inScheme    vlcs:chemische_stof ;
        skos:notation    "CHEMONTID:0001722" ;
        skos:prefLabel   "Fatty alcohol esters"@en .

csc:CHEMONTID_0004111
        a                skos:Concept ;
        skos:altLabel    "dimethoxybenzene"@en ;
        skos:broader     csc:CHEMONTID_0004113 ;
        skos:definition  "Organic aromatic compounds containing a monocyclic benzene moiety carrying exactly two methoxy groups."@en ;
        skos:inScheme    vlcs:chemische_stof ;
        skos:notation    "CHEMONTID:0004111" ;
        skos:prefLabel   "Dimethoxybenzenes"@en .

csc:CHEMONTID_0000074
        a                skos:Concept ;
        rdfs:seeAlso     tax_nodes:C0000074 ;
        skos:altLabel    "Pyridazines"@en , "pyridazines"@en ;
        skos:broader     csc:CHEMONTID_0001346 ;
        skos:definition  "Compounds containing a pyridazine ring, which is a six-member aromatic ring containing two nitrogen atoms at positions 1 and 2, and four carbon atoms."@en ;
        skos:inScheme    vlcs:chemische_stof ;
        skos:notation    "CHEMONTID:0000074" ;
        skos:prefLabel   "Pyridazines and derivatives"@en .

csc:CHEMONTID_0002452
        a                skos:Concept ;
        skos:altLabel    "tertiary amine"@en , "a tertiary amine"@en ;
        skos:broader     csc:CHEMONTID_0002449 ;
        skos:definition  "Amines having the nitrogen atom linked to exactly three hydrocarbyl groups."@en ;
        skos:inScheme    vlcs:chemische_stof ;
        skos:notation    "CHEMONTID:0002452" ;
        skos:prefLabel   "Tertiary amines"@en .

csc:CHEMONTID_0004830
        a                skos:Concept ;
        skos:altLabel    "alpha-dipeptides"@en ;
        skos:broader     csc:CHEMONTID_0000348 ;
        skos:definition  "Organic compounds containing a sequence of exactly two alpha-amino acids joined by a peptide bond."@en ;
        skos:inScheme    vlcs:chemische_stof ;
        skos:notation    "CHEMONTID:0004830" ;
        skos:prefLabel   "Dipeptides"@en .

csc:CHEMONTID_0000295
        a                skos:Concept ;
        rdfs:seeAlso     tax_nodes:C0000295 ;
        skos:altLabel    "Benzodiazepines"@en ;
        skos:broader     csc:CHEMONTID_0000002 ;
        skos:definition  "Organic compounds containing a benzene ring fused to either isomers of diazepine(unsaturated seven-member heterocycle with two nitrogen atoms replacing two carbon atoms)."@en ;
        skos:inScheme    vlcs:chemische_stof ;
        skos:notation    "CHEMONTID:0000295" ;
        skos:prefLabel   "Benzodiazepines"@en .

csc:CHEMONTID_0003357
        a                skos:Concept ;
        skos:altLabel    "N-alkylpiperazine"@en ;
        skos:broader     csc:CHEMONTID_0000189 ;
        skos:definition  "Organic compounds containing a piperazine ring where the nitrogen ring atom carries an alkyl group."@en ;
        skos:inScheme    vlcs:chemische_stof ;
        skos:notation    "CHEMONTID:0003357" ;
        skos:prefLabel   "N-alkylpiperazines"@en .

csc:CHEMONTID_0001270
        a                skos:Concept ;
        rdfs:seeAlso     tax_nodes:C0001270 ;
        skos:broader     csc:CHEMONTID_0000424 ;
        skos:definition  "Inorganic compounds containing non-metal as well as metal atoms but not belonging to afore mentioned classes."@en ;
        skos:inScheme    vlcs:chemische_stof ;
        skos:notation    "CHEMONTID:0001270" ;
        skos:prefLabel   "Miscellaneous mixed metal/non-metals"@en .

csc:CHEMONTID_0004009
        a                skos:Concept ;
        skos:altLabel    "phthalate ester"@en ;
        skos:broader     csc:CHEMONTID_0001105 ;
        skos:definition  "Ester derivatives of phthalic acids, which are based on a benzene dicarboxylic acid skeleton."@en ;
        skos:inScheme    vlcs:chemische_stof ;
        skos:notation    "CHEMONTID:0004009" ;
        skos:prefLabel   "Phthalate esters"@en .

csc:CHEMONTID_0001168
        a                skos:Concept ;
        rdfs:seeAlso     tax_nodes:C0001168 ;
        skos:altLabel    "acetal"@en ;
        skos:broader     csc:CHEMONTID_0000323 ;
        skos:definition  "Organic compounds comprising the ketene acetal functional group, with the general structure XC(Y)=C(R3)R4 (R1,R2=H, alkyl, aryl; X,Y=any hetero atom)."@en ;
        skos:inScheme    vlcs:chemische_stof ;
        skos:notation    "CHEMONTID:0001168" ;
        skos:prefLabel   "Ketene acetals"@en .

csc:CHEMONTID_0004521
        a                skos:Concept ;
        skos:broader     csc:CHEMONTID_0001026 ;
        skos:definition  "Alkyhalide compounds that are composed only of chlorine, fluorine, and carbon atoms."@en ;
        skos:inScheme    vlcs:chemische_stof ;
        skos:notation    "CHEMONTID:0004521" ;
        skos:prefLabel   "Chlorofluorocarbons"@en .

csc:CHEMONTID_0004742
        a                skos:Concept ;
        rdfs:seeAlso     tax_nodes:C0004742 ;
        skos:broader     csc:CHEMONTID_0002279 ;
        skos:definition  "Aromatic compounds contaning a phenoxy group."@en ;
        skos:inScheme    vlcs:chemische_stof ;
        skos:notation    "CHEMONTID:0004742" ;
        skos:prefLabel   "Phenoxy compounds"@en .

csc:CHEMONTID_0003094
        a                skos:Concept ;
        rdfs:seeAlso     tax_nodes:C0003094 ;
        skos:altLabel    "thiadiazinane"@en ;
        skos:broader     csc:CHEMONTID_0000002 ;
        skos:definition  "Organic heterocyclic compounds containing a six-membered saturated heterocycle with two nitrogen, one sulfur, and three carbon atoms."@en ;
        skos:inScheme    vlcs:chemische_stof ;
        skos:notation    "CHEMONTID:0003094" ;
        skos:prefLabel   "Thiadiazinanes"@en .

csc:CHEMONTID_0001357
        a                skos:Concept ;
        skos:altLabel    "diterpenoid"@en , "Acyclic diterpenoids"@en ;
        skos:broader     csc:CHEMONTID_0001551 ;
        skos:definition  "Diterpenoids (compounds made of four consecutive isoprene units) that do not contain a cycle."@en ;
        skos:inScheme    vlcs:chemische_stof ;
        skos:notation    "CHEMONTID:0001357" ;
        skos:prefLabel   "Acyclic diterpenoids"@en .

csc:CHEMONTID_0000129
        a                skos:Concept ;
        rdfs:seeAlso     tax_nodes:C0000129 ;
        skos:altLabel    "An alcohol"@en , "an alcohol"@en ;
        skos:broader     csc:CHEMONTID_0000323 ;
        skos:definition  "Organic compounds in which at least one hydroxyl functional group (-OH) is bound to a carbon atom, usually connected to other carbon or hydrogen atoms."@en ;
        skos:inScheme    vlcs:chemische_stof ;
        skos:notation    "CHEMONTID:0000129" ;
        skos:prefLabel   "Alcohols and polyols"@en .

csc:CHEMONTID_0002507
        a                skos:Concept ;
        rdfs:seeAlso     tax_nodes:C0002507 ;
        skos:altLabel    "homoflavonoid"@en ;
        skos:broader     csc:CHEMONTID_0000261 ;
        skos:definition  "Naturally occurring oxygen heterocycles with a structure based on a 16-carbon skeleton including a chromanone, chromone or chromane system with a benzyl group at position C-3."@en ;
        skos:inScheme    vlcs:chemische_stof ;
        skos:notation    "CHEMONTID:0002507" ;
        skos:prefLabel   "Homoisoflavonoids"@en .

csc:CHEMONTID_0000420
        a                skos:Concept ;
        skos:altLabel    "Chlorodibenzo-para-dioxins"@en , "Chlorinated Dibenzo-para-dioxins"@en , "dibenzodioxine"@en , "Chlorodibenzo-p-dioxins"@en ;
        skos:broader     csc:CHEMONTID_0001381 ;
        skos:definition  "Organic compounds containing a chlorine atom attached to a dibenzo-p-dioxin moiety."@en ;
        skos:inScheme    vlcs:chemische_stof ;
        skos:notation    "CHEMONTID:0000420" ;
        skos:prefLabel   "Chlorinated dibenzo-p-dioxins"@en .

csc:CHEMONTID_0001150
        a                skos:Concept ;
        skos:altLabel    "imidazolidinone"@en ;
        skos:broader     csc:CHEMONTID_0001149 ;
        skos:definition  "Organic compounds containing an imidazolidinedione moiety, which is an imidazolidine ring bearing two ketones."@en ;
        skos:inScheme    vlcs:chemische_stof ;
        skos:notation    "CHEMONTID:0001150" ;
        skos:prefLabel   "Imidazolidinediones"@en .

csc:CHEMONTID_0004212
        a                skos:Concept ;
        skos:broader     csc:CHEMONTID_0004208 ;
        skos:definition  "Aromatic compounds that contain a xylene moiety, which is a monocyclic benzene carrying exactly two methyl groups, and at least one hydroxyl group."@en ;
        skos:inScheme    vlcs:chemische_stof ;
        skos:notation    "CHEMONTID:0004212" ;
        skos:prefLabel   "Xylenols"@en .

csc:CHEMONTID_0000175
        a                skos:Concept ;
        rdfs:seeAlso     tax_nodes:C0000175 ;
        skos:altLabel    "glycerolipid"@en , "Glycerolipids"@en ;
        skos:broader     csc:CHEMONTID_0000012 ;
        skos:definition  "Lipids formed by joining fatty acids to glycerol by ester bonds."@en ;
        skos:inScheme    vlcs:chemische_stof ;
        skos:notation    "CHEMONTID:0000175" ;
        skos:prefLabel   "Glycerolipids"@en .

csc:CHEMONTID_0001578
        a                skos:Concept ;
        rdfs:seeAlso     tax_nodes:C0001578 ;
        skos:altLabel    "benzofurans"@en ;
        skos:broader     csc:CHEMONTID_0000301 ;
        skos:definition  "Organic compounds containing a benzene ring fused to a furanone."@en ;
        skos:inScheme    vlcs:chemische_stof ;
        skos:notation    "CHEMONTID:0001578" ;
        skos:prefLabel   "Benzofuranones"@en .

csc:CHEMONTID_0003956
        a                skos:Concept ;
        skos:altLabel    "aromatic amine"@en , "biphenyls"@en ;
        skos:broader     csc:CHEMONTID_0003955 ;
        skos:definition  "Organic compounds containing a benzidine skeleton, which is substituted only at the 3-  and 3'-positions."@en ;
        skos:inScheme    vlcs:chemische_stof ;
        skos:notation    "CHEMONTID:0003956" ;
        skos:prefLabel   "3,3'-disubstituted benzidines"@en .

csc:CHEMONTID_0003030
        a                skos:Concept ;
        skos:altLabel    "Polychlorinated Biphenyls"@en , "polychlorobiphenyl"@en , "PCBs"@en ;
        skos:broader     csc:CHEMONTID_0000500 ;
        skos:definition  "Organic compounds containing at least two chlorine atoms attached to either benzene ring of the biphenyl moiety."@en ;
        skos:inScheme    vlcs:chemische_stof ;
        skos:notation    "CHEMONTID:0003030" ;
        skos:prefLabel   "Polychlorinated biphenyls"@en .

csc:CHEMONTID_0000143
        a                skos:Concept ;
        skos:altLabel    "bisphenols"@en , "bisphenol"@en ;
        skos:broader     csc:CHEMONTID_0000369 ;
        skos:definition  "Methylenediphenols, HOC6H4CH2C6H4OH, commonly p,p-methylenediphenol, and their substitution products (generally derived from condensation of two equivalent amounts of a phenol with an aldehyde or ketone)."@en ;
        skos:inScheme    vlcs:chemische_stof ;
        skos:notation    "CHEMONTID:0000143" ;
        skos:prefLabel   "Bisphenols"@en .

csc:CHEMONTID_0003205
        a                skos:Concept ;
        skos:altLabel    "siloxane"@en ;
        skos:broader     csc:CHEMONTID_0004446 ;
        skos:definition  "Organosilicon compounds with the general formula H[Si](R)(R')O[Si](H)(R'')R'''  (R= organyl, R'-R'''= H or organyl)."@en ;
        skos:inScheme    vlcs:chemische_stof ;
        skos:notation    "CHEMONTID:0003205" ;
        skos:prefLabel   "Disiloxanes"@en .

csc:CHEMONTID_0003924
        a                skos:Concept ;
        skos:altLabel    "phenylalkylamine"@en ;
        skos:broader     csc:CHEMONTID_0003899 ;
        skos:definition  "Organic amines where the amine group is secondary and linked on one end to a phenyl group and on the other end, to an alkyl group."@en ;
        skos:inScheme    vlcs:chemische_stof ;
        skos:notation    "CHEMONTID:0003924" ;
        skos:prefLabel   "Phenylalkylamines"@en .

csc:CHEMONTID_0001546
        a                skos:Concept ;
        skos:altLabel    "Vitamin E"@en , "tocol"@en ;
        skos:broader     csc:CHEMONTID_0001534 ;
        skos:definition  "A group of fat-soluble compounds containing or derived either from a tocopherol or a tocotrienol skeleton."@en ;
        skos:inScheme    vlcs:chemische_stof ;
        skos:notation    "CHEMONTID:0001546" ;
        skos:prefLabel   "Vitamin E compounds"@en .

csc:CHEMONTID_0002949
        a                skos:Concept ;
        skos:altLabel    "LCFA"@en , "Long-chain fatty acid"@en , "LCFAs"@en , " a long-chain fatty acid"@en , "long-chain fatty acid"@en ;
        skos:broader     csc:CHEMONTID_0000262 ;
        skos:definition  "Fatty acids with an aliphatic tail that contains between 13 and 21 carbon atoms."@en ;
        skos:inScheme    vlcs:chemische_stof ;
        skos:notation    "CHEMONTID:0002949" ;
        skos:prefLabel   "Long-chain fatty acids"@en .

csc:CHEMONTID_0000318
        a                skos:Concept ;
        skos:broader     csc:CHEMONTID_0000347 ;
        skos:definition  "Compounds comprising the carbamic acid functional group or a derivative thereof. They have the general structure RN(R')C(=O)OH or RN(R')C(=O)R\", where R,R'= H or organyl group, R\"= OH, alkyloxy, acyloxy, or halogen."@en ;
        skos:inScheme    vlcs:chemische_stof ;
        skos:notation    "CHEMONTID:0000318" ;
        skos:prefLabel   "Carbamic acids and derivatives"@en .

csc:CHEMONTID_0002995
        a                skos:Concept ;
        rdfs:seeAlso     tax_nodes:C0002995 ;
        skos:broader     csc:CHEMONTID_0000265 ;
        skos:definition  "Carboxylic acids containing exactly five carboxyl groups."@en ;
        skos:inScheme    vlcs:chemische_stof ;
        skos:notation    "CHEMONTID:0002995" ;
        skos:prefLabel   "Pentacarboxylic acids and derivatives"@en .

csc:CHEMONTID_0003970
        a                skos:Concept ;
        rdfs:seeAlso     tax_nodes:C0003970 ;
        skos:altLabel    "pyridines"@en , "organohalogen compound"@en ;
        skos:broader     csc:CHEMONTID_0000089 ;
        skos:definition  "Organic compounds containing a pyridine ring substituted at one or more positions by a halogen atom."@en ;
        skos:inScheme    vlcs:chemische_stof ;
        skos:notation    "CHEMONTID:0003970" ;
        skos:prefLabel   "Halopyridines"@en .

csc:CHEMONTID_0000364
        a                skos:Concept ;
        rdfs:seeAlso     tax_nodes:C0000364 ;
        skos:altLabel    "organooxygen compound"@en ;
        skos:broader     csc:CHEMONTID_0000264 ;
        skos:definition  "Compounds comprising the organic carbonic acid or a derivative thereof."@en ;
        skos:inScheme    vlcs:chemische_stof ;
        skos:notation    "CHEMONTID:0000364" ;
        skos:prefLabel   "Organic carbonic acids and derivatives"@en .

csc:CHEMONTID_0001767
        a                skos:Concept ;
        skos:altLabel    "gibberellin"@en , "Gibberellins"@en ;
        skos:broader     csc:CHEMONTID_0001551 ;
        skos:definition  "Diterpenoids containing the gibberellane skeleton ((8S)-4,4,8-trimethyl-13-methylidenetetracyclo[10.2.1.0^{1,9}.0^{3,8}]pentadecane), an aliphatic four-ring system."@en ;
        skos:inScheme    vlcs:chemische_stof ;
        skos:notation    "CHEMONTID:0001767" ;
        skos:prefLabel   "Gibberellins"@en .

csc:CHEMONTID_0002497
        a                skos:Concept ;
        rdfs:seeAlso     tax_nodes:C0002497 ;
        skos:altLabel    "Indoles"@en , "indoles"@en ;
        skos:broader     csc:CHEMONTID_0000211 ;
        skos:definition  "Compounds containing an indole moiety, which consists of pyrrole ring fused to benzene  to form 2,3-benzopyrrole."@en ;
        skos:inScheme    vlcs:chemische_stof ;
        skos:notation    "CHEMONTID:0002497" ;
        skos:prefLabel   "Indoles"@en .

csc:CHEMONTID_0004622
        a                skos:Concept ;
        rdfs:seeAlso     tax_nodes:C0004622 ;
        skos:broader     csc:CHEMONTID_0004475 ;
        skos:definition  "Hydrocarbons that contains one or more unsaturated carbon atoms, and an aliphatic branch."@en ;
        skos:inScheme    vlcs:chemische_stof ;
        skos:notation    "CHEMONTID:0004622" ;
        skos:prefLabel   "Branched unsaturated hydrocarbons"@en .

csc:CHEMONTID_0001016
        a                skos:Concept ;
        rdfs:seeAlso     tax_nodes:C0001016 ;
        skos:altLabel    "cycloalkanes"@en , "cycloalkane"@en ;
        skos:broader     csc:CHEMONTID_0004474 ;
        skos:definition  "Saturated monocyclic hydrocarbons (with or without side chains)."@en ;
        skos:inScheme    vlcs:chemische_stof ;
        skos:notation    "CHEMONTID:0001016" ;
        skos:prefLabel   "Cycloalkanes"@en .

csc:CHEMONTID_0000087
        a                skos:Concept ;
        rdfs:seeAlso     tax_nodes:C0000087 ;
        skos:altLabel    "Pyrazoles"@en ;
        skos:broader     csc:CHEMONTID_0000436 ;
        skos:definition  "Compounds containing a pyrazole ring, which is a five-member aromatic ring with two nitrogen atoms (at positions 1 and 2) and three carbon atoms."@en ;
        skos:inScheme    vlcs:chemische_stof ;
        skos:notation    "CHEMONTID:0000087" ;
        skos:prefLabel   "Pyrazoles"@en .

csc:CHEMONTID_0001062
        a                skos:Concept ;
        rdfs:seeAlso     tax_nodes:C0001062 ;
        skos:altLabel    "inorganic nitrate salt"@en , "p-block molecular entity"@en ;
        skos:broader     csc:CHEMONTID_0000435 ;
        skos:definition  "Inorganic non-metallic compounds containing a nitrate as its largest oxoanion."@en , "Inorganic non-metallic compoundscontaining a nitrate as its largest oxoanion."@en ;
        skos:inScheme    vlcs:chemische_stof ;
        skos:notation    "CHEMONTID:0001062" ;
        skos:prefLabel   "Non-metal nitrates"@en .

csc:CHEMONTID_0000553
        a                skos:Concept ;
        rdfs:seeAlso     tax_nodes:C0000553 ;
        skos:altLabel    "nitride"@en ;
        skos:broader     csc:CHEMONTID_0000453 ;
        skos:definition  "Inorganic compounds of nitrogen where nitrogen has a formal oxidation state of -3, and the heaviest atom bonded to it belongs to the class of 'other non-metals'."@en , "Inorganic compounds of nitrogen where nitrogen has a formal oxidation state of −3, and the heaviest atom bonded to it belongs to the class of 'other non-metals'."@en ;
        skos:inScheme    vlcs:chemische_stof ;
        skos:notation    "CHEMONTID:0000553" ;
        skos:prefLabel   "Other non-metal nitrides"@en .

csc:CHEMONTID_0001030
        a                skos:Concept ;
        rdfs:seeAlso     tax_nodes:C0001030 ;
        skos:altLabel    "organochlorine compound"@en ;
        skos:broader     csc:CHEMONTID_0002866 ;
        skos:definition  "Organic compounds containing the acyl chloride functional group."@en ;
        skos:inScheme    vlcs:chemische_stof ;
        skos:notation    "CHEMONTID:0001030" ;
        skos:prefLabel   "Aryl chlorides"@en .

csc:CHEMONTID_0000055
        a                skos:Concept ;
        rdfs:seeAlso     tax_nodes:C0000055 ;
        skos:altLabel    "dibenzothiazepine"@en , "Dibenzothiazepines"@en ;
        skos:broader     csc:CHEMONTID_0000317 ;
        skos:definition  "Compounds containing a dibenzothiazepine moiety, which consists of two benzene connected by a thiazepine ring."@en ;
        skos:inScheme    vlcs:chemische_stof ;
        skos:notation    "CHEMONTID:0000055" ;
        skos:prefLabel   "Dibenzothiazepines"@en .

csc:CHEMONTID_0002433
        a                skos:Concept ;
        skos:altLabel    "alpha,beta-unsaturated aldehyde"@en ;
        skos:broader     csc:CHEMONTID_0003131 ;
        skos:definition  "Aldehydes of general formula R(1)R(2)C=CR(3)-CH=O or RC#C-CH=O in which the aldehydic C=O function is conjugated to an unsaturated C-C bond at the alpha,beta position."@en ;
        skos:inScheme    vlcs:chemische_stof ;
        skos:notation    "CHEMONTID:0002433" ;
        skos:prefLabel   "Alpha,beta-unsaturated aldehydes"@en .

csc:CHEMONTID_0001205
        a                skos:Concept ;
        rdfs:seeAlso     tax_nodes:C0001205 ;
        skos:altLabel    "carboxylic acids"@en , "a carboxylate"@en , "Carboxylic Acids"@en ;
        skos:broader     csc:CHEMONTID_0000265 ;
        skos:definition  "Compounds containing a carboxylic acid group with the formula -C(=O)OH."@en ;
        skos:inScheme    vlcs:chemische_stof ;
        skos:notation    "CHEMONTID:0001205" ;
        skos:prefLabel   "Carboxylic acids"@en .

csc:CHEMONTID_0002608
        a                skos:Concept ;
        rdfs:seeAlso     tax_nodes:C0002608 ;
        skos:altLabel    "organochlorine compound"@en , "alcohol"@en ;
        skos:broader     csc:CHEMONTID_0002528 ;
        skos:definition  "Alcohols substituted by a chlorine atom at a saturated carbon atom otherwise bearing only hydrogen or hydrocarbyl groups."@en ;
        skos:inScheme    vlcs:chemische_stof ;
        skos:notation    "CHEMONTID:0002608" ;
        skos:prefLabel   "Chlorohydrins"@en .

csc:CHEMONTID_0001924
        a                skos:Concept ;
        skos:altLabel    "pyridazines"@en ;
        skos:broader     csc:CHEMONTID_0000074 ;
        skos:definition  "Organic compounds containing an amino group attached to a pyridazine ring."@en ;
        skos:inScheme    vlcs:chemische_stof ;
        skos:notation    "CHEMONTID:0001924" ;
        skos:prefLabel   "Aminopyridazines"@en .

csc:CHEMONTID_0003338
        a                skos:Concept ;
        skos:altLabel    "a polyethylene oxide"@en , "a polyethylene glycol"@en , "poly(ethylene glycol)"@en , "Polyethylene oxides"@en ;
        skos:broader     csc:CHEMONTID_0001167 ;
        skos:definition  "Oligomers or polymers of ethylene oxide, with the general formula (C2H4O)n (with n>=3)."@en ;
        skos:inScheme    vlcs:chemische_stof ;
        skos:notation    "CHEMONTID:0003338" ;
        skos:prefLabel   "Polyethylene glycols"@en .

csc:CHEMONTID_0000023
        a                skos:Concept ;
        rdfs:seeAlso     tax_nodes:C0000023 ;
        skos:altLabel    "naphthalenes"@en , "Naphthalenes"@en ;
        skos:broader     csc:CHEMONTID_0002448 ;
        skos:definition  "Compounds containing a naphthalene moiety, which consists of two fused benzene rings."@en ;
        skos:inScheme    vlcs:chemische_stof ;
        skos:notation    "CHEMONTID:0000023" ;
        skos:prefLabel   "Naphthalenes"@en .

csc:CHEMONTID_0003384
        a                skos:Concept ;
        skos:altLabel    "organic thiophosphate"@en , "phosphorothioic acid triesters"@en ;
        skos:broader     csc:CHEMONTID_0001572 ;
        skos:definition  "Organic compounds containing the thiophosphoric acid functional group or a derivative thereof, with the general structure ROP(OR')(OR'')=S, where exactly three R-groups are organyl groups."@en ;
        skos:inScheme    vlcs:chemische_stof ;
        skos:notation    "CHEMONTID:0003384" ;
        skos:prefLabel   "Thiophosphate triesters"@en .

csc:CHEMONTID_0004787
        a                skos:Concept ;
        skos:broader     csc:CHEMONTID_0001162 ;
        skos:definition  "Methyl esters of carbamic acid."@en ;
        skos:inScheme    vlcs:chemische_stof ;
        skos:notation    "CHEMONTID:0004787" ;
        skos:prefLabel   "Methylcarbamates"@en .

csc:CHEMONTID_0003131
        a                skos:Concept ;
        skos:altLabel    "carbonyl compound"@en ;
        skos:broader     csc:CHEMONTID_0001831 ;
        skos:definition  "Carbonyl compounds with the general structure R#CC(=O)R' or R=CC(=O)R', where R=organyl, R'=H, N, O, organyl group or halide group."@en ;
        skos:inScheme    vlcs:chemische_stof ;
        skos:notation    "CHEMONTID:0003131" ;
        skos:prefLabel   "Alpha,beta-unsaturated carbonyl compounds"@en .

csc:CHEMONTID_0004289
        a                skos:Concept ;
        skos:broader     csc:CHEMONTID_0004024 ;
        skos:definition  "Compounds containing a lead compound bonded to four carbon atoms."@en ;
        skos:inScheme    vlcs:chemische_stof ;
        skos:notation    "CHEMONTID:0004289" ;
        skos:prefLabel   "Tetraorganolead compounds"@en .

csc:CHEMONTID_0000419
        a                skos:Concept ;
        rdfs:seeAlso     tax_nodes:C0000419 ;
        skos:altLabel    "phosphonic acids"@en ;
        skos:broader     csc:CHEMONTID_0000264 ;
        skos:definition  "Organic compounds containing phosphonic acid or a derivative thereof."@en ;
        skos:inScheme    vlcs:chemische_stof ;
        skos:notation    "CHEMONTID:0000419" ;
        skos:prefLabel   "Organic phosphonic acids and derivatives"@en .

csc:CHEMONTID_0001693
        a                skos:Concept ;
        rdfs:seeAlso     tax_nodes:C0001693 ;
        skos:altLabel    "triazines"@en , "Triazinamines"@en ;
        skos:broader     csc:CHEMONTID_0000098 ;
        skos:definition  "Organic compounds containing an amino group attached to a triazine ring."@en ;
        skos:inScheme    vlcs:chemische_stof ;
        skos:notation    "CHEMONTID:0001693" ;
        skos:prefLabel   "Aminotriazines"@en .

csc:CHEMONTID_0004755
        a                skos:Concept ;
        skos:broader     csc:CHEMONTID_0004712 ;
        skos:definition  "Aromatic anilides with the general structure RC(=O)N(R')R\", where R=furan, and R\"=benzene."@en ;
        skos:inScheme    vlcs:chemische_stof ;
        skos:notation    "CHEMONTID:0004755" ;
        skos:prefLabel   "Furanilides"@en .

csc:CHEMONTID_0001149
        a                skos:Concept ;
        skos:altLabel    "imidazolidinone"@en ;
        skos:broader     csc:CHEMONTID_0000250 ;
        skos:definition  "Organic compounds containing an imidazolidinone moiety, which is an imidazolidine ring bearing a ketone."@en ;
        skos:inScheme    vlcs:chemische_stof ;
        skos:notation    "CHEMONTID:0001149" ;
        skos:prefLabel   "Imidazolidinones"@en .

csc:CHEMONTID_0004502
        a                skos:Concept ;
        rdfs:seeAlso     tax_nodes:C0004502 ;
        skos:broader     csc:CHEMONTID_0000289 ;
        skos:definition  "Nucleosides in which the oxygen atom at the 5'position of the ribose moiety has been replaced by another atom. The nucleobases here are limited to purine, pyrimidine, and pyridine derivatives."@en ;
        skos:inScheme    vlcs:chemische_stof ;
        skos:notation    "CHEMONTID:0004502" ;
        skos:prefLabel   "5'-deoxyribonucleosides"@en .

csc:CHEMONTID_0003573
        a                skos:Concept ;
        skos:altLabel    "2-deoxystreptamine derivative"@en ;
        skos:broader     csc:CHEMONTID_0003575 ;
        skos:definition  "2-deoxystreptamine aminoglycosides that a glycosidically linked to a pyranose of furanose unit at the C4- and C5-positions."@en ;
        skos:inScheme    vlcs:chemische_stof ;
        skos:notation    "CHEMONTID:0003573" ;
        skos:prefLabel   "4,5-disubstituted 2-deoxystreptamines"@en .

csc:CHEMONTID_0003029
        a                skos:Concept ;
        skos:altLabel    "dibenzofurans"@en , "organochlorine compound"@en ;
        skos:broader     csc:CHEMONTID_0001378 ;
        skos:definition  "Organic compounds containing two or more chlorine atoms attached to a dibenzofuran moiety."@en ;
        skos:inScheme    vlcs:chemische_stof ;
        skos:notation    "CHEMONTID:0003029" ;
        skos:prefLabel   "Polychlorinated dibenzofurans"@en .

csc:CHEMONTID_0002345
        a                skos:Concept ;
        skos:altLabel    "methoxybenzoic acid"@en ;
        skos:broader     csc:CHEMONTID_0002344 ;
        skos:definition  "Benzoic acids in which the hydrogen atom at position 2 of the benzene ring is replaced by a methoxy group."@en ;
        skos:inScheme    vlcs:chemische_stof ;
        skos:notation    "CHEMONTID:0002345" ;
        skos:prefLabel   "O-methoxybenzoic acids and derivatives"@en .

csc:CHEMONTID_0001661
        a                skos:Concept ;
        skos:altLabel    "secondary alcohol"@en ;
        skos:broader     csc:CHEMONTID_0000129 ;
        skos:definition  "Compounds containing a secondary alcohol functional group, with the general structure HOC(R)(R') (R,R'=alkyl, aryl)."@en ;
        skos:inScheme    vlcs:chemische_stof ;
        skos:notation    "CHEMONTID:0001661" ;
        skos:prefLabel   "Secondary alcohols"@en .

csc:CHEMONTID_0000433
        a                skos:Concept ;
        rdfs:seeAlso     tax_nodes:C0000433 ;
        skos:altLabel    "noble gas molecular entity"@en ;
        skos:broader     csc:CHEMONTID_0000423 ;
        skos:definition  "Inorganic non-metallic compounds in which the largest atom is a halogen atom."@en ;
        skos:inScheme    vlcs:chemische_stof ;
        skos:notation    "CHEMONTID:0000433" ;
        skos:prefLabel   "Homogeneous noble gases"@en .

csc:CHEMONTID_0004050
        a                skos:Concept ;
        skos:broader     csc:CHEMONTID_0001027 ;
        skos:definition  "Organic compounds containing an alkyl chain attached to the sulfur of an organosulfonyl fluoride group, where all hydrogens of the alkyl chain are replaced by fluorine atoms."@en ;
        skos:inScheme    vlcs:chemische_stof ;
        skos:notation    "CHEMONTID:0004050" ;
        skos:prefLabel   "Perfluoroalkanesulfonyl fluorides"@en .

csc:CHEMONTID_0002811
        a                skos:Concept ;
        rdfs:seeAlso     tax_nodes:C0002811 ;
        skos:altLabel    "alkylbenzene"@en ;
        skos:broader     csc:CHEMONTID_0002279 ;
        skos:definition  "Organic compounds containing a phenylpropane moiety."@en ;
        skos:inScheme    vlcs:chemische_stof ;
        skos:notation    "CHEMONTID:0002811" ;
        skos:prefLabel   "Phenylpropanes"@en .

csc:CHEMONTID_0004478
        a                skos:Concept ;
        rdfs:seeAlso     tax_nodes:C0004478 ;
        skos:altLabel    "acetylide"@en , "acetylides"@en ;
        skos:broader     csc:CHEMONTID_0000000 ;
        skos:definition  "Compounds arising by replacement of one or both hydrogen atoms of acetylene (ethyne) by a metal or other cationic group. E.g. NaC#CH monosodium acetylide. By extension, analogous compounds derived from terminal acetylenes, RC#CH. The class is limited here to derivatives of acetylene where the hydrogen atom is replaced with an element with similar or lower electronegativity that carbon."@en ;
        skos:inScheme    vlcs:chemische_stof ;
        skos:notation    "CHEMONTID:0004478" ;
        skos:prefLabel   "Acetylides"@en .

csc:CHEMONTID_0004225
        a                skos:Concept ;
        skos:broader     csc:CHEMONTID_0000503 ;
        skos:definition  "Organonitrogen compounds containing a quaternary ammonium substituted with four alkyl chains."@en ;
        skos:inScheme    vlcs:chemische_stof ;
        skos:notation    "CHEMONTID:0004225" ;
        skos:prefLabel   "Tetraalkylammonium salts"@en .

csc:CHEMONTID_0000188
        a                skos:Concept ;
        skos:altLabel    "amphetamines"@en ;
        skos:broader     csc:CHEMONTID_0000186 ;
        skos:definition  "Organic compounds containing or derived from 1-phenylpropan-2-amine."@en ;
        skos:inScheme    vlcs:chemische_stof ;
        skos:notation    "CHEMONTID:0000188" ;
        skos:prefLabel   "Amphetamines and derivatives"@en .

csc:CHEMONTID_0002566
        a                skos:Concept ;
        rdfs:seeAlso     tax_nodes:C0002566 ;
        skos:altLabel    "isoquinolines"@en ;
        skos:broader     csc:CHEMONTID_0000002 ;
        skos:definition  "Aromatic polycyclic compounds containing an isoquinoline moiety, which consists of a benzene ring fused to a pyridine ring and forming benzo[c]pyridine."@en ;
        skos:inScheme    vlcs:chemische_stof ;
        skos:notation    "CHEMONTID:0002566" ;
        skos:prefLabel   "Isoquinolines and derivatives"@en .

csc:CHEMONTID_0003969
        a                skos:Concept ;
        skos:altLabel    "dinitrotoluene"@en ;
        skos:broader     csc:CHEMONTID_0004108 ;
        skos:definition  "Organic aromatic compounds containing a benzene that carries a single methyl group and exactly two nitro groups."@en ;
        skos:inScheme    vlcs:chemische_stof ;
        skos:notation    "CHEMONTID:0003969" ;
        skos:prefLabel   "Dinitrotoluenes"@en .

csc:CHEMONTID_0001804
        a                skos:Concept ;
        rdfs:seeAlso     tax_nodes:C0001804 ;
        skos:altLabel    "organic diphosphate"@en ;
        skos:broader     csc:CHEMONTID_0000463 ;
        skos:definition  "Organic compounds containing the pyrophosphate oxoanion, with the structure OP([O-])(=O)OP(O)([O-])=O."@en ;
        skos:inScheme    vlcs:chemische_stof ;
        skos:notation    "CHEMONTID:0001804" ;
        skos:prefLabel   "Organic pyrophosphates"@en .

csc:CHEMONTID_0004446
        a                skos:Concept ;
        skos:altLabel    "siloxanes"@en , "siloxane"@en , "Organosilicon Compounds"@en ;
        skos:broader     csc:CHEMONTID_0003194 ;
        skos:definition  "Saturated silicon-oxygen hydrides with unbranched or branched chains of alternating silicon and oxygen atoms (each silicon atom is separated from its nearest silicon neighbours by single oxygen atoms). The general structure of unbranched siloxanes is H3Si[OSiH2]nOSiH3. H3Si[OSiH2]nOSiH[OSiH2OSiH3]2 is an example of a branched siloxane. By extension hydrocarbyl derivatives are commonly included."@en ;
        skos:inScheme    vlcs:chemische_stof ;
        skos:notation    "CHEMONTID:0004446" ;
        skos:prefLabel   "Siloxanes"@en .

csc:CHEMONTID_0001850
        a                skos:Concept ;
        rdfs:seeAlso     tax_nodes:C0001850 ;
        skos:altLabel    "thiol"@en ;
        skos:broader     csc:CHEMONTID_0002448 ;
        skos:definition  "Compounds containing a thiophenol ring, which a phenol derivative obtained by replacing the oxygen atom from the hydroxyl group (attached to the benzene) by a sulfur atom."@en ;
        skos:inScheme    vlcs:chemische_stof ;
        skos:notation    "CHEMONTID:0001850" ;
        skos:prefLabel   "Thiophenols"@en .

csc:CHEMONTID_0004667
        a                skos:Concept ;
        skos:broader     csc:CHEMONTID_0000375 ;
        skos:definition  "Organonitrogen compounds containing a nitro group, which is N-linked to a guanidine."@en ;
        skos:inScheme    vlcs:chemische_stof ;
        skos:notation    "CHEMONTID:0004667" ;
        skos:prefLabel   "Nitroguanidines"@en .

csc:CHEMONTID_0003983
        a                skos:Concept ;
        skos:altLabel    "diisocyanate"@en , "toluenes"@en ;
        skos:broader     csc:CHEMONTID_0001091 ;
        skos:definition  "Organic compounds containing a benzene ring, which is substituted by a methyl group and two isocyanate groups."@en ;
        skos:inScheme    vlcs:chemische_stof ;
        skos:notation    "CHEMONTID:0003983" ;
        skos:prefLabel   "Toluene diisocyanates"@en .

csc:CHEMONTID_0000124
        a                skos:Concept ;
        skos:altLabel    "An aldehyde"@en , "aldehydes"@en , "Aldehydes"@en , "aldehyde"@en ;
        skos:broader     csc:CHEMONTID_0001831 ;
        skos:definition  "Organic compounds containing the aldehyde functional group."@en ;
        skos:inScheme    vlcs:chemische_stof ;
        skos:notation    "CHEMONTID:0000124" ;
        skos:prefLabel   "Aldehydes"@en .

csc:CHEMONTID_0001527
        a                skos:Concept ;
        rdfs:seeAlso     tax_nodes:C0001527 ;
        skos:altLabel    "nitrile"@en , "a diphenylacetonitrile"@en ;
        skos:broader     csc:CHEMONTID_0002279 ;
        skos:definition  "Cyclic aromatic compounds containing a diphenylacetonitrile moiety, which consists of a diphenylmethane linked to and acetonitrile to form 2,2-diphenylacetonitrile."@en ;
        skos:inScheme    vlcs:chemische_stof ;
        skos:notation    "CHEMONTID:0001527" ;
        skos:prefLabel   "Diphenylacetonitriles"@en .

csc:CHEMONTID_0002257
        a                skos:Concept ;
        rdfs:seeAlso     tax_nodes:C0002257 ;
        skos:altLabel    "pyrroles"@en ;
        skos:broader     csc:CHEMONTID_0000090 ;
        skos:definition  "Heterocyclic compounds containing a pyrrole ring substituted at one or more positions."@en ;
        skos:inScheme    vlcs:chemische_stof ;
        skos:notation    "CHEMONTID:0002257" ;
        skos:prefLabel   "Substituted pyrroles"@en .

csc:CHEMONTID_0004681
        a                skos:Concept ;
        rdfs:seeAlso     tax_nodes:C0004681 ;
        skos:broader     csc:CHEMONTID_0001443 ;
        skos:definition  "Polycyclic aromatic compounds containing a 1,2,4-triazolo[1,5-a]pyrimidine ring system, which is substituted with a sulfonamide at the 2-position."@en ;
        skos:inScheme    vlcs:chemische_stof ;
        skos:notation    "CHEMONTID:0004681" ;
        skos:prefLabel   "1,2,4-triazolopyrimidine-2-sulfonamides"@en .

csc:CHEMONTID_0003628
        a                skos:Concept ;
        skos:altLabel    "alpha,beta-unsaturated carboxylic ester"@en ;
        skos:broader     csc:CHEMONTID_0001238 ;
        skos:definition  "Carboxylic esters of general structure R1C(R2)=C(R3)C(=O)OR4 (R4= organyl compound) or R1C#CC(=O)OR2 (R2= organyl compound), in which the ester group is conjugated to an unsaturated C-C bond."@en ;
        skos:inScheme    vlcs:chemische_stof ;
        skos:notation    "CHEMONTID:0003628" ;
        skos:prefLabel   "Alpha,beta-unsaturated carboxylic esters"@en .

csc:CHEMONTID_0004603
        a                skos:Concept ;
        rdfs:seeAlso     tax_nodes:C0004603 ;
        skos:broader     csc:CHEMONTID_0000000 ;
        skos:definition  "Organic compounds that contain one or more oxygen atoms."@en ;
        skos:inScheme    vlcs:chemische_stof ;
        skos:notation    "CHEMONTID:0004603" ;
        skos:prefLabel   "Organic oxygen compounds"@en .

csc:CHEMONTID_0001716
        a                skos:Concept ;
        skos:altLabel    "quinolines"@en ;
        skos:broader     csc:CHEMONTID_0000056 ;
        skos:definition  "Compounds containing a hydrogenated quinoline bearing a ketone group."@en ;
        skos:inScheme    vlcs:chemische_stof ;
        skos:notation    "CHEMONTID:0001716" ;
        skos:prefLabel   "Hydroquinolones"@en .

csc:CHEMONTID_0004105
        a                skos:Concept ;
        rdfs:seeAlso     tax_nodes:C0004105 ;
        skos:altLabel    "s-Triazines"@en , "sym-Triazines"@en ;
        skos:broader     csc:CHEMONTID_0000098 ;
        skos:definition  "Compounds containing a triazine ring, which is a heterocyclic ring, similar to the six-member benzene ring but with three carbons replaced by nitrogen atoms, at ring positions 1, 3, and 5."@en ;
        skos:inScheme    vlcs:chemische_stof ;
        skos:notation    "CHEMONTID:0004105" ;
        skos:prefLabel   "1,3,5-triazines"@en .

csc:CHEMONTID_0002446
        a                skos:Concept ;
        skos:altLabel    "peroxy acid"@en , "Peroxycarboxylates"@en , "a peroxycarboxylic acid"@en ;
        skos:broader     csc:CHEMONTID_0002445 ;
        skos:definition  "Organic acids with the general formula [H]OOC(R)=O (R = H, organyl group)."@en ;
        skos:inScheme    vlcs:chemische_stof ;
        skos:notation    "CHEMONTID:0002446" ;
        skos:prefLabel   "Peroxycarboxylic acids"@en .

csc:CHEMONTID_0000534
        a                skos:Concept ;
        rdfs:seeAlso     tax_nodes:C0000534 ;
        skos:altLabel    "Metalloids"@en , "Inorganic Chemicals"@en , "p-block molecular entity"@en , "inorganic oxide"@en ;
        skos:broader     csc:CHEMONTID_0000460 ;
        skos:definition  "Inorganic compounds containing an oxygen atom of an oxidation state of -2, in which the heaviest atom bonded to the oxygen is a metalloid."@en ;
        skos:inScheme    vlcs:chemische_stof ;
        skos:notation    "CHEMONTID:0000534" ;
        skos:prefLabel   "Metalloid oxides"@en .

csc:CHEMONTID_0000289
        a                skos:Concept ;
        rdfs:seeAlso     tax_nodes:C0000289 ;
        skos:altLabel    "nucleobase-containing molecular entity"@en ;
        skos:broader     csc:CHEMONTID_0000000 ;
        skos:definition  "Compounds containing a nucleobase linked to a ribose or deoxyribose sugar via a beta-glycosidic linkage. The ribose or deoxyribose moiety bears at least a phosphate group in case of nucleotides."@en ;
        skos:inScheme    vlcs:chemische_stof ;
        skos:notation    "CHEMONTID:0000289" ;
        skos:prefLabel   "Nucleosides, nucleotides, and analogues"@en .

csc:CHEMONTID_0001983
        a                skos:Concept ;
        rdfs:seeAlso     tax_nodes:C0001983 ;
        skos:altLabel    "dihydrofuran"@en ;
        skos:broader     csc:CHEMONTID_0000002 ;
        skos:definition  "Compounds containing a dihydrofuran moiety, which is a furan derivative with only one double bond."@en ;
        skos:inScheme    vlcs:chemische_stof ;
        skos:notation    "CHEMONTID:0001983" ;
        skos:prefLabel   "Dihydrofurans"@en .

csc:CHEMONTID_0000036
        a                skos:Concept ;
        rdfs:seeAlso     tax_nodes:C0000036 ;
        skos:altLabel    "nitrobenzenes"@en , "Nitrobenzyl compounds"@en , "Nitrobenzenes"@en ;
        skos:broader     csc:CHEMONTID_0002279 ;
        skos:definition  "Compounds containing a nitrobenzene moiety, which consists of a benzene ring with a carbon bearing a nitro group."@en ;
        skos:inScheme    vlcs:chemische_stof ;
        skos:notation    "CHEMONTID:0000036" ;
        skos:prefLabel   "Nitrobenzenes"@en .

csc:CHEMONTID_0002414
        a                skos:Concept ;
        skos:altLabel    "aromatic carboxylic acid"@en , "pyridines"@en ;
        skos:broader     csc:CHEMONTID_0001322 ;
        skos:definition  "Compounds containing a pyridine ring bearing a carboxylic acid group."@en ;
        skos:inScheme    vlcs:chemische_stof ;
        skos:notation    "CHEMONTID:0002414" ;
        skos:prefLabel   "Pyridinecarboxylic acids"@en .

csc:CHEMONTID_0002460
        a                skos:Concept ;
        skos:altLabel    "amino alcohol"@en ;
        skos:broader     csc:CHEMONTID_0002449 ;
        skos:definition  "Organic compounds that carry a hydroxy and an amino functional groups on an alkane backbone."@en ;
        skos:inScheme    vlcs:chemische_stof ;
        skos:notation    "CHEMONTID:0002460" ;
        skos:prefLabel   "Alkanolamines"@en .

csc:CHEMONTID_0002635
        a                skos:Concept ;
        skos:altLabel    "thiazoles"@en ;
        skos:broader     csc:CHEMONTID_0000095 ;
        skos:definition  "Compounds containing a thiazole ring substituted at positions 2 and 5 only."@en ;
        skos:inScheme    vlcs:chemische_stof ;
        skos:notation    "CHEMONTID:0002635" ;
        skos:prefLabel   "2,5-disubstituted thiazoles"@en .

csc:CHEMONTID_0000004
        a                skos:Concept ;
        rdfs:seeAlso     tax_nodes:C0000004 ;
        skos:altLabel    "organosulfur compound"@en ;
        skos:broader     csc:CHEMONTID_0000000 ;
        skos:definition  "Organic compounds containing a carbon-sulfur bond."@en ;
        skos:inScheme    vlcs:chemische_stof ;
        skos:notation    "CHEMONTID:0000004" ;
        skos:prefLabel   "Organosulfur compounds"@en .

csc:CHEMONTID_0000050
        a                skos:Concept ;
        rdfs:seeAlso     tax_nodes:C0000050 ;
        skos:altLabel    "lactones"@en , "lactone"@en , "a lactone"@en , "Lactones"@en ;
        skos:broader     csc:CHEMONTID_0000002 ;
        skos:definition  "Cyclic esters of hydroxy carboxylic acids, containing a 1-oxacycloalkan-2-one structure, or analogues having unsaturation or heteroatoms replacing one or more carbon atoms of the ring."@en ;
        skos:inScheme    vlcs:chemische_stof ;
        skos:notation    "CHEMONTID:0000050" ;
        skos:prefLabel   "Lactones"@en .

csc:CHEMONTID_0002183
        a                skos:Concept ;
        skos:altLabel    "triazoles"@en ;
        skos:broader     csc:CHEMONTID_0000099 ;
        skos:definition  "Organic aromatic compounds containing a phenyl group substituted with a triazole ring."@en ;
        skos:inScheme    vlcs:chemische_stof ;
        skos:notation    "CHEMONTID:0002183" ;
        skos:prefLabel   "Phenyltriazoles"@en .

csc:CHEMONTID_0002105
        a                skos:Concept ;
        skos:altLabel    "glycoside"@en ;
        skos:broader     csc:CHEMONTID_0000011 ;
        skos:definition  "Carbohydrate derivatives in which a sugar group is bonded through its anomeric carbon to another group via a C-, S-,N-,O-, or Se- glycosidic bond."@en ;
        skos:inScheme    vlcs:chemische_stof ;
        skos:notation    "CHEMONTID:0002105" ;
        skos:prefLabel   "Glycosyl compounds"@en .

csc:CHEMONTID_0000446
        a                skos:Concept ;
        rdfs:seeAlso     tax_nodes:C0000446 ;
        skos:altLabel    "oxoanion"@en ;
        skos:broader     csc:CHEMONTID_0000424 ;
        skos:definition  "Inorganic oxoanionic compounds in which the heaviest atom not in an oxoanion is an alkaline earth metal."@en ;
        skos:inScheme    vlcs:chemische_stof ;
        skos:notation    "CHEMONTID:0000446" ;
        skos:prefLabel   "Alkaline earth metal oxoanionic compounds"@en .

csc:CHEMONTID_0004238
        a                skos:Concept ;
        skos:broader     csc:CHEMONTID_0000405 ;
        skos:definition  "Organoarsenic compounds, where the arsenic atom is tetrasubstituted by organic groups. They have the general structure R4[As+]X-, X=any atom but H."@en ;
        skos:inScheme    vlcs:chemische_stof ;
        skos:notation    "CHEMONTID:0004238" ;
        skos:prefLabel   "Tetraorganoarsonium salts"@en .

csc:CHEMONTID_0003522
        a                skos:Concept ;
        skos:altLabel    "1-benzopyran"@en ;
        skos:broader     csc:CHEMONTID_0003410 ;
        skos:definition  "Organic compounds containing a 1-benzopyran moiety that carries two methyl groups at the 2-position."@en ;
        skos:inScheme    vlcs:chemische_stof ;
        skos:notation    "CHEMONTID:0003522" ;
        skos:prefLabel   "2,2-dimethyl-1-benzopyrans"@en .

csc:CHEMONTID_0002547
        a                skos:Concept ;
        skos:altLabel    "imidazolidines"@en ;
        skos:broader     csc:CHEMONTID_0000250 ;
        skos:definition  "Polycyclic compounds containing an imidazoline substituted by a phenyl group."@en ;
        skos:inScheme    vlcs:chemische_stof ;
        skos:notation    "CHEMONTID:0002547" ;
        skos:prefLabel   "Phenylimidazolidines"@en .

csc:CHEMONTID_0000460
        a                skos:Concept ;
        rdfs:seeAlso     tax_nodes:C0000460 ;
        skos:altLabel    "Metalloids"@en , "Inorganic Chemicals"@en ;
        skos:broader     csc:CHEMONTID_0000424 ;
        skos:definition  "Inorganic compounds belonging to either of the metalloid hydrides, metalloid nitrides, metalloid oxides, metalloid sulfides."@en ;
        skos:inScheme    vlcs:chemische_stof ;
        skos:notation    "CHEMONTID:0000460" ;
        skos:prefLabel   "Metalloid organides"@en .

csc:CHEMONTID_0002049
        a                skos:Concept ;
        rdfs:seeAlso     tax_nodes:C0002049 ;
        skos:altLabel    "terpene glycoside"@en ;
        skos:broader     csc:CHEMONTID_0000259 ;
        skos:definition  "Prenol lipids containing a carbohydrate moiety glycosidically bound to a terpene backbone."@en ;
        skos:inScheme    vlcs:chemische_stof ;
        skos:notation    "CHEMONTID:0002049" ;
        skos:prefLabel   "Terpene glycosides"@en .

csc:CHEMONTID_0002340
        a                skos:Concept ;
        rdfs:seeAlso     tax_nodes:C0002340 ;
        skos:altLabel    "aza-steroid"@en ;
        skos:broader     csc:CHEMONTID_0000258 ;
        skos:definition  "Steroid derivatives in which one carbon atom in the steroidal skeleton has been substituted with a nitrogen atom."@en ;
        skos:inScheme    vlcs:chemische_stof ;
        skos:notation    "CHEMONTID:0002340" ;
        skos:prefLabel   "Azasteroids and derivatives"@en .

csc:CHEMONTID_0002768
        a                skos:Concept ;
        skos:altLabel    "bromophenol"@en ;
        skos:broader     csc:CHEMONTID_0002764 ;
        skos:definition  "Bromophenols carrying a iodine at the C2 position of the benzene ring."@en ;
        skos:inScheme    vlcs:chemische_stof ;
        skos:notation    "CHEMONTID:0002768" ;
        skos:prefLabel   "O-bromophenols"@en .

csc:CHEMONTID_0000137
        a                skos:Concept ;
        skos:altLabel    "a resorcinol"@en , "resorcinols"@en , "Resorcinols"@en ;
        skos:broader     csc:CHEMONTID_0001286 ;
        skos:definition  "Compounds containing a resorcinol moiety, which is a benzene ring bearing two hydroxyl groups at positions 1 and 3."@en ;
        skos:inScheme    vlcs:chemische_stof ;
        skos:notation    "CHEMONTID:0000137" ;
        skos:prefLabel   "Resorcinols"@en .

csc:CHEMONTID_0001831
        a                skos:Concept ;
        rdfs:seeAlso     tax_nodes:C0001831 ;
        skos:altLabel    "carbonyl"@en , "carbonyl compound"@en ;
        skos:broader     csc:CHEMONTID_0000323 ;
        skos:definition  "Organic compounds containing a carbonyl group, with the general structure RC(=O)R', where R=organyl, R'=H, N, O, organyl group or halide group."@en ;
        skos:inScheme    vlcs:chemische_stof ;
        skos:notation    "CHEMONTID:0001831" ;
        skos:prefLabel   "Carbonyl compounds"@en .

csc:CHEMONTID_0004220
        a                skos:Concept ;
        skos:broader     csc:CHEMONTID_0004219 ;
        skos:definition  "Aromatic compounds containing a toluene, which carries a carboxamide group a the 3-position."@en ;
        skos:inScheme    vlcs:chemische_stof ;
        skos:notation    "CHEMONTID:0004220" ;
        skos:prefLabel   "m-Toluamides"@en .

csc:CHEMONTID_0002017
        a                skos:Concept ;
        rdfs:seeAlso     tax_nodes:C0002017 ;
        skos:broader     csc:CHEMONTID_0000097 ;
        skos:definition  "Compounds containing a thiophene ring which bears a carboxylic acid group (or a salt/ester thereof)."@en ;
        skos:inScheme    vlcs:chemische_stof ;
        skos:notation    "CHEMONTID:0002017" ;
        skos:prefLabel   "Thiophene carboxylic acids and derivatives"@en .

csc:CHEMONTID_0003964
        a                skos:Concept ;
        skos:altLabel    "aminotoluene"@en ;
        skos:broader     csc:CHEMONTID_0001091 ;
        skos:definition  "Organic aromatic compounds containing a benzene that carries a single methyl group and one amino group."@en ;
        skos:inScheme    vlcs:chemische_stof ;
        skos:notation    "CHEMONTID:0003964" ;
        skos:prefLabel   "Aminotoluenes"@en .

csc:CHEMONTID_0004441
        a                skos:Concept ;
        rdfs:seeAlso     tax_nodes:C0004441 ;
        skos:altLabel    "Allyl-metals"@en ;
        skos:broader     csc:CHEMONTID_0000462 ;
        skos:definition  "Organometallic compounds containing an allylic group attached to the metal atom."@en ;
        skos:inScheme    vlcs:chemische_stof ;
        skos:notation    "CHEMONTID:0004441" ;
        skos:prefLabel   "Metal allyls"@en .

csc:CHEMONTID_0003213
        a                skos:Concept ;
        skos:altLabel    "an aromatic aldehyde"@en , "an aryl-aldehyde"@en , "arenecarbaldehyde"@en , "Aromatic aldehydes"@en ;
        skos:broader     csc:CHEMONTID_0000124 ;
        skos:definition  "Compounds containing an aldehyde group directly attached to an aromatic ring."@en ;
        skos:inScheme    vlcs:chemische_stof ;
        skos:notation    "CHEMONTID:0003213" ;
        skos:prefLabel   "Aryl-aldehydes"@en .

csc:CHEMONTID_0004616
        a                skos:Concept ;
        skos:altLabel    "aryl phosphate"@en ;
        skos:broader     csc:CHEMONTID_0000408 ;
        skos:definition  "Organophosphorus compounds having a phosphate group substituted by one or more aryl groups."@en ;
        skos:inScheme    vlcs:chemische_stof ;
        skos:notation    "CHEMONTID:0004616" ;
        skos:prefLabel   "Aryl phosphates"@en .

csc:CHEMONTID_0000151
        a                skos:Concept ;
        rdfs:seeAlso     tax_nodes:C0000151 ;
        skos:altLabel    "Anthraquinones"@en ;
        skos:broader     csc:CHEMONTID_0000018 ;
        skos:definition  "Organic compounds containing either anthracene-9,10-quinone, 1,4-anthraquinone, or 1,2-anthraquinone."@en ;
        skos:inScheme    vlcs:chemische_stof ;
        skos:notation    "CHEMONTID:0000151" ;
        skos:prefLabel   "Anthraquinones"@en .

csc:CHEMONTID_0004196
        a                skos:Concept ;
        skos:broader     csc:CHEMONTID_0002497 ;
        skos:definition  "Compounds containing an indole moiety that carries an alkyl chain at the 3-position."@en ;
        skos:inScheme    vlcs:chemische_stof ;
        skos:notation    "CHEMONTID:0004196" ;
        skos:prefLabel   "3-alkylindoles"@en .

csc:CHEMONTID_0000326
        a                skos:Concept ;
        rdfs:seeAlso     tax_nodes:C0000326 ;
        skos:altLabel    "bipyridines"@en ;
        skos:broader     csc:CHEMONTID_0000089 ;
        skos:definition  "Organic compounds containing two pyridine rings linked to each other."@en ;
        skos:inScheme    vlcs:chemische_stof ;
        skos:notation    "CHEMONTID:0000326" ;
        skos:prefLabel   "Bipyridines and oligopyridines"@en .

csc:CHEMONTID_0001729
        a                skos:Concept ;
        rdfs:seeAlso     tax_nodes:C0001729 ;
        skos:altLabel    "an oxepane"@en , "oxacycle"@en ;
        skos:broader     csc:CHEMONTID_0000002 ;
        skos:definition  "Compounds containing an oxepane ring, which is a seven-member saturated aliphatic heterocycle with one oxygen and six carbon atoms."@en ;
        skos:inScheme    vlcs:chemische_stof ;
        skos:notation    "CHEMONTID:0001729" ;
        skos:prefLabel   "Oxepanes"@en .

csc:CHEMONTID_0002031
        a                skos:Concept ;
        rdfs:seeAlso     tax_nodes:C0002031 ;
        skos:altLabel    "Stigmastane steroids"@en , "Stigmasterols and C24-ethyl derivatives"@en , "steroid"@en ;
        skos:broader     csc:CHEMONTID_0000258 ;
        skos:definition  "Sterol lipids with a structure based on the stigmastane skeleton, which consists of a cholestane moiety bearing an ethyl group at the carbon atom C24."@en ;
        skos:inScheme    vlcs:chemische_stof ;
        skos:notation    "CHEMONTID:0002031" ;
        skos:prefLabel   "Stigmastanes and derivatives"@en .

csc:CHEMONTID_0000372
        a                skos:Concept ;
        rdfs:seeAlso     tax_nodes:C0000372 ;
        skos:altLabel    "piperidines"@en ;
        skos:broader     csc:CHEMONTID_0000195 ;
        skos:definition  "Compounds containing the fentanyl moiety or a derivative, which is based on a N-(1-(2-phenylethyl)-4-piperidinyl)-N-phenylpropanamide skeleton."@en ;
        skos:inScheme    vlcs:chemische_stof ;
        skos:notation    "CHEMONTID:0000372" ;
        skos:prefLabel   "Fentanyls"@en .

csc:CHEMONTID_0004164
        a                skos:Concept ;
        rdfs:seeAlso     tax_nodes:C0004164 ;
        skos:altLabel    "organic thiophosphate"@en , "a dithiophosphate O-ester"@en ;
        skos:broader     csc:CHEMONTID_0003385 ;
        skos:definition  "O-ester derivatives of dithiophosphates, with the general structure RSP(O)(O)=S (R = organyl group)."@en ;
        skos:inScheme    vlcs:chemische_stof ;
        skos:notation    "CHEMONTID:0004164" ;
        skos:prefLabel   "Dithiophosphate O-esters"@en .

csc:CHEMONTID_0003480
        a                skos:Concept ;
        rdfs:seeAlso     tax_nodes:C0003480 ;
        skos:altLabel    "cinnamate ester"@en , "a cinnamic acid ester"@en ;
        skos:broader     csc:CHEMONTID_0000476 ;
        skos:definition  "Compound containing an ester derivative of cinnamic acid."@en ;
        skos:inScheme    vlcs:chemische_stof ;
        skos:notation    "CHEMONTID:0003480" ;
        skos:prefLabel   "Cinnamic acid esters"@en .

csc:CHEMONTID_0000049
        a                skos:Concept ;
        rdfs:seeAlso     tax_nodes:C0000049 ;
        skos:broader     csc:CHEMONTID_0000048 ;
        skos:definition  "Compounds containing a tametraline moiety, which consists of a tetrahydronaphthalene linked to a phenyl group to form N-methyl-4-phenyl-1,2,3,4-tetrahydronaphthalen-1-amine skeleton."@en ;
        skos:inScheme    vlcs:chemische_stof ;
        skos:notation    "CHEMONTID:0000049" ;
        skos:prefLabel   "Tametralines"@en .

csc:CHEMONTID_0000095
        a                skos:Concept ;
        rdfs:seeAlso     tax_nodes:C0000095 ;
        skos:altLabel    "Thiazoles"@en ;
        skos:broader     csc:CHEMONTID_0000436 ;
        skos:definition  "Heterocyclic compounds containing a five-member aromatic ring made up of one sulfur atom, one nitrogen, and three carbon atoms."@en ;
        skos:inScheme    vlcs:chemische_stof ;
        skos:notation    "CHEMONTID:0000095" ;
        skos:prefLabel   "Thiazoles"@en .

csc:CHEMONTID_0001498
        a                skos:Concept ;
        skos:altLabel    "hexose"@en ;
        skos:broader     csc:CHEMONTID_0001540 ;
        skos:definition  "Monosaccharides in which the sugar unit is a is a six-carbon containing moeity."@en ;
        skos:inScheme    vlcs:chemische_stof ;
        skos:notation    "CHEMONTID:0001498" ;
        skos:prefLabel   "Hexoses"@en .

csc:CHEMONTID_0001245
        a                skos:Concept ;
        rdfs:seeAlso     tax_nodes:C0001245 ;
        skos:altLabel    "gamma-lactone"@en ;
        skos:broader     csc:CHEMONTID_0000050 ;
        skos:definition  "Compounds containing a gamma butyrolactone moiety, which consists of an aliphatic five-member ring with four carbon atoms, one oxygen atom, and bears a ketone group on the carbon adjacent to the oxygen atom."@en ;
        skos:inScheme    vlcs:chemische_stof ;
        skos:notation    "CHEMONTID:0001245" ;
        skos:prefLabel   "Gamma butyrolactones"@en .

csc:CHEMONTID_0002648
        a                skos:Concept ;
        rdfs:seeAlso     tax_nodes:C0002648 ;
        skos:altLabel    "oxolanes"@en ;
        skos:broader     csc:CHEMONTID_0000002 ;
        skos:definition  "Heterocyclic compounds containing a saturated, aliphatic, five-membered ring where a carbon is replaced by an oxygen."@en ;
        skos:inScheme    vlcs:chemische_stof ;
        skos:notation    "CHEMONTID:0002648" ;
        skos:prefLabel   "Tetrahydrofurans"@en .

csc:CHEMONTID_0000017
        a                skos:Concept ;
        skos:altLabel    "cyclic olefin"@en ;
        skos:broader     csc:CHEMONTID_0002840 ;
        skos:definition  "Unsaturated monocyclic hydrocarbons having one endocyclic double bond."@en ;
        skos:inScheme    vlcs:chemische_stof ;
        skos:notation    "CHEMONTID:0000017" ;
        skos:prefLabel   "Cycloalkenes"@en .

csc:CHEMONTID_0002441
        a                skos:Concept ;
        rdfs:seeAlso     tax_nodes:C0002441 ;
        skos:altLabel    "naphthols"@en , "Naphthols"@en ;
        skos:broader     csc:CHEMONTID_0000023 ;
        skos:definition  "Naphthalene derivatives carrying one or more hydroxyl (-OH) groups at any ring position."@en ;
        skos:inScheme    vlcs:chemische_stof ;
        skos:notation    "CHEMONTID:0002441" ;
        skos:prefLabel   "Naphthols and derivatives"@en .

csc:CHEMONTID_0001466
        a                skos:Concept ;
        rdfs:seeAlso     tax_nodes:C0001466 ;
        skos:altLabel    "steroid"@en , "C18 steroids (estrogens) and derivatives"@en ;
        skos:broader     csc:CHEMONTID_0000258 ;
        skos:definition  "Steroids with a structure based on the estrane skeleton."@en ;
        skos:inScheme    vlcs:chemische_stof ;
        skos:notation    "CHEMONTID:0001466" ;
        skos:prefLabel   "Estrane steroids"@en .

csc:CHEMONTID_0000238
        a                skos:Concept ;
        rdfs:seeAlso     tax_nodes:C0000238 ;
        skos:altLabel    "tannin"@en ;
        skos:broader     csc:CHEMONTID_0000261 ;
        skos:definition  "Naturally occurring polyphenols which be categorized into four main classes: hydrolyzable tannin (based on ellagic acid or gallic acid), condensed tannins (made of oligomeric or polymeric proanthocyanidins), complex tannins (made of a catechin bound to a gallotannin or elagitannin), and phlorotannins (oligomers of phloroglucinol)."@en ;
        skos:inScheme    vlcs:chemische_stof ;
        skos:notation    "CHEMONTID:0000238" ;
        skos:prefLabel   "Tannins"@en .

csc:CHEMONTID_0004749
        a                skos:Concept ;
        skos:broader     csc:CHEMONTID_0001820 ;
        skos:definition  "Aromatic heterocyclic compounds containing a 1,3-dioxoisoindoline moiety. They are imide derivatives of phthalic anhydrides."@en ;
        skos:inScheme    vlcs:chemische_stof ;
        skos:notation    "CHEMONTID:0004749" ;
        skos:prefLabel   "Phthalimides"@en .

csc:CHEMONTID_0004321
        a                skos:Concept ;
        skos:broader     csc:CHEMONTID_0000060 ;
        skos:definition  "Compounds containing phenylalanine or a derivative thereof resulting from reaction of phenylalanine at the amino group or the carboxy group, or from the replacement of any hydrogen of glycine by a heteroatom."@en ;
        skos:inScheme    vlcs:chemische_stof ;
        skos:notation    "CHEMONTID:0004321" ;
        skos:prefLabel   "Phenylalanine and derivatives"@en .

csc:CHEMONTID_0000284
        a                skos:Concept ;
        rdfs:seeAlso     tax_nodes:C0000284 ;
        skos:altLabel    "Substituted anilines"@en ;
        skos:broader     csc:CHEMONTID_0002279 ;
        skos:definition  "Organic compounds containing an aminobenzene moiety."@en ;
        skos:inScheme    vlcs:chemische_stof ;
        skos:notation    "CHEMONTID:0000284" ;
        skos:prefLabel   "Aniline and substituted anilines"@en .

csc:CHEMONTID_0002118
        a                skos:Concept ;
        rdfs:seeAlso     tax_nodes:C0002118 ;
        skos:altLabel    "oxazolopyridine"@en ;
        skos:broader     csc:CHEMONTID_0000002 ;
        skos:definition  "Polycyclic compounds containing an oxazole ring fused to a pyridine ring."@en ;
        skos:inScheme    vlcs:chemische_stof ;
        skos:notation    "CHEMONTID:0002118" ;
        skos:prefLabel   "Oxazolopyridines"@en .

csc:CHEMONTID_0000031
        a                skos:Concept ;
        rdfs:seeAlso     tax_nodes:C0000031 ;
        skos:broader     csc:CHEMONTID_0002279 ;
        skos:definition  "Organic compounds containing a sulfonamide group that is S-linked to a benzene ring."@en ;
        skos:inScheme    vlcs:chemische_stof ;
        skos:notation    "CHEMONTID:0000031" ;
        skos:prefLabel   "Benzenesulfonamides"@en .

csc:CHEMONTID_0000459
        a                skos:Concept ;
        rdfs:seeAlso     tax_nodes:C0000459 ;
        skos:broader     csc:CHEMONTID_0000424 ;
        skos:definition  "Inorganic compounds belonging to either the lanthanide hydrides, lanthanide nitrides, lanthanide oxides, lanthanide sulfides."@en ;
        skos:inScheme    vlcs:chemische_stof ;
        skos:notation    "CHEMONTID:0000459" ;
        skos:prefLabel   "Lanthanide organides"@en .

csc:CHEMONTID_0002837
        a                skos:Concept ;
        rdfs:seeAlso     tax_nodes:C0002837 ;
        skos:altLabel    "hydrocarbon"@en ;
        skos:broader     csc:CHEMONTID_0000000 ;
        skos:definition  "Organic compounds made up only of carbon and hydrogen atoms."@en ;
        skos:inScheme    vlcs:chemische_stof ;
        skos:notation    "CHEMONTID:0002837" ;
        skos:prefLabel   "Hydrocarbons"@en .

csc:CHEMONTID_0000206
        a                skos:Concept ;
        skos:altLabel    "1,2-diazanaphthalenes"@en , "cinnolines"@en ;
        skos:broader     csc:CHEMONTID_0004789 ;
        skos:definition  "Organic aromatic compounds containing a benzene fused to a pyridazine ring."@en ;
        skos:inScheme    vlcs:chemische_stof ;
        skos:notation    "CHEMONTID:0000206" ;
        skos:prefLabel   "Cinnolines"@en .

csc:CHEMONTID_0001189
        a                skos:Concept ;
        skos:altLabel    "N-acyl-amino acid"@en ;
        skos:broader     csc:CHEMONTID_0000060 ;
        skos:definition  "Compounds containing an alpha amino acid (or a derivative thereof) which bears an acyl group at its terminal nitrogen atom."@en ;
        skos:inScheme    vlcs:chemische_stof ;
        skos:notation    "CHEMONTID:0001189" ;
        skos:prefLabel   "N-acyl-alpha amino acids and derivatives"@en .

csc:CHEMONTID_0003567
        a                skos:Concept ;
        rdfs:seeAlso     tax_nodes:C0003567 ;
        skos:altLabel    "24-methylcholestane steroids"@en , "<new synonym>"@en , "Ergosterols and C24-methyl derivatives"@en , "ergostanoid"@en ;
        skos:broader     csc:CHEMONTID_0000258 ;
        skos:definition  "Steroids with a structure based on the ergostane skeleton, which arises from the methylation of cholestane at the 24-position."@en ;
        skos:inScheme    vlcs:chemische_stof ;
        skos:notation    "CHEMONTID:0003567" ;
        skos:prefLabel   "Ergostane steroids"@en .

csc:CHEMONTID_0003314
        a                skos:Concept ;
        skos:altLabel    "a phenyl-1,2,4-triazole"@en , "triazoles"@en ;
        skos:broader     csc:CHEMONTID_0002183 ;
        skos:definition  "Organic compounds containing a 1,2,4-triazole substituted by a phenyl group."@en ;
        skos:inScheme    vlcs:chemische_stof ;
        skos:notation    "CHEMONTID:0003314" ;
        skos:prefLabel   "Phenyl-1,2,4-triazoles"@en .

csc:CHEMONTID_0004297
        a                skos:Concept ;
        skos:broader     csc:CHEMONTID_0004296 ;
        skos:definition  "Aromatic compounds containing a ketone substituted by one aryl group, and a phenyl group."@en ;
        skos:inScheme    vlcs:chemische_stof ;
        skos:notation    "CHEMONTID:0004297" ;
        skos:prefLabel   "Aryl-phenylketones"@en .

csc:CHEMONTID_0000427
        a                skos:Concept ;
        rdfs:seeAlso     tax_nodes:C0000427 ;
        skos:broader     csc:CHEMONTID_0000422 ;
        skos:definition  "Inorganic compounds containing only metal atoms,with the largest atom being a post-transition metal atom."@en ;
        skos:inScheme    vlcs:chemische_stof ;
        skos:notation    "CHEMONTID:0000427" ;
        skos:prefLabel   "Homogeneous post-transition metal compounds"@en .

csc:CHEMONTID_0001157
        a                skos:Concept ;
        rdfs:seeAlso     tax_nodes:C0001157 ;
        skos:altLabel    "sulfone"@en ;
        skos:broader     csc:CHEMONTID_0000004 ;
        skos:definition  "Compounds containing the sulfonyl group, with the general structure RS(=O)2R' ( R,R' must not be H)."@en ;
        skos:inScheme    vlcs:chemische_stof ;
        skos:notation    "CHEMONTID:0001157" ;
        skos:prefLabel   "Sulfonyls"@en .

csc:CHEMONTID_0004219
        a                skos:Concept ;
        skos:broader     csc:CHEMONTID_0001091 ;
        skos:definition  "Aromatic compounds containing a toluene, which carries a carboxamide group."@en ;
        skos:inScheme    vlcs:chemische_stof ;
        skos:notation    "CHEMONTID:0004219" ;
        skos:prefLabel   "Toluamides"@en .

csc:CHEMONTID_0002132
        a                skos:Concept ;
        rdfs:seeAlso     tax_nodes:C0002132 ;
        skos:altLabel    "dithioacetal"@en ;
        skos:broader     csc:CHEMONTID_0001187 ;
        skos:definition  "Compounds containing a dithioacetal functional group with the general structure R2C(SR')2."@en ;
        skos:inScheme    vlcs:chemische_stof ;
        skos:notation    "CHEMONTID:0002132" ;
        skos:prefLabel   "Dithioacetals"@en .

csc:CHEMONTID_0004012
        a                skos:Concept ;
        skos:broader     csc:CHEMONTID_0004009 ;
        skos:definition  "Ester derivatives of p-phthalic acids, which are based on a benzene 1,4-dicarboxylic acid skeleton."@en ;
        skos:inScheme    vlcs:chemische_stof ;
        skos:notation    "CHEMONTID:0004012" ;
        skos:prefLabel   "p-Phthalate esters"@en .

csc:CHEMONTID_0001378
        a                skos:Concept ;
        skos:altLabel    "dibenzofurans"@en , "organochlorine compound"@en ;
        skos:broader     csc:CHEMONTID_0000015 ;
        skos:definition  "Organic compounds containing a chlorine atom attached to a dibenzofuran moiety."@en ;
        skos:inScheme    vlcs:chemische_stof ;
        skos:notation    "CHEMONTID:0001378" ;
        skos:prefLabel   "Chlorinated dibenzofurans"@en .

csc:CHEMONTID_0004731
        a                skos:Concept ;
        skos:altLabel    "Methoxytriazines"@en , "methoxy-1,3,5-triazine"@en ;
        skos:broader     csc:CHEMONTID_0004638 ;
        skos:definition  "Aromatic heterocyclic compounds containing a 1,3,5-triazine ring, which is substituted at the 2-position with a methoxy group."@en ;
        skos:inScheme    vlcs:chemische_stof ;
        skos:notation    "CHEMONTID:0004731" ;
        skos:prefLabel   "2-methoxy-1,3,5-triazines"@en .

csc:CHEMONTID_0002100
        a                skos:Concept ;
        rdfs:seeAlso     tax_nodes:C0002100 ;
        skos:altLabel    "benzodioxine"@en ;
        skos:broader     csc:CHEMONTID_0000002 ;
        skos:definition  "Organic compounds containing a benzene ring fused to a dioxin ring. Dioxin a six-membered unsaturated ring of two oxygen atoms and four carbon atoms."@en ;
        skos:inScheme    vlcs:chemische_stof ;
        skos:notation    "CHEMONTID:0002100" ;
        skos:prefLabel   "Benzodioxins"@en .

csc:CHEMONTID_0002528
        a                skos:Concept ;
        rdfs:seeAlso     tax_nodes:C0002528 ;
        skos:altLabel    "alcohol"@en , "organohalogen compound"@en , "Haloalcohols"@en ;
        skos:broader     csc:CHEMONTID_0000267 ;
        skos:definition  "Alcohols substituted by a halogen atom at a saturated carbon atom otherwise bearing only hydrogen or hydrocarbyl groups (usually used to mean beta-halo alcohols)."@en ;
        skos:inScheme    vlcs:chemische_stof ;
        skos:notation    "CHEMONTID:0002528" ;
        skos:prefLabel   "Halohydrins"@en .

csc:CHEMONTID_0004233
        a                skos:Concept ;
        rdfs:seeAlso     tax_nodes:C0004233 ;
        skos:altLabel    "benzenes"@en ;
        skos:broader     csc:CHEMONTID_0002279 ;
        skos:definition  "Aromatic compounds containing a benzenesulfonyl group, which consists of a monocyclic benzene moiety that carries a sulfonyl group."@en ;
        skos:inScheme    vlcs:chemische_stof ;
        skos:notation    "CHEMONTID:0004233" ;
        skos:prefLabel   "Benzenesulfonyl compounds"@en .

csc:CHEMONTID_0001346
        a                skos:Concept ;
        rdfs:seeAlso     tax_nodes:C0001346 ;
        skos:altLabel    "diazines"@en ;
        skos:broader     csc:CHEMONTID_0000002 ;
        skos:definition  "Organic compounds containing a five-member heterocyclic compound with five nitrogen atoms, and two nitrogen atoms at positions 1 and 2 (Pyridazines), 1 and 3 (Pyrimidines), or 1 and 4 (Pyrazines)."@en ;
        skos:inScheme    vlcs:chemische_stof ;
        skos:notation    "CHEMONTID:0001346" ;
        skos:prefLabel   "Diazines"@en .

csc:CHEMONTID_0002749
        a                skos:Concept ;
        rdfs:seeAlso     tax_nodes:C0002749 ;
        skos:altLabel    "S-type indole alkaloids"@en ;
        skos:broader     csc:CHEMONTID_0000279 ;
        skos:definition  "Alkaloids having a core structure based on the strychnan, stemmadenine (seco-curan), or the akuammicine (curan) skeleton."@en ;
        skos:inScheme    vlcs:chemische_stof ;
        skos:notation    "CHEMONTID:0002749" ;
        skos:prefLabel   "Strychnos alkaloids"@en .

csc:CHEMONTID_0000118
        a                skos:Concept ;
        skos:altLabel    "ketone"@en , "ketones"@en , "Ketones"@en ;
        skos:broader     csc:CHEMONTID_0001831 ;
        skos:definition  "Organic compounds  in which a carbonyl group is bonded to two carbon atoms R2C=O (neither R may be a hydrogen atom). Ketones that have one or more alpha-hydrogen atoms undergo keto-enol tautomerization, the tautomer being an enol."@en ;
        skos:inScheme    vlcs:chemische_stof ;
        skos:notation    "CHEMONTID:0000118" ;
        skos:prefLabel   "Ketones"@en .

csc:CHEMONTID_0001392
        a                skos:Concept ;
        rdfs:seeAlso     tax_nodes:C0001392 ;
        skos:altLabel    "phenylpropanoid"@en ;
        skos:broader     csc:CHEMONTID_0000000 ;
        skos:definition  "Plant products of low molecular weight formed primarily from oxidative coupling of two p-propylphenol moieties. They can also be described as micromolecules with two phenylpropanoid units coupled together. They can be attached in various manners, like C5-C5', C8-C8'. Most known natural lignans are oxidized at C9 and C9´ and, based upon the way in which oxygen is incorporated into the skeleton and on the cyclization patterns, a wide range of lignans of very different structural types can be formed."@en ;
        skos:inScheme    vlcs:chemische_stof ;
        skos:notation    "CHEMONTID:0001392" ;
        skos:prefLabel   "Lignans, neolignans and related compounds"@en .

csc:CHEMONTID_0004201
        a                skos:Concept ;
        rdfs:seeAlso     tax_nodes:C0004201 ;
        skos:altLabel    "Thiazolobenzotriazoles"@en , "triazolobenzothiazole"@en , "a triazolobenzothiazole"@en ;
        skos:broader     csc:CHEMONTID_0000315 ;
        skos:definition  "Compound containing a triazole ring fused to the benzene or the thiazole moiety of the benzothiazole ring system."@en ;
        skos:inScheme    vlcs:chemische_stof ;
        skos:notation    "CHEMONTID:0004201" ;
        skos:prefLabel   "Triazolobenzothiazoles"@en .

csc:CHEMONTID_0002542
        a                skos:Concept ;
        rdfs:seeAlso     tax_nodes:C0002542 ;
        skos:altLabel    "benzyl ether"@en ;
        skos:broader     csc:CHEMONTID_0002279 ;
        skos:definition  "Aromatic ethers with the general formula ROCR' (R = alkyl, aryl; R'=benzene)."@en ;
        skos:inScheme    vlcs:chemische_stof ;
        skos:notation    "CHEMONTID:0002542" ;
        skos:prefLabel   "Benzylethers"@en .

csc:CHEMONTID_0001314
        a                skos:Concept ;
        rdfs:seeAlso     tax_nodes:C0001314 ;
        skos:altLabel    "dioxanes"@en , "m-Dioxanes"@en , "Meta-Dioxanes"@en ;
        skos:broader     csc:CHEMONTID_0000368 ;
        skos:definition  "Organic compounds containing 1,3-dioxane, an aliphatic six-member ring with two oxygen atoms in ring positions 1 and 3."@en ;
        skos:inScheme    vlcs:chemische_stof ;
        skos:notation    "CHEMONTID:0001314" ;
        skos:prefLabel   "1,3-dioxanes"@en .

csc:CHEMONTID_0002044
        a                skos:Concept ;
        rdfs:seeAlso     tax_nodes:C0002044 ;
        skos:altLabel    "naphthalenes"@en , "benzenes"@en , "ring assembly"@en ;
        skos:broader     csc:CHEMONTID_0000023 ;
        skos:definition  "Compounds containing a phenylnaphthalene skeleton, which consists of a naphthalene bound to a phenyl group."@en ;
        skos:inScheme    vlcs:chemische_stof ;
        skos:notation    "CHEMONTID:0002044" ;
        skos:prefLabel   "Phenylnaphthalenes"@en .

csc:CHEMONTID_0000132
        a                skos:Concept ;
        rdfs:seeAlso     tax_nodes:C0000132 ;
        skos:altLabel    "enol"@en ;
        skos:broader     csc:CHEMONTID_0000323 ;
        skos:definition  "Compounds containing the enol functional group, with the structure HO(R)C=CR'. Ketones that have one or more alpha-hydrogen atoms undergo keto-enol tautomerization, the tautomer being an enol."@en ;
        skos:inScheme    vlcs:chemische_stof ;
        skos:notation    "CHEMONTID:0000132" ;
        skos:prefLabel   "Enols"@en .

csc:CHEMONTID_0000307
        a                skos:Concept ;
        rdfs:seeAlso     tax_nodes:C0000307 ;
        skos:altLabel    "azepanes"@en ;
        skos:broader     csc:CHEMONTID_0000002 ;
        skos:definition  "Organic compounds containing a saturated seven member heterocycle, with one nitrogen atom."@en ;
        skos:inScheme    vlcs:chemische_stof ;
        skos:notation    "CHEMONTID:0000307" ;
        skos:prefLabel   "Azepanes"@en .

csc:CHEMONTID_0002012
        a                skos:Concept ;
        rdfs:seeAlso     tax_nodes:C0002012 ;
        skos:altLabel    "oxanes"@en , "Tetrahydropyranes"@en , "Tetrahydropyrans"@en ;
        skos:broader     csc:CHEMONTID_0000002 ;
        skos:definition  "Compounds containing an oxane (tetrahydropyran) ring, which is a six-member saturated aliphatic heterocycle with one oxygen atom and five carbon atoms."@en ;
        skos:inScheme    vlcs:chemische_stof ;
        skos:notation    "CHEMONTID:0002012" ;
        skos:prefLabel   "Oxanes"@en .

csc:CHEMONTID_0001581
        a                skos:Concept ;
        rdfs:seeAlso     tax_nodes:C0001581 ;
        skos:altLabel    "a piperidinone"@en , "piperidones"@en ;
        skos:broader     csc:CHEMONTID_0000195 ;
        skos:definition  "Compounds containing a piperidine ring which bears a ketone."@en ;
        skos:inScheme    vlcs:chemische_stof ;
        skos:notation    "CHEMONTID:0001581" ;
        skos:prefLabel   "Piperidinones"@en .

csc:CHEMONTID_0000321
        a                skos:Concept ;
        rdfs:seeAlso     tax_nodes:C0000321 ;
        skos:altLabel    "carbonyl compound"@en ;
        skos:broader     csc:CHEMONTID_0002279 ;
        skos:definition  "Organic compounds containing an acyl moiety of benzoic acid with the formula (C6H5CO-)."@en ;
        skos:inScheme    vlcs:chemische_stof ;
        skos:notation    "CHEMONTID:0000321" ;
        skos:prefLabel   "Benzoyl derivatives"@en .

csc:CHEMONTID_0001724
        a                skos:Concept ;
        skos:altLabel    "pyrethrins"@en ;
        skos:broader     csc:CHEMONTID_0001461 ;
        skos:definition  "Pyrethroids with a structure based on a skeleton that is characterized by the presence of a chrysanthemic acid esterified with a cyclopentenone derivative."@en ;
        skos:inScheme    vlcs:chemische_stof ;
        skos:notation    "CHEMONTID:0001724" ;
        skos:prefLabel   "Pyrethrins"@en .

csc:CHEMONTID_0004113
        a                skos:Concept ;
        rdfs:seeAlso     tax_nodes:C0004113 ;
        skos:altLabel    "methoxybenzene"@en ;
        skos:broader     csc:CHEMONTID_0002279 ;
        skos:definition  "Organic aromatic compounds containing a monocyclic benzene moiety carrying exactly or one more methoxy groups."@en ;
        skos:inScheme    vlcs:chemische_stof ;
        skos:notation    "CHEMONTID:0004113" ;
        skos:prefLabel   "Methoxybenzenes"@en .

csc:CHEMONTID_0000076
        a                skos:Concept ;
        rdfs:seeAlso     tax_nodes:C0000076 ;
        skos:altLabel    "Furans"@en , "Oxoles"@en ;
        skos:broader     csc:CHEMONTID_0000002 ;
        skos:definition  "Compounds containing a furan ring, which is a five-member aromatic ring with one oxygen atom, four carbon atoms."@en ;
        skos:inScheme    vlcs:chemische_stof ;
        skos:notation    "CHEMONTID:0000076" ;
        skos:prefLabel   "Furans"@en .

csc:CHEMONTID_0002454
        a                skos:Concept ;
        skos:altLabel    "tertiary amine"@en , "a tertiary alkylarylamine"@en ;
        skos:broader     csc:CHEMONTID_0002452 ;
        skos:definition  "Tertiary amines where the nitrogen atom is linked to at least one alkyl group and at least one aryl group."@en ;
        skos:inScheme    vlcs:chemische_stof ;
        skos:notation    "CHEMONTID:0002454" ;
        skos:prefLabel   "Tertiary alkylarylamines"@en .

csc:CHEMONTID_0000542
        a                skos:Concept ;
        rdfs:seeAlso     tax_nodes:C0000542 ;
        skos:altLabel    "inorganic oxide"@en ;
        skos:broader     csc:CHEMONTID_0000459 ;
        skos:definition  "Inorganic compounds containing an oxygen atom of an oxidation state of -2, in which the heaviest atom bonded to the oxygen is a lanthanide."@en ;
        skos:inScheme    vlcs:chemische_stof ;
        skos:notation    "CHEMONTID:0000542" ;
        skos:prefLabel   "Lanthanide oxides"@en .

csc:CHEMONTID_0001272
        a                skos:Concept ;
        rdfs:seeAlso     tax_nodes:C0001272 ;
        skos:altLabel    "phenols"@en , "methoxybenzene"@en ;
        skos:broader     csc:CHEMONTID_0000134 ;
        skos:definition  "Aromatic compounds containing a methoxyphenol moiety."@en ;
        skos:inScheme    vlcs:chemische_stof ;
        skos:notation    "CHEMONTID:0001272" ;
        skos:prefLabel   "Cresols"@en .

vlcs:chemische_stof
        skos:altLabel    "a chemical entity"@en ;
        skos:definition  "Constitutionally or isotopically distinct atoms, molecules, ions, ion pairs, radicals, radical ions, complexes, conformers etc., identifiable as a separately distinguishable entity."@en ;
        skos:notation    "CHEMONTID:9999999" ;
        skos:prefLabel   "Chemical entities"@en .

csc:CHEMONTID_0004089
        a                skos:Concept ;
        rdfs:seeAlso     tax_nodes:C0004089 ;
        skos:broader     csc:CHEMONTID_0002800 ;
        skos:definition  "Organic compounds containing a disulfide group R-SS-R' where R and R' are both alkyl groups."@en ;
        skos:inScheme    vlcs:chemische_stof ;
        skos:notation    "CHEMONTID:0004089" ;
        skos:prefLabel   "Dialkyldisulfides"@en .

csc:CHEMONTID_0000510
        a                skos:Concept ;
        rdfs:seeAlso     tax_nodes:C0000510 ;
        skos:altLabel    "Thioamides"@en , "Thionamides"@en , "thiocarboxamide"@en ;
        skos:broader     csc:CHEMONTID_0000004 ;
        skos:definition  "Organic compounds containing the functional group with the general structure R-CS-NR'R, where R, R', and R are organic groups."@en ;
        skos:inScheme    vlcs:chemische_stof ;
        skos:notation    "CHEMONTID:0000510" ;
        skos:prefLabel   "Thioamides"@en .

csc:CHEMONTID_0000090
        a                skos:Concept ;
        rdfs:seeAlso     tax_nodes:C0000090 ;
        skos:altLabel    "Pyrroles"@en ;
        skos:broader     csc:CHEMONTID_0000002 ;
        skos:definition  "Compounds containing a pyrrole ring, which is a five-member aromatic heterocycle with one nitrogen atom and four carbon atoms."@en ;
        skos:inScheme    vlcs:chemische_stof ;
        skos:notation    "CHEMONTID:0000090" ;
        skos:prefLabel   "Pyrroles"@en .

csc:CHEMONTID_0000265
        a                skos:Concept ;
        rdfs:seeAlso     tax_nodes:C0000265 ;
        skos:broader     csc:CHEMONTID_0000264 ;
        skos:definition  "Compounds containing a carboxylic acid group with the formula -C(=O)OH or a derivative thereof."@en ;
        skos:inScheme    vlcs:chemische_stof ;
        skos:notation    "CHEMONTID:0000265" ;
        skos:prefLabel   "Carboxylic acids and derivatives"@en .

csc:CHEMONTID_0000012
        a                skos:Concept ;
        rdfs:seeAlso     tax_nodes:C0000012 ;
        skos:altLabel    "lipid"@en , "Lipids"@en , "lipids"@en ;
        skos:broader     csc:CHEMONTID_0000000 ;
        skos:definition  "Fatty acids and their derivatives, and substances related biosynthetically or functionally to these compounds."@en ;
        skos:inScheme    vlcs:chemische_stof ;
        skos:notation    "CHEMONTID:0000012" ;
        skos:prefLabel   "Lipids and lipid-like molecules"@en .

csc:CHEMONTID_0004776
        a                skos:Concept ;
        rdfs:seeAlso     tax_nodes:C0004776 ;
        skos:broader     csc:CHEMONTID_0000278 ;
        skos:definition  "Organic compounds having the nitroso group, -NO, attached to carbon, or to another element, most commonly nitrogen or oxygen."@en ;
        skos:inScheme    vlcs:chemische_stof ;
        skos:notation    "CHEMONTID:0004776" ;
        skos:prefLabel   "Organic nitroso compounds"@en .

csc:CHEMONTID_0000486
        a                skos:Concept ;
        skos:altLabel    "1,4-diazanaphthalenes"@en , "quinoxaline derivative"@en , "Quinoxalines"@en ;
        skos:broader     csc:CHEMONTID_0004789 ;
        skos:definition  "Compounds containing a quinoxaline moiety, a bicyclic heterocycle made up of a benzene ring fused to a pyrazine ring."@en ;
        skos:inScheme    vlcs:chemische_stof ;
        skos:notation    "CHEMONTID:0000486" ;
        skos:prefLabel   "Quinoxalines"@en .

csc:CHEMONTID_0001461
        a                skos:Concept ;
        skos:altLabel    "cyclopropanes"@en , "carboxylic ester"@en ;
        skos:broader     csc:CHEMONTID_0000324 ;
        skos:definition  "Organic compounds similar to the pyrethrins. Some pyrethroids containing a chrysanthemic acid esterified with a cyclopentenone (pyrethrins), or with a phenoxybenzyl group."@en ;
        skos:inScheme    vlcs:chemische_stof ;
        skos:notation    "CHEMONTID:0001461" ;
        skos:prefLabel   "Pyrethroids"@en .

csc:CHEMONTID_0002864
        a                skos:Concept ;
        rdfs:seeAlso     tax_nodes:C0002864 ;
        skos:altLabel    "organobromine compound"@en ;
        skos:broader     csc:CHEMONTID_0002868 ;
        skos:definition  "Vinyl halides in which a bromine atom is bonded to an sp2-hybridised carbon atom."@en ;
        skos:inScheme    vlcs:chemische_stof ;
        skos:notation    "CHEMONTID:0002864" ;
        skos:prefLabel   "Vinyl bromides"@en .

csc:CHEMONTID_0000233
        a                skos:Concept ;
        rdfs:seeAlso     tax_nodes:C0000233 ;
        skos:altLabel    "tetrahydrothiophenes"@en ;
        skos:broader     csc:CHEMONTID_0000002 ;
        skos:definition  "Organic compounds containing thiolane, a five-member saturated ring containing four carbon atoms and a sulfur atom."@en ;
        skos:inScheme    vlcs:chemische_stof ;
        skos:notation    "CHEMONTID:0000233" ;
        skos:prefLabel   "Thiolanes"@en .

csc:CHEMONTID_0002611
        a                skos:Concept ;
        skos:altLabel    "chlorobenzoic acid"@en ;
        skos:broader     csc:CHEMONTID_0002565 ;
        skos:definition  "Benzoic acids having two chlorine atoms attached to the carboxylated benzene ring."@en ;
        skos:inScheme    vlcs:chemische_stof ;
        skos:notation    "CHEMONTID:0002611" ;
        skos:prefLabel   "Dichlorobenzoic acids"@en .

csc:CHEMONTID_0000408
        a                skos:Concept ;
        rdfs:seeAlso     tax_nodes:C0000408 ;
        skos:altLabel    "phosphoric ester"@en ;
        skos:broader     csc:CHEMONTID_0000402 ;
        skos:definition  "Organic compounds containing phosphoric acid ester functional group, with the general structure R1P(=O)(R2)OR3. R1,R2 = O,N,  or halogen atom; R3 = organyl group."@en ;
        skos:inScheme    vlcs:chemische_stof ;
        skos:notation    "CHEMONTID:0000408" ;
        skos:prefLabel   "Phosphate esters"@en .

csc:CHEMONTID_0001857
        a                skos:Concept ;
        rdfs:seeAlso     tax_nodes:C0001857 ;
        skos:altLabel    "naphthyridine derivative"@en , "a naphthyridine"@en ;
        skos:broader     csc:CHEMONTID_0004788 ;
        skos:definition  "Compounds containing a naphthyridine moiety, a naphthalene in which a carbon atom has been replaced by a nitrogen in each of the two rings. The naphthyridine skeleton can also be described as an assembly two fused pyridine rings, which do not share their nitrogen atom."@en ;
        skos:inScheme    vlcs:chemische_stof ;
        skos:notation    "CHEMONTID:0001857" ;
        skos:prefLabel   "Naphthyridines"@en .

csc:CHEMONTID_0000454
        a                skos:Concept ;
        rdfs:seeAlso     tax_nodes:C0000454 ;
        skos:altLabel    "halogen molecular entity"@en ;
        skos:broader     csc:CHEMONTID_0000423 ;
        skos:definition  "Inorganic compounds belonging to either the halogen hydrides, halogen nitrides, halogen oxides, or halogen sulfides."@en ;
        skos:inScheme    vlcs:chemische_stof ;
        skos:notation    "CHEMONTID:0000454" ;
        skos:prefLabel   "Halogen organides"@en .

csc:CHEMONTID_0003096
        a                skos:Concept ;
        skos:altLabel    "carbonyl compound"@en , "organohalogen compound"@en ;
        skos:broader     csc:CHEMONTID_0000176 ;
        skos:definition  "Benzoic acids or derivatives carrying a halogen atom on the benzene ring."@en ;
        skos:inScheme    vlcs:chemische_stof ;
        skos:notation    "CHEMONTID:0003096" ;
        skos:prefLabel   "Halobenzoic acids and derivatives"@en .

csc:CHEMONTID_0000201
        a                skos:Concept ;
        skos:altLabel    "Tocopherols"@en , "Vitamin E"@en , "tocopherol"@en ;
        skos:broader     csc:CHEMONTID_0001546 ;
        skos:definition  "Vitamin E derivatives containing a saturated trimethyltridecyl chain attached to the carbon C6 atom of a benzopyran ring system. The differ from tocotrienols that contain an unsaturated trimethyltrideca-3,7,11-trien-1-yl chain."@en ;
        skos:inScheme    vlcs:chemische_stof ;
        skos:notation    "CHEMONTID:0000201" ;
        skos:prefLabel   "Tocopherols"@en .

csc:CHEMONTID_0001184
        a                skos:Concept ;
        skos:altLabel    "a sulfuric acid diester"@en , "Sulfuric Acid Esters"@en , "sulfuric ester"@en ;
        skos:broader     csc:CHEMONTID_0003455 ;
        skos:definition  "Organic compounds containing the sulfuric acid diester functional group with the generic structure ROS(OR')(=O)=O, (R,R'=organyl group)."@en ;
        skos:inScheme    vlcs:chemische_stof ;
        skos:notation    "CHEMONTID:0001184" ;
        skos:prefLabel   "Sulfuric acid diesters"@en .

csc:CHEMONTID_0001359
        a                skos:Concept ;
        rdfs:seeAlso     tax_nodes:C0001359 ;
        skos:altLabel    "hydroxy monocarboxylic acid"@en , "2-hydroxy-carboxylic acids and derivatives"@en ;
        skos:broader     csc:CHEMONTID_0000472 ;
        skos:definition  "Organic compounds containing a carboxylic acid substituted with a hydroxyl group on the adjacent carbon."@en ;
        skos:inScheme    vlcs:chemische_stof ;
        skos:notation    "CHEMONTID:0001359" ;
        skos:prefLabel   "Alpha hydroxy acids and derivatives"@en .

csc:CHEMONTID_0002334
        a                skos:Concept ;
        skos:altLabel    "pyrroles"@en ;
        skos:broader     csc:CHEMONTID_0002257 ;
        skos:definition  "Polycyclic aromatic compounds containing a benzene ring linked to a pyrrole ring through a CC or CN bond."@en ;
        skos:inScheme    vlcs:chemische_stof ;
        skos:notation    "CHEMONTID:0002334" ;
        skos:prefLabel   "Phenylpyrroles"@en .

csc:CHEMONTID_0004712
        a                skos:Concept ;
        skos:broader     csc:CHEMONTID_0000285 ;
        skos:definition  "Aromatic compounds containing an anilide group in which the carboxamide group is substituted with an aromatic group. They have the general structure RNC(=O)R', where R= benzene, and R = aryl group."@en ;
        skos:inScheme    vlcs:chemische_stof ;
        skos:notation    "CHEMONTID:0004712" ;
        skos:prefLabel   "Aromatic anilides"@en .

csc:CHEMONTID_0004292
        a                skos:Concept ;
        skos:broader     csc:CHEMONTID_0000308 ;
        skos:definition  "Aromatic heterocyclic compounds containing a 1,2,4-benzothiadiazine ring system with two S=O bonds at the 1-position."@en ;
        skos:inScheme    vlcs:chemische_stof ;
        skos:notation    "CHEMONTID:0004292" ;
        skos:prefLabel   "1,2,4-benzothiadiazine-1,1-dioxides"@en .

csc:CHEMONTID_0000422
        a                skos:Concept ;
        rdfs:seeAlso     tax_nodes:C0000422 ;
        skos:broader     csc:CHEMONTID_0000001 ;
        skos:definition  "Inorganic compounds that contain only metal atoms."@en ;
        skos:inScheme    vlcs:chemische_stof ;
        skos:notation    "CHEMONTID:0000422" ;
        skos:prefLabel   "Homogeneous metal compounds"@en .

csc:CHEMONTID_0002800
        a                skos:Concept ;
        rdfs:seeAlso     tax_nodes:C0002800 ;
        skos:altLabel    "Disulfides"@en , "organic disulfide"@en , "disulfide"@en ;
        skos:broader     csc:CHEMONTID_0000004 ;
        skos:definition  "Organosulfur compounds with the general formula RSSR' (R,R' = alkyl, aryl)."@en ;
        skos:inScheme    vlcs:chemische_stof ;
        skos:notation    "CHEMONTID:0002800" ;
        skos:prefLabel   "Organic disulfides"@en .

csc:CHEMONTID_0002380
        a                skos:Concept ;
        skos:altLabel    "limonoid"@en , "a tetranortriterpenoid"@en , "Limonins"@en , "a limonoid"@en , "Tetranotriterpenoids"@en ;
        skos:broader     csc:CHEMONTID_0001553 ;
        skos:definition  "Highly oxygenated, modified terpenoids with a prototypical structure either containing or derived from a precursor with a 4,4,8-trimethyl-17-furanylsteroid skeleton. All naturally occurring citrus limonoids contain a furan ring attached to the D-ring, at C-17, as well as oxygen containing functional groups at C-3, C-4, C-7, C-16 and C-17."@en ;
        skos:inScheme    vlcs:chemische_stof ;
        skos:notation    "CHEMONTID:0002380" ;
        skos:prefLabel   "Limonoids"@en .

csc:CHEMONTID_0001152
        a                skos:Concept ;
        rdfs:seeAlso     tax_nodes:C0001152 ;
        skos:altLabel    "Nitro Compounds"@en , "nitro compounds"@en ;
        skos:broader     csc:CHEMONTID_0003631 ;
        skos:definition  "Compounds having the nitro group, -NO2 (free valence on nitrogen), which may be attached to carbon, nitrogen (as in nitramines), or oxygen (as in nitrates), among other elements (in the absence of specification, C-nitro compounds are usually implied)."@en ;
        skos:inScheme    vlcs:chemische_stof ;
        skos:notation    "CHEMONTID:0001152" ;
        skos:prefLabel   "Organic nitro compounds"@en .

csc:CHEMONTID_0003958
        a                skos:Concept ;
        skos:altLabel    "organofluorine compound"@en , "carbonyl compound"@en ;
        skos:broader     csc:CHEMONTID_0003962 ;
        skos:definition  "Organic compounds containing an octyl chain attached to the C-alpha of a carboxylic acid group (or a derivative thereof), where all hydrogens of the octyl chain are replaced by fluorine atoms."@en ;
        skos:inScheme    vlcs:chemische_stof ;
        skos:notation    "CHEMONTID:0003958" ;
        skos:prefLabel   "Perfluorooctanoic acid and derivatives"@en .

csc:CHEMONTID_0001871
        a                skos:Concept ;
        rdfs:seeAlso     tax_nodes:C0001871 ;
        skos:altLabel    "carbonyl compound"@en , "naphthalenes"@en , "Naphthoic acids and derivatives"@en ;
        skos:broader     csc:CHEMONTID_0000023 ;
        skos:definition  "Compounds containing a naphthalene moiety, which bears a carboxylic acid group or a derivative at one or more positions. Naphthalene is a bicyclic compound that is made up of two fused benzene ring."@en ;
        skos:inScheme    vlcs:chemische_stof ;
        skos:notation    "CHEMONTID:0001871" ;
        skos:prefLabel   "Naphthalenecarboxylic acids and derivatives"@en .

csc:CHEMONTID_0001373
        a                skos:Concept ;
        skos:altLabel    "ynone"@en ;
        skos:broader     csc:CHEMONTID_0003672 ;
        skos:definition  "Organic compounds containing the ynone functional group, an alpha,beta unsaturated ketone group with the general structure  RC#C-C(=O)R' (R'  not H)."@en ;
        skos:inScheme    vlcs:chemische_stof ;
        skos:notation    "CHEMONTID:0001373" ;
        skos:prefLabel   "Ynones"@en .

csc:CHEMONTID_0000398
        a                skos:Concept ;
        rdfs:seeAlso     tax_nodes:C0000398 ;
        skos:altLabel    "nitrogen mustard"@en , "Nitrogen Mustard Compounds"@en ;
        skos:broader     csc:CHEMONTID_0000278 ;
        skos:definition  "Compounds having two beta-haloalkyl groups bound to a nitrogen atom."@en ;
        skos:inScheme    vlcs:chemische_stof ;
        skos:notation    "CHEMONTID:0000398" ;
        skos:prefLabel   "Nitrogen mustard compounds"@en .

csc:CHEMONTID_0000145
        a                skos:Concept ;
        rdfs:seeAlso     tax_nodes:C0000145 ;
        skos:altLabel    "Coumarins"@en ;
        skos:broader     csc:CHEMONTID_0000261 ;
        skos:definition  "Polycyclic aromatic compounds containing a 1-benzopyran moiety with a ketone group at the C2 carbon atom (1-benzopyran-2-one)."@en ;
        skos:inScheme    vlcs:chemische_stof ;
        skos:notation    "CHEMONTID:0000145" ;
        skos:prefLabel   "Coumarins and derivatives"@en .

csc:CHEMONTID_0001548
        a                skos:Concept ;
        rdfs:seeAlso     tax_nodes:C0001548 ;
        skos:altLabel    "organohalogen compound"@en ;
        skos:broader     csc:CHEMONTID_0000265 ;
        skos:definition  "Carboxylic acids (or derivative thereof) containing a halogen atom bonded to the alpha carbon atom."@en ;
        skos:inScheme    vlcs:chemische_stof ;
        skos:notation    "CHEMONTID:0001548" ;
        skos:prefLabel   "Alpha-halocarboxylic acids and derivatives"@en .

csc:CHEMONTID_0003000
        a                skos:Concept ;
        skos:altLabel    "carboxylic acid"@en , "organohalogen compound"@en ;
        skos:broader     csc:CHEMONTID_0001548 ;
        skos:definition  "Carboxylic acids containing a halogen atom bonded to the alpha carbon atom."@en ;
        skos:inScheme    vlcs:chemische_stof ;
        skos:notation    "CHEMONTID:0003000" ;
        skos:prefLabel   "Alpha-halocarboxylic acids"@en .

csc:CHEMONTID_0000113
        a                skos:Concept ;
        rdfs:seeAlso     tax_nodes:C0000113 ;
        skos:altLabel    "phenylhydrazines"@en , "Phenylhydrazines"@en ;
        skos:broader     csc:CHEMONTID_0002279 ;
        skos:definition  "Compounds containing a phenylhydrazide moiety, which consists of a hydrazide substituent attached to a phenyl group."@en ;
        skos:inScheme    vlcs:chemische_stof ;
        skos:notation    "CHEMONTID:0000113" ;
        skos:prefLabel   "Phenylhydrazines"@en .

csc:CHEMONTID_0001516
        a                skos:Concept ;
        rdfs:seeAlso     tax_nodes:C0001516 ;
        skos:altLabel    "Chlorocarbons"@en , "organochlorine compound"@en ;
        skos:broader     csc:CHEMONTID_0000267 ;
        skos:definition  "Compounds containing a chemical bond between a carbon atom and a chlorine atom."@en ;
        skos:inScheme    vlcs:chemische_stof ;
        skos:notation    "CHEMONTID:0001516" ;
        skos:prefLabel   "Organochlorides"@en .

csc:CHEMONTID_0001096
        a                skos:Concept ;
        skos:altLabel    "fatty amide"@en , "N-acyl amines"@en ;
        skos:broader     csc:CHEMONTID_0000331 ;
        skos:definition  "Compounds containing a fatty acid moiety linked to an amine group through an ester linkage."@en ;
        skos:inScheme    vlcs:chemische_stof ;
        skos:notation    "CHEMONTID:0001096" ;
        skos:prefLabel   "N-acyl amines"@en .

csc:CHEMONTID_0003940
        a                skos:Concept ;
        rdfs:seeAlso     tax_nodes:C0003940 ;
        skos:altLabel    "organic oxide"@en ;
        skos:broader     csc:CHEMONTID_0004603 ;
        skos:definition  "Organic compounds containing an oxide group."@en ;
        skos:inScheme    vlcs:chemische_stof ;
        skos:notation    "CHEMONTID:0003940" ;
        skos:prefLabel   "Organic oxides"@en .

csc:CHEMONTID_0004670
        a                skos:Concept ;
        rdfs:seeAlso     tax_nodes:C0004670 ;
        skos:broader     csc:CHEMONTID_0002341 ;
        skos:definition  "Aromatic compounds that contain a phenol ether, which carries an amine group on the benzene ring."@en ;
        skos:inScheme    vlcs:chemische_stof ;
        skos:notation    "CHEMONTID:0004670" ;
        skos:prefLabel   "Aminophenyl ethers"@en .

csc:CHEMONTID_0000089
        a                skos:Concept ;
        rdfs:seeAlso     tax_nodes:C0000089 ;
        skos:altLabel    "Pyridines"@en ;
        skos:broader     csc:CHEMONTID_0000002 ;
        skos:definition  "Compounds containing a pyridine ring, which is a six-member aromatic heterocycle which consists of one nitrogen atom and five carbon atoms."@en ;
        skos:inScheme    vlcs:chemische_stof ;
        skos:notation    "CHEMONTID:0000089" ;
        skos:prefLabel   "Pyridines and derivatives"@en .

csc:CHEMONTID_0002467
        a                skos:Concept ;
        skos:altLabel    "polyol"@en ;
        skos:broader     csc:CHEMONTID_0002286 ;
        skos:definition  "Polyols containing an alcohol group at two adjacent positions."@en ;
        skos:inScheme    vlcs:chemische_stof ;
        skos:notation    "CHEMONTID:0002467" ;
        skos:prefLabel   "1,2-diols"@en .

csc:CHEMONTID_0001530
        a                skos:Concept ;
        rdfs:seeAlso     tax_nodes:C0001530 ;
        skos:altLabel    "a benzylnitrile"@en , "benzenes"@en , "nitrile"@en ;
        skos:broader     csc:CHEMONTID_0002279 ;
        skos:definition  "Organic compounds containing a benzene bearing a nitrile substituent."@en ;
        skos:inScheme    vlcs:chemische_stof ;
        skos:notation    "CHEMONTID:0001530" ;
        skos:prefLabel   "Benzonitriles"@en .

csc:CHEMONTID_0000555
        a                skos:Concept ;
        rdfs:seeAlso     tax_nodes:C0000555 ;
        skos:altLabel    "sulfide salt"@en ;
        skos:broader     csc:CHEMONTID_0000453 ;
        skos:definition  "Inorganic compounds containing a sulfur atom of an oxidation state of -2, in which the heaviest atom bonded to the oxygen belongs to the class of other non-metals."@en ;
        skos:inScheme    vlcs:chemische_stof ;
        skos:notation    "CHEMONTID:0000555" ;
        skos:prefLabel   "Other non-metal sulfides"@en .

csc:CHEMONTID_0000302
        a                skos:Concept ;
        rdfs:seeAlso     tax_nodes:C0000302 ;
        skos:altLabel    "Benzoxazoles"@en ;
        skos:broader     csc:CHEMONTID_0000002 ;
        skos:definition  "Organic compounds containing a benzene fused to an oxazole ring Oxazole is five-membered aromatic ring with a nitrogen and an oxygen atoms at the 1- and 3-position, respectively."@en ;
        skos:inScheme    vlcs:chemische_stof ;
        skos:notation    "CHEMONTID:0000302" ;
        skos:prefLabel   "Benzoxazoles"@en .

csc:CHEMONTID_0004347
        a                skos:Concept ;
        skos:broader     csc:CHEMONTID_0004348 ;
        skos:definition  "Tetraorganotin compounds where the tin atom is linked to exactly four alkyl groups."@en ;
        skos:inScheme    vlcs:chemische_stof ;
        skos:notation    "CHEMONTID:0004347" ;
        skos:prefLabel   "Tetraalkyltins"@en .

csc:CHEMONTID_0003410
        a                skos:Concept ;
        rdfs:seeAlso     tax_nodes:C0003410 ;
        skos:altLabel    "Chromenes"@en , "1-benzopyran"@en ;
        skos:broader     csc:CHEMONTID_0000123 ;
        skos:definition  "Organic aromatic compounds that 1-benzopyran, a bicyclic compound made up of a benzene ring fused to a pyran, so that the oxygen atom is at the 1-position."@en ;
        skos:inScheme    vlcs:chemische_stof ;
        skos:notation    "CHEMONTID:0003410" ;
        skos:prefLabel   "1-benzopyrans"@en .

csc:CHEMONTID_0001207
        a                skos:Concept ;
        skos:altLabel    "carbohydrazide"@en ;
        skos:broader     csc:CHEMONTID_0000112 ;
        skos:definition  "Compounds containing a derivative of thiosemicarbazide with the general structure R1N(R2)N(R3)C(=S)N(R4)R5 (R1-R5=H, alkyl, aryl) where the ketone group has carbonyl group has been replaced with a thiocarbonyl group."@en ;
        skos:inScheme    vlcs:chemische_stof ;
        skos:notation    "CHEMONTID:0001207" ;
        skos:prefLabel   "Thiosemicarbazides"@en .

csc:CHEMONTID_0002901
        a                skos:Concept ;
        rdfs:seeAlso     tax_nodes:C0002901 ;
        skos:altLabel    "isoflavonoid"@en , "2-Isoflavenes"@en ;
        skos:broader     csc:CHEMONTID_0002506 ;
        skos:definition  "Flavonoids with a structure based on the 3-phenylchromene skeleton, with a double bond between the C2 and C3 carbon atoms of the chromene moiety."@en ;
        skos:inScheme    vlcs:chemische_stof ;
        skos:notation    "CHEMONTID:0002901" ;
        skos:prefLabel   "Isoflav-2-enes"@en .

csc:CHEMONTID_0001253
        a                skos:Concept ;
        rdfs:seeAlso     tax_nodes:C0001253 ;
        skos:altLabel    "Quinolines"@en , "quinolines"@en ;
        skos:broader     csc:CHEMONTID_0000002 ;
        skos:definition  "Compounds containing a quinoline moiety, which consists of a benzene ring fused to a pyrimidine ring to form benzo[b]azabenzene."@en ;
        skos:inScheme    vlcs:chemische_stof ;
        skos:notation    "CHEMONTID:0001253" ;
        skos:prefLabel   "Quinolines and derivatives"@en .

csc:CHEMONTID_0000278
        a                skos:Concept ;
        rdfs:seeAlso     tax_nodes:C0000278 ;
        skos:altLabel    "organonitrogen compound"@en ;
        skos:broader     csc:CHEMONTID_0004707 ;
        skos:definition  "Organic compounds containing a nitrogen atom."@en ;
        skos:inScheme    vlcs:chemische_stof ;
        skos:notation    "CHEMONTID:0000278" ;
        skos:prefLabel   "Organonitrogen compounds"@en .

csc:CHEMONTID_0003631
        a                skos:Concept ;
        rdfs:seeAlso     tax_nodes:C0003631 ;
        skos:altLabel    "dipolar compound"@en ;
        skos:broader     csc:CHEMONTID_0003630 ;
        skos:definition  "Organic 1,3-dipolar compounds with the general structure  X=Y+-Z- <-> X--Y+=Z<-> X+-Y-Z-<-> X-=Y-Z+ (X, Z = C, N, or O; Y = N or O)."@en ;
        skos:inScheme    vlcs:chemische_stof ;
        skos:notation    "CHEMONTID:0003631" ;
        skos:prefLabel   "Allyl-type 1,3-dipolar organic compounds"@en .

csc:CHEMONTID_0000025
        a                skos:Concept ;
        rdfs:seeAlso     tax_nodes:C0000025 ;
        skos:altLabel    "Phenanthrenes"@en , "phenanthrenes"@en ;
        skos:broader     csc:CHEMONTID_0002448 ;
        skos:definition  "Polycyclic compounds containing a phenanthrene moiety, which is a tricyclic aromatic compound with three non-linearly fused benzene."@en ;
        skos:inScheme    vlcs:chemische_stof ;
        skos:notation    "CHEMONTID:0000025" ;
        skos:prefLabel   "Phenanthrenes and derivatives"@en .

csc:CHEMONTID_0004361
        a                skos:Concept ;
        skos:broader     csc:CHEMONTID_0000176 ;
        skos:definition  "Derivatives of amino benzoic acid derivatives where the amine group is N-acylated."@en ;
        skos:inScheme    vlcs:chemische_stof ;
        skos:notation    "CHEMONTID:0004361" ;
        skos:prefLabel   "Acylaminobenzoic acid and derivatives"@en .

csc:CHEMONTID_0004789
        a                skos:Concept ;
        rdfs:seeAlso     tax_nodes:C0004789 ;
        skos:broader     csc:CHEMONTID_0004788 ;
        skos:definition  "Aromatic heterocyclic compounds containing a benzene ring fused to a diazine ring. The diazine ring is an analogue of benzene, where two carbon atoms are replaced by nitrogen atoms."@en ;
        skos:inScheme    vlcs:chemische_stof ;
        skos:notation    "CHEMONTID:0004789" ;
        skos:prefLabel   "Benzodiazines"@en .

csc:CHEMONTID_0000292
        a                skos:Concept ;
        skos:altLabel    "barbiturates"@en ;
        skos:broader     csc:CHEMONTID_0000291 ;
        skos:definition  "Compounds containing a perhydropyrimidine ring substituted at C-2, -4 and -6 by oxo groups."@en ;
        skos:inScheme    vlcs:chemische_stof ;
        skos:notation    "CHEMONTID:0000292" ;
        skos:prefLabel   "Barbituric acid derivatives"@en .

csc:CHEMONTID_0002126
        a                skos:Concept ;
        skos:altLabel    "para-terphenyl"@en ;
        skos:broader     csc:CHEMONTID_0002042 ;
        skos:definition  "Terphenyls with a structure containing the 1,4-diphenylbenzene skeleton."@en ;
        skos:inScheme    vlcs:chemische_stof ;
        skos:notation    "CHEMONTID:0002126" ;
        skos:prefLabel   "P-terphenyls"@en .

csc:CHEMONTID_0004504
        a                skos:Concept ;
        rdfs:seeAlso     tax_nodes:C0004504 ;
        skos:altLabel    "cyanides"@en ;
        skos:broader     csc:CHEMONTID_0000278 ;
        skos:definition  "Organic nitrogen compounds that contain the cyano (C#N) group. The group can be present either in the anionic or covalently bond form."@en ;
        skos:inScheme    vlcs:chemische_stof ;
        skos:notation    "CHEMONTID:0004504" ;
        skos:prefLabel   "Organic cyanides"@en .

csc:CHEMONTID_0004084
        a                skos:Concept ;
        skos:broader     csc:CHEMONTID_0000362 ;
        skos:definition  "Organonitrogen compounds of the form NC-CN or X-CN, where X is a halogen."@en ;
        skos:inScheme    vlcs:chemische_stof ;
        skos:notation    "CHEMONTID:0004084" ;
        skos:prefLabel   "Cyanogens"@en .

csc:CHEMONTID_0003575
        a                skos:Concept ;
        skos:altLabel    "amino cyclitol"@en ;
        skos:broader     csc:CHEMONTID_0001675 ;
        skos:definition  "Aminoglycosides containing the 2-deoxystreptamine (1,3-diaminocyclohexane-4,5,6-triol) core."@en ;
        skos:inScheme    vlcs:chemische_stof ;
        skos:notation    "CHEMONTID:0003575" ;
        skos:prefLabel   "2-deoxystreptamine aminoglycosides"@en .

csc:CHEMONTID_0003322
        a                skos:Concept ;
        skos:altLabel    "wax ester"@en , "Wax monoesters"@en ;
        skos:broader     csc:CHEMONTID_0001723 ;
        skos:definition  "Waxes bearing an ester group at exactly one position."@en ;
        skos:inScheme    vlcs:chemische_stof ;
        skos:notation    "CHEMONTID:0003322" ;
        skos:prefLabel   "Wax monoesters"@en .

csc:CHEMONTID_0001663
        a                skos:Concept ;
        skos:altLabel    "carboxamide"@en ;
        skos:broader     csc:CHEMONTID_0000475 ;
        skos:definition  "Compounds containing a secondary carboxylic acid amide functional group, with the general structure RC(=O)N(R')H (R,R'=alkyl, aryl)."@en ;
        skos:inScheme    vlcs:chemische_stof ;
        skos:notation    "CHEMONTID:0001663" ;
        skos:prefLabel   "Secondary carboxylic acid amides"@en .

csc:CHEMONTID_0000435
        a                skos:Concept ;
        rdfs:seeAlso     tax_nodes:C0000435 ;
        skos:altLabel    "oxoanion"@en ;
        skos:broader     csc:CHEMONTID_0000423 ;
        skos:definition  "Inorganic non-metallic compounds containing an oxoanion."@en ;
        skos:inScheme    vlcs:chemische_stof ;
        skos:notation    "CHEMONTID:0000435" ;
        skos:prefLabel   "Non-metal oxoanionic compounds"@en .

csc:CHEMONTID_0004771
        a                skos:Concept ;
        skos:broader     csc:CHEMONTID_0004623 ;
        skos:definition  "Organic compounds containing the thiophosphoric acid functional group or a derivative thereof, with the general structure ROP(OR')(OR'')=S, where R= pyrimidine, R' = organyl group , and R\" = any atom."@en ;
        skos:inScheme    vlcs:chemische_stof ;
        skos:notation    "CHEMONTID:0004771" ;
        skos:prefLabel   "Pyrimidinyl phosphorothioates"@en .

csc:CHEMONTID_0000901
        a                skos:Concept ;
        rdfs:seeAlso     tax_nodes:C0000901 ;
        skos:altLabel    "alkali metal salt"@en ;
        skos:broader     csc:CHEMONTID_0000445 ;
        skos:definition  "Inorganic compounds in which the largest oxoanion is silicate, and in which the heaviest atom not in an oxoanion is an alkali metal."@en ;
        skos:inScheme    vlcs:chemische_stof ;
        skos:notation    "CHEMONTID:0000901" ;
        skos:prefLabel   "Alkali metal silicates"@en .

csc:CHEMONTID_0000403
        a                skos:Concept ;
        rdfs:seeAlso     tax_nodes:C0000403 ;
        skos:altLabel    "sulfuric acid derivative"@en ;
        skos:broader     csc:CHEMONTID_0000264 ;
        skos:definition  "Organic compounds containing the sulfuric acid or a derivative thereof."@en ;
        skos:inScheme    vlcs:chemische_stof ;
        skos:notation    "CHEMONTID:0000403" ;
        skos:prefLabel   "Organic sulfuric acids and derivatives"@en .

csc:CHEMONTID_0001133
        a                skos:Concept ;
        skos:altLabel    "Monoglycerides"@en , "monoglyceride"@en , "Monoacylglycerol"@en , "Monoacylglycerols"@en ;
        skos:broader     csc:CHEMONTID_0003808 ;
        skos:definition  "Glycerides consisting of one fatty acid chain covalently bonded to a glycerol molecule through an ester linkage."@en ;
        skos:inScheme    vlcs:chemische_stof ;
        skos:notation    "CHEMONTID:0001133" ;
        skos:prefLabel   "Monoacylglycerols"@en .

csc:CHEMONTID_0001820
        a                skos:Concept ;
        skos:altLabel    "isoindoles"@en ;
        skos:broader     csc:CHEMONTID_0002496 ;
        skos:definition  "Aromatic polycyclic compounds that an isoindole bearing a ketone."@en ;
        skos:inScheme    vlcs:chemische_stof ;
        skos:notation    "CHEMONTID:0001820" ;
        skos:prefLabel   "Isoindolones"@en .

csc:CHEMONTID_0003487
        a                skos:Concept ;
        skos:altLabel    "cyclic ketone"@en ;
        skos:broader     csc:CHEMONTID_0000118 ;
        skos:definition  "Organic compounds containing a ketone that is conjugated to a cyclic moiety."@en ;
        skos:inScheme    vlcs:chemische_stof ;
        skos:notation    "CHEMONTID:0003487" ;
        skos:prefLabel   "Cyclic ketones"@en .

csc:CHEMONTID_0004637
        a                skos:Concept ;
        skos:broader     csc:CHEMONTID_0004105 ;
        skos:definition  "Aromatic compounds containing a 1,3,5-triazine ring that is substituted at the 2-position with a S-alkyl group."@en ;
        skos:inScheme    vlcs:chemische_stof ;
        skos:notation    "CHEMONTID:0004637" ;
        skos:prefLabel   "Alkyl-2-thio-S-triazines"@en .

csc:CHEMONTID_0000172
        a                skos:Concept ;
        skos:altLabel    "penams"@en ;
        skos:broader     csc:CHEMONTID_0000162 ;
        skos:definition  "Organic heterocyclic compounds containing the 4-thia-1-azabicyclo[3.2.0]heptan-7-one structure."@en ;
        skos:inScheme    vlcs:chemische_stof ;
        skos:notation    "CHEMONTID:0000172" ;
        skos:prefLabel   "Penams"@en .

csc:CHEMONTID_0000347
        a                skos:Concept ;
        skos:altLabel    "organonitrogen compound"@en , "organooxygen compound"@en , "Amino Acids"@en ;
        skos:broader     csc:CHEMONTID_0000013 ;
        skos:definition  "Organic compounds containing an amine group, a carboxylic acid group (or a derivative thereof), and a side-chain that is specific to each amino acid."@en ;
        skos:inScheme    vlcs:chemische_stof ;
        skos:notation    "CHEMONTID:0000347" ;
        skos:prefLabel   "Amino acids and derivatives"@en .

csc:CHEMONTID_0003953
        a                skos:Concept ;
        rdfs:seeAlso     tax_nodes:C0003953 ;
        skos:altLabel    "hydroxyquinoline"@en ;
        skos:broader     csc:CHEMONTID_0001253 ;
        skos:definition  "Compounds containing a quinoline moiety, which carries a hydroxy group at the 8-position. Quinoline consists of a benzene ring fused to a pyrimidine ring to form benzo[b]azabenzene."@en ;
        skos:inScheme    vlcs:chemische_stof ;
        skos:notation    "CHEMONTID:0003953" ;
        skos:prefLabel   "8-hydroxyquinolines"@en .

csc:CHEMONTID_0001322
        a                skos:Concept ;
        rdfs:seeAlso     tax_nodes:C0001322 ;
        skos:altLabel    "aromatic carboxylic acid"@en ;
        skos:broader     csc:CHEMONTID_0000089 ;
        skos:definition  "Compounds containing a pyridine ring bearing a carboxylic acid group or a derivative thereof."@en ;
        skos:inScheme    vlcs:chemische_stof ;
        skos:notation    "CHEMONTID:0001322" ;
        skos:prefLabel   "Pyridinecarboxylic acids and derivatives"@en .

csc:CHEMONTID_0001077
        a                skos:Concept ;
        rdfs:seeAlso     tax_nodes:C0001077 ;
        skos:altLabel    "p-block molecular entity"@en , "inorganic sulfate salt"@en ;
        skos:broader     csc:CHEMONTID_0000435 ;
        skos:definition  "Inorganic non-metallic compoundscontaining a sulfate as its largest oxoanion."@en , "Inorganic non-metallic compounds containing a sulfate as its largest oxoanion."@en ;
        skos:inScheme    vlcs:chemische_stof ;
        skos:notation    "CHEMONTID:0001077" ;
        skos:prefLabel   "Non-metal sulfates"@en .

csc:CHEMONTID_0003455
        a                skos:Concept ;
        rdfs:seeAlso     tax_nodes:C0003455 ;
        skos:altLabel    "sulfuric ester"@en ;
        skos:broader     csc:CHEMONTID_0000403 ;
        skos:definition  "Organic compounds containing a sulfate group that carries one or two O-ester groups."@en ;
        skos:inScheme    vlcs:chemische_stof ;
        skos:notation    "CHEMONTID:0003455" ;
        skos:prefLabel   "Sulfuric acid esters"@en .

csc:CHEMONTID_0002771
        a                skos:Concept ;
        skos:altLabel    "monochlorophenol"@en ;
        skos:broader     csc:CHEMONTID_0002766 ;
        skos:definition  "Chlorophenols carrying a iodine at the C2 position of the benzene ring."@en ;
        skos:inScheme    vlcs:chemische_stof ;
        skos:notation    "CHEMONTID:0002771" ;
        skos:prefLabel   "O-chlorophenols"@en .

csc:CHEMONTID_0000315
        a                skos:Concept ;
        rdfs:seeAlso     tax_nodes:C0000315 ;
        skos:altLabel    "benzotriazoles"@en ;
        skos:broader     csc:CHEMONTID_0000002 ;
        skos:definition  "Organic compounds containing a benzene fused to a triazole ring (a five-membered ring with two carbon atoms and three nitrogen atoms)."@en ;
        skos:inScheme    vlcs:chemische_stof ;
        skos:notation    "CHEMONTID:0000315" ;
        skos:prefLabel   "Benzotriazoles"@en .

csc:CHEMONTID_0002273
        a                skos:Concept ;
        skos:altLabel    "imidazolidine-2,4-dione"@en , "an  imidazolidine-2,4-dione"@en , " Imidazolidine-2,4-diones"@en ;
        skos:broader     csc:CHEMONTID_0001150 ;
        skos:definition  "Heterocyclic compounds containing an imidazolidine  substituted by ketone group at positions 2 and 4."@en ;
        skos:inScheme    vlcs:chemische_stof ;
        skos:notation    "CHEMONTID:0002273" ;
        skos:prefLabel   "Hydantoins"@en .

csc:CHEMONTID_0004107
        a                skos:Concept ;
        rdfs:seeAlso     tax_nodes:C0004107 ;
        skos:broader     csc:CHEMONTID_0000098 ;
        skos:definition  "Compounds containing a triazine ring, which is a heterocyclic ring, similar to the six-member benzene ring but with three carbons replaced by nitrogen atoms, at ring positions 1, 2, and 4."@en ;
        skos:inScheme    vlcs:chemische_stof ;
        skos:notation    "CHEMONTID:0004107" ;
        skos:prefLabel   "1,2,4-triazines"@en .

csc:CHEMONTID_0002448
        a                skos:Concept ;
        rdfs:seeAlso     tax_nodes:C0002448 ;
        skos:altLabel    "benzenoid aromatic compound"@en ;
        skos:broader     csc:CHEMONTID_0000000 ;
        skos:definition  "Aromatic compounds containing one or more benzene rings."@en ;
        skos:inScheme    vlcs:chemische_stof ;
        skos:notation    "CHEMONTID:0002448" ;
        skos:prefLabel   "Benzenoids"@en .

csc:CHEMONTID_0001764
        a                skos:Concept ;
        rdfs:seeAlso     tax_nodes:C0001764 ;
        skos:altLabel    "pyridinium ion"@en ;
        skos:broader     csc:CHEMONTID_0000089 ;
        skos:definition  "Compounds containing a pyridinium ring, which is the cationic form of pyridine."@en ;
        skos:inScheme    vlcs:chemische_stof ;
        skos:notation    "CHEMONTID:0001764" ;
        skos:prefLabel   "Pyridinium derivatives"@en .

csc:CHEMONTID_0001091
        a                skos:Concept ;
        rdfs:seeAlso     tax_nodes:C0001091 ;
        skos:altLabel    "a toluene"@en , "toluenes"@en ;
        skos:broader     csc:CHEMONTID_0002279 ;
        skos:definition  "Compounds containing a benzene ring which bears a methane group."@en ;
        skos:inScheme    vlcs:chemische_stof ;
        skos:notation    "CHEMONTID:0001091" ;
        skos:prefLabel   "Toluenes"@en .

csc:CHEMONTID_0002494
        a                skos:Concept ;
        skos:altLabel    "benzoquinones"@en , "p-quinone"@en , "Benzoquinones"@en ;
        skos:broader     csc:CHEMONTID_0002384 ;
        skos:definition  "Benzoquinones where the two C=O groups are attached at the 1- and 4-positions, respectively."@en ;
        skos:inScheme    vlcs:chemische_stof ;
        skos:notation    "CHEMONTID:0002494" ;
        skos:prefLabel   "P-benzoquinones"@en .

csc:CHEMONTID_0000038
        a                skos:Concept ;
        rdfs:seeAlso     tax_nodes:C0000038 ;
        skos:altLabel    "a sulfanilide"@en , "a sulfonanilide"@en , "Sulfonanilides"@en ;
        skos:broader     csc:CHEMONTID_0002279 ;
        skos:definition  "Organic aromatic compounds containing a sulfanilide moiety, with the general structure RS(=O)(=O)NC1=CC=CC=C1."@en ;
        skos:inScheme    vlcs:chemische_stof ;
        skos:notation    "CHEMONTID:0000038" ;
        skos:prefLabel   "Sulfanilides"@en .

csc:CHEMONTID_0000504
        a                skos:Concept ;
        rdfs:seeAlso     tax_nodes:C0000504 ;
        skos:altLabel    "lipid"@en , "Linoleic Acids"@en ;
        skos:broader     csc:CHEMONTID_0003909 ;
        skos:definition  "Derivatives of lineolic acid. Lineolic acid is a polyunsaturated omega-6 18 carbon long fatty acid, with two CC double bonds at the 9- and 12-positions."@en ;
        skos:inScheme    vlcs:chemische_stof ;
        skos:notation    "CHEMONTID:0000504" ;
        skos:prefLabel   "Lineolic acids and derivatives"@en .

csc:CHEMONTID_0003865
        a                skos:Concept ;
        rdfs:seeAlso     tax_nodes:C0003865 ;
        skos:broader     csc:CHEMONTID_0000000 ;
        skos:definition  "Organic compounds consisting of an assembly of cations and anions."@en ;
        skos:inScheme    vlcs:chemische_stof ;
        skos:notation    "CHEMONTID:0003865" ;
        skos:prefLabel   "Organic salts"@en .

csc:CHEMONTID_0001234
        a                skos:Concept ;
        rdfs:seeAlso     tax_nodes:C0001234 ;
        skos:altLabel    "isothiocyanate"@en , "isothiocyanates"@en , "Isothiocyanates"@en ;
        skos:broader     csc:CHEMONTID_0000004 ;
        skos:definition  "Organic compounds containing the isothiocyanate group, an isocyanate analogue with the general formula RN=C=S."@en ;
        skos:inScheme    vlcs:chemische_stof ;
        skos:notation    "CHEMONTID:0001234" ;
        skos:prefLabel   "Isothiocyanates"@en .

csc:CHEMONTID_0000259
        a                skos:Concept ;
        rdfs:seeAlso     tax_nodes:C0000259 ;
        skos:altLabel    "Prenyllipids"@en ;
        skos:broader     csc:CHEMONTID_0000012 ;
        skos:definition  "Lipids synthesized from the five-carbon-unit precursors isopentenyl diphosphate and dimethylallyl diphosphate."@en ;
        skos:inScheme    vlcs:chemische_stof ;
        skos:notation    "CHEMONTID:0000259" ;
        skos:prefLabel   "Prenol lipids"@en .

csc:CHEMONTID_0000550
        a                skos:Concept ;
        rdfs:seeAlso     tax_nodes:C0000550 ;
        skos:altLabel    "halogen oxide"@en ;
        skos:broader     csc:CHEMONTID_0000454 ;
        skos:definition  "Inorganic compounds containing an oxygen atom of an oxidation state of -2, in which the heaviest atom bonded to the oxygen is a halogen."@en ;
        skos:inScheme    vlcs:chemische_stof ;
        skos:notation    "CHEMONTID:0000550" ;
        skos:prefLabel   "Halogen oxides"@en .

csc:CHEMONTID_0002858
        a                skos:Concept ;
        rdfs:seeAlso     tax_nodes:C0002858 ;
        skos:altLabel    "ifosfamides"@en ;
        skos:broader     csc:CHEMONTID_0002466 ;
        skos:definition  "Oxazaphospholanes containing the isofamide skeleton. Isofamide is a heterocyclic compound made up of a 1,3,2-oxazaphospholane, where the phosphorus atom is part of a phosphodiamide group, and the oxazaphospholane is substituted by two haloalkyl chains."@en ;
        skos:inScheme    vlcs:chemische_stof ;
        skos:notation    "CHEMONTID:0002858" ;
        skos:prefLabel   "Isofamides"@en .

csc:CHEMONTID_0000052
        a                skos:Concept ;
        skos:altLabel    "Bromobiphenyls"@en ;
        skos:broader     csc:CHEMONTID_0000041 ;
        skos:definition  "Organic compounds containing a biphenyl moiety substituted at one or more positions by a bromine atom."@en ;
        skos:inScheme    vlcs:chemische_stof ;
        skos:notation    "CHEMONTID:0000052" ;
        skos:prefLabel   "Brominated biphenyls"@en .

csc:CHEMONTID_0004517
        a                skos:Concept ;
        skos:broader     csc:CHEMONTID_0003276 ;
        skos:definition  "Aromatic heterocyclic compounds containing a toluene that is p-substituted with a sulfonamide group."@en ;
        skos:inScheme    vlcs:chemische_stof ;
        skos:notation    "CHEMONTID:0004517" ;
        skos:prefLabel   "P-toluenesulfonamides"@en .

csc:CHEMONTID_0001455
        a                skos:Concept ;
        rdfs:seeAlso     tax_nodes:C0001455 ;
        skos:altLabel    "tetrapyrrole"@en ;
        skos:broader     csc:CHEMONTID_0000002 ;
        skos:definition  "Polycyclic aromatic compounds containing four pyrrole rings joined by one-carbon units linking position 2 of one pyrrole ring to position 5 of the next."@en ;
        skos:inScheme    vlcs:chemische_stof ;
        skos:notation    "CHEMONTID:0001455" ;
        skos:prefLabel   "Tetrapyrroles and derivatives"@en .

csc:CHEMONTID_0004097
        a                skos:Concept ;
        rdfs:seeAlso     tax_nodes:C0004097 ;
        skos:broader     csc:CHEMONTID_0000295 ;
        skos:definition  "Organic compounds containing a benzene ring fused to a 1,4-azepine."@en ;
        skos:inScheme    vlcs:chemische_stof ;
        skos:notation    "CHEMONTID:0004097" ;
        skos:prefLabel   "1,4-benzodiazepines"@en .

csc:CHEMONTID_0001202
        a                skos:Concept ;
        rdfs:seeAlso     tax_nodes:C0001202 ;
        skos:altLabel    "thioethers"@en , "organic sulfide"@en ;
        skos:broader     csc:CHEMONTID_0000004 ;
        skos:definition  "Compounds containing the ester derivative of thiocarboxylic acid, with the general structure R-S-R' (R,R'=alkyl, aryl)."@en ;
        skos:inScheme    vlcs:chemische_stof ;
        skos:notation    "CHEMONTID:0001202" ;
        skos:prefLabel   "Thioethers"@en .

csc:CHEMONTID_0004310
        a                skos:Concept ;
        skos:broader     csc:CHEMONTID_0000060 ;
        skos:definition  "Compounds containing valine or a derivative thereof resulting from reaction of valine at the amino group or the carboxy group, or from the replacement of any hydrogen of glycine by a heteroatom."@en ;
        skos:inScheme    vlcs:chemische_stof ;
        skos:notation    "CHEMONTID:0004310" ;
        skos:prefLabel   "Valine and derivatives"@en .

csc:CHEMONTID_0002651
        a                skos:Concept ;
        rdfs:seeAlso     tax_nodes:C0002651 ;
        skos:altLabel    "diarylheptanoid"@en ;
        skos:broader     csc:CHEMONTID_0002650 ;
        skos:definition  "Diarylheptanoids with an open heptane chain. The two aromatic rings are linked only by the heptane chain."@en ;
        skos:inScheme    vlcs:chemische_stof ;
        skos:notation    "CHEMONTID:0002651" ;
        skos:prefLabel   "Linear diarylheptanoids"@en .

csc:CHEMONTID_0000020
        a                skos:Concept ;
        rdfs:seeAlso     tax_nodes:C0000020 ;
        skos:altLabel    "fluorenes"@en ;
        skos:broader     csc:CHEMONTID_0002448 ;
        skos:definition  "Compounds containing a fluorene moiety, which consists of two benzene rings connected through either a cyclopentane, cyclopentene, or cyclopenta-1,3-diene."@en ;
        skos:inScheme    vlcs:chemische_stof ;
        skos:notation    "CHEMONTID:0000020" ;
        skos:prefLabel   "Fluorenes"@en .

csc:CHEMONTID_0001423
        a                skos:Concept ;
        skos:altLabel    "Thia fatty acids"@en , "thia fatty acid"@en ;
        skos:broader     csc:CHEMONTID_0000262 ;
        skos:definition  "Fatty acid derivatives obtained by insertion of a sulfur atom at specific positions in the chain."@en ;
        skos:inScheme    vlcs:chemische_stof ;
        skos:notation    "CHEMONTID:0001423" ;
        skos:prefLabel   "Thia fatty acids"@en .

csc:CHEMONTID_0000494
        a                skos:Concept ;
        skos:altLabel    "Isoflavonoids"@en , "3-Phenylchromones"@en , "Isoflavones"@en , "isoflavones"@en ;
        skos:broader     csc:CHEMONTID_0002901 ;
        skos:definition  "Polycyclic compounds containing a 2-isoflavene skeleton which bears a ketone group at the C4 carbon atom."@en ;
        skos:inScheme    vlcs:chemische_stof ;
        skos:notation    "CHEMONTID:0000494" ;
        skos:prefLabel   "Isoflavones"@en .

csc:CHEMONTID_0001897
        a                skos:Concept ;
        skos:altLabel    "amino alcohol"@en ;
        skos:broader     csc:CHEMONTID_0002460 ;
        skos:definition  "Organic compounds containing an alkyl chain with an amine group bound to the C1 atom and an alcohol group bound to the C2 atom."@en ;
        skos:inScheme    vlcs:chemische_stof ;
        skos:notation    "CHEMONTID:0001897" ;
        skos:prefLabel   "1,2-aminoalcohols"@en .

csc:CHEMONTID_0004706
        a                skos:Concept ;
        skos:altLabel    "triazines"@en ;
        skos:broader     csc:CHEMONTID_0000490 ;
        skos:definition  "Aromatic heterocyclic compounds containing a s-triazine ring which is substituted with a urea at the ring 2-position."@en ;
        skos:inScheme    vlcs:chemische_stof ;
        skos:notation    "CHEMONTID:0004706" ;
        skos:prefLabel   "S-triazinyl-2-sulfonylureas"@en .

csc:CHEMONTID_0001644
        a                skos:Concept ;
        skos:altLabel    "Diglycerides"@en , "a 1,2-diacyl-sn-glycerol"@en , "1,2-diglyceride"@en , "1,2-diacyl-sn-glycerol"@en ;
        skos:broader     csc:CHEMONTID_0001129 ;
        skos:definition  "Diacylglycerols containing a glycerol acylated at positions 1 and 2."@en ;
        skos:inScheme    vlcs:chemische_stof ;
        skos:notation    "CHEMONTID:0001644" ;
        skos:prefLabel   "1,2-diacylglycerols"@en .

csc:CHEMONTID_0001819
        a                skos:Concept ;
        rdfs:seeAlso     tax_nodes:C0001819 ;
        skos:altLabel    "isoindoles"@en ;
        skos:broader     csc:CHEMONTID_0000002 ;
        skos:definition  "Polycyclic compounds containing an isoindole moiety, which is structurally characterized by a cyclohexadiene fused to a pyrrole ring."@en ;
        skos:inScheme    vlcs:chemische_stof ;
        skos:notation    "CHEMONTID:0001819" ;
        skos:prefLabel   "Isoindoles and derivatives"@en .

csc:CHEMONTID_0003058
        a                skos:Concept ;
        skos:altLabel    "20-oxo steroid"@en ;
        skos:broader     csc:CHEMONTID_0001194 ;
        skos:definition  "Steroid derivatives carrying a C=O group at the 20-position of the steroid skeleton."@en ;
        skos:inScheme    vlcs:chemische_stof ;
        skos:notation    "CHEMONTID:0003058" ;
        skos:prefLabel   "20-oxosteroids"@en .

csc:CHEMONTID_0004752
        a                skos:Concept ;
        rdfs:seeAlso     tax_nodes:C0004752 ;
        skos:broader     csc:CHEMONTID_0000278 ;
        skos:definition  "Oxime ether derivatives with the general formula CC(R)=NOC(=O)N(R')R\\\", where R-R\\\" = H or organyl."@en , "Oxime ether derivatives with the general formula CC(R)=NOC(=O)N(R')R\", where R-R\" = H or organyl."@en ;
        skos:inScheme    vlcs:chemische_stof ;
        skos:notation    "CHEMONTID:0004752" ;
        skos:prefLabel   "Oxime carbamates"@en .

csc:CHEMONTID_0004208
        a                skos:Concept ;
        rdfs:seeAlso     tax_nodes:C0004208 ;
        skos:altLabel    "xylene"@en ;
        skos:broader     csc:CHEMONTID_0002279 ;
        skos:definition  "Aromatic compounds that contain a xylene moiety, which is a monocyclic benzene carrying exactly two methyl groups."@en ;
        skos:inScheme    vlcs:chemische_stof ;
        skos:notation    "CHEMONTID:0004208" ;
        skos:prefLabel   "Xylenes"@en .

csc:CHEMONTID_0000462
        a                skos:Concept ;
        rdfs:seeAlso     tax_nodes:C0000462 ;
        skos:altLabel    "an organometallic compound"@en , "organometallic compound"@en ;
        skos:broader     csc:CHEMONTID_0000000 ;
        skos:definition  "Organic compounds containing a bond between a carbon atom and metal atom."@en ;
        skos:inScheme    vlcs:chemische_stof ;
        skos:notation    "CHEMONTID:0000462" ;
        skos:prefLabel   "Organometallic compounds"@en .

csc:CHEMONTID_0002840
        a                skos:Concept ;
        skos:altLabel    "cyclic olefin"@en ;
        skos:broader     csc:CHEMONTID_0002838 ;
        skos:definition  "Olefins that contain at least one ring in their structure."@en ;
        skos:inScheme    vlcs:chemische_stof ;
        skos:notation    "CHEMONTID:0002840" ;
        skos:prefLabel   "Cyclic olefins"@en .

csc:CHEMONTID_0003570
        a                skos:Concept ;
        skos:altLabel    "estrogen"@en ;
        skos:broader     csc:CHEMONTID_0001466 ;
        skos:definition  "Steroids with a structure containing a 3-hydroxylated estrane."@en ;
        skos:inScheme    vlcs:chemische_stof ;
        skos:notation    "CHEMONTID:0003570" ;
        skos:prefLabel   "Estrogens and derivatives"@en .

csc:CHEMONTID_0001192
        a                skos:Concept ;
        skos:altLabel    "halide"@en ;
        skos:broader     csc:CHEMONTID_0000318 ;
        skos:definition  "Compounds containing a carbamic acid derivative linked to a halogen atom."@en ;
        skos:inScheme    vlcs:chemische_stof ;
        skos:notation    "CHEMONTID:0001192" ;
        skos:prefLabel   "Carbamic acid halides"@en .

csc:CHEMONTID_0004001
        a                skos:Concept ;
        skos:broader     csc:CHEMONTID_0002562 ;
        skos:definition  "Thiadiazoles with an amino group attached to the 2-position of a 1,3,4-thiadiazole ring."@en ;
        skos:inScheme    vlcs:chemische_stof ;
        skos:notation    "CHEMONTID:0004001" ;
        skos:prefLabel   "2-amino-1,3,4-thiadiazoles"@en .

csc:CHEMONTID_0001114
        a                skos:Concept ;
        rdfs:seeAlso     tax_nodes:C0001114 ;
        skos:altLabel    "a 3-oxo acid"@en ;
        skos:broader     csc:CHEMONTID_0000389 ;
        skos:definition  "Organic compounds containing an aldehyde substituted with a keto group on the C3 carbon atom."@en ;
        skos:inScheme    vlcs:chemische_stof ;
        skos:notation    "CHEMONTID:0001114" ;
        skos:prefLabel   "Beta-keto acids and derivatives"@en .

csc:CHEMONTID_0000139
        a                skos:Concept ;
        rdfs:seeAlso     tax_nodes:C0000139 ;
        skos:broader     csc:CHEMONTID_0000134 ;
        skos:definition  "Compounds containing a hydroxyethyl group attached to the C4 carbon of a phenol group."@en ;
        skos:inScheme    vlcs:chemische_stof ;
        skos:notation    "CHEMONTID:0000139" ;
        skos:prefLabel   "Tyrosols and derivatives"@en .

csc:CHEMONTID_0000430
        a                skos:Concept ;
        rdfs:seeAlso     tax_nodes:C0000430 ;
        skos:broader     csc:CHEMONTID_0000422 ;
        skos:definition  "Inorganic compounds containing only metal atoms,with the largest atom being a transition metal atom."@en ;
        skos:inScheme    vlcs:chemische_stof ;
        skos:notation    "CHEMONTID:0000430" ;
        skos:prefLabel   "Homogeneous actinide compounds"@en .

csc:CHEMONTID_0004475
        a                skos:Concept ;
        rdfs:seeAlso     tax_nodes:C0004475 ;
        skos:broader     csc:CHEMONTID_0002837 ;
        skos:definition  "Hydrocarbons that contains one or more unsaturated carbon atoms. These compounds contain one or more double, triple, or aromatic bonds."@en ;
        skos:inScheme    vlcs:chemische_stof ;
        skos:notation    "CHEMONTID:0004475" ;
        skos:prefLabel   "Unsaturated hydrocarbons"@en .

csc:CHEMONTID_0000185
        a                skos:Concept ;
        rdfs:seeAlso     tax_nodes:C0000185 ;
        skos:altLabel    "aromatic amine"@en ;
        skos:broader     csc:CHEMONTID_0002279 ;
        skos:definition  "Compounds containing a phenylmethtylamine moiety, which consists of a phenyl group substituted by an methanamine."@en ;
        skos:inScheme    vlcs:chemische_stof ;
        skos:notation    "CHEMONTID:0000185" ;
        skos:prefLabel   "Phenylmethylamines"@en .

csc:CHEMONTID_0002019
        a                skos:Concept ;
        skos:altLabel    "ring assembly"@en , "pyrazoles"@en ;
        skos:broader     csc:CHEMONTID_0000087 ;
        skos:definition  "Compounds containing a phenylpyrazole skeleton, which consists of a pyrazole bound to a phenyl group."@en ;
        skos:inScheme    vlcs:chemische_stof ;
        skos:notation    "CHEMONTID:0002019" ;
        skos:prefLabel   "Phenylpyrazoles"@en .

csc:CHEMONTID_0002310
        a                skos:Concept ;
        skos:altLabel    "imidazoles"@en ;
        skos:broader     csc:CHEMONTID_0000078 ;
        skos:definition  "Heterocyclic compounds containing an imidazole ring substituted at one or more positions."@en ;
        skos:inScheme    vlcs:chemische_stof ;
        skos:notation    "CHEMONTID:0002310" ;
        skos:prefLabel   "Substituted imidazoles"@en .

csc:CHEMONTID_0000107
        a                skos:Concept ;
        rdfs:seeAlso     tax_nodes:C0000107 ;
        skos:altLabel    "oxazinane"@en ;
        skos:broader     csc:CHEMONTID_0000002 ;
        skos:definition  "Compounds containing an oxazinane moiety, which consists of a saturated aliphatic six-member ring with one oxygen atom, a nitrogen atom, and four carbon atoms. Isomers  of oxaphospholane include 1,2-oxazinane, 1,3-oxazinane, and 1,4-oxazinane."@en ;
        skos:inScheme    vlcs:chemische_stof ;
        skos:notation    "CHEMONTID:0000107" ;
        skos:prefLabel   "Oxazinanes"@en .

csc:CHEMONTID_0004443
        a                skos:Concept ;
        rdfs:seeAlso     tax_nodes:C0004443 ;
        skos:broader     csc:CHEMONTID_0004436 ;
        skos:definition  "Metal alkyls, where the alkyl group is attached to a transition metal atom."@en ;
        skos:inScheme    vlcs:chemische_stof ;
        skos:notation    "CHEMONTID:0004443" ;
        skos:prefLabel   "Transition metal alkyls"@en .

csc:CHEMONTID_0001381
        a                skos:Concept ;
        skos:altLabel    "dibenzodioxine"@en , "a dibenzo-p-dioxin"@en , "a dibenzodioxin"@en , "Dibenzodioxins"@en ;
        skos:broader     csc:CHEMONTID_0001379 ;
        skos:definition  "Compounds containing a dibenzo-p-dioxin moiety, which consists of two benzene connected by a para-dioxin ring."@en ;
        skos:inScheme    vlcs:chemische_stof ;
        skos:notation    "CHEMONTID:0001381" ;
        skos:prefLabel   "Dibenzo-p-dioxins"@en .

csc:CHEMONTID_0000153
        a                skos:Concept ;
        rdfs:seeAlso     tax_nodes:C0000153 ;
        skos:altLabel    "Naphthoquinones"@en ;
        skos:broader     csc:CHEMONTID_0000023 ;
        skos:definition  "Compounds containing a naphthohydroquinone moiety, which consists of a benzene ring linearly fused to a bezene-1,4-dione (quinone)."@en ;
        skos:inScheme    vlcs:chemische_stof ;
        skos:notation    "CHEMONTID:0000153" ;
        skos:prefLabel   "Naphthoquinones"@en .

csc:CHEMONTID_0003934
        a                skos:Concept ;
        rdfs:seeAlso     tax_nodes:C0003934 ;
        skos:altLabel    "organosulfur compound"@en ;
        skos:broader     csc:CHEMONTID_0000264 ;
        skos:definition  "Organosulfur compounds with the general formula SC(=S)N(R1)R2; R1-R2 =  H or organyl group."@en ;
        skos:inScheme    vlcs:chemische_stof ;
        skos:notation    "CHEMONTID:0003934" ;
        skos:prefLabel   "Dithiocarbamic acids and derivatives"@en .

csc:CHEMONTID_0001303
        a                skos:Concept ;
        rdfs:seeAlso     tax_nodes:C0001303 ;
        skos:altLabel    "organic thiophosphate"@en ;
        skos:broader     csc:CHEMONTID_0000264 ;
        skos:definition  "Organic compounds containing the thiophosphoric acid functional group or a derivative thereof, with the general structure RP(R')(R'')=S, where R,R',R'' = O,N, halogen residue."@en ;
        skos:inScheme    vlcs:chemische_stof ;
        skos:notation    "CHEMONTID:0001303" ;
        skos:prefLabel   "Organic thiophosphoric acids and derivatives"@en .

csc:CHEMONTID_0002286
        a                skos:Concept ;
        skos:altLabel    "polyol"@en ;
        skos:broader     csc:CHEMONTID_0000129 ;
        skos:definition  "Organic compounds containing more than one hydroxyl groups."@en ;
        skos:inScheme    vlcs:chemische_stof ;
        skos:notation    "CHEMONTID:0002286" ;
        skos:prefLabel   "Polyols"@en .

csc:CHEMONTID_0003980
        a                skos:Concept ;
        skos:altLabel    "benzyl chlorides"@en , "a benzyl chloride"@en , "Alpha chlorotoluenes"@en ;
        skos:broader     csc:CHEMONTID_0003981 ;
        skos:definition  "Organic compounds containing  a benzene skeleton substituted with a chloromethyl group."@en ;
        skos:inScheme    vlcs:chemische_stof ;
        skos:notation    "CHEMONTID:0003980" ;
        skos:prefLabel   "Benzyl chlorides"@en .

csc:CHEMONTID_0001524
        a                skos:Concept ;
        rdfs:seeAlso     tax_nodes:C0001524 ;
        skos:altLabel    "organotin compound"@en ;
        skos:broader     csc:CHEMONTID_0001523 ;
        skos:definition  "Compounds containing bond between a carbon atom and a tin atom."@en ;
        skos:inScheme    vlcs:chemische_stof ;
        skos:notation    "CHEMONTID:0001524" ;
        skos:prefLabel   "Organotin compounds"@en .

csc:CHEMONTID_0000549
        a                skos:Concept ;
        rdfs:seeAlso     tax_nodes:C0000549 ;
        skos:altLabel    "nitride"@en , "halogen molecular entity"@en ;
        skos:broader     csc:CHEMONTID_0000454 ;
        skos:definition  "Inorganic compounds of nitrogen where nitrogen has a formal oxidation state of -3, and the heaviest atom bonded to it is a halogen."@en ;
        skos:inScheme    vlcs:chemische_stof ;
        skos:notation    "CHEMONTID:0000549" ;
        skos:prefLabel   "Halogen nitrides"@en .

csc:CHEMONTID_0001279
        a                skos:Concept ;
        rdfs:seeAlso     tax_nodes:C0001279 ;
        skos:altLabel    "aliphatic sulfide"@en , "organohalogen compound"@en ;
        skos:broader     csc:CHEMONTID_0001202 ;
        skos:definition  "Compounds containing having two beta-haloalkyl groups bound to a sulfur atom."@en ;
        skos:inScheme    vlcs:chemische_stof ;
        skos:notation    "CHEMONTID:0001279" ;
        skos:prefLabel   "Sulfur mustard compounds"@en .

csc:CHEMONTID_0004632
        a                skos:Concept ;
        rdfs:seeAlso     tax_nodes:C0004632 ;
        skos:altLabel    "Sulfoxides"@en ;
        skos:broader     csc:CHEMONTID_0002279 ;
        skos:definition  "Organosulfur compounds containing a sulfoxide group substituted with a phenyl group."@en ;
        skos:inScheme    vlcs:chemische_stof ;
        skos:notation    "CHEMONTID:0004632" ;
        skos:prefLabel   "Phenyl sulfoxides"@en .

csc:CHEMONTID_0001026
        a                skos:Concept ;
        rdfs:seeAlso     tax_nodes:C0001026 ;
        skos:altLabel    "an alkyl chloride"@en , "chloroalkane"@en , "a chloroalkane"@en , "organochlorine compound"@en ;
        skos:broader     csc:CHEMONTID_0002867 ;
        skos:definition  "Organic compounds containing the alkyl chloride functional group with formula R-Cl , where R is an alkyl group."@en ;
        skos:inScheme    vlcs:chemische_stof ;
        skos:notation    "CHEMONTID:0001026" ;
        skos:prefLabel   "Alkyl chlorides"@en .

csc:CHEMONTID_0004387
        a                skos:Concept ;
        rdfs:seeAlso     tax_nodes:C0004387 ;
        skos:broader     csc:CHEMONTID_0000305 ;
        skos:definition  "Aromatic heterocyclic compounds containing a pyrazolo[3,4-d]pyrimidine ring system, which consists of a pyrazole ring fused to but and not sharing a nitrogen atom with a pyrimidine ring."@en ;
        skos:inScheme    vlcs:chemische_stof ;
        skos:notation    "CHEMONTID:0004387" ;
        skos:prefLabel   "Pyrazolo[3,4-d]pyrimidines"@en .

csc:CHEMONTID_0000517
        a                skos:Concept ;
        rdfs:seeAlso     tax_nodes:C0000517 ;
        skos:altLabel    "a carbamide"@en , "Carbamides"@en , "ureas"@en ;
        skos:broader     csc:CHEMONTID_0000364 ;
        skos:definition  "Compounds containing two amine groups joined by a carbonyl (C=O) functional group."@en ;
        skos:inScheme    vlcs:chemische_stof ;
        skos:notation    "CHEMONTID:0000517" ;
        skos:prefLabel   "Ureas"@en .

csc:CHEMONTID_0000097
        a                skos:Concept ;
        rdfs:seeAlso     tax_nodes:C0000097 ;
        skos:altLabel    "Thiophenes"@en ;
        skos:broader     csc:CHEMONTID_0000002 ;
        skos:definition  "Compounds containing a five-membered aromatic moiety made up of one sulfur atom and four carbon atoms."@en ;
        skos:inScheme    vlcs:chemische_stof ;
        skos:notation    "CHEMONTID:0000097" ;
        skos:prefLabel   "Thiophenes"@en .

csc:CHEMONTID_0004309
        a                skos:Concept ;
        skos:altLabel    "benzenesulfonate ester"@en ;
        skos:broader     csc:CHEMONTID_0000032 ;
        skos:definition  "Arenesulfonate esters that result from the formal condensation of the hydroxy group of an alcohol, enol, phenol or heteroarenol with benzenesulfonic acid."@en ;
        skos:inScheme    vlcs:chemische_stof ;
        skos:notation    "CHEMONTID:0004309" ;
        skos:prefLabel   "Benzenesulfonate esters"@en .

csc:CHEMONTID_0000019
        a                skos:Concept ;
        rdfs:seeAlso     tax_nodes:C0000019 ;
        skos:altLabel    "dibenzannulene"@en , "Dibenzocycloheptenes"@en ;
        skos:broader     csc:CHEMONTID_0002448 ;
        skos:definition  "Compounds containing a dibenzocycloheptene moiety, which consists of two benzene rings connected by a cycloheptene ring."@en ;
        skos:inScheme    vlcs:chemische_stof ;
        skos:notation    "CHEMONTID:0000019" ;
        skos:prefLabel   "Dibenzocycloheptenes"@en .

csc:CHEMONTID_0000310
        a                skos:Concept ;
        rdfs:seeAlso     tax_nodes:C0000310 ;
        skos:altLabel    "Phenothiazines"@en ;
        skos:broader     csc:CHEMONTID_0000309 ;
        skos:definition  "Polycyclic aromatic compounds containing a phenothiazine moiety, which is a linear tricyclic system that consists of a two benzene rings joined by a para-thiazine ring."@en ;
        skos:inScheme    vlcs:chemische_stof ;
        skos:notation    "CHEMONTID:0000310" ;
        skos:prefLabel   "Phenothiazines"@en .

csc:CHEMONTID_0003671
        a                skos:Concept ;
        skos:altLabel    "aromatic ketone"@en ;
        skos:broader     csc:CHEMONTID_0003670 ;
        skos:definition  "Ketones have the generic structure RC(=O)R', where R = aryl group and R'=alkyl group."@en ;
        skos:inScheme    vlcs:chemische_stof ;
        skos:notation    "CHEMONTID:0003671" ;
        skos:prefLabel   "Aryl alkyl ketones"@en .

csc:CHEMONTID_0001468
        a                skos:Concept ;
        skos:altLabel    "corticosteroid hormone"@en ;
        skos:broader     csc:CHEMONTID_0003569 ;
        skos:definition  "Steroids with a structure based on a hydroxylated prostane moiety."@en ;
        skos:inScheme    vlcs:chemische_stof ;
        skos:notation    "CHEMONTID:0001468" ;
        skos:prefLabel   "Gluco/mineralocorticoids, progestogins and derivatives"@en .

csc:CHEMONTID_0004576
        a                skos:Concept ;
        skos:broader     csc:CHEMONTID_0000487 ;
        skos:definition  "Salicylic acids or derivatives, that are O-acylated."@en ;
        skos:inScheme    vlcs:chemische_stof ;
        skos:notation    "CHEMONTID:0004576" ;
        skos:prefLabel   "Acylsalicylic acids and derivatives"@en .

csc:CHEMONTID_0004323
        a                skos:Concept ;
        skos:broader     csc:CHEMONTID_0000060 ;
        skos:definition  "Compounds containing glutamic acid or a derivative thereof resulting from reaction of glutamic acid at the amino group or the carboxy group, or from the replacement of any hydrogen of glycine by a heteroatom."@en ;
        skos:inScheme    vlcs:chemische_stof ;
        skos:notation    "CHEMONTID:0004323" ;
        skos:prefLabel   "Glutamic acid and derivatives"@en .

csc:CHEMONTID_0000286
        a                skos:Concept ;
        skos:altLabel    "primary alcohol"@en ;
        skos:broader     csc:CHEMONTID_0000129 ;
        skos:definition  "Compounds comprising the primary alcohol functional group, with the general structure RCOH (R=alkyl, aryl)."@en ;
        skos:inScheme    vlcs:chemische_stof ;
        skos:notation    "CHEMONTID:0000286" ;
        skos:prefLabel   "Primary alcohols"@en .

csc:CHEMONTID_0000033
        a                skos:Concept ;
        rdfs:seeAlso     tax_nodes:C0000033 ;
        skos:altLabel    "benzyl alcohols"@en , "Benzyl Alcohols"@en ;
        skos:broader     csc:CHEMONTID_0002279 ;
        skos:definition  "Organic compounds containing the phenylmethanol substructure."@en ;
        skos:inScheme    vlcs:chemische_stof ;
        skos:notation    "CHEMONTID:0000033" ;
        skos:prefLabel   "Benzyl alcohols"@en .

csc:CHEMONTID_0002411
        a                skos:Concept ;
        skos:altLabel    "carboxylic acid"@en , "piperidines"@en ;
        skos:broader     csc:CHEMONTID_0001974 ;
        skos:definition  "Compounds containing a piperidine ring which bears a carboxylic acid group."@en ;
        skos:inScheme    vlcs:chemische_stof ;
        skos:notation    "CHEMONTID:0002411" ;
        skos:prefLabel   "Piperidinecarboxylic acids"@en .

csc:CHEMONTID_0002839
        a                skos:Concept ;
        skos:altLabel    "acyclic olefin"@en ;
        skos:broader     csc:CHEMONTID_0002838 ;
        skos:definition  "Olefins that do not contain a ring in their structure."@en ;
        skos:inScheme    vlcs:chemische_stof ;
        skos:notation    "CHEMONTID:0002839" ;
        skos:prefLabel   "Acyclic olefins"@en .

csc:CHEMONTID_0000208
        a                skos:Concept ;
        skos:altLabel    "pyridazinone"@en ;
        skos:broader     csc:CHEMONTID_0000074 ;
        skos:definition  "Compounds containing a pyridazine ring which bears a ketone."@en ;
        skos:inScheme    vlcs:chemische_stof ;
        skos:notation    "CHEMONTID:0000208" ;
        skos:prefLabel   "Pyridazinones"@en .

csc:CHEMONTID_0003569
        a                skos:Concept ;
        rdfs:seeAlso     tax_nodes:C0003569 ;
        skos:altLabel    "A C(21) steroid"@en , "C21 steroids (gluco/mineralocorticoids, progestogins) and derivatives"@en , "steroid"@en , "Pregnanes"@en ;
        skos:broader     csc:CHEMONTID_0000258 ;
        skos:definition  "Steroids with a structure based on the 21-carbon pregnane skeleton."@en ;
        skos:inScheme    vlcs:chemische_stof ;
        skos:notation    "CHEMONTID:0003569" ;
        skos:prefLabel   "Pregnane steroids"@en .

csc:CHEMONTID_0000254
        a                skos:Concept ;
        rdfs:seeAlso     tax_nodes:C0000254 ;
        skos:altLabel    "Ethers"@en , "ether"@en , "ethers"@en , "an ether"@en ;
        skos:broader     csc:CHEMONTID_0000323 ;
        skos:definition  "Compounds bearing an ether group with the formula Compounds ROR (R not H)."@en ;
        skos:inScheme    vlcs:chemische_stof ;
        skos:notation    "CHEMONTID:0000254" ;
        skos:prefLabel   "Ethers"@en .

csc:CHEMONTID_0001657
        a                skos:Concept ;
        skos:altLabel    "dicarboximide"@en ;
        skos:broader     csc:CHEMONTID_0001093 ;
        skos:definition  "Carboxylic acid derivatives containing two carbonyl groups where the carbon atoms are both linked to the same nitrogen atom."@en ;
        skos:inScheme    vlcs:chemische_stof ;
        skos:notation    "CHEMONTID:0001657" ;
        skos:prefLabel   "Carboxylic acid imides"@en .

csc:CHEMONTID_0000001
        a                  skos:Concept ;
        rdfs:seeAlso       tax_nodes:C0000001 ;
        skos:altLabel      "inorganic molecular entity"@en ;
        skos:definition    "Compounds that do not contain a C atom. Exceptions are made for isocyanide/cyanide and their non-hydrocarbyl derivatives, thiophosgene, carbon diselenide, carbon monosulfide, carbon disulfide, carbon subsulfide, carbon monoxide, carbon trioxide, carbon suboxide, and dicarbon monoxide."@en , "Compounds that do not contain a C atom."@en ;
        skos:inScheme      vlcs:chemische_stof ;
        skos:notation      "CHEMONTID:0000001" ;
        skos:prefLabel     "Inorganic compounds"@en ;
        skos:topConceptOf  vlcs:chemische_stof .

csc:CHEMONTID_0000429
        a                skos:Concept ;
        rdfs:seeAlso     tax_nodes:C0000429 ;
        skos:broader     csc:CHEMONTID_0000422 ;
        skos:definition  "Inorganic compounds containing only metal atoms, with the largest atom being a lanthanide atom."@en ;
        skos:inScheme    vlcs:chemische_stof ;
        skos:notation    "CHEMONTID:0000429" ;
        skos:prefLabel   "Homogeneous lanthanide compounds"@en .

csc:CHEMONTID_0000475
        a                skos:Concept ;
        skos:altLabel    "amide"@en ;
        skos:broader     csc:CHEMONTID_0001093 ;
        skos:definition  "Carboxylic acid derivatives containing a carbonyl group in which the carbon atom is linked to a nitrogen atom (substituted or not). The general formula of the carboxylic acid amide is R1C(=O)N(R2)R3 (R1,R2,R3=H, alkyl, aryl)."@en ;
        skos:inScheme    vlcs:chemische_stof ;
        skos:notation    "CHEMONTID:0000475" ;
        skos:prefLabel   "Carboxylic acid amides"@en .

csc:CHEMONTID_0002309
        a                skos:Concept ;
        skos:altLabel    "amino acid amide"@en ;
        skos:broader     csc:CHEMONTID_0000060 ;
        skos:definition  "Amide derivatives of alpha amino acids."@en ;
        skos:inScheme    vlcs:chemische_stof ;
        skos:notation    "CHEMONTID:0002309" ;
        skos:prefLabel   "Alpha amino acid amides"@en .

csc:CHEMONTID_0002180
        a                skos:Concept ;
        rdfs:seeAlso     tax_nodes:C0002180 ;
        skos:altLabel    "nucleobase-containing molecular entity"@en ;
        skos:broader     csc:CHEMONTID_0000480 ;
        skos:definition  "Compounds consisting of a pyrimidine linked to a ribose which lacks a hydroxyl group at position 2."@en ;
        skos:inScheme    vlcs:chemische_stof ;
        skos:notation    "CHEMONTID:0002180" ;
        skos:prefLabel   "Pyrimidine 2'-deoxyribonucleosides"@en .

csc:CHEMONTID_0001127
        a                skos:Concept ;
        skos:altLabel    "Acyclic monoterpenoids"@en , "Linear monoterpenes"@en , "monoterpenoid"@en ;
        skos:broader     csc:CHEMONTID_0001549 ;
        skos:definition  "Monoterpenes that do not contain a cycle."@en ;
        skos:inScheme    vlcs:chemische_stof ;
        skos:notation    "CHEMONTID:0001127" ;
        skos:prefLabel   "Acyclic monoterpenoids"@en .

csc:CHEMONTID_0001846
        a                skos:Concept ;
        skos:broader     csc:CHEMONTID_0000285 ;
        skos:definition  "Organic compounds containing an acetamide group conjugated to a phenyl group."@en ;
        skos:inScheme    vlcs:chemische_stof ;
        skos:notation    "CHEMONTID:0001846" ;
        skos:prefLabel   "Acetanilides"@en .

csc:CHEMONTID_0000198
        a                skos:Concept ;
        skos:altLabel    "oligosaccharide"@en ;
        skos:broader     csc:CHEMONTID_0000011 ;
        skos:definition  "Carbohydrates made up of 3 to 10 monosaccharide units linked to each other through glycosidic bonds."@en ;
        skos:inScheme    vlcs:chemische_stof ;
        skos:notation    "CHEMONTID:0000198" ;
        skos:prefLabel   "Oligosaccharides"@en .

csc:CHEMONTID_0003979
        a                skos:Concept ;
        skos:altLabel    "benzyl bromides"@en , "Alpha bromotoluenes"@en , "a benzyl bromide"@en ;
        skos:broader     csc:CHEMONTID_0003981 ;
        skos:definition  "Organic compounds containing  a benzene skeleton substituted with a bromomethyl group."@en ;
        skos:inScheme    vlcs:chemische_stof ;
        skos:notation    "CHEMONTID:0003979" ;
        skos:prefLabel   "Benzyl bromides"@en .

csc:CHEMONTID_0002323
        a                skos:Concept ;
        rdfs:seeAlso     tax_nodes:C0002323 ;
        skos:altLabel    "benzothiadiazole"@en ;
        skos:broader     csc:CHEMONTID_0000002 ;
        skos:definition  "Heterocyclic aromatic compounds containing a benzene ring fused to a thiadiazole ring. Thiadiazole is a five-membered aromatic heterocycle made up of one sulfur atom and two nitrogen atoms."@en ;
        skos:inScheme    vlcs:chemische_stof ;
        skos:notation    "CHEMONTID:0002323" ;
        skos:prefLabel   "Benzothiadiazoles"@en .

csc:CHEMONTID_0004701
        a                skos:Concept ;
        skos:broader     csc:CHEMONTID_0001350 ;
        skos:definition  "Benzoic acid esters where the benzene ring is para-substituted with a hydroxy group."@en ;
        skos:inScheme    vlcs:chemische_stof ;
        skos:notation    "CHEMONTID:0004701" ;
        skos:prefLabel   "p-Hydroxybenzoic acid esters"@en .

csc:CHEMONTID_0001814
        a                skos:Concept ;
        rdfs:seeAlso     tax_nodes:C0001814 ;
        skos:altLabel    "phosphine"@en ;
        skos:broader     csc:CHEMONTID_0002279 ;
        skos:definition  "Compounds containing a phenylphosphine, which consists of phosphine substituent bound to a phenyl group."@en ;
        skos:inScheme    vlcs:chemische_stof ;
        skos:notation    "CHEMONTID:0001814" ;
        skos:prefLabel   "Phenylphosphines and derivatives"@en .

csc:CHEMONTID_0000411
        a                skos:Concept ;
        rdfs:seeAlso     tax_nodes:C0000411 ;
        skos:altLabel    "oxime"@en , "Oximes"@en ;
        skos:broader     csc:CHEMONTID_0000278 ;
        skos:definition  "Compounds containing the oxime functional group, with the general structure R1(R2)C=NOH."@en ;
        skos:inScheme    vlcs:chemische_stof ;
        skos:notation    "CHEMONTID:0000411" ;
        skos:prefLabel   "Oximes"@en .

csc:CHEMONTID_0003053
        a                skos:Concept ;
        skos:altLabel    "aza-steroid"@en ;
        skos:broader     csc:CHEMONTID_0002340 ;
        skos:definition  "Azasteroids where the carbon atom at position 25 is replaced by a nitrogen atom."@en ;
        skos:inScheme    vlcs:chemische_stof ;
        skos:notation    "CHEMONTID:0003053" ;
        skos:prefLabel   "25-azasteroids and derivatives"@en .

csc:CHEMONTID_0004456
        a                skos:Concept ;
        rdfs:seeAlso     tax_nodes:C0004456 ;
        skos:altLabel    "organic molecular entity"@en ;
        skos:broader     csc:CHEMONTID_0000463 ;
        skos:definition  "Organic compounds containing the selenite oxoanion, with the formula  [SO3]2-, or its conjugated base."@en ;
        skos:inScheme    vlcs:chemische_stof ;
        skos:notation    "CHEMONTID:0004456" ;
        skos:prefLabel   "Organic sulfites"@en .

csc:CHEMONTID_0004203
        a                skos:Concept ;
        rdfs:seeAlso     tax_nodes:C0004203 ;
        skos:broader     csc:CHEMONTID_0002279 ;
        skos:definition  "Aromatic compounds containing a methyl-3-methoxyacrylate moiety that carries a benzyl group at the C-alpha carbon."@en ;
        skos:inScheme    vlcs:chemische_stof ;
        skos:notation    "CHEMONTID:0004203" ;
        skos:prefLabel   "Phenyl-beta-methoxyacrylates"@en .

csc:CHEMONTID_0004677
        a                skos:Concept ;
        rdfs:seeAlso     tax_nodes:C0004677 ;
        skos:broader     csc:CHEMONTID_0002279 ;
        skos:definition  "Aromatic compounds hat contain a phenol ether attached to the C2-atom of a phenylpropionic acid ester."@en ;
        skos:inScheme    vlcs:chemische_stof ;
        skos:notation    "CHEMONTID:0004677" ;
        skos:prefLabel   "2-phenoxypropionic acid esters"@en .

csc:CHEMONTID_0003449
        a                skos:Concept ;
        rdfs:seeAlso     tax_nodes:C0003449 ;
        skos:altLabel    "N-alkylpyrrolidine"@en ;
        skos:broader     csc:CHEMONTID_0000218 ;
        skos:definition  "Compounds containing a pyrrolidine moiety that is substituted at the N1-position with an alkyl group. Pyrrolidine is a five-membered saturated aliphatic heterocycle with one nitrogen atom and four carbon atoms."@en ;
        skos:inScheme    vlcs:chemische_stof ;
        skos:notation    "CHEMONTID:0003449" ;
        skos:prefLabel   "N-alkylpyrrolidines"@en .

csc:CHEMONTID_0000134
        a                skos:Concept ;
        rdfs:seeAlso     tax_nodes:C0000134 ;
        skos:altLabel    "phenols"@en , "a phenol"@en , "Phenols"@en ;
        skos:broader     csc:CHEMONTID_0002448 ;
        skos:definition  "Compounds containing a phenol moiety, which is a benzene bearing a hydroxyl group."@en ;
        skos:inScheme    vlcs:chemische_stof ;
        skos:notation    "CHEMONTID:0000134" ;
        skos:prefLabel   "Phenols"@en .

csc:CHEMONTID_0000309
        a                skos:Concept ;
        rdfs:seeAlso     tax_nodes:C0000309 ;
        skos:altLabel    "benzothiazine"@en ;
        skos:broader     csc:CHEMONTID_0000002 ;
        skos:definition  "Organic compounds containing a benzene fused to a thiazine ring (a six-membered ring with four carbon atoms, one nitrogen atom and one sulfur atom)."@en ;
        skos:inScheme    vlcs:chemische_stof ;
        skos:notation    "CHEMONTID:0000309" ;
        skos:prefLabel   "Benzothiazines"@en .

csc:CHEMONTID_0003961
        a                skos:Concept ;
        skos:altLabel    "organofluorine compound"@en , "organophosphorus compound"@en , "PFASs"@en ;
        skos:broader     csc:CHEMONTID_0001027 ;
        skos:definition  "Organic compounds containing an alkyl chain attached to the sulfur of a sulfonic acid group (or a derivative thereof), where all hydrogens of the alkyl chain are replaced by fluorine atoms."@en ;
        skos:inScheme    vlcs:chemische_stof ;
        skos:notation    "CHEMONTID:0003961" ;
        skos:prefLabel   "Perfluoroalkyl sulfonic acid and derivatives"@en .

csc:CHEMONTID_0003417
        a                skos:Concept ;
        skos:altLabel    "fatty acid methyl ester"@en ;
        skos:broader     csc:CHEMONTID_0000324 ;
        skos:definition  "Compounds containing a fatty acid that is esterified with a methyl group. They have the general structure RC(=O)OR', where R=fatty aliphatic tail or organyl group and R'=methyl group."@en ;
        skos:inScheme    vlcs:chemische_stof ;
        skos:notation    "CHEMONTID:0003417" ;
        skos:prefLabel   "Fatty acid methyl esters"@en .

csc:CHEMONTID_0000355
        a                skos:Concept ;
        rdfs:seeAlso     tax_nodes:C0000355 ;
        skos:altLabel    "alkylbenzene"@en ;
        skos:broader     csc:CHEMONTID_0002279 ;
        skos:definition  "Aromatic compounds containing a prop-2-ylbenzene moiety."@en ;
        skos:inScheme    vlcs:chemische_stof ;
        skos:notation    "CHEMONTID:0000355" ;
        skos:prefLabel   "Cumenes"@en .

csc:CHEMONTID_0004147
        a                skos:Concept ;
        skos:broader     csc:CHEMONTID_0000074 ;
        skos:definition  "Organic compounds containing a pyridazine ring substituted by a phenyl group."@en ;
        skos:inScheme    vlcs:chemische_stof ;
        skos:notation    "CHEMONTID:0004147" ;
        skos:prefLabel   "Phenylpyridazines"@en .

csc:CHEMONTID_0001551
        a                skos:Concept ;
        rdfs:seeAlso     tax_nodes:C0001551 ;
        skos:altLabel    "diterpenoid"@en , "C20 isoprenoids (diterpenes)"@en ;
        skos:broader     csc:CHEMONTID_0000259 ;
        skos:definition  "Terpene compounds formed by four isoprene units."@en ;
        skos:inScheme    vlcs:chemische_stof ;
        skos:notation    "CHEMONTID:0001551" ;
        skos:prefLabel   "Diterpenoids"@en .

csc:CHEMONTID_0000323
        a                skos:Concept ;
        rdfs:seeAlso     tax_nodes:C0000323 ;
        skos:altLabel    "organooxygen compound"@en ;
        skos:broader     csc:CHEMONTID_0004603 ;
        skos:definition  "Organic compounds containing a bond between a carbon atom and an oxygen atom."@en ;
        skos:inScheme    vlcs:chemische_stof ;
        skos:notation    "CHEMONTID:0000323" ;
        skos:prefLabel   "Organooxygen compounds"@en .

csc:CHEMONTID_0000078
        a                skos:Concept ;
        rdfs:seeAlso     tax_nodes:C0000078 ;
        skos:altLabel    "Imidazoles"@en , "an imidazole"@en ;
        skos:broader     csc:CHEMONTID_0000436 ;
        skos:definition  "Compounds containing an imidazole ring, which is an aromatic five-member ring with two nitrogen atoms at positions 1 and 3, and three carbon atoms."@en ;
        skos:inScheme    vlcs:chemische_stof ;
        skos:notation    "CHEMONTID:0000078" ;
        skos:prefLabel   "Imidazoles"@en .

csc:CHEMONTID_0004161
        a                skos:Concept ;
        skos:altLabel    "hydroxypyrimidine"@en ;
        skos:broader     csc:CHEMONTID_0000075 ;
        skos:definition  "Organic compounds containing a hydroxyl group attached to a pyrimidine ring. Pyrimidine is a 6-membered ring consisting of four carbon atoms and two nitrogen centers at the 1- and 3- ring positions."@en ;
        skos:inScheme    vlcs:chemische_stof ;
        skos:notation    "CHEMONTID:0004161" ;
        skos:prefLabel   "Hydroxypyrimidines"@en .

csc:CHEMONTID_0000299
        a                skos:Concept ;
        rdfs:seeAlso     tax_nodes:C0000299 ;
        skos:broader     csc:CHEMONTID_0000472 ;
        skos:definition  "Hydroxy acids with a 6 to 12 carbon atoms long side chain."@en ;
        skos:inScheme    vlcs:chemische_stof ;
        skos:notation    "CHEMONTID:0000299" ;
        skos:prefLabel   "Medium-chain hydroxy acids and derivatives"@en .

csc:CHEMONTID_0001274
        a                skos:Concept ;
        skos:altLabel    "a 1,2-cresol"@en , "a o-cresol"@en , "hydroxytoluene"@en , "o-Cresols"@en , "1,2-Cresols"@en ;
        skos:broader     csc:CHEMONTID_0001272 ;
        skos:definition  "Organic compounds containing an ortho-cresol moiety, which consists of a benzene bearing one hydroxyl group at ring positions 1 and 2, respectively."@en ;
        skos:inScheme    vlcs:chemische_stof ;
        skos:notation    "CHEMONTID:0001274" ;
        skos:prefLabel   "Ortho cresols"@en .

csc:CHEMONTID_0000512
        a                skos:Concept ;
        skos:altLabel    "lipid"@en , "Jasmonic acids"@en ;
        skos:broader     csc:CHEMONTID_0000504 ;
        skos:definition  "Lipids containing or derived from a jasmonic acid, with a structure characterized by the presence of an alkene chain linked to a 2-(3-oxocyclopentyl)acetic acid moiety."@en ;
        skos:inScheme    vlcs:chemische_stof ;
        skos:notation    "CHEMONTID:0000512" ;
        skos:prefLabel   "Jasmonic acids"@en .

csc:CHEMONTID_0000267
        a                skos:Concept ;
        rdfs:seeAlso     tax_nodes:C0000267 ;
        skos:altLabel    "organohalogen compound"@en ;
        skos:broader     csc:CHEMONTID_0000000 ;
        skos:definition  "Organic compounds containing a bond between a carbon atom and a halogen atom (At, F, Cl, Br, I)."@en ;
        skos:inScheme    vlcs:chemische_stof ;
        skos:notation    "CHEMONTID:0000267" ;
        skos:prefLabel   "Organohalogen compounds"@en .

csc:CHEMONTID_0000014
        a                skos:Concept ;
        rdfs:seeAlso     tax_nodes:C0000014 ;
        skos:broader     csc:CHEMONTID_0002279 ;
        skos:definition  "Compounds containing a phenylbutylamine moiety, which consists of a phenyl group substituted at the fourth carbon by an butan-1-amine."@en ;
        skos:inScheme    vlcs:chemische_stof ;
        skos:notation    "CHEMONTID:0000014" ;
        skos:prefLabel   "Phenylbutylamines"@en .

csc:CHEMONTID_0001961
        a                skos:Concept ;
        rdfs:seeAlso     tax_nodes:C0001961 ;
        skos:altLabel    "depsipeptide"@en ;
        skos:broader     csc:CHEMONTID_0001813 ;
        skos:definition  "Natural or synthetic compounds having sequences of amino and hydroxy carboxylic acid residues (usually α-amino and α-hydroxy acids), commonly but not necessarily regularly alternating."@en ;
        skos:inScheme    vlcs:chemische_stof ;
        skos:notation    "CHEMONTID:0001961" ;
        skos:prefLabel   "Depsipeptides"@en .

csc:CHEMONTID_0000060
        a                skos:Concept ;
        skos:broader     csc:CHEMONTID_0000347 ;
        skos:definition  "Amino acids in which the amino group is attached to the carbon atom immediately adjacent to the carboxylate group (alpha carbon), or a derivative thereof."@en ;
        skos:inScheme    vlcs:chemische_stof ;
        skos:notation    "CHEMONTID:0000060" ;
        skos:prefLabel   "Alpha amino acids and derivatives"@en .

csc:CHEMONTID_0004525
        a                skos:Concept ;
        skos:broader     csc:CHEMONTID_0000417 ;
        skos:definition  "Compounds containing a phenoxyacetate that carries one or more chlorine atoms on the benzene ring."@en ;
        skos:inScheme    vlcs:chemische_stof ;
        skos:notation    "CHEMONTID:0004525" ;
        skos:prefLabel   "Chlorophenoxyacetates"@en .

csc:CHEMONTID_0002866
        a                skos:Concept ;
        rdfs:seeAlso     tax_nodes:C0002866 ;
        skos:altLabel    "haloarene"@en ;
        skos:broader     csc:CHEMONTID_0000267 ;
        skos:definition  "Organic compounds containing an aromatic ring (or ring system) carrying a C-X bond."@en ;
        skos:inScheme    vlcs:chemische_stof ;
        skos:notation    "CHEMONTID:0002866" ;
        skos:prefLabel   "Aryl halides"@en .

csc:CHEMONTID_0000281
        a                skos:Concept ;
        skos:broader     csc:CHEMONTID_0000176 ;
        skos:definition  "Benzoic acids (or derivative thereof) containing an amine group attached to the benzene moiety."@en ;
        skos:inScheme    vlcs:chemische_stof ;
        skos:notation    "CHEMONTID:0000281" ;
        skos:prefLabel   "Aminobenzoic acids and derivatives"@en .

csc:CHEMONTID_0003098
        a                skos:Concept ;
        skos:altLabel    "carbonyl compound"@en , "organohalogen compound"@en ;
        skos:broader     csc:CHEMONTID_0003096 ;
        skos:definition  "Benzoic acids or derivatives carrying a halogen atom at the 2-position of the benzene ring."@en ;
        skos:inScheme    vlcs:chemische_stof ;
        skos:notation    "CHEMONTID:0003098" ;
        skos:prefLabel   "2-halobenzoic acids and derivatives"@en .

csc:CHEMONTID_0000456
        a                skos:Concept ;
        rdfs:seeAlso     tax_nodes:C0000456 ;
        skos:altLabel    "alkali metal molecular entity"@en ;
        skos:broader     csc:CHEMONTID_0000424 ;
        skos:definition  "Inorganic compounds belonging either to the alkali metal hydrides, the alkali metal nitrides, the alkali metal oxides, or the alkali metal sulfides."@en ;
        skos:inScheme    vlcs:chemische_stof ;
        skos:notation    "CHEMONTID:0000456" ;
        skos:prefLabel   "Alkali metal organides"@en .

csc:CHEMONTID_0001859
        a                skos:Concept ;
        rdfs:seeAlso     tax_nodes:C0001859 ;
        skos:altLabel    "pyridopyrimidine"@en ;
        skos:broader     csc:CHEMONTID_0000002 ;
        skos:definition  "Compounds containing a pyridopyrimidine, which consists of a pyridine fused to a pyrimidine. Pyridine is 6-membered ring consisting of five carbon atoms and a nitrogen atom. Pyrimidine is a 6-membered ring consisting of four carbon atoms and two nitrogen centers at the 1- and 3- ring positions."@en ;
        skos:inScheme    vlcs:chemische_stof ;
        skos:notation    "CHEMONTID:0001859" ;
        skos:prefLabel   "Pyridopyrimidines"@en .

csc:CHEMONTID_0002336
        a                skos:Concept ;
        rdfs:seeAlso     tax_nodes:C0002336 ;
        skos:altLabel    "pyrrolidines"@en , "a phenylpyrrolidine"@en ;
        skos:broader     csc:CHEMONTID_0000218 ;
        skos:definition  "Polycyclic aromatic compounds containing a benzene ring linked to a pyrrolidine ring through a CC or CN bond. Pyrrolidine is a five-membered saturated aliphatic heterocycle with one nitrogen atom and four carbon atoms."@en ;
        skos:inScheme    vlcs:chemische_stof ;
        skos:notation    "CHEMONTID:0002336" ;
        skos:prefLabel   "Phenylpyrrolidines"@en .

csc:CHEMONTID_0004714
        a                skos:Concept ;
        rdfs:seeAlso     tax_nodes:C0004714 ;
        skos:altLabel    "Carbanilates"@en ;
        skos:broader     csc:CHEMONTID_0002279 ;
        skos:definition  "Ester derivatives of phenylcarbamic acids."@en ;
        skos:inScheme    vlcs:chemische_stof ;
        skos:notation    "CHEMONTID:0004714" ;
        skos:prefLabel   "Phenylcarbamic acid esters"@en .

csc:CHEMONTID_0001108
        a                skos:Concept ;
        skos:altLabel    "benzenedicarboxylic acid"@en ;
        skos:broader     csc:CHEMONTID_0001105 ;
        skos:definition  "Compounds containing a benzene ring bearing a carboxylic acid group at ring carbon atoms 1 and 4."@en ;
        skos:inScheme    vlcs:chemische_stof ;
        skos:notation    "CHEMONTID:0001108" ;
        skos:prefLabel   "P-phthalic acid and derivatives"@en .

csc:CHEMONTID_0000424
        a                skos:Concept ;
        rdfs:seeAlso     tax_nodes:C0000424 ;
        skos:broader     csc:CHEMONTID_0000001 ;
        skos:definition  "Compounds that contains both metal and non metal atoms."@en ;
        skos:inScheme    vlcs:chemische_stof ;
        skos:notation    "CHEMONTID:0000424" ;
        skos:prefLabel   "Mixed metal/non-metal compounds"@en .

csc:CHEMONTID_0000147
        a                skos:Concept ;
        rdfs:seeAlso     tax_nodes:C0000147 ;
        skos:altLabel    "macrolides"@en , "macrolide"@en ;
        skos:broader     csc:CHEMONTID_0000261 ;
        skos:definition  "Organic compounds containing a lactone ring of at least twelve members."@en ;
        skos:inScheme    vlcs:chemische_stof ;
        skos:notation    "CHEMONTID:0000147" ;
        skos:prefLabel   "Macrolides and analogues"@en .

csc:CHEMONTID_0001122
        a                skos:Concept ;
        skos:altLabel    "barbiturates"@en ;
        skos:broader     csc:CHEMONTID_0000291 ;
        skos:definition  "Organic compounds containing a 2-thioxodihydropyrimidine-4,6(1H,5H)-dione skeleton."@en ;
        skos:inScheme    vlcs:chemische_stof ;
        skos:notation    "CHEMONTID:0001122" ;
        skos:prefLabel   "Thiobarbituric acid derivatives"@en .

csc:CHEMONTID_0003080
        a                skos:Concept ;
        skos:altLabel    "1,3,5-triazines"@en ;
        skos:broader     csc:CHEMONTID_0001693 ;
        skos:definition  "N-aliphatic amine derivatives of 1,3,5-triazines. 1,3,5-triazines are aromatic compounds having three nitrogen ring atoms at the 1-, 3-, and 5- positions."@en ;
        skos:inScheme    vlcs:chemische_stof ;
        skos:notation    "CHEMONTID:0003080" ;
        skos:prefLabel   "N-aliphatic s-triazines"@en .

csc:CHEMONTID_0000368
        a                skos:Concept ;
        rdfs:seeAlso     tax_nodes:C0000368 ;
        skos:altLabel    "dioxanes"@en ;
        skos:broader     csc:CHEMONTID_0000002 ;
        skos:definition  "Compounds containing a dioxane ring, which is a six-membered saturated ring of two oxygen atoms and four carbon atoms. The dioxanes are divided in 1,2-dioxanes, 1,3-dioxanes, and 1,4-dioxanes."@en ;
        skos:inScheme    vlcs:chemische_stof ;
        skos:notation    "CHEMONTID:0000368" ;
        skos:prefLabel   "Dioxanes"@en .

csc:CHEMONTID_0002746
        a                skos:Concept ;
        skos:altLabel    "ergoline alkaloid"@en ;
        skos:broader     csc:CHEMONTID_0002680 ;
        skos:definition  "Amides of Lysergic acids."@en ;
        skos:inScheme    vlcs:chemische_stof ;
        skos:notation    "CHEMONTID:0002746" ;
        skos:prefLabel   "Lysergamides"@en .

csc:CHEMONTID_0001518
        a                skos:Concept ;
        rdfs:seeAlso     tax_nodes:C0001518 ;
        skos:altLabel    "an organoiodide"@en , "organoiodine compound"@en ;
        skos:broader     csc:CHEMONTID_0000267 ;
        skos:definition  "Compounds containing a chemical bond between a carbon atom and an iodine atom."@en ;
        skos:inScheme    vlcs:chemische_stof ;
        skos:notation    "CHEMONTID:0001518" ;
        skos:prefLabel   "Organoiodides"@en .

csc:CHEMONTID_0001098
        a                skos:Concept ;
        skos:altLabel    "organobromine compound"@en ;
        skos:broader     csc:CHEMONTID_0000035 ;
        skos:definition  "Organic compounds containing a bromine atom attached to a benzene ring."@en ;
        skos:inScheme    vlcs:chemische_stof ;
        skos:notation    "CHEMONTID:0001098" ;
        skos:prefLabel   "Bromobenzenes"@en .

csc:CHEMONTID_0004451
        a                skos:Concept ;
        skos:broader     csc:CHEMONTID_0004450 ;
        skos:definition  "Organic compounds containing acrylic acid CH2=CHCO2H."@en ;
        skos:inScheme    vlcs:chemische_stof ;
        skos:notation    "CHEMONTID:0004451" ;
        skos:prefLabel   "Acrylic acids"@en .

csc:CHEMONTID_0001564
        a                skos:Concept ;
        skos:altLabel    "monoterpenoid"@en ;
        skos:broader     csc:CHEMONTID_0001549 ;
        skos:definition  "Monoterpenoids containing exactly 2 rings, which are fused to each other."@en ;
        skos:inScheme    vlcs:chemische_stof ;
        skos:notation    "CHEMONTID:0001564" ;
        skos:prefLabel   "Bicyclic monoterpenoids"@en .

csc:CHEMONTID_0004640
        a                skos:Concept ;
        rdfs:seeAlso     tax_nodes:C0004640 ;
        skos:broader     csc:CHEMONTID_0002279 ;
        skos:definition  "Aromatic compounds containing a methylcarbamic acid esterified with a phenyl group."@en ;
        skos:inScheme    vlcs:chemische_stof ;
        skos:notation    "CHEMONTID:0004640" ;
        skos:prefLabel   "Phenyl methylcarbamates"@en .

csc:CHEMONTID_0003412
        a                skos:Concept ;
        rdfs:seeAlso     tax_nodes:C0003412 ;
        skos:altLabel    "thiochromane"@en ;
        skos:broader     csc:CHEMONTID_0000002 ;
        skos:definition  "Organic heterocyclic compounds containing a benzene ring fused to a pyran ring. Pyran a six-membered heterocyclic, non-aromatic ring, made up of five carbon atoms and one oxygen atom and containing two double bonds."@en ;
        skos:inScheme    vlcs:chemische_stof ;
        skos:notation    "CHEMONTID:0003412" ;
        skos:prefLabel   "Benzothiopyrans"@en .

csc:CHEMONTID_0001753
        a                skos:Concept ;
        rdfs:seeAlso     tax_nodes:C0001753 ;
        skos:altLabel    "N-acylindole"@en ;
        skos:broader     csc:CHEMONTID_0000211 ;
        skos:definition  "Organic compounds containing an indole attached to a benzoyl moiety through the acyl group."@en ;
        skos:inScheme    vlcs:chemische_stof ;
        skos:notation    "CHEMONTID:0001753" ;
        skos:prefLabel   "Benzoylindoles"@en .

csc:CHEMONTID_0001209
        a                skos:Concept ;
        rdfs:seeAlso     tax_nodes:C0001209 ;
        skos:altLabel    "thioureas"@en ;
        skos:broader     csc:CHEMONTID_0000004 ;
        skos:definition  "Organic compounds containing the thiourea functional group, a derivative of urea with the general structure (R1(N)R2C(=S)(R3)R4, R1-R4=H, alkyl, aryl), obtained by replacing the carbonyl group of urea with a thiocarbonyl group."@en ;
        skos:inScheme    vlcs:chemische_stof ;
        skos:notation    "CHEMONTID:0001209" ;
        skos:prefLabel   "Thioureas"@en .

csc:CHEMONTID_0000525
        a                skos:Concept ;
        rdfs:seeAlso     tax_nodes:C0000525 ;
        skos:altLabel    "nitride"@en , "alkali metal salt"@en ;
        skos:broader     csc:CHEMONTID_0000456 ;
        skos:definition  "Inorganic compounds of nitrogen where nitrogen has a formal oxidation state of -3, and the heaviest metal atom is an alkali metal."@en ;
        skos:inScheme    vlcs:chemische_stof ;
        skos:notation    "CHEMONTID:0000525" ;
        skos:prefLabel   "Alkali metal nitrides"@en .

csc:CHEMONTID_0003886
        a                skos:Concept ;
        rdfs:seeAlso     tax_nodes:C0003886 ;
        skos:altLabel    "dicarboximide"@en , "heterocyclic compound"@en ;
        skos:broader     csc:CHEMONTID_0000002 ;
        skos:definition  "Cyclic organooxygen compounds containing the structure RC(=N)N where the central carbon atom and one of the linked nitrogen atoms are part of the same ring( R here is an organyl group). They can also be viewed as analogs of lactams where the oxygen atom is replaced by a nitrogen atom."@en ;
        skos:inScheme    vlcs:chemische_stof ;
        skos:notation    "CHEMONTID:0003886" ;
        skos:prefLabel   "Imidolactams"@en .

csc:CHEMONTID_0002230
        a                skos:Concept ;
        skos:altLabel    "aliphatic aldehyde"@en ;
        skos:broader     csc:CHEMONTID_0000124 ;
        skos:definition  "An aldehyde with a chain length containing between 2 and 5 carbon atoms."@en ;
        skos:inScheme    vlcs:chemische_stof ;
        skos:notation    "CHEMONTID:0002230" ;
        skos:prefLabel   "Short-chain aldehydes"@en .

csc:CHEMONTID_0003633
        a                skos:Concept ;
        rdfs:seeAlso     tax_nodes:C0003633 ;
        skos:altLabel    "dipolar compound"@en ;
        skos:broader     csc:CHEMONTID_0003630 ;
        skos:definition  "Organic 1,3-dipolar compounds with the general structure  X#N+-Z- <-> X-=N+=Z <-> X-=N-Z+ <-> X-N=Z (X = C or O, Z = C, N, or O)."@en ;
        skos:inScheme    vlcs:chemische_stof ;
        skos:notation    "CHEMONTID:0003633" ;
        skos:prefLabel   "Propargyl-type 1,3-dipolar organic compounds"@en .

csc:CHEMONTID_0000027
        a                skos:Concept ;
        rdfs:seeAlso     tax_nodes:C0000027 ;
        skos:altLabel    "indanes"@en ;
        skos:broader     csc:CHEMONTID_0002448 ;
        skos:definition  "Compounds containing an indane moiety, which consists of a cyclopentane fused to a benzene ring."@en ;
        skos:inScheme    vlcs:chemische_stof ;
        skos:notation    "CHEMONTID:0000027" ;
        skos:prefLabel   "Indanes"@en .

csc:CHEMONTID_0001974
        a                skos:Concept ;
        rdfs:seeAlso     tax_nodes:C0001974 ;
        skos:altLabel    "carbonyl compound"@en , "piperidines"@en ;
        skos:broader     csc:CHEMONTID_0000195 ;
        skos:definition  "Compounds containing a piperidine ring which bears a carboxylic acid group (or a derivative thereof)."@en ;
        skos:inScheme    vlcs:chemische_stof ;
        skos:notation    "CHEMONTID:0001974" ;
        skos:prefLabel   "Piperidinecarboxylic acids and derivatives"@en .

csc:CHEMONTID_0003808
        a                skos:Concept ;
        rdfs:seeAlso     tax_nodes:C0003808 ;
        skos:altLabel    "monosubstituted glycerol"@en , "a monoorganylglycerol"@en , "Monoradylglyerols"@en ;
        skos:broader     csc:CHEMONTID_0000175 ;
        skos:definition  "Glycerolipids that carry exactly one acyl chain attached to the glycerol moiety."@en ;
        skos:inScheme    vlcs:chemische_stof ;
        skos:notation    "CHEMONTID:0003808" ;
        skos:prefLabel   "Monoradylglycerols"@en .

csc:CHEMONTID_0001476
        a                skos:Concept ;
        skos:broader     csc:CHEMONTID_0001470 ;
        skos:definition  "Inorganic compounds in which the largest metallic oxoanion is borate, to which either no atom or a non metal atom is bonded."@en ;
        skos:inScheme    vlcs:chemische_stof ;
        skos:notation    "CHEMONTID:0001476" ;
        skos:prefLabel   "Miscellaneous borates"@en .

csc:CHEMONTID_0002451
        a                skos:Concept ;
        skos:altLabel    "secondary amine"@en ;
        skos:broader     csc:CHEMONTID_0002449 ;
        skos:definition  "Amines having the nitrogen atom linked to exactly two hydrocarbyl groups."@en ;
        skos:inScheme    vlcs:chemische_stof ;
        skos:notation    "CHEMONTID:0002451" ;
        skos:prefLabel   "Secondary amines"@en .

csc:CHEMONTID_0001223
        a                skos:Concept ;
        skos:altLabel    "alpha-diketone"@en ;
        skos:broader     csc:CHEMONTID_0000118 ;
        skos:definition  "Organic compounds containing two ketone groups on two adjacent carbon atoms."@en ;
        skos:inScheme    vlcs:chemische_stof ;
        skos:notation    "CHEMONTID:0001223" ;
        skos:prefLabel   "Alpha-diketones"@en .

csc:CHEMONTID_0003601
        a                skos:Concept ;
        skos:altLabel    "naphthalenesulfonic acid"@en ;
        skos:broader     csc:CHEMONTID_0003310 ;
        skos:definition  "Organic aromatic compounds that contain a naphthalene moiety that carries a sulfonic acid group at the 2-position. Naphthalene is a bicyclic compound that is made up of two fused benzene ring."@en ;
        skos:inScheme    vlcs:chemische_stof ;
        skos:notation    "CHEMONTID:0003601" ;
        skos:prefLabel   "2-naphthalene sulfonates"@en .

csc:CHEMONTID_0000294
        a                skos:Concept ;
        rdfs:seeAlso     tax_nodes:C0000294 ;
        skos:altLabel    "Benzimidazoles"@en ;
        skos:broader     csc:CHEMONTID_0000002 ;
        skos:definition  "Organic compounds containing a benzene ring fused to an imidazole ring (five member ring containing a nitrogen atom, 4 carbon atoms, and two double bonds)."@en ;
        skos:inScheme    vlcs:chemische_stof ;
        skos:notation    "CHEMONTID:0000294" ;
        skos:prefLabel   "Benzimidazoles"@en .

csc:CHEMONTID_0004759
        a                skos:Concept ;
        skos:broader     csc:CHEMONTID_0004758 ;
        skos:definition  "Aromatic heterocyclic compounds containing a furan ring, which carries a carboxyl group or a derivative thereof at the ring 3-position."@en ;
        skos:inScheme    vlcs:chemische_stof ;
        skos:notation    "CHEMONTID:0004759" ;
        skos:prefLabel   "Furan-3-carboxylic acid and derivatives"@en .

csc:CHEMONTID_0000041
        a                skos:Concept ;
        rdfs:seeAlso     tax_nodes:C0000041 ;
        skos:altLabel    "biphenyls"@en , "Diphenyl ethers, biphenyls, dibenzyls and stilbenes"@en , "Biphenyl Compounds"@en ;
        skos:broader     csc:CHEMONTID_0002279 ;
        skos:definition  "Organic compounds containing to benzene rings linked together by a C-C bond."@en ;
        skos:inScheme    vlcs:chemische_stof ;
        skos:notation    "CHEMONTID:0000041" ;
        skos:prefLabel   "Biphenyls and derivatives"@en .

csc:CHEMONTID_0000469
        a                skos:Concept ;
        skos:altLabel    "alkylamine"@en , "a monoalkylamine"@en ;
        skos:broader     csc:CHEMONTID_0002450 ;
        skos:definition  "Organic compounds containing an primary aliphatic amine group."@en ;
        skos:inScheme    vlcs:chemische_stof ;
        skos:notation    "CHEMONTID:0000469" ;
        skos:prefLabel   "Monoalkylamines"@en .

csc:CHEMONTID_0001619
        a                skos:Concept ;
        skos:altLabel    "purine ribonucleoside triphosphate"@en ;
        skos:broader     csc:CHEMONTID_0001544 ;
        skos:definition  "Purine ribobucleotides with a triphosphate group  linked to the ribose moiety."@en ;
        skos:inScheme    vlcs:chemische_stof ;
        skos:notation    "CHEMONTID:0001619" ;
        skos:prefLabel   "Purine ribonucleoside triphosphates"@en .

csc:CHEMONTID_0000262
        a                skos:Concept ;
        rdfs:seeAlso     tax_nodes:C0000262 ;
        skos:altLabel    "Fatty Acids and Conjugates"@en , "a fatty acid"@en , "monocarboxylic acid"@en , "Fatty Acids"@en ;
        skos:broader     csc:CHEMONTID_0003909 ;
        skos:definition  "Aliphatic monocarboxylic acids with a saturated or unsaturated aliphatic tail (with at least 4 Carbon atoms)."@en ;
        skos:inScheme    vlcs:chemische_stof ;
        skos:notation    "CHEMONTID:0000262" ;
        skos:prefLabel   "Fatty acids and conjugates"@en .

csc:CHEMONTID_0000437
        a                skos:Concept ;
        rdfs:seeAlso     tax_nodes:C0000437 ;
        skos:altLabel    "halide"@en ;
        skos:broader     csc:CHEMONTID_0000423 ;
        skos:definition  "Inorganic compounds containing 'other non-metals' and halogen."@en ;
        skos:inScheme    vlcs:chemische_stof ;
        skos:notation    "CHEMONTID:0000437" ;
        skos:prefLabel   "Other non-metal halides"@en .

csc:CHEMONTID_0003370
        a                skos:Concept ;
        rdfs:seeAlso     tax_nodes:C0003370 ;
        skos:altLabel    "Diphenyldiazenes"@en , "a diphenyldiazene"@en , "azobenzenes"@en ;
        skos:broader     csc:CHEMONTID_0000002 ;
        skos:definition  "Organonitrogen aromatic compounds that contain a central azo group, where each nitrogen atom is conjugated to a benzene ring."@en ;
        skos:inScheme    vlcs:chemische_stof ;
        skos:notation    "CHEMONTID:0003370" ;
        skos:prefLabel   "Azobenzenes"@en .

csc:CHEMONTID_0001167
        a                skos:Concept ;
        skos:altLabel    "ether"@en ;
        skos:broader     csc:CHEMONTID_0000254 ;
        skos:definition  "Organic compounds containing the dialkyl ether functional group, with the formula ROR', where R and R' are alkyl groups."@en ;
        skos:inScheme    vlcs:chemische_stof ;
        skos:notation    "CHEMONTID:0001167" ;
        skos:prefLabel   "Dialkyl ethers"@en .

csc:CHEMONTID_0002861
        a                skos:Concept ;
        rdfs:seeAlso     tax_nodes:C0002861 ;
        skos:altLabel    "organofluorine compound"@en ;
        skos:broader     csc:CHEMONTID_0002868 ;
        skos:definition  "Vinyl halides in which a fluorine atom is bonded to an sp2-hybridised carbon atom."@en ;
        skos:inScheme    vlcs:chemische_stof ;
        skos:notation    "CHEMONTID:0002861" ;
        skos:prefLabel   "Vinyl fluorides"@en .

csc:CHEMONTID_0002317
        a                skos:Concept ;
        rdfs:seeAlso     tax_nodes:C0002317 ;
        skos:altLabel    "phenylpyridine"@en ;
        skos:broader     csc:CHEMONTID_0000089 ;
        skos:definition  "Polycyclic aromatic compounds containing a benzene ring linked to a pyridine ring through a CC or CN bond."@en ;
        skos:inScheme    vlcs:chemische_stof ;
        skos:notation    "CHEMONTID:0002317" ;
        skos:prefLabel   "Phenylpyridines"@en .

csc:CHEMONTID_0001633
        a                skos:Concept ;
        rdfs:seeAlso     tax_nodes:C0001633 ;
        skos:altLabel    "homoflavonoid"@en ;
        skos:broader     csc:CHEMONTID_0002507 ;
        skos:definition  "Homoisoflavonoids with a structure based on the chromone system. Chromone is a bicyclic compound consisting of a 1-benzopyran, which bears a ketone group at the 4-position."@en ;
        skos:inScheme    vlcs:chemische_stof ;
        skos:notation    "CHEMONTID:0001633" ;
        skos:prefLabel   "Homoisoflavones"@en .

csc:CHEMONTID_0000405
        a                skos:Concept ;
        rdfs:seeAlso     tax_nodes:C0000405 ;
        skos:altLabel    "organoarsenic compound"@en , "Organic Chemicals"@en ;
        skos:broader     csc:CHEMONTID_0001370 ;
        skos:definition  "Compounds containing bond between a carbon atom and an arsenic atom."@en ;
        skos:inScheme    vlcs:chemische_stof ;
        skos:notation    "CHEMONTID:0000405" ;
        skos:prefLabel   "Organoarsenic compounds"@en .

csc:CHEMONTID_0002363
        a                skos:Concept ;
        rdfs:seeAlso     tax_nodes:C0002363 ;
        skos:altLabel    "acetamides"@en ;
        skos:broader     csc:CHEMONTID_0002279 ;
        skos:definition  "Amide derivatives of phenylacetic acids."@en ;
        skos:inScheme    vlcs:chemische_stof ;
        skos:notation    "CHEMONTID:0002363" ;
        skos:prefLabel   "Phenylacetamides"@en .

csc:CHEMONTID_0001135
        a                skos:Concept ;
        skos:altLabel    "Triacylglycerols"@en , "Triacylglycerol"@en , "Triglycerides"@en , "triglyceride"@en ;
        skos:broader     csc:CHEMONTID_0003815 ;
        skos:definition  "Glycerides consisting of three fatty acid chains covalently bonded to a glycerol molecule through ester linkages."@en ;
        skos:inScheme    vlcs:chemische_stof ;
        skos:notation    "CHEMONTID:0001135" ;
        skos:prefLabel   "Triacylglycerols"@en .

csc:CHEMONTID_0000128
        a                skos:Concept ;
        skos:broader     csc:CHEMONTID_0000254 ;
        skos:definition  "Organic compounds containing the alkyl aryl ether functional group with the generic formula R-O-R' , where R is an alkyl group and R' is an aryl group."@en ;
        skos:inScheme    vlcs:chemische_stof ;
        skos:notation    "CHEMONTID:0000128" ;
        skos:prefLabel   "Alkyl aryl ethers"@en .

csc:CHEMONTID_0002506
        a                skos:Concept ;
        rdfs:seeAlso     tax_nodes:C0002506 ;
        skos:altLabel    "isoflavonoid"@en , "Isoflavonoids"@en , "3-phenylbenzopyrans"@en ;
        skos:broader     csc:CHEMONTID_0000261 ;
        skos:definition  "Natural products derived from 3-phenylchromen-4-one."@en ;
        skos:inScheme    vlcs:chemische_stof ;
        skos:notation    "CHEMONTID:0002506" ;
        skos:prefLabel   "Isoflavonoids"@en .

csc:CHEMONTID_0003909
        a                skos:Concept ;
        rdfs:seeAlso     tax_nodes:C0003909 ;
        skos:altLabel    "lipid"@en , "Fatty Acyls"@en ;
        skos:broader     csc:CHEMONTID_0000012 ;
        skos:definition  "Organic molecules synthesized by chain elongation of an acetyl-CoA primer with malonyl-CoA (or methylmalonyl-CoA) groups that might contain a cyclic functionality and/or are substituted with heteroatoms."@en ;
        skos:inScheme    vlcs:chemische_stof ;
        skos:notation    "CHEMONTID:0003909" ;
        skos:prefLabel   "Fatty Acyls"@en .

csc:CHEMONTID_0000174
        a                skos:Concept ;
        skos:altLabel    "penicillin"@en , "Penicillins"@en , "penicillins"@en ;
        skos:broader     csc:CHEMONTID_0000172 ;
        skos:definition  "Organic compounds containing the penicillin core structure, which is structurally characterized by a penam ring bearing two methyl groups at position 2, and an amide group at position 6 [starting from the sulfur atom at position 1]."@en ;
        skos:inScheme    vlcs:chemische_stof ;
        skos:notation    "CHEMONTID:0000174" ;
        skos:prefLabel   "Penicillins"@en .

csc:CHEMONTID_0004211
        a                skos:Concept ;
        skos:broader     csc:CHEMONTID_0004208 ;
        skos:definition  "Aromatic compounds that contain a p-xylene moiety, which is a monocyclic benzene carrying exactly two methyl groups at the 1- and 4-positions."@en ;
        skos:inScheme    vlcs:chemische_stof ;
        skos:notation    "CHEMONTID:0004211" ;
        skos:prefLabel   "p-Xylenes"@en .

csc:CHEMONTID_0004639
        a                skos:Concept ;
        skos:broader     csc:CHEMONTID_0004105 ;
        skos:definition  "Aromatic compounds containing a 1,3,5-triazine ring that is substituted at the 2-position with a halogen atom."@en ;
        skos:inScheme    vlcs:chemische_stof ;
        skos:notation    "CHEMONTID:0004639" ;
        skos:prefLabel   "Halo-S-triazines"@en .

csc:CHEMONTID_0002552
        a                skos:Concept ;
        rdfs:seeAlso     tax_nodes:C0002552 ;
        skos:broader     csc:CHEMONTID_0001253 ;
        skos:definition  "Quinolines in which the quinoline ring system is substituted by a carboxyl group at one or more positions."@en ;
        skos:inScheme    vlcs:chemische_stof ;
        skos:notation    "CHEMONTID:0002552" ;
        skos:prefLabel   "Quinoline carboxylic acids"@en .

csc:CHEMONTID_0003955
        a                skos:Concept ;
        skos:altLabel    "aromatic amine"@en , "biphenyls"@en , "Benzidines"@en ;
        skos:broader     csc:CHEMONTID_0000041 ;
        skos:definition  "Organic compounds containing the benzidine skeleton, made up of a biphenyl ring system substituted at the 4- and 4'-positions with a unsubstituted amine group."@en ;
        skos:inScheme    vlcs:chemische_stof ;
        skos:notation    "CHEMONTID:0003955" ;
        skos:prefLabel   "Benzidines"@en .

csc:CHEMONTID_0000640
        a                skos:Concept ;
        rdfs:seeAlso     tax_nodes:C0000640 ;
        skos:altLabel    "alkali metal salt"@en ;
        skos:broader     csc:CHEMONTID_0000445 ;
        skos:definition  "Inorganic compounds in which the largest oxoanion is hypochlorite, and in which the heaviest atom not in an oxoanion is an alkali metal."@en ;
        skos:inScheme    vlcs:chemische_stof ;
        skos:notation    "CHEMONTID:0000640" ;
        skos:prefLabel   "Alkali metal hypochlorites"@en .

csc:CHEMONTID_0000395
        a                skos:Concept ;
        rdfs:seeAlso     tax_nodes:C0000395 ;
        skos:altLabel    "nitrates"@en ;
        skos:broader     csc:CHEMONTID_0000463 ;
        skos:definition  "Organic compounds containing the nitrate oxoanion, with the formula NO3-."@en ;
        skos:inScheme    vlcs:chemische_stof ;
        skos:notation    "CHEMONTID:0000395" ;
        skos:prefLabel   "Organic nitrates"@en .

csc:CHEMONTID_0003457
        a                skos:Concept ;
        skos:altLabel    "alkyl phosphate"@en ;
        skos:broader     csc:CHEMONTID_0000408 ;
        skos:definition  "Organic compounds containing a phosphate group that is linked to one or more alkyl chains."@en ;
        skos:inScheme    vlcs:chemische_stof ;
        skos:notation    "CHEMONTID:0003457" ;
        skos:prefLabel   "Alkyl phosphates"@en .

csc:CHEMONTID_0001370
        a                skos:Concept ;
        rdfs:seeAlso     tax_nodes:C0001370 ;
        skos:altLabel    "organic molecular entity"@en , "Metalloids"@en , "Organic Chemicals"@en ;
        skos:broader     csc:CHEMONTID_0000462 ;
        skos:definition  "Organic compounds containing a metalloid atom."@en ;
        skos:inScheme    vlcs:chemische_stof ;
        skos:notation    "CHEMONTID:0001370" ;
        skos:prefLabel   "Organometalloid compounds"@en .

csc:CHEMONTID_0002229
        a                skos:Concept ;
        skos:altLabel    "fatty aldehyde"@en ;
        skos:broader     csc:CHEMONTID_0000124 ;
        skos:definition  "An aldehyde with a chain length containing between 6 and 12 carbon atoms."@en ;
        skos:inScheme    vlcs:chemische_stof ;
        skos:notation    "CHEMONTID:0002229" ;
        skos:prefLabel   "Medium-chain aldehydes"@en .

csc:CHEMONTID_0002948
        a                skos:Concept ;
        skos:altLabel    "aminobenzoic acid"@en ;
        skos:broader     csc:CHEMONTID_0000281 ;
        skos:definition  "Benzoic acids containing an amine group attached to the benzene moiety."@en ;
        skos:inScheme    vlcs:chemische_stof ;
        skos:notation    "CHEMONTID:0002948" ;
        skos:prefLabel   "Aminobenzoic acids"@en .

csc:CHEMONTID_0000317
        a                skos:Concept ;
        rdfs:seeAlso     tax_nodes:C0000317 ;
        skos:altLabel    "benzothiazepine"@en ;
        skos:broader     csc:CHEMONTID_0000002 ;
        skos:definition  "Organic compounds containing a benzene fused to a thiazepine ring (a seven-membered ring with a nitrogen atom and a sulfur atom replacing two carbon atoms)."@en ;
        skos:inScheme    vlcs:chemische_stof ;
        skos:notation    "CHEMONTID:0000317" ;
        skos:prefLabel   "Benzothiazepines"@en .

csc:CHEMONTID_0002275
        a                skos:Concept ;
        rdfs:seeAlso     tax_nodes:C0002275 ;
        skos:altLabel    "nitronaphthalene"@en ;
        skos:broader     csc:CHEMONTID_0000023 ;
        skos:definition  "Polycyclic aromatic compounds containing a naphthalene moiety substituted by one or more nitro groups."@en ;
        skos:inScheme    vlcs:chemische_stof ;
        skos:notation    "CHEMONTID:0002275" ;
        skos:prefLabel   "Nitronaphthalenes"@en .

csc:CHEMONTID_0000363
        a                skos:Concept ;
        rdfs:seeAlso     tax_nodes:C0000363 ;
        skos:altLabel    "Cyanates"@en , "cyanates"@en ;
        skos:broader     csc:CHEMONTID_0000463 ;
        skos:definition  "Organic compounds containing the cyanate functional group with the formula [OCN]-."@en ;
        skos:inScheme    vlcs:chemische_stof ;
        skos:notation    "CHEMONTID:0000363" ;
        skos:prefLabel   "Cyanates"@en .

csc:CHEMONTID_0000538
        a                skos:Concept ;
        rdfs:seeAlso     tax_nodes:C0000538 ;
        skos:altLabel    "inorganic oxide"@en ;
        skos:broader     csc:CHEMONTID_0000461 ;
        skos:definition  "Inorganic compounds containing an oxygen atom of an oxidation state of -2, in which the heaviest atom bonded to the oxygen is a transition metal."@en ;
        skos:inScheme    vlcs:chemische_stof ;
        skos:notation    "CHEMONTID:0000538" ;
        skos:prefLabel   "Transition metal oxides"@en .

csc:CHEMONTID_0004155
        a                skos:Concept ;
        rdfs:seeAlso     tax_nodes:C0004155 ;
        skos:broader     csc:CHEMONTID_0002279 ;
        skos:definition  "Aromatic compounds containing two benzene rings linked to each other through an ether group."@en ;
        skos:inScheme    vlcs:chemische_stof ;
        skos:notation    "CHEMONTID:0004155" ;
        skos:prefLabel   "Diphenylethers"@en .

csc:CHEMONTID_0001093
        a                skos:Concept ;
        rdfs:seeAlso     tax_nodes:C0001093 ;
        skos:altLabel    "organooxygen compound"@en ;
        skos:broader     csc:CHEMONTID_0000265 ;
        skos:definition  "Derivatives of carboxylic acid."@en ;
        skos:inScheme    vlcs:chemische_stof ;
        skos:notation    "CHEMONTID:0001093" ;
        skos:prefLabel   "Carboxylic acid derivatives"@en .

csc:CHEMONTID_0002496
        a                skos:Concept ;
        rdfs:seeAlso     tax_nodes:C0002496 ;
        skos:altLabel    "isoindoles"@en ;
        skos:broader     csc:CHEMONTID_0001819 ;
        skos:definition  "Heterocyclic compounds containing a 2,3-dihydro-1H-iso-indole moiety."@en ;
        skos:inScheme    vlcs:chemische_stof ;
        skos:notation    "CHEMONTID:0002496" ;
        skos:prefLabel   "Isoindolines"@en .

csc:CHEMONTID_0003899
        a                skos:Concept ;
        skos:altLabel    "aralkylamine"@en ;
        skos:broader     csc:CHEMONTID_0002449 ;
        skos:definition  "Alkylamines in which the alkyl group is substituted at one carbon atom by an aromatic hydrocarbyl group."@en ;
        skos:inScheme    vlcs:chemische_stof ;
        skos:notation    "CHEMONTID:0003899" ;
        skos:prefLabel   "Aralkylamines"@en .

csc:CHEMONTID_0000584
        a                skos:Concept ;
        rdfs:seeAlso     tax_nodes:C0000584 ;
        skos:altLabel    "fluoride salt"@en , "Metalloids"@en , "Inorganic Chemicals"@en , "inorganic salt"@en ;
        skos:broader     csc:CHEMONTID_0000442 ;
        skos:definition  "Inorganic compounds in which the largest halogen atom is fluorine, and the heaviest metal atom is a metalloid."@en ;
        skos:inScheme    vlcs:chemische_stof ;
        skos:notation    "CHEMONTID:0000584" ;
        skos:prefLabel   "Metalloid fluorides"@en .

csc:CHEMONTID_0001987
        a                skos:Concept ;
        rdfs:seeAlso     tax_nodes:C0001987 ;
        skos:altLabel    "glucitol derivative"@en ;
        skos:broader     csc:CHEMONTID_0001816 ;
        skos:definition  "Organic polycyclic compounds containing an isosorbide(1,4-Dianhydrosorbitol) moiety, which consists of two -oxolan-3-ol rings."@en ;
        skos:inScheme    vlcs:chemische_stof ;
        skos:notation    "CHEMONTID:0001987" ;
        skos:prefLabel   "Isosorbides"@en .

csc:CHEMONTID_0000331
        a                skos:Concept ;
        rdfs:seeAlso     tax_nodes:C0000331 ;
        skos:altLabel    "Fatty amides"@en , "fatty amide"@en ;
        skos:broader     csc:CHEMONTID_0003909 ;
        skos:definition  "Carboxylic acid amide derivatives of fatty acids, that are formed from a fatty acid and an amine."@en ;
        skos:inScheme    vlcs:chemische_stof ;
        skos:notation    "CHEMONTID:0000331" ;
        skos:prefLabel   "Fatty amides"@en .

csc:CHEMONTID_0002464
        a                skos:Concept ;
        skos:altLabel    "nitrogen molecular entity"@en ;
        skos:broader     csc:CHEMONTID_0000112 ;
        skos:definition  "Hydrazine derivatives with the general formula RC(NHNH2)2=NNH2."@en ;
        skos:inScheme    vlcs:chemische_stof ;
        skos:notation    "CHEMONTID:0002464" ;
        skos:prefLabel   "Hydrazidines"@en .

csc:CHEMONTID_0002930
        a                skos:Concept ;
        skos:altLabel    "diterpenoid"@en ;
        skos:broader     csc:CHEMONTID_0001551 ;
        skos:definition  "Diterpenoids with a structure based on the mutilane skeleton."@en ;
        skos:inScheme    vlcs:chemische_stof ;
        skos:notation    "CHEMONTID:0002930" ;
        skos:prefLabel   "Mutilane diterpenoids"@en .

csc:CHEMONTID_0000552
        a                skos:Concept ;
        rdfs:seeAlso     tax_nodes:C0000552 ;
        skos:altLabel    "inorganic hydride"@en ;
        skos:broader     csc:CHEMONTID_0000453 ;
        skos:definition  "Inorganic compounds in which the heaviest atom bonded to a hydrogen atom is belongs to the class of 'other non-metals'."@en ;
        skos:inScheme    vlcs:chemische_stof ;
        skos:notation    "CHEMONTID:0000552" ;
        skos:prefLabel   "Other non-metal hydrides"@en .

csc:CHEMONTID_0003194
        a                skos:Concept ;
        rdfs:seeAlso     tax_nodes:C0003194 ;
        skos:altLabel    "organosilicon compound"@en ;
        skos:broader     csc:CHEMONTID_0001370 ;
        skos:definition  "Organic compounds containing a C[Si] bond."@en ;
        skos:inScheme    vlcs:chemische_stof ;
        skos:notation    "CHEMONTID:0003194" ;
        skos:prefLabel   "Organosilicon compounds"@en .

csc:CHEMONTID_0001204
        a                skos:Concept ;
        rdfs:seeAlso     tax_nodes:C0001204 ;
        skos:altLabel    "phosphoramides"@en , "Organic phosphoric acid amides"@en , "phosphoramide"@en ;
        skos:broader     csc:CHEMONTID_0000402 ;
        skos:definition  "Organic compounds containing the phosphoric acid amide functional group."@en ;
        skos:inScheme    vlcs:chemische_stof ;
        skos:notation    "CHEMONTID:0001204" ;
        skos:prefLabel   "Organic phosphoramides"@en .

csc:CHEMONTID_0000229
        a                skos:Concept ;
        rdfs:seeAlso     tax_nodes:C0000229 ;
        skos:altLabel    "thiazoles"@en ;
        skos:broader     csc:CHEMONTID_0002490 ;
        skos:definition  "Heterocyclic compounds containing a five-member unsaturated aliphatic ring with one nitrogen atom, one sulfur atom, three carbon atoms."@en ;
        skos:inScheme    vlcs:chemische_stof ;
        skos:notation    "CHEMONTID:0000229" ;
        skos:prefLabel   "Thiazolines"@en .

csc:CHEMONTID_0001923
        a                skos:Concept ;
        skos:altLabel    "thiazolidines"@en , "thiocarbonyl compound"@en ;
        skos:broader     csc:CHEMONTID_0000226 ;
        skos:definition  "Heterocyclic compounds containing a thiazolidinethione ring which bears one thioketone group."@en ;
        skos:inScheme    vlcs:chemische_stof ;
        skos:notation    "CHEMONTID:0001923" ;
        skos:prefLabel   "Thiazolidinethiones"@en .

csc:CHEMONTID_0003305
        a                skos:Concept ;
        skos:altLabel    "amino sugar"@en ;
        skos:broader     csc:CHEMONTID_0000011 ;
        skos:definition  "Saccharides containing a sugar unit that bears an amino group."@en ;
        skos:inScheme    vlcs:chemische_stof ;
        skos:notation    "CHEMONTID:0003305" ;
        skos:prefLabel   "Aminosaccharides"@en .

csc:CHEMONTID_0000211
        a                skos:Concept ;
        rdfs:seeAlso     tax_nodes:C0000211 ;
        skos:altLabel    "indoles"@en ;
        skos:broader     csc:CHEMONTID_0000002 ;
        skos:definition  "Organic compounds containing an indole, which is a bicyclic ring system made up of a six-membered benzene ring fused to a five-membered nitrogen-containing pyrrole ring."@en ;
        skos:inScheme    vlcs:chemische_stof ;
        skos:notation    "CHEMONTID:0000211" ;
        skos:prefLabel   "Indoles and derivatives"@en .

csc:CHEMONTID_0001614
        a                skos:Concept ;
        rdfs:seeAlso     tax_nodes:C0001614 ;
        skos:altLabel    "4-phenylbenzopyrans"@en , "neoflavonoid"@en , "Neoflavonoids"@en ;
        skos:broader     csc:CHEMONTID_0000261 ;
        skos:definition  "Compounds with a structure based on the 4-phenylchromene backbone."@en ;
        skos:inScheme    vlcs:chemische_stof ;
        skos:notation    "CHEMONTID:0001614" ;
        skos:prefLabel   "Neoflavonoids"@en .

csc:CHEMONTID_0001194
        a                skos:Concept ;
        rdfs:seeAlso     tax_nodes:C0001194 ;
        skos:altLabel    "Ketosteroids"@en , "oxo steroid"@en ;
        skos:broader     csc:CHEMONTID_0000258 ;
        skos:definition  "Steroid derivatives carrying a C=O group attached to steroid skeleton."@en ;
        skos:inScheme    vlcs:chemische_stof ;
        skos:notation    "CHEMONTID:0001194" ;
        skos:prefLabel   "Oxosteroids"@en .

csc:CHEMONTID_0002344
        a                skos:Concept ;
        skos:altLabel    "methoxybenzoic acid"@en ;
        skos:broader     csc:CHEMONTID_0000176 ;
        skos:definition  "Benzoic acids in which a hydrogen atom of the benzene ring is replaced by a methoxy group."@en ;
        skos:inScheme    vlcs:chemische_stof ;
        skos:notation    "CHEMONTID:0002344" ;
        skos:prefLabel   "Methoxybenzoic acids and derivatives"@en .

csc:CHEMONTID_0000432
        a                skos:Concept ;
        rdfs:seeAlso     tax_nodes:C0000432 ;
        skos:broader     csc:CHEMONTID_0000423 ;
        skos:definition  "Inorganic non-metallic compounds in which the largest atom is a nobel gas."@en ;
        skos:inScheme    vlcs:chemische_stof ;
        skos:notation    "CHEMONTID:0000432" ;
        skos:prefLabel   "Homogeneous halogens"@en .

csc:CHEMONTID_0004477
        a                skos:Concept ;
        rdfs:seeAlso     tax_nodes:C0004477 ;
        skos:broader     csc:CHEMONTID_0002837 ;
        skos:definition  "Aromatic compounds that are made up of carbon and hydrogen atoms only."@en ;
        skos:inScheme    vlcs:chemische_stof ;
        skos:notation    "CHEMONTID:0004477" ;
        skos:prefLabel   "Aromatic hydrocarbons"@en .

csc:CHEMONTID_0001162
        a                skos:Concept ;
        skos:altLabel    "Carbamic Acid Esters"@en , "carbamate ester"@en ;
        skos:broader     csc:CHEMONTID_0000318 ;
        skos:definition  "Compounds containing an ester of carbamic acid with the general structure R2NC(=O)OR' (R' not H). They are esters of carbamic acids."@en ;
        skos:inScheme    vlcs:chemische_stof ;
        skos:notation    "CHEMONTID:0001162" ;
        skos:prefLabel   "Carbamate esters"@en .

csc:CHEMONTID_0002565
        a                skos:Concept ;
        skos:altLabel    "benzoic acids"@en ;
        skos:broader     csc:CHEMONTID_0000176 ;
        skos:definition  "Organic Compounds containing a benzene ring which bears at least one carboxyl group."@en ;
        skos:inScheme    vlcs:chemische_stof ;
        skos:notation    "CHEMONTID:0002565" ;
        skos:prefLabel   "Benzoic acids"@en .

csc:CHEMONTID_0003968
        a                skos:Concept ;
        skos:altLabel    "substituted aniline"@en ;
        skos:broader     csc:CHEMONTID_0000284 ;
        skos:definition  "Organic compounds containing an aniline moiety, which is substituted at 2 positions by a nitro group."@en ;
        skos:inScheme    vlcs:chemische_stof ;
        skos:notation    "CHEMONTID:0003968" ;
        skos:prefLabel   "Dinitroanilines"@en .

csc:CHEMONTID_0000400
        a                skos:Concept ;
        rdfs:seeAlso     tax_nodes:C0000400 ;
        skos:altLabel    "organophosphorus compound"@en , "Organophosphorus Compounds"@en ;
        skos:broader     csc:CHEMONTID_0000000 ;
        skos:definition  "Organic compounds containing the phosphorus atom."@en ;
        skos:inScheme    vlcs:chemische_stof ;
        skos:notation    "CHEMONTID:0000400" ;
        skos:prefLabel   "Organophosphorus compounds"@en .

csc:CHEMONTID_0004445
        a                skos:Concept ;
        skos:altLabel    "Organosilicon Compounds"@en ;
        skos:broader     csc:CHEMONTID_0003194 ;
        skos:definition  "Organosilicon compounds where the tetravalent silicon atom is linked to one or more heteroatoms."@en ;
        skos:inScheme    vlcs:chemische_stof ;
        skos:notation    "CHEMONTID:0004445" ;
        skos:prefLabel   "Organoheterosilanes"@en .

csc:CHEMONTID_0003936
        a                skos:Concept ;
        rdfs:seeAlso     tax_nodes:C0003936 ;
        skos:altLabel    "organosulfur compound"@en ;
        skos:broader     csc:CHEMONTID_0003934 ;
        skos:definition  "Organosulfur compounds with the general formula R3SC(=S)N(R1)R2; R1-R2 =  H or organyl group, R3 = organyl."@en ;
        skos:inScheme    vlcs:chemische_stof ;
        skos:notation    "CHEMONTID:0003936" ;
        skos:prefLabel   "Dithiocarbamic acid esters"@en .

csc:CHEMONTID_0004413
        a                skos:Concept ;
        skos:broader     csc:CHEMONTID_0000178 ;
        skos:definition  "Aromatic compound containing a benzene carboxamide moiety that carries an amine group at the 2-position of the benzene ring."@en ;
        skos:inScheme    vlcs:chemische_stof ;
        skos:notation    "CHEMONTID:0004413" ;
        skos:prefLabel   "Anthranilamides"@en .

csc:CHEMONTID_0002754
        a                skos:Concept ;
        rdfs:seeAlso     tax_nodes:C0002754 ;
        skos:altLabel    "phenylpropanoid"@en ;
        skos:broader     csc:CHEMONTID_0000261 ;
        skos:definition  "Aromatic alcohols containing a 3-phenylprop-2-en-1-ol moiety."@en ;
        skos:inScheme    vlcs:chemische_stof ;
        skos:notation    "CHEMONTID:0002754" ;
        skos:prefLabel   "Cinnamyl alcohols"@en .

csc:CHEMONTID_0000123
        a                skos:Concept ;
        rdfs:seeAlso     tax_nodes:C0000123 ;
        skos:altLabel    "benzopyran"@en , "Benzopyranoids"@en ;
        skos:broader     csc:CHEMONTID_0000002 ;
        skos:definition  "Organic compounds containing a benzene ring fused to a pyran ring. Pyran a six-membered heterocyclic, non-aromatic ring, made up of five carbon atoms and one oxygen atom and containing two double bonds."@en ;
        skos:inScheme    vlcs:chemische_stof ;
        skos:notation    "CHEMONTID:0000123" ;
        skos:prefLabel   "Benzopyrans"@en .

csc:CHEMONTID_0001572
        a                skos:Concept ;
        rdfs:seeAlso     tax_nodes:C0001572 ;
        skos:altLabel    "Thiophosphate esters"@en ;
        skos:broader     csc:CHEMONTID_0001303 ;
        skos:definition  "Organic compounds containing the thiophosphoric acid functional group or a derivative thereof, with the general structure ROP(OR')(OR'')=S, where at least one R-group is an organyl group."@en ;
        skos:inScheme    vlcs:chemische_stof ;
        skos:notation    "CHEMONTID:0001572" ;
        skos:prefLabel   "Thiophosphoric acid esters"@en .

csc:CHEMONTID_0002003
        a                skos:Concept ;
        skos:altLabel    "cyclic ketone"@en , "carbotricyclic compound"@en , "carboxylic ester"@en ;
        skos:broader     csc:CHEMONTID_0002002 ;
        skos:definition  "Mutilins with a hydroxyacetate derivative attached to the C8 carbon atom of the cyclopenta[8]annulene moiety."@en ;
        skos:inScheme    vlcs:chemische_stof ;
        skos:notation    "CHEMONTID:0002003" ;
        skos:prefLabel   "Pleuromutilin and derivatives"@en .

csc:CHEMONTID_0004809
        a                skos:Concept ;
        skos:broader     csc:CHEMONTID_0004808 ;
        skos:definition  "Organic compounds contaning a chlorine atom attached to the alpha carbon atom relative to C=O group."@en ;
        skos:inScheme    vlcs:chemische_stof ;
        skos:notation    "CHEMONTID:0004809" ;
        skos:prefLabel   "Alpha-chloroketones"@en .

csc:CHEMONTID_0000099
        a                skos:Concept ;
        rdfs:seeAlso     tax_nodes:C0000099 ;
        skos:altLabel    "Triazoles"@en ;
        skos:broader     csc:CHEMONTID_0000436 ;
        skos:definition  "Compounds containing  a five-member aromatic ring of two carbon atoms and three nitrogen atoms."@en ;
        skos:inScheme    vlcs:chemische_stof ;
        skos:notation    "CHEMONTID:0000099" ;
        skos:prefLabel   "Triazoles"@en .

csc:CHEMONTID_0001540
        a                skos:Concept ;
        skos:altLabel    "monosaccharide"@en ;
        skos:broader     csc:CHEMONTID_0000011 ;
        skos:definition  "Compounds containing one carbohydrate unit not glycosidically linked to another such unit, and no set of two or more glycosidically linked carbohydrate units. Monosaccharides have the general formula CnH2nOn."@en ;
        skos:inScheme    vlcs:chemische_stof ;
        skos:notation    "CHEMONTID:0001540" ;
        skos:prefLabel   "Monosaccharides"@en .

csc:CHEMONTID_0001715
        a                skos:Concept ;
        rdfs:seeAlso     tax_nodes:C0001715 ;
        skos:altLabel    "quinolines"@en ;
        skos:broader     csc:CHEMONTID_0001253 ;
        skos:definition  "Derivatives of  quinoline in which in which at least one double bond in the quinoline moiety are reduced by adding two hydrogen atoms."@en ;
        skos:inScheme    vlcs:chemische_stof ;
        skos:notation    "CHEMONTID:0001715" ;
        skos:prefLabel   "Hydroquinolines"@en .

csc:CHEMONTID_0001295
        a                skos:Concept ;
        rdfs:seeAlso     tax_nodes:C0001295 ;
        skos:altLabel    "Hydroxysteroids"@en , "hydroxy steroid"@en ;
        skos:broader     csc:CHEMONTID_0000258 ;
        skos:definition  "Compounds containing an steroid backbone, with at least one hydrogen substituted by a hydroxyl group."@en ;
        skos:inScheme    vlcs:chemische_stof ;
        skos:notation    "CHEMONTID:0001295" ;
        skos:prefLabel   "Hydroxysteroids"@en .

csc:CHEMONTID_0000067
        a                skos:Concept ;
        rdfs:seeAlso     tax_nodes:C0000067 ;
        skos:altLabel    "Pyrazines"@en ;
        skos:broader     csc:CHEMONTID_0001346 ;
        skos:definition  "Compounds containing a pyrazine ring, which is a six-member aromatic heterocycle, that consists of two nitrogen atoms (at positions 1 and 4) and four carbon atoms."@en ;
        skos:inScheme    vlcs:chemische_stof ;
        skos:notation    "CHEMONTID:0000067" ;
        skos:prefLabel   "Pyrazines"@en .

csc:CHEMONTID_0002445
        a                skos:Concept ;
        rdfs:seeAlso     tax_nodes:C0002445 ;
        skos:altLabel    "carbonyl compound"@en ;
        skos:broader     csc:CHEMONTID_0000265 ;
        skos:definition  "Organic acids with the general formula OOC(R)=O (R = H, organyl group)."@en ;
        skos:inScheme    vlcs:chemische_stof ;
        skos:notation    "CHEMONTID:0002445" ;
        skos:prefLabel   "Peroxycarboxylic acids and derivatives"@en .

csc:CHEMONTID_0004150
        a                skos:Concept ;
        rdfs:seeAlso     tax_nodes:C0004150 ;
        skos:broader     csc:CHEMONTID_0000000 ;
        skos:definition  "Derivatives of hydrocarbons obtained by substituting one or more carbon atoms by an heteroatom. They contain at least one carbon atom and heteroatom."@en ;
        skos:inScheme    vlcs:chemische_stof ;
        skos:notation    "CHEMONTID:0004150" ;
        skos:prefLabel   "Hydrocarbon derivatives"@en .

csc:CHEMONTID_0002491
        a                skos:Concept ;
        rdfs:seeAlso     tax_nodes:C0002491 ;
        skos:altLabel    "organonitrogen heterocyclic compound"@en ;
        skos:broader     csc:CHEMONTID_0000002 ;
        skos:definition  "Azole derivatives obtained by conversion of both double bonds of the azole ring to single bonds, yielding a saturated ring."@en ;
        skos:inScheme    vlcs:chemische_stof ;
        skos:notation    "CHEMONTID:0002491" ;
        skos:prefLabel   "Azolidines"@en .

csc:CHEMONTID_0004325
        a                skos:Concept ;
        skos:altLabel    "cyclohexenones"@en ;
        skos:broader     csc:CHEMONTID_0003487 ;
        skos:definition  "Compounds containing a cylohexenone moiety, which is a six-membered aliphatic ring that carries a ketone and has one endocyclic double bond."@en ;
        skos:inScheme    vlcs:chemische_stof ;
        skos:notation    "CHEMONTID:0004325" ;
        skos:prefLabel   "Cyclohexenones"@en .

csc:CHEMONTID_0000035
        a                skos:Concept ;
        rdfs:seeAlso     tax_nodes:C0000035 ;
        skos:broader     csc:CHEMONTID_0002279 ;
        skos:definition  "Aromatic compounds containing a halogen atom linked to a benzene ring."@en ;
        skos:inScheme    vlcs:chemische_stof ;
        skos:notation    "CHEMONTID:0000035" ;
        skos:prefLabel   "Halobenzenes"@en .

csc:CHEMONTID_0001982
        a                skos:Concept ;
        rdfs:seeAlso     tax_nodes:C0001982 ;
        skos:broader     csc:CHEMONTID_0001983 ;
        skos:definition  "Compounds containing a furan ring bearing a ketone group."@en ;
        skos:inScheme    vlcs:chemische_stof ;
        skos:notation    "CHEMONTID:0001982" ;
        skos:prefLabel   "Furanones"@en .

csc:CHEMONTID_0001010
        a                skos:Concept ;
        skos:altLabel    "oxime O-ethers"@en , "oxime O-ether"@en , "O-Hydrocarbyl oximes"@en ;
        skos:broader     csc:CHEMONTID_0000411 ;
        skos:definition  "Compounds containing the oxime ether functional group, with the general structure R1(R2)C=NOR3 ( R3 not H)."@en ;
        skos:inScheme    vlcs:chemische_stof ;
        skos:notation    "CHEMONTID:0001010" ;
        skos:prefLabel   "Oxime ethers"@en .

csc:CHEMONTID_0001438
        a                skos:Concept ;
        rdfs:seeAlso     tax_nodes:C0001438 ;
        skos:altLabel    "organothiophosphorus compound"@en ;
        skos:broader     csc:CHEMONTID_0000400 ;
        skos:definition  "Organic derivatives of thiophosphonic acid, thiophosphoric acid, dithiophosphoric acid, or phosphorotrithioic acid, or derivatives thereof. Thiophosphonic acid, dithiophosphoric acid, thiophosphoric acid, and phosphorotrithioic acid are thiophosphorus compounds with the formula OP(O)(=S), OP(S)(=S)O, OP(O)(=S)O, and OP(=S)(S)S, respectively."@en ;
        skos:inScheme    vlcs:chemische_stof ;
        skos:notation    "CHEMONTID:0001438" ;
        skos:prefLabel   "Organothiophosphorus compounds"@en .

csc:CHEMONTID_0000501
        a                skos:Concept ;
        rdfs:seeAlso     tax_nodes:C0000501 ;
        skos:altLabel    "isocyanates"@en , "Isocyanates"@en ;
        skos:broader     csc:CHEMONTID_0000278 ;
        skos:definition  "Organic compounds containing the isocyanic acid tautomer, HN=C=O, of cyanic acid, HOC#N or its hydrocarbyl derivatives RN=C=O."@en ;
        skos:inScheme    vlcs:chemische_stof ;
        skos:notation    "CHEMONTID:0000501" ;
        skos:prefLabel   "Isocyanates"@en .

csc:CHEMONTID_0000081
        a                skos:Concept ;
        rdfs:seeAlso     tax_nodes:C0000081 ;
        skos:altLabel    "Isoxazoles"@en ;
        skos:broader     csc:CHEMONTID_0000436 ;
        skos:definition  "Heterocyclic organic compounds containing an isoxazole moiety, with a structure characterized by a five-member aromatic ring with one oxygen atom and one nitrogen atom at ring positions 1 and 2, respectively."@en ;
        skos:inScheme    vlcs:chemische_stof ;
        skos:notation    "CHEMONTID:0000081" ;
        skos:prefLabel   "Isoxazoles"@en .

csc:CHEMONTID_0003862
        a                skos:Concept ;
        rdfs:seeAlso     tax_nodes:C0003862 ;
        skos:altLabel    "aliphatic sulfide"@en ;
        skos:broader     csc:CHEMONTID_0001202 ;
        skos:definition  "Organosulfur compounds containing a thioether group that is substituted by two alkyl groups."@en ;
        skos:inScheme    vlcs:chemische_stof ;
        skos:notation    "CHEMONTID:0003862" ;
        skos:prefLabel   "Dialkylthioethers"@en .

csc:CHEMONTID_0002389
        a                skos:Concept ;
        rdfs:seeAlso     tax_nodes:C0002389 ;
        skos:altLabel    "organic heterocyclic compound"@en , "organonitrogen heterocyclic compound"@en ;
        skos:broader     csc:CHEMONTID_0000002 ;
        skos:definition  "Organic compounds containing diazinane, a six-membered saturated heterocycle containing four carbon atoms and two nitrogen atoms."@en ;
        skos:inScheme    vlcs:chemische_stof ;
        skos:notation    "CHEMONTID:0002389" ;
        skos:prefLabel   "Diazinanes"@en .

csc:CHEMONTID_0004767
        a                skos:Concept ;
        skos:broader     csc:CHEMONTID_0004766 ;
        skos:definition  "Aromatic compounds containing a phenylphosphonothioate group, which is O-esterified with another phenyl group. They have the general structure OP(R)(=S)OR', where R,R'=phenyl groups."@en ;
        skos:inScheme    vlcs:chemische_stof ;
        skos:notation    "CHEMONTID:0004767" ;
        skos:prefLabel   "Phenyl phenylphosphonothioates"@en .

csc:CHEMONTID_0002680
        a                skos:Concept ;
        rdfs:seeAlso     tax_nodes:C0002680 ;
        skos:altLabel    "ergoline alkaloid"@en ;
        skos:broader     csc:CHEMONTID_0002679 ;
        skos:definition  "Alkaloids with a structure based on the lysergic acid skeleton."@en ;
        skos:inScheme    vlcs:chemische_stof ;
        skos:notation    "CHEMONTID:0002680" ;
        skos:prefLabel   "Lysergic acids and derivatives"@en .

csc:CHEMONTID_0000224
        a                skos:Concept ;
        rdfs:seeAlso     tax_nodes:C0000224 ;
        skos:altLabel    "Thiadiazines"@en ;
        skos:broader     csc:CHEMONTID_0000002 ;
        skos:definition  "Cyclic organic compounds containing a thiadiazine ring, which is a six-member unsaturated heterocycle made up of one sulfur atom and two nitrogen atoms."@en ;
        skos:inScheme    vlcs:chemische_stof ;
        skos:notation    "CHEMONTID:0000224" ;
        skos:prefLabel   "Thiadiazines"@en .

csc:CHEMONTID_0000270
        a                skos:Concept ;
        rdfs:seeAlso     tax_nodes:C0000270 ;
        skos:altLabel    "sulfonic acid derivative"@en ;
        skos:broader     csc:CHEMONTID_0004434 ;
        skos:definition  "Compounds containing a sulfonic acid or derivative, with the general structure RS(=O)2X (R=alkyl, aryl; X=any heteroatom)."@en ;
        skos:inScheme    vlcs:chemische_stof ;
        skos:notation    "CHEMONTID:0000270" ;
        skos:prefLabel   "Organosulfonic acids and derivatives"@en .

csc:CHEMONTID_0004735
        a                skos:Concept ;
        skos:altLabel    "Methylthio-1,3,5-triazines"@en ;
        skos:broader     csc:CHEMONTID_0004105 ;
        skos:definition  "Aromatic compounds containing a 1,3,5-triazine ring that is substituted at the 2-position with a methylthio group."@en ;
        skos:inScheme    vlcs:chemische_stof ;
        skos:notation    "CHEMONTID:0004735" ;
        skos:prefLabel   "Methylthio-s-triazines"@en .

csc:CHEMONTID_0001129
        a                skos:Concept ;
        skos:altLabel    "Diglycerides"@en , "diglyceride"@en , "diacylglycerol"@en , " Diacylglycerols"@en ;
        skos:broader     csc:CHEMONTID_0003809 ;
        skos:definition  "Glycerides consisting of two fatty acid chains covalently bonded to a glycerol molecule through ester linkages."@en ;
        skos:inScheme    vlcs:chemische_stof ;
        skos:notation    "CHEMONTID:0001129" ;
        skos:prefLabel   "Diacylglycerols"@en .

csc:CHEMONTID_0000445
        a                skos:Concept ;
        rdfs:seeAlso     tax_nodes:C0000445 ;
        skos:altLabel    "alkali metal molecular entity"@en , "oxoanion"@en ;
        skos:broader     csc:CHEMONTID_0000424 ;
        skos:definition  "Inorganic oxoanionic compounds in which the heaviest atom not in an oxoanion is an alkali metal."@en ;
        skos:inScheme    vlcs:chemische_stof ;
        skos:notation    "CHEMONTID:0000445" ;
        skos:prefLabel   "Alkali metal oxoanionic compounds"@en .

csc:CHEMONTID_0000491
        a                skos:Concept ;
        rdfs:seeAlso     tax_nodes:C0000491 ;
        skos:altLabel    "sulfoxides"@en , "Sulfoxides"@en , "sulfoxide"@en ;
        skos:broader     csc:CHEMONTID_0000004 ;
        skos:definition  "Compounds containing a sulfoxide functional group, with the structure RS(=O)R' (R,R' not H)."@en ;
        skos:inScheme    vlcs:chemische_stof ;
        skos:notation    "CHEMONTID:0000491" ;
        skos:prefLabel   "Sulfoxides"@en .

csc:CHEMONTID_0001816
        a                skos:Concept ;
        rdfs:seeAlso     tax_nodes:C0001816 ;
        skos:altLabel    "furofuran"@en ;
        skos:broader     csc:CHEMONTID_0000002 ;
        skos:definition  "Organic compounds containing a two furan rings fused to each other. Furan is a five-membered aromatic ring with four carbon atoms and one oxygen atom."@en ;
        skos:inScheme    vlcs:chemische_stof ;
        skos:notation    "CHEMONTID:0001816" ;
        skos:prefLabel   "Furofurans"@en .

csc:CHEMONTID_0001396
        a                skos:Concept ;
        rdfs:seeAlso     tax_nodes:C0001396 ;
        skos:altLabel    "benzoxazine"@en , "Benzoxazines"@en ;
        skos:broader     csc:CHEMONTID_0000002 ;
        skos:definition  "Organic compounds containing a benzene fused to an oxazine ring (a six-membered aliphatic ring with four carbon atoms, one oxygen atom, and one nitrogen atom)."@en ;
        skos:inScheme    vlcs:chemische_stof ;
        skos:notation    "CHEMONTID:0001396" ;
        skos:prefLabel   "Benzoxazines"@en .

csc:CHEMONTID_0002799
        a                skos:Concept ;
        rdfs:seeAlso     tax_nodes:C0002799 ;
        skos:altLabel    "organic trisulfide"@en ;
        skos:broader     csc:CHEMONTID_0000004 ;
        skos:definition  "Organosulfur compounds with the general formula RSSSR' (R,R'=alkyl, aryl)."@en ;
        skos:inScheme    vlcs:chemische_stof ;
        skos:notation    "CHEMONTID:0002799" ;
        skos:prefLabel   "Organic trisulfides"@en .

csc:CHEMONTID_0000168
        a                skos:Concept ;
        skos:altLabel    "cephems"@en , "a cephem"@en , "2,3-Didehydrocephams"@en , "cephem"@en ;
        skos:broader     csc:CHEMONTID_0000162 ;
        skos:definition  "Organic compounds containing the 5-thia-1-azabicyclo[4.2.0]oct-2-en-8-one nucleus."@en ;
        skos:inScheme    vlcs:chemische_stof ;
        skos:notation    "CHEMONTID:0000168" ;
        skos:prefLabel   "Cephems"@en .

csc:CHEMONTID_0001862
        a                skos:Concept ;
        rdfs:seeAlso     tax_nodes:C0001862 ;
        skos:altLabel    "trithiane"@en ;
        skos:broader     csc:CHEMONTID_0000002 ;
        skos:definition  "Organic compounds containing a six-member aliphatic saturated heterocycle made up of three sulfur atoms and three carbon atoms."@en ;
        skos:inScheme    vlcs:chemische_stof ;
        skos:notation    "CHEMONTID:0001862" ;
        skos:prefLabel   "Trithianes"@en .

csc:CHEMONTID_0003276
        a                skos:Concept ;
        skos:altLabel    "sulfonic acid derivative"@en , "a tosyl compound"@en ;
        skos:broader     csc:CHEMONTID_0001091 ;
        skos:definition  "Organosulfur compounds containing a tosyl group, with the general formula CH3C6H4S(O2)R (R =  any atom)."@en ;
        skos:inScheme    vlcs:chemische_stof ;
        skos:notation    "CHEMONTID:0003276" ;
        skos:prefLabel   "Tosyl compounds"@en .

csc:CHEMONTID_0000389
        a                skos:Concept ;
        rdfs:seeAlso     tax_nodes:C0000389 ;
        skos:altLabel    "oxo carboxylic acid"@en ;
        skos:broader     csc:CHEMONTID_0000264 ;
        skos:definition  "Organic compounds containing a ketone group and a carboxylic acid group."@en ;
        skos:inScheme    vlcs:chemische_stof ;
        skos:notation    "CHEMONTID:0000389" ;
        skos:prefLabel   "Keto acids and derivatives"@en .

csc:CHEMONTID_0002767
        a                skos:Concept ;
        skos:altLabel    "bromophenol"@en ;
        skos:broader     csc:CHEMONTID_0002764 ;
        skos:definition  "Bromophenols carrying a iodine at the C3 position of the benzene ring."@en ;
        skos:inScheme    vlcs:chemische_stof ;
        skos:notation    "CHEMONTID:0002767" ;
        skos:prefLabel   "M-bromophenols"@en .

csc:CHEMONTID_0000136
        a                skos:Concept ;
        skos:altLabel    "hydroquinones"@en , "Hydroquinones"@en , "a quinol"@en ;
        skos:broader     csc:CHEMONTID_0001286 ;
        skos:definition  "Compounds containing a hydroquinone moiety, which consists of a benzene ring with a hydroxyl groups at positions 1 and 4."@en ;
        skos:inScheme    vlcs:chemische_stof ;
        skos:notation    "CHEMONTID:0000136" ;
        skos:prefLabel   "Hydroquinones"@en .

csc:CHEMONTID_0002514
        a                skos:Concept ;
        skos:altLabel    "hydroxybenzoic acid"@en ;
        skos:broader     csc:CHEMONTID_0000487 ;
        skos:definition  "Ortho-hydroxylated benzoic acids."@en ;
        skos:inScheme    vlcs:chemische_stof ;
        skos:notation    "CHEMONTID:0002514" ;
        skos:prefLabel   "Salicylic acids"@en .

csc:CHEMONTID_0004472
        a                skos:Concept ;
        skos:altLabel    "ketal"@en ;
        skos:broader     csc:CHEMONTID_0001656 ;
        skos:definition  "Acetals derived from ketones by replacement of the oxo group by two hydrocarbyloxy groups R2C(OR)2 ( R not Hydrogen ). This term, once abandoned, has been reinstated as a subclass of acetals."@en ;
        skos:inScheme    vlcs:chemische_stof ;
        skos:notation    "CHEMONTID:0004472" ;
        skos:prefLabel   "Ketals"@en .

csc:CHEMONTID_0004647
        a                skos:Concept ;
        rdfs:seeAlso     tax_nodes:C0004647 ;
        skos:broader     csc:CHEMONTID_0000134 ;
        skos:definition  "Phenols that are unsubstituted at the 4-position."@en ;
        skos:inScheme    vlcs:chemische_stof ;
        skos:notation    "CHEMONTID:0004647" ;
        skos:prefLabel   "1-hydroxy-4-unsubstituted benzenoids"@en .

csc:CHEMONTID_0001585
        a                skos:Concept ;
        skos:altLabel    "sulfonamide"@en ;
        skos:broader     csc:CHEMONTID_0000270 ;
        skos:definition  "Compounds containing the sulfonamide functional group, an amide of sulfonic acid with the general structure R1S(=O)2N(R2)R3 (R1=alkyl, aryl; R2,R3=H, alkyl, aryl)."@en ;
        skos:inScheme    vlcs:chemische_stof ;
        skos:notation    "CHEMONTID:0001585" ;
        skos:prefLabel   "Organosulfonamides"@en .

csc:CHEMONTID_0004149
        a                skos:Concept ;
        rdfs:seeAlso     tax_nodes:C0004149 ;
        skos:broader     csc:CHEMONTID_0002837 ;
        skos:definition  "Polycyclic organic compounds made up only of carbon and hydrogen atoms."@en ;
        skos:inScheme    vlcs:chemische_stof ;
        skos:notation    "CHEMONTID:0004149" ;
        skos:prefLabel   "Polycyclic hydrocarbons"@en .

csc:CHEMONTID_0001553
        a                skos:Concept ;
        rdfs:seeAlso     tax_nodes:C0001553 ;
        skos:altLabel    "C30 isoprenoids (triterpenes)"@en , "triterpenoid"@en ;
        skos:broader     csc:CHEMONTID_0000259 ;
        skos:definition  "Terpene molecules containing six isoprene units."@en , "Terpene molecules containing 8 isoprene units."@en ;
        skos:inScheme    vlcs:chemische_stof ;
        skos:notation    "CHEMONTID:0001553" ;
        skos:prefLabel   "Triterpenoids"@en .

csc:CHEMONTID_0004117
        a                skos:Concept ;
        skos:altLabel    "Nitro Compounds"@en ;
        skos:broader     csc:CHEMONTID_0001152 ;
        skos:definition  "Compounds having the nitro group, -NO2 (free valence on nitrogen), which is attached to carbon."@en ;
        skos:inScheme    vlcs:chemische_stof ;
        skos:notation    "CHEMONTID:0004117" ;
        skos:prefLabel   "C-nitro compounds"@en .

csc:CHEMONTID_0001055
        a                skos:Concept ;
        rdfs:seeAlso     tax_nodes:C0001055 ;
        skos:altLabel    "inorganic hydroxy compound"@en , "p-block molecular entity"@en ;
        skos:broader     csc:CHEMONTID_0000435 ;
        skos:definition  "Inorganic non-metallic compounds containing the hydroxide group as its largest oxoanion."@en ;
        skos:inScheme    vlcs:chemische_stof ;
        skos:notation    "CHEMONTID:0001055" ;
        skos:prefLabel   "Non-metal hydroxides"@en .

csc:CHEMONTID_0002205
        a                skos:Concept ;
        skos:altLabel    "S-glycosyl compound"@en ;
        skos:broader     csc:CHEMONTID_0002105 ;
        skos:definition  "Glycoside in which a sugar group is bonded through one carbon to another group via a S-glycosidic bond."@en ;
        skos:inScheme    vlcs:chemische_stof ;
        skos:notation    "CHEMONTID:0002205" ;
        skos:prefLabel   "Thioglycosides"@en .

csc:CHEMONTID_0000546
        a                skos:Concept ;
        rdfs:seeAlso     tax_nodes:C0000546 ;
        skos:altLabel    "inorganic oxide"@en ;
        skos:broader     csc:CHEMONTID_0000457 ;
        skos:definition  "Inorganic compounds containing an oxygen atom of an oxidation state of -2, in which the heaviest atom bonded to the oxygen is an alkaline earth metal."@en ;
        skos:inScheme    vlcs:chemische_stof ;
        skos:notation    "CHEMONTID:0000546" ;
        skos:prefLabel   "Alkaline earth metal oxides"@en .

csc:CHEMONTID_0002679
        a                skos:Concept ;
        rdfs:seeAlso     tax_nodes:C0002679 ;
        skos:altLabel    "ergoline alkaloid"@en , "Ergolines"@en ;
        skos:broader     csc:CHEMONTID_0000279 ;
        skos:definition  "Compounds containing an ergoline moiety, which is structurally characterized by he presence of a 4,6,6a,7,8,9,10,10a-octahydroindolo[4,3-fg] quinoline."@en ;
        skos:inScheme    vlcs:chemische_stof ;
        skos:notation    "CHEMONTID:0002679" ;
        skos:prefLabel   "Ergoline and derivatives"@en .

csc:CHEMONTID_0000048
        a                skos:Concept ;
        rdfs:seeAlso     tax_nodes:C0000048 ;
        skos:altLabel    "tetralins"@en , "Tetrahydronaphthalenes"@en ;
        skos:broader     csc:CHEMONTID_0002448 ;
        skos:definition  "Polycyclic aromatic compounds containing a tetralin moiety, which consists of a benzene fused to a cyclohexane."@en ;
        skos:inScheme    vlcs:chemische_stof ;
        skos:notation    "CHEMONTID:0000048" ;
        skos:prefLabel   "Tetralins"@en .

csc:CHEMONTID_0001917
        a                skos:Concept ;
        skos:broader     csc:CHEMONTID_0000281 ;
        skos:definition  "Organic compounds containing a benzamide moiety with an amine group attached to the benzene ring."@en ;
        skos:inScheme    vlcs:chemische_stof ;
        skos:notation    "CHEMONTID:0001917" ;
        skos:prefLabel   "Aminobenzamides"@en .

csc:CHEMONTID_0001244
        a                skos:Concept ;
        rdfs:seeAlso     tax_nodes:C0001244 ;
        skos:altLabel    "delta-lactone"@en ;
        skos:broader     csc:CHEMONTID_0000050 ;
        skos:definition  "Cyclic organic compounds containing an oxan-2- one moiety."@en ;
        skos:inScheme    vlcs:chemische_stof ;
        skos:notation    "CHEMONTID:0001244" ;
        skos:prefLabel   "Delta valerolactones"@en .

csc:CHEMONTID_0002647
        a                skos:Concept ;
        skos:altLabel    "cyclohexanols"@en , "Cyclohexanols"@en ;
        skos:broader     csc:CHEMONTID_0001661 ;
        skos:definition  "Compounds containing an alcohol group attached to a cyclohexane ring."@en ;
        skos:inScheme    vlcs:chemische_stof ;
        skos:notation    "CHEMONTID:0002647" ;
        skos:prefLabel   "Cyclohexanols"@en .

csc:CHEMONTID_0001710
        a                skos:Concept ;
        rdfs:seeAlso     tax_nodes:C0001710 ;
        skos:broader     csc:CHEMONTID_0000238 ;
        skos:definition  "Tannins with a structure characterized by either of the following models. In model 1, the structure contains galloyl units (in some cases, shikimic acid units) are linked to diverse polyol carbohydrate-, catechin-, or triterpenoid units. In model 2, contains at least two galloyl units C-C coupled to each other, and do not contain a glycosidically linked catechin unit."@en , "Tannins with a structure characterized by either of the following models. In model 1, the structure contains galloyl units (in some cases, shikimic acid units) that are linked to diverse polyol carbohydrate-, catechin-, or triterpenoid units. In model 2, contains at least two galloyl units C-C coupled to each other, and do not contain a glycosidically linked catechin unit."@en ;
        skos:inScheme    vlcs:chemische_stof ;
        skos:notation    "CHEMONTID:0001710" ;
        skos:prefLabel   "Hydrolyzable tannins"@en .

csc:CHEMONTID_0001290
        a                skos:Concept ;
        rdfs:seeAlso     tax_nodes:C0001290 ;
        skos:altLabel    "indolyl carboxylic acid"@en ;
        skos:broader     csc:CHEMONTID_0000211 ;
        skos:definition  "Compounds containing a carboxylic acid chain (of at least 2 carbon atoms) linked to an indole ring."@en ;
        skos:inScheme    vlcs:chemische_stof ;
        skos:notation    "CHEMONTID:0001290" ;
        skos:prefLabel   "Indolyl carboxylic acids and derivatives"@en .

csc:CHEMONTID_0002693
        a                skos:Concept ;
        rdfs:seeAlso     tax_nodes:C0002693 ;
        skos:altLabel    "triazinanes"@en ;
        skos:broader     csc:CHEMONTID_0000002 ;
        skos:definition  "Compounds containing a triazinane ring, which is a six-membered saturated heterocycle with  three nitrogen ring atoms and three ring carbon atoms."@en ;
        skos:inScheme    vlcs:chemische_stof ;
        skos:notation    "CHEMONTID:0002693" ;
        skos:prefLabel   "Triazinanes"@en .

csc:CHEMONTID_0004527
        a                skos:Concept ;
        skos:broader     csc:CHEMONTID_0000475 ;
        skos:definition  "Organic compounds with the general formula RNHC(=O)CH2Cl, where R= organyl group."@en ;
        skos:inScheme    vlcs:chemische_stof ;
        skos:notation    "CHEMONTID:0004527" ;
        skos:prefLabel   "Chloroacetamides"@en .

csc:CHEMONTID_0001465
        a                skos:Concept ;
        rdfs:seeAlso     tax_nodes:C0001465 ;
        skos:altLabel    "tropane alkaloid"@en ;
        skos:broader     csc:CHEMONTID_0000279 ;
        skos:definition  "Organic compounds containing or derived from anatoxin, homoanatoxin or other analogues. Anatoxins constitute a class of potent neurotoxic alkaloids."@en ;
        skos:inScheme    vlcs:chemische_stof ;
        skos:notation    "CHEMONTID:0001465" ;
        skos:prefLabel   "Anatoxins"@en .

csc:CHEMONTID_0002868
        a                skos:Concept ;
        rdfs:seeAlso     tax_nodes:C0002868 ;
        skos:altLabel    "organohalogen compound"@en ;
        skos:broader     csc:CHEMONTID_0000267 ;
        skos:definition  "Organic compounds in which the halogen atom is bonded to an sp2-hybridised carbon atom of a carbon-carbon double bond (C=C)."@en ;
        skos:inScheme    vlcs:chemische_stof ;
        skos:notation    "CHEMONTID:0002868" ;
        skos:prefLabel   "Vinyl halides"@en .

csc:CHEMONTID_0001212
        a                skos:Concept ;
        rdfs:seeAlso     tax_nodes:C0001212 ;
        skos:altLabel    "alkanethiol"@en ;
        skos:broader     csc:CHEMONTID_0002485 ;
        skos:definition  "Organic compounds containing the thiol functional group linked to an alkyl chain."@en ;
        skos:inScheme    vlcs:chemische_stof ;
        skos:notation    "CHEMONTID:0001212" ;
        skos:prefLabel   "Alkylthiols"@en .

csc:CHEMONTID_0004748
        a                skos:Concept ;
        skos:broader     csc:CHEMONTID_0004623 ;
        skos:definition  "Organothiophosphorus compounds that contain a thiophosphoric acid O-esterified with a phenyl group."@en ;
        skos:inScheme    vlcs:chemische_stof ;
        skos:notation    "CHEMONTID:0004748" ;
        skos:prefLabel   "Phenyl thiophosphates"@en .

csc:CHEMONTID_0000458
        a                skos:Concept ;
        rdfs:seeAlso     tax_nodes:C0000458 ;
        skos:broader     csc:CHEMONTID_0000424 ;
        skos:definition  "Inorganic compounds belonging either to the post-transition metal hydrides, post-transition metal nitrides, post-transition metal oxides, or the post-transition metal sulfides."@en ;
        skos:inScheme    vlcs:chemische_stof ;
        skos:notation    "CHEMONTID:0000458" ;
        skos:prefLabel   "Post-transition metal organides"@en .

csc:CHEMONTID_0004794
        a                skos:Concept ;
        rdfs:seeAlso     tax_nodes:C0004794 ;
        skos:broader     csc:CHEMONTID_0000023 ;
        skos:definition  "Aromatic heterocyclic compounds containing a naphthalene moiety substituted at one or more positions by a chlorine atom."@en ;
        skos:inScheme    vlcs:chemische_stof ;
        skos:notation    "CHEMONTID:0004794" ;
        skos:prefLabel   "Chloronaphthalenes"@en .

csc:CHEMONTID_0003566
        a                skos:Concept ;
        rdfs:seeAlso     tax_nodes:C0003566 ;
        skos:altLabel    "a cholestanoid"@en , "a cholestane steroid"@en , "cholestanoid"@en , "Sterol Lipids"@en , "Cholestanoids"@en ;
        skos:broader     csc:CHEMONTID_0000258 ;
        skos:definition  "Steroids with a structure containing the 27-carbon cholestane skeleton."@en ;
        skos:inScheme    vlcs:chemische_stof ;
        skos:notation    "CHEMONTID:0003566" ;
        skos:prefLabel   "Cholestane steroids"@en .

csc:CHEMONTID_0002338
        a                skos:Concept ;
        rdfs:seeAlso     tax_nodes:C0002338 ;
        skos:altLabel    "organosulfur heterocyclic compound"@en ;
        skos:broader     csc:CHEMONTID_0000002 ;
        skos:definition  "Polycyclic compounds containing a thiophene ring fused to a 7 member carbocyclic moiety. Thiophene is 5-membered ring consisting of four carbon atoms and one sulfur atom."@en ;
        skos:inScheme    vlcs:chemische_stof ;
        skos:notation    "CHEMONTID:0002338" ;
        skos:prefLabel   "Cycloheptathiophenes"@en .

csc:CHEMONTID_0004716
        a                skos:Concept ;
        skos:broader     csc:CHEMONTID_0001846 ;
        skos:definition  "Organic compounds containing an acetamide group conjugated to a phenyl group, which is in turn substituted with one or more halogen atoms."@en ;
        skos:inScheme    vlcs:chemische_stof ;
        skos:notation    "CHEMONTID:0004716" ;
        skos:prefLabel   "Haloacetanilides"@en .

csc:CHEMONTID_0001401
        a                skos:Concept ;
        skos:altLabel    "p-menthane monoterpenoid"@en , "Menthane monoterpenoids"@en ;
        skos:broader     csc:CHEMONTID_0001549 ;
        skos:definition  "Monoterpenoids with a structure based on the o-, m-, or p-menthane backbone. P-menthane consists of the cyclohexane ring with a methyl group and a (2-methyl)-propyl group at the 1 and 4 ring position, respectively. The o- and m- menthanes are much rarer, and presumably arise by alkyl migration of p-menthanes."@en ;
        skos:inScheme    vlcs:chemische_stof ;
        skos:notation    "CHEMONTID:0001401" ;
        skos:prefLabel   "Menthane monoterpenoids"@en .

csc:CHEMONTID_0004296
        a                skos:Concept ;
        skos:broader     csc:CHEMONTID_0003670 ;
        skos:definition  "Aromatic compounds containing a ketone substituted by one aryl group."@en ;
        skos:inScheme    vlcs:chemische_stof ;
        skos:notation    "CHEMONTID:0004296" ;
        skos:prefLabel   "Phenylketones"@en .

csc:CHEMONTID_0000426
        a                skos:Concept ;
        rdfs:seeAlso     tax_nodes:C0000426 ;
        skos:broader     csc:CHEMONTID_0000422 ;
        skos:definition  "Inorganic compounds containing only metal atoms,with the largest atom being a transition metal atom."@en ;
        skos:inScheme    vlcs:chemische_stof ;
        skos:notation    "CHEMONTID:0000426" ;
        skos:prefLabel   "Homogeneous transition metal compounds"@en .

csc:CHEMONTID_0002384
        a                skos:Concept ;
        skos:altLabel    "benzoquinones"@en , "Benzoquinones"@en ;
        skos:broader     csc:CHEMONTID_0002495 ;
        skos:definition  "Organic compounds containing a benzene ring that carries two ketone group at the 1- and 4-positions (cyclohexa-2,5-diene-1,4-dione)."@en ;
        skos:inScheme    vlcs:chemische_stof ;
        skos:notation    "CHEMONTID:0002384" ;
        skos:prefLabel   "Benzoquinones"@en .

csc:CHEMONTID_0000472
        a                skos:Concept ;
        rdfs:seeAlso     tax_nodes:C0000472 ;
        skos:altLabel    "hydroxy carboxylic acid"@en ;
        skos:broader     csc:CHEMONTID_0000264 ;
        skos:definition  "Compounds comprising one or more hydroxy acid groups."@en ;
        skos:inScheme    vlcs:chemische_stof ;
        skos:notation    "CHEMONTID:0000472" ;
        skos:prefLabel   "Hydroxy acids and derivatives"@en .

csc:CHEMONTID_0004485
        a                skos:Concept ;
        rdfs:seeAlso     tax_nodes:C0004485 ;
        skos:altLabel    "a halocyclohexane"@en , "a halogenocyclohexane"@en , "Halogenocyclohexanes"@en , "Halocyclohexanes"@en , "a cyclohexyl halide"@en ;
        skos:broader     csc:CHEMONTID_0002867 ;
        skos:definition  "Organohalogen compounds containing a monocyclic cyclohexane moiety that is substituted at one or more positions by an halogen atom."@en ;
        skos:inScheme    vlcs:chemische_stof ;
        skos:notation    "CHEMONTID:0004485" ;
        skos:prefLabel   "Cyclohexyl halides"@en .

csc:CHEMONTID_0000195
        a                skos:Concept ;
        rdfs:seeAlso     tax_nodes:C0000195 ;
        skos:altLabel    "Piperidines"@en ;
        skos:broader     csc:CHEMONTID_0000002 ;
        skos:definition  "Compounds containing a piperidine ring, which is a saturated aliphatic six-member ring with one nitrogen atom and five carbon atoms."@en ;
        skos:inScheme    vlcs:chemische_stof ;
        skos:notation    "CHEMONTID:0000195" ;
        skos:prefLabel   "Piperidines"@en .

csc:CHEMONTID_0002320
        a                skos:Concept ;
        rdfs:seeAlso     tax_nodes:C0002320 ;
        skos:altLabel    "halophenol"@en ;
        skos:broader     csc:CHEMONTID_0000134 ;
        skos:definition  "Aromatic compounds containing benzene substituted by a hydroxyl group and a halogen atom."@en ;
        skos:inScheme    vlcs:chemische_stof ;
        skos:notation    "CHEMONTID:0002320" ;
        skos:prefLabel   "Halophenols"@en .

csc:CHEMONTID_0000163
        a                skos:Concept ;
        rdfs:seeAlso     tax_nodes:C0000163 ;
        skos:altLabel    "caprolactams"@en ;
        skos:broader     csc:CHEMONTID_0000160 ;
        skos:definition  "Cyclic amides of caproic acid. Caproic acid is the carboxylic acid derived from hexane with the general formula C5H11COOH."@en ;
        skos:inScheme    vlcs:chemische_stof ;
        skos:notation    "CHEMONTID:0000163" ;
        skos:prefLabel   "Caprolactams"@en .

csc:CHEMONTID_0004628
        a                skos:Concept ;
        rdfs:seeAlso     tax_nodes:C0004628 ;
        skos:broader     csc:CHEMONTID_0000134 ;
        skos:definition  "Phenols that carry an alkoxy group at the 4-position of the benzene ring."@en ;
        skos:inScheme    vlcs:chemische_stof ;
        skos:notation    "CHEMONTID:0004628" ;
        skos:prefLabel   "4-alkoxyphenols"@en .

csc:CHEMONTID_0000338
        a                skos:Concept ;
        skos:altLabel    "Branched fatty acids"@en , "branched-chain fatty acid"@en ;
        skos:broader     csc:CHEMONTID_0000262 ;
        skos:definition  "Fatty acids containing a branched chain."@en ;
        skos:inScheme    vlcs:chemische_stof ;
        skos:notation    "CHEMONTID:0000338" ;
        skos:prefLabel   "Branched fatty acids"@en .

csc:CHEMONTID_0001313
        a                skos:Concept ;
        rdfs:seeAlso     tax_nodes:C0001313 ;
        skos:altLabel    "p-Dioxanes"@en , "dioxanes"@en , "Para-Dioxanes"@en ;
        skos:broader     csc:CHEMONTID_0000368 ;
        skos:definition  "Organic compounds containing 1,4-dioxane, an aliphatic six-member ring with two oxygen atoms in ring positions 1 and 4."@en ;
        skos:inScheme    vlcs:chemische_stof ;
        skos:notation    "CHEMONTID:0001313" ;
        skos:prefLabel   "1,4-dioxanes"@en .

csc:CHEMONTID_0004674
        a                skos:Concept ;
        skos:broader     csc:CHEMONTID_0004676 ;
        skos:definition  "Aromatic compounds containing a phenoxypropionic acid that is para-substituted with an aryl group."@en ;
        skos:inScheme    vlcs:chemische_stof ;
        skos:notation    "CHEMONTID:0004674" ;
        skos:prefLabel   "Aryloxyphenoxypropionic acids"@en .

csc:CHEMONTID_0001534
        a                skos:Concept ;
        rdfs:seeAlso     tax_nodes:C0001534 ;
        skos:altLabel    "lipid"@en , "Quinones and hydroquinones"@en ;
        skos:broader     csc:CHEMONTID_0000259 ;
        skos:definition  "Lipids structurally characterized by the presence of a quinone or hydroquinone moiety."@en ;
        skos:inScheme    vlcs:chemische_stof ;
        skos:notation    "CHEMONTID:0001534" ;
        skos:prefLabel   "Quinone and hydroquinone lipids"@en .

csc:CHEMONTID_0001755
        a                skos:Concept ;
        skos:altLabel    "diterpene glycoside"@en ;
        skos:broader     csc:CHEMONTID_0002049 ;
        skos:definition  "Diterpenoids in which an isoprene unit is glycosylated."@en ;
        skos:inScheme    vlcs:chemische_stof ;
        skos:notation    "CHEMONTID:0001755" ;
        skos:prefLabel   "Diterpene glycosides"@en .

csc:CHEMONTID_0004144
        a                skos:Concept ;
        rdfs:seeAlso     tax_nodes:C0004144 ;
        skos:broader     csc:CHEMONTID_0000002 ;
        skos:definition  "Compounds containing an aromatic ring where a carbon atom is linked to an hetero atom."@en ;
        skos:inScheme    vlcs:chemische_stof ;
        skos:notation    "CHEMONTID:0004144" ;
        skos:prefLabel   "Heteroaromatic compounds"@en .

csc:CHEMONTID_0002485
        a                skos:Concept ;
        rdfs:seeAlso     tax_nodes:C0002485 ;
        skos:altLabel    "thiols"@en , "Sulfhydryl Compounds"@en , "a mercaptan"@en , "thiol"@en , "Mercapto Compounds"@en , "Mercaptans"@en ;
        skos:broader     csc:CHEMONTID_0000004 ;
        skos:definition  "Organic compounds containing a functional group with the structure RSH (R = organyl)."@en ;
        skos:inScheme    vlcs:chemische_stof ;
        skos:notation    "CHEMONTID:0002485" ;
        skos:prefLabel   "Thiols"@en .

csc:CHEMONTID_0003460
        a                skos:Concept ;
        skos:altLabel    "trialkyl phosphate"@en ;
        skos:broader     csc:CHEMONTID_0003457 ;
        skos:definition  "Organic compounds containing a phosphate group that is linked to exactly three alkyl chains."@en ;
        skos:inScheme    vlcs:chemische_stof ;
        skos:notation    "CHEMONTID:0003460" ;
        skos:prefLabel   "Trialkyl phosphates"@en .

csc:CHEMONTID_0000029
        a                skos:Concept ;
        rdfs:seeAlso     tax_nodes:C0000029 ;
        skos:broader     csc:CHEMONTID_0000261 ;
        skos:definition  "Organic aromatic compounds containing a cinnamlaldehyde moiety, consisting of a benzene and an aldehyde group to form 3-phenylprop-2-enal."@en ;
        skos:inScheme    vlcs:chemische_stof ;
        skos:notation    "CHEMONTID:0000029" ;
        skos:prefLabel   "Cinnamaldehydes"@en .

csc:CHEMONTID_0002951
        a                skos:Concept ;
        skos:altLabel    "long-chain fatty alcohol"@en , "a long-chain alcohol"@en , "long-chain alcohol"@en , "long chain alcohols"@en , "long-chain alcohols"@en ;
        skos:broader     csc:CHEMONTID_0001334 ;
        skos:definition  "Fatty alcohols that have an aliphatic tail of 13 to 21 carbon atoms."@en ;
        skos:inScheme    vlcs:chemische_stof ;
        skos:notation    "CHEMONTID:0002951" ;
        skos:prefLabel   "Long-chain fatty alcohols"@en .

csc:CHEMONTID_0000320
        a                skos:Concept ;
        rdfs:seeAlso     tax_nodes:C0000320 ;
        skos:altLabel    "Dibenzazepines"@en , "Iminostilbenes"@en , "an iminostilbene"@en , "Dibenzoazepines"@en ;
        skos:broader     csc:CHEMONTID_0000293 ;
        skos:definition  "Compounds with two benzene rings connected by an azepine ring. Azepine is an unsaturated seven-member heterocycle with one nitrogen atom replacing a carbon atom."@en ;
        skos:inScheme    vlcs:chemische_stof ;
        skos:notation    "CHEMONTID:0000320" ;
        skos:prefLabel   "Dibenzazepines"@en .

csc:CHEMONTID_0001723
        a                skos:Concept ;
        skos:altLabel    "wax ester"@en ;
        skos:broader     csc:CHEMONTID_0000324 ;
        skos:definition  "Mixtures of long-chain apolar lipids. They are usually esters of an alcohol other than glycerol and a long chain acid."@en ;
        skos:inScheme    vlcs:chemische_stof ;
        skos:notation    "CHEMONTID:0001723" ;
        skos:prefLabel   "Wax esters"@en .

csc:CHEMONTID_0004112
        a                skos:Concept ;
        rdfs:seeAlso     tax_nodes:C0004112 ;
        skos:broader     csc:CHEMONTID_0002279 ;
        skos:definition  "Organic compounds containing two benzoyl groups O-linked to each other via a peroxide group. Their skeleton has the general formula [C6H5C(O)]2O2."@en ;
        skos:inScheme    vlcs:chemische_stof ;
        skos:notation    "CHEMONTID:0004112" ;
        skos:prefLabel   "Benzoyl peroxides"@en .

csc:CHEMONTID_0000075
        a                skos:Concept ;
        rdfs:seeAlso     tax_nodes:C0000075 ;
        skos:altLabel    "Pyrimidines"@en ;
        skos:broader     csc:CHEMONTID_0001346 ;
        skos:definition  "Compounds containing a pyrimidne ring, which is a six-member aromatic heterocycle which consists of two nitrogen atoms (at positions 1 and 3) and four carbon atoms."@en ;
        skos:inScheme    vlcs:chemische_stof ;
        skos:notation    "CHEMONTID:0000075" ;
        skos:prefLabel   "Pyrimidines and pyrimidine derivatives"@en .

csc:CHEMONTID_0004831
        a                skos:Concept ;
        skos:altLabel    "oligopeptide"@en , "Oligopeptides"@en , "alpha-oligopeptides"@en ;
        skos:broader     csc:CHEMONTID_0000348 ;
        skos:definition  "Organic compounds containing a sequence of between three and ten alpha-amino acids joined by peptide bonds."@en ;
        skos:inScheme    vlcs:chemische_stof ;
        skos:notation    "CHEMONTID:0004831" ;
        skos:prefLabel   "Oligopeptides"@en .

csc:CHEMONTID_0000716
        a                skos:Concept ;
        rdfs:seeAlso     tax_nodes:C0000716 ;
        skos:altLabel    "chlorins"@en ;
        skos:broader     csc:CHEMONTID_0001455 ;
        skos:definition  "Large heterocyclic aromatic ring systems consisting, at the core, of three pyrroles and one pyrroline coupled through four methine linkages."@en ;
        skos:inScheme    vlcs:chemische_stof ;
        skos:notation    "CHEMONTID:0000716" ;
        skos:prefLabel   "Chlorins"@en .

csc:CHEMONTID_0000296
        a                skos:Concept ;
        rdfs:seeAlso     tax_nodes:C0000296 ;
        skos:altLabel    "Benzodioxoles"@en ;
        skos:broader     csc:CHEMONTID_0000002 ;
        skos:definition  "Organic compounds containing a benzene ring fused to either isomers of dioxole. Dioxole is a five-membered unsaturated ring of two oxygen atoms and three carbon atoms."@en ;
        skos:inScheme    vlcs:chemische_stof ;
        skos:notation    "CHEMONTID:0000296" ;
        skos:prefLabel   "Benzodioxoles"@en .

csc:CHEMONTID_0002421
        a                skos:Concept ;
        skos:altLabel    "a naphthoic acid"@en , "naphthoic acid"@en , "Naphthoic acids"@en ;
        skos:broader     csc:CHEMONTID_0001871 ;
        skos:definition  "Compounds containing a naphthalene moiety, which bears a carboxylic acid group one or more positions. Naphthalene is a bicyclic compound that is made up of two fused benzene ring."@en ;
        skos:inScheme    vlcs:chemische_stof ;
        skos:notation    "CHEMONTID:0002421" ;
        skos:prefLabel   "Naphthalenecarboxylic acids"@en .

csc:CHEMONTID_0000218
        a                skos:Concept ;
        rdfs:seeAlso     tax_nodes:C0000218 ;
        skos:altLabel    "Pyrrolidines"@en ;
        skos:broader     csc:CHEMONTID_0000002 ;
        skos:definition  "Compounds containing a pyrrolidine ring, which is a five-membered saturated aliphatic heterocycle with one nitrogen atom and four carbon atoms."@en ;
        skos:inScheme    vlcs:chemische_stof ;
        skos:notation    "CHEMONTID:0000218" ;
        skos:prefLabel   "Pyrrolidines"@en .

csc:CHEMONTID_0000264
        a                skos:Concept ;
        rdfs:seeAlso     tax_nodes:C0000264 ;
        skos:broader     csc:CHEMONTID_0000000 ;
        skos:definition  "Compounds an organic acid or a derivative thereof."@en ;
        skos:inScheme    vlcs:chemische_stof ;
        skos:notation    "CHEMONTID:0000264" ;
        skos:prefLabel   "Organic acids and derivatives"@en .

csc:CHEMONTID_0000011
        a                skos:Concept ;
        rdfs:seeAlso     tax_nodes:C0000011 ;
        skos:altLabel    "carbohydrates and carbohydrate derivatives"@en , "carbohydrates"@en , "Carbohydrates"@en ;
        skos:broader     csc:CHEMONTID_0000323 ;
        skos:definition  "Monosaccharides, disaccharides, oligosaccharides, polysaccharides, and their derivatives."@en ;
        skos:inScheme    vlcs:chemische_stof ;
        skos:notation    "CHEMONTID:0000011" ;
        skos:prefLabel   "Carbohydrates and carbohydrate conjugates"@en .

csc:CHEMONTID_0002817
        a                skos:Concept ;
        skos:altLabel    "dibenzopyran"@en ;
        skos:broader     csc:CHEMONTID_0003410 ;
        skos:definition  "Organic heterocyclic compounds with a structure containing a dibenzopyran moiety, made up of two benzene rings fused to a central pyran ring."@en ;
        skos:inScheme    vlcs:chemische_stof ;
        skos:notation    "CHEMONTID:0002817" ;
        skos:prefLabel   "Dibenzopyrans"@en .

csc:CHEMONTID_0004056
        a                skos:Concept ;
        skos:altLabel    "Pentavalent organic arsenicals"@en ;
        skos:broader     csc:CHEMONTID_0000405 ;
        skos:definition  "Organoarsenic compounds in which a carbon is linked to a pentavalent arsenic atom."@en ;
        skos:inScheme    vlcs:chemische_stof ;
        skos:notation    "CHEMONTID:0004056" ;
        skos:prefLabel   "Pentavalent organic arsenic compounds"@en .

csc:CHEMONTID_0002319
        a                skos:Concept ;
        rdfs:seeAlso     tax_nodes:C0002319 ;
        skos:altLabel    "benzoate ester"@en , "phenols"@en ;
        skos:broader     csc:CHEMONTID_0002448 ;
        skos:definition  "Aromatic compounds containing a benzene ring substituted by a hydroxyl group and an ester group."@en ;
        skos:inScheme    vlcs:chemische_stof ;
        skos:notation    "CHEMONTID:0002319" ;
        skos:prefLabel   "Phenol esters"@en .

csc:CHEMONTID_0000485
        a                skos:Concept ;
        skos:altLabel    "Quinazolines"@en , "1,3-diazanaphthalenes"@en , "quinazolines"@en ;
        skos:broader     csc:CHEMONTID_0004789 ;
        skos:definition  "Compounds containing a quinazoline moiety, which is made up of two fused six-member aromatic rings, a benzene ring and a pyrimidine ring."@en ;
        skos:inScheme    vlcs:chemische_stof ;
        skos:notation    "CHEMONTID:0000485" ;
        skos:prefLabel   "Quinazolines"@en .

csc:CHEMONTID_0002863
        a                skos:Concept ;
        rdfs:seeAlso     tax_nodes:C0002863 ;
        skos:altLabel    "organochlorine compound"@en ;
        skos:broader     csc:CHEMONTID_0002868 ;
        skos:definition  "Vinyl halides in which a chlorine atom is bonded to an sp2-hybridised carbon atom."@en ;
        skos:inScheme    vlcs:chemische_stof ;
        skos:notation    "CHEMONTID:0002863" ;
        skos:prefLabel   "Vinyl chlorides"@en .

csc:CHEMONTID_0001460
        a                skos:Concept ;
        rdfs:seeAlso     tax_nodes:C0001460 ;
        skos:altLabel    "vitamin D"@en ;
        skos:broader     csc:CHEMONTID_0000258 ;
        skos:definition  "Compounds containing a secosteroid backbone, usually secoergostane or secocholestane."@en ;
        skos:inScheme    vlcs:chemische_stof ;
        skos:notation    "CHEMONTID:0001460" ;
        skos:prefLabel   "Vitamin D and derivatives"@en .

csc:CHEMONTID_0001888
        a                skos:Concept ;
        rdfs:seeAlso     tax_nodes:C0001888 ;
        skos:altLabel    "sultone"@en ;
        skos:broader     csc:CHEMONTID_0000106 ;
        skos:definition  "Organic compounds containing a gamma-sultone, a Intramolecular cyclic ester of hydroxy sulfonic acid, with a SO ring bond, and three ring carbon atoms."@en ;
        skos:inScheme    vlcs:chemische_stof ;
        skos:notation    "CHEMONTID:0001888" ;
        skos:prefLabel   "Gamma sultones"@en .

csc:CHEMONTID_0004024
        a                skos:Concept ;
        rdfs:seeAlso     tax_nodes:C0004024 ;
        skos:altLabel    "organolead compound"@en ;
        skos:broader     csc:CHEMONTID_0001523 ;
        skos:definition  "Compounds containing bond between a carbon atom and a lead atom."@en ;
        skos:inScheme    vlcs:chemische_stof ;
        skos:notation    "CHEMONTID:0004024" ;
        skos:prefLabel   "Organolead compounds"@en .

csc:CHEMONTID_0000453
        a                skos:Concept ;
        rdfs:seeAlso     tax_nodes:C0000453 ;
        skos:broader     csc:CHEMONTID_0000423 ;
        skos:definition  "Inorganic compounds belonging to either of the other non-metal Hydrides, other non-metal nitrides, other non-metal oxides, or the other non-metal sulfides."@en ;
        skos:inScheme    vlcs:chemische_stof ;
        skos:notation    "CHEMONTID:0000453" ;
        skos:prefLabel   "Other non-metal organides"@en .

csc:CHEMONTID_0003095
        a                skos:Concept ;
        skos:altLabel    "21-hydroxy steroid"@en ;
        skos:broader     csc:CHEMONTID_0001295 ;
        skos:definition  "Steroids carrying a hydroxyl group at the 21-position of the steroid backbone."@en ;
        skos:inScheme    vlcs:chemische_stof ;
        skos:notation    "CHEMONTID:0003095" ;
        skos:prefLabel   "21-hydroxysteroids"@en .

csc:CHEMONTID_0000200
        a                skos:Concept ;
        skos:altLabel    "Xanthenes"@en ;
        skos:broader     csc:CHEMONTID_0002817 ;
        skos:definition  "Polycyclic aromatic compounds containing a xanthene moiety, which consists of two benzene rings joined to each other by a pyran ring."@en ;
        skos:inScheme    vlcs:chemische_stof ;
        skos:notation    "CHEMONTID:0000200" ;
        skos:prefLabel   "Xanthenes"@en .

csc:CHEMONTID_0001603
        a                skos:Concept ;
        skos:altLabel    "a 2-monoglyceride"@en , "2-monoglyceride"@en , "a 2-monoacylglycerol"@en , "2-monoglycerides"@en , "2-acylglycerol"@en ;
        skos:broader     csc:CHEMONTID_0001133 ;
        skos:definition  "Monoacylglycerols containing a glycerol acylated at the 2-position."@en ;
        skos:inScheme    vlcs:chemische_stof ;
        skos:notation    "CHEMONTID:0001603" ;
        skos:prefLabel   "2-monoacylglycerols"@en .

csc:CHEMONTID_0001183
        a                skos:Concept ;
        rdfs:seeAlso     tax_nodes:C0001183 ;
        skos:altLabel    "sulfamides"@en ;
        skos:broader     csc:CHEMONTID_0000403 ;
        skos:definition  "Organic compounds containing the sulfuric acid diamide functional group, with the generic structure R1N(R2)S(=O)(=O)ON(R3)R4 (R1-R4 = H or organyl."@en ;
        skos:inScheme    vlcs:chemische_stof ;
        skos:notation    "CHEMONTID:0001183" ;
        skos:prefLabel   "Sulfuric acid diamides"@en .

csc:CHEMONTID_0003017
        a                skos:Concept ;
        skos:altLabel    "organonitrogen heterocyclic compound"@en , "polycyclic heteroarene"@en ;
        skos:broader     csc:CHEMONTID_0000274 ;
        skos:definition  "Organic heterocyclic compounds with a structure characterized by a benzene ring fused to an acridine ring system."@en ;
        skos:inScheme    vlcs:chemische_stof ;
        skos:notation    "CHEMONTID:0003017" ;
        skos:prefLabel   "Benzacridines"@en .

csc:CHEMONTID_0004711
        a                skos:Concept ;
        rdfs:seeAlso     tax_nodes:C0004711 ;
        skos:altLabel    "a 2-benzimidazolylcarbamic acid ester"@en ;
        skos:broader     csc:CHEMONTID_0000294 ;
        skos:definition  "Aromatic heteropolycyclic compounds that contain a carbamic acid ester group, which is N-linked to the C2-atom of a benzimidazole moiety."@en ;
        skos:inScheme    vlcs:chemische_stof ;
        skos:notation    "CHEMONTID:0004711" ;
        skos:prefLabel   "2-benzimidazolylcarbamic acid esters"@en .

csc:CHEMONTID_0001105
        a                skos:Concept ;
        skos:altLabel    "benzenedicarboxylic acid"@en ;
        skos:broader     csc:CHEMONTID_0000176 ;
        skos:definition  "Compounds containing a phthalic acid moiety (or a derivative thereof), which is a benzene ring bearing a carboxylic acid group at two different ring positions. Isomers of phthalic acid include meta-phthalic acid (benzene-1,3-dioic acid), ortho-phthalic acid (benzene-1,2-dioic acid), and para-phthalic acid (benzene-1,4-dioic acid)."@en ;
        skos:inScheme    vlcs:chemische_stof ;
        skos:notation    "CHEMONTID:0001105" ;
        skos:prefLabel   "Phthalic acid and derivatives"@en .

csc:CHEMONTID_0000176
        a                skos:Concept ;
        rdfs:seeAlso     tax_nodes:C0000176 ;
        skos:broader     csc:CHEMONTID_0002279 ;
        skos:definition  "Organic compounds containing a carboxylic acid substituent attached to a benzene ring."@en ;
        skos:inScheme    vlcs:chemische_stof ;
        skos:notation    "CHEMONTID:0000176" ;
        skos:prefLabel   "Benzoic acids and derivatives"@en .

csc:CHEMONTID_0001151
        a                skos:Concept ;
        rdfs:seeAlso     tax_nodes:C0001151 ;
        skos:altLabel    "indanones"@en ;
        skos:broader     csc:CHEMONTID_0000027 ;
        skos:definition  "Compounds containing an indane ring bearing a ketone group."@en ;
        skos:inScheme    vlcs:chemische_stof ;
        skos:notation    "CHEMONTID:0001151" ;
        skos:prefLabel   "Indanones"@en .

csc:CHEMONTID_0001326
        a                skos:Concept ;
        skos:altLabel    "phosphoramide"@en ;
        skos:broader     csc:CHEMONTID_0001322 ;
        skos:definition  "Compounds containing a pyridine ring bearing a carboxamide."@en ;
        skos:inScheme    vlcs:chemische_stof ;
        skos:notation    "CHEMONTID:0001326" ;
        skos:prefLabel   "Pyridinecarboxamides"@en .

csc:CHEMONTID_0000895
        a                skos:Concept ;
        rdfs:seeAlso     tax_nodes:C0000895 ;
        skos:altLabel    "alkali metal salt"@en ;
        skos:broader     csc:CHEMONTID_0000445 ;
        skos:definition  "Inorganic compounds in which the largest oxoanion is borate, and in which the heaviest atom not in an oxoanion is an alkali metal."@en ;
        skos:inScheme    vlcs:chemische_stof ;
        skos:notation    "CHEMONTID:0000895" ;
        skos:prefLabel   "Alkali metal borates"@en .

csc:CHEMONTID_0004434
        a                skos:Concept ;
        rdfs:seeAlso     tax_nodes:C0004434 ;
        skos:broader     csc:CHEMONTID_0000264 ;
        skos:definition  "Compounds containing a sulfonic acid or derivative, with the general structure RS(=O)2X (R= H or organyl group, X=any heteroatom)."@en ;
        skos:inScheme    vlcs:chemische_stof ;
        skos:notation    "CHEMONTID:0004434" ;
        skos:prefLabel   "Organic sulfonic acids and derivatives"@en .

csc:CHEMONTID_0003031
        a                skos:Concept ;
        skos:altLabel    "a pyrrolidin-2-one"@en , "pyrrolidin-2-ones"@en ;
        skos:broader     csc:CHEMONTID_0001158 ;
        skos:definition  "Pyrrolidines which bear a C=O group at position 2 of the pyrrolidine ring."@en ;
        skos:inScheme    vlcs:chemische_stof ;
        skos:notation    "CHEMONTID:0003031" ;
        skos:prefLabel   "Pyrrolidine-2-ones"@en .

csc:CHEMONTID_0003459
        a                skos:Concept ;
        skos:altLabel    "dialkyl phosphate"@en ;
        skos:broader     csc:CHEMONTID_0003457 ;
        skos:definition  "Organic compounds containing a phosphate group that is linked to exactly two alkyl chain."@en ;
        skos:inScheme    vlcs:chemische_stof ;
        skos:notation    "CHEMONTID:0003459" ;
        skos:prefLabel   "Dialkyl phosphates"@en .

csc:CHEMONTID_0004189
        a                skos:Concept ;
        rdfs:seeAlso     tax_nodes:C0004189 ;
        skos:altLabel    "Phthalanes"@en , "1,3-dihydroisobenzofurans"@en ;
        skos:broader     csc:CHEMONTID_0000002 ;
        skos:definition  "Compounds containing the coumaran skeleton, which consists of a benzene ring fused to a 2,3-dihydrofuran ring."@en ;
        skos:inScheme    vlcs:chemische_stof ;
        skos:notation    "CHEMONTID:0004189" ;
        skos:prefLabel   "Coumarans"@en .

csc:CHEMONTID_0000190
        a                skos:Concept ;
        rdfs:seeAlso     tax_nodes:C0000190 ;
        skos:altLabel    "phenols"@en ;
        skos:broader     csc:CHEMONTID_0000134 ;
        skos:definition  "Compounds containing a methoxy group attached to the benzene ring of a phenol moiety."@en ;
        skos:inScheme    vlcs:chemische_stof ;
        skos:notation    "CHEMONTID:0000190" ;
        skos:prefLabel   "Methoxyphenols"@en .

csc:CHEMONTID_0003971
        a                skos:Concept ;
        skos:altLabel    "pyridines"@en , "organohalogen compound"@en ;
        skos:broader     csc:CHEMONTID_0003970 ;
        skos:definition  "Organic compounds containing a pyridine ring substituted at two or more positions by a halogen atom."@en ;
        skos:inScheme    vlcs:chemische_stof ;
        skos:notation    "CHEMONTID:0003971" ;
        skos:prefLabel   "Polyhalopyridines"@en .

csc:CHEMONTID_0000365
        a                skos:Concept ;
        rdfs:seeAlso     tax_nodes:C0000365 ;
        skos:altLabel    "Cyclamates"@en , "sulfamic acids"@en ;
        skos:broader     csc:CHEMONTID_0000039 ;
        skos:definition  "Compounds containing a cyclohexylsulfamic acid moiety."@en ;
        skos:inScheme    vlcs:chemische_stof ;
        skos:notation    "CHEMONTID:0000365" ;
        skos:prefLabel   "Cyclamates"@en .

csc:CHEMONTID_0000112
        a                skos:Concept ;
        rdfs:seeAlso     tax_nodes:C0000112 ;
        skos:altLabel    "hydrazines"@en ;
        skos:broader     csc:CHEMONTID_0000278 ;
        skos:definition  "Compounds comprising the hydrazine functional group, with the general formula R1R2NNR3R4."@en ;
        skos:inScheme    vlcs:chemische_stof ;
        skos:notation    "CHEMONTID:0000112" ;
        skos:prefLabel   "Hydrazines and derivatives"@en .

csc:CHEMONTID_0001515
        a                skos:Concept ;
        rdfs:seeAlso     tax_nodes:C0001515 ;
        skos:altLabel    "organobromine compound"@en ;
        skos:broader     csc:CHEMONTID_0000267 ;
        skos:definition  "Compounds containing a chemical bond between a carbon atom and a bromine atom."@en ;
        skos:inScheme    vlcs:chemische_stof ;
        skos:notation    "CHEMONTID:0001515" ;
        skos:prefLabel   "Organobromides"@en .

csc:CHEMONTID_0004157
        a                skos:Concept ;
        rdfs:seeAlso     tax_nodes:C0004157 ;
        skos:altLabel    "halomethane"@en ;
        skos:broader     csc:CHEMONTID_0002867 ;
        skos:definition  "Organic compounds in which at least one of the four hydrogen atoms of methane (CH4) are replaced by halogen atoms."@en ;
        skos:inScheme    vlcs:chemische_stof ;
        skos:notation    "CHEMONTID:0004157" ;
        skos:prefLabel   "Halomethanes"@en .

csc:CHEMONTID_0004623
        a                skos:Concept ;
        skos:broader     csc:CHEMONTID_0001572 ;
        skos:definition  "Organic compounds containing the thiophosphoric acid functional group or a derivative thereof, with the general structure ROP(OR')(OR'')=S, where at least one R-group is an aryl group."@en ;
        skos:inScheme    vlcs:chemische_stof ;
        skos:notation    "CHEMONTID:0004623" ;
        skos:prefLabel   "Aryl thiophosphates"@en .

csc:CHEMONTID_0000333
        a                skos:Concept ;
        skos:altLabel    "Straight chain fatty acids"@en , "straight-chain fatty acid"@en ;
        skos:broader     csc:CHEMONTID_0000262 ;
        skos:definition  "Fatty acids with a straight aliphatic chain."@en ;
        skos:inScheme    vlcs:chemische_stof ;
        skos:notation    "CHEMONTID:0000333" ;
        skos:prefLabel   "Straight chain fatty acids"@en .

csc:CHEMONTID_0002466
        a                skos:Concept ;
        rdfs:seeAlso     tax_nodes:C0002466 ;
        skos:altLabel    "organophosphorus compound"@en , "organonitrogen heterocyclic compound"@en ;
        skos:broader     csc:CHEMONTID_0000002 ;
        skos:definition  "Organic heterocyclic compounds containing an oxazaphosphinane ring, which consists of three carbon atoms, one nitrogen atom, and one phosphorus atom."@en ;
        skos:inScheme    vlcs:chemische_stof ;
        skos:notation    "CHEMONTID:0002466" ;
        skos:prefLabel   "Oxazaphosphinanes"@en .

csc:CHEMONTID_0001238
        a                skos:Concept ;
        skos:altLabel    "A carboxylic ester"@en , "carboxylic ester"@en ;
        skos:broader     csc:CHEMONTID_0001093 ;
        skos:definition  "Carboxylic acid derivatives in which the carbon atom from the carbonyl group is attached to an alkyl or an aryl moiety through an oxygen atom (forming an ester group)."@en ;
        skos:inScheme    vlcs:chemische_stof ;
        skos:notation    "CHEMONTID:0001238" ;
        skos:prefLabel   "Carboxylic acid esters"@en .

csc:CHEMONTID_0000554
        a                skos:Concept ;
        rdfs:seeAlso     tax_nodes:C0000554 ;
        skos:altLabel    "inorganic oxide"@en ;
        skos:broader     csc:CHEMONTID_0000453 ;
        skos:definition  "Inorganic compounds containing an oxygen atom of an oxidation state of -2, in which the heaviest atom bonded to the oxygen belongs to the class of 'other non-metals'."@en ;
        skos:inScheme    vlcs:chemische_stof ;
        skos:notation    "CHEMONTID:0000554" ;
        skos:prefLabel   "Other non-metal oxides"@en .

csc:CHEMONTID_0000301
        a                skos:Concept ;
        rdfs:seeAlso     tax_nodes:C0000301 ;
        skos:altLabel    "Benzofurans"@en , "Coumarones"@en ;
        skos:broader     csc:CHEMONTID_0000002 ;
        skos:definition  "Organic compounds containing a benzene ring fused to a furan. Furan is a five-membered aromatic ring with four carbon atoms and one oxygen atom."@en ;
        skos:inScheme    vlcs:chemische_stof ;
        skos:notation    "CHEMONTID:0000301" ;
        skos:prefLabel   "Benzofurans"@en .

csc:CHEMONTID_0000056
        a                skos:Concept ;
        rdfs:seeAlso     tax_nodes:C0000056 ;
        skos:altLabel    "Quinolones"@en , "quinolone"@en ;
        skos:broader     csc:CHEMONTID_0001253 ;
        skos:definition  "Compounds containing a quinoline moiety which bears a ketone group."@en ;
        skos:inScheme    vlcs:chemische_stof ;
        skos:notation    "CHEMONTID:0000056" ;
        skos:prefLabel   "Quinolones and derivatives"@en .

csc:CHEMONTID_0002434
        a                skos:Concept ;
        skos:altLabel    "aldehyde"@en ;
        skos:broader     csc:CHEMONTID_0000124 ;
        skos:definition  "Aldehydes with the general formula HC(H)(R)C(=O)H, where R is an organyl group."@en ;
        skos:inScheme    vlcs:chemische_stof ;
        skos:notation    "CHEMONTID:0002434" ;
        skos:prefLabel   "Alpha-hydrogen aldehydes"@en .

csc:CHEMONTID_0004812
        a                skos:Concept ;
        rdfs:seeAlso     tax_nodes:C0004812 ;
        skos:altLabel    "acenaphthylenes"@en ;
        skos:broader     csc:CHEMONTID_0002448 ;
        skos:definition  "Aromatic polycyclic compounds containing an acenaphthylene moiety. Acenaphthylene is a carbotricyclic compound, consisting of a naphthalene with positions C1 and C8 connected by an ethylene bridge."@en ;
        skos:inScheme    vlcs:chemische_stof ;
        skos:notation    "CHEMONTID:0004812" ;
        skos:prefLabel   "Acenaphthylenes"@en .

csc:CHEMONTID_0000522
        a                skos:Concept ;
        rdfs:seeAlso     tax_nodes:C0000522 ;
        skos:altLabel    "actinoid molecular entity"@en , "inorganic oxide"@en ;
        skos:broader     csc:CHEMONTID_0000455 ;
        skos:definition  "Inorganic compounds containing an oxygen atom of an oxidation state of -2, in which the heaviest atom bonded to the oxygen is an actinide."@en ;
        skos:inScheme    vlcs:chemische_stof ;
        skos:notation    "CHEMONTID:0000522" ;
        skos:prefLabel   "Actinide oxides"@en .

csc:CHEMONTID_0001925
        a                skos:Concept ;
        skos:altLabel    "sulfonamide"@en , "benzenes"@en ;
        skos:broader     csc:CHEMONTID_0000031 ;
        skos:definition  "Organic compounds containing a benzenesulfonamide moiety with an amine group attached to the benzene ring."@en ;
        skos:inScheme    vlcs:chemische_stof ;
        skos:notation    "CHEMONTID:0001925" ;
        skos:prefLabel   "Aminobenzenesulfonamides"@en .

csc:CHEMONTID_0001252
        a                skos:Concept ;
        skos:altLabel    "indole-3-acetic acids"@en ;
        skos:broader     csc:CHEMONTID_0001290 ;
        skos:definition  "Compounds containing an acetic acid (or a derivative) linked to the C3 carbon atom of an indole."@en ;
        skos:inScheme    vlcs:chemische_stof ;
        skos:notation    "CHEMONTID:0001252" ;
        skos:prefLabel   "Indole-3-acetic acid derivatives"@en .

csc:CHEMONTID_0003630
        a                skos:Concept ;
        rdfs:seeAlso     tax_nodes:C0003630 ;
        skos:altLabel    "dipolar compound"@en ;
        skos:broader     csc:CHEMONTID_0000000 ;
        skos:definition  "Electrically neutral organic molecules carrying a positive and a negative charge in one of their major canonical descriptions. In most dipolar compounds the charges are delocalized; however the term is also applied to species where this is not the case. The term 1,3-dipolar compounds is used for those in which a significant canonical resonance form can be represented by a separation of charge over three atoms (in connection with 1,3-dipolar cycloadditions)."@en ;
        skos:inScheme    vlcs:chemische_stof ;
        skos:notation    "CHEMONTID:0003630" ;
        skos:prefLabel   "Organic 1,3-dipolar compounds"@en .

csc:CHEMONTID_0002402
        a                skos:Concept ;
        skos:altLabel    "N-acyl-amino acid"@en ;
        skos:broader     csc:CHEMONTID_0001189 ;
        skos:definition  "Compounds containing an alpha amino acid which bears an acyl group at its terminal nitrogen atom."@en ;
        skos:inScheme    vlcs:chemische_stof ;
        skos:notation    "CHEMONTID:0002402" ;
        skos:prefLabel   "N-acyl-alpha amino acids"@en .

csc:CHEMONTID_0003385
        a                skos:Concept ;
        rdfs:seeAlso     tax_nodes:C0003385 ;
        skos:altLabel    "organic thiophosphate"@en ;
        skos:broader     csc:CHEMONTID_0000264 ;
        skos:definition  "Organic compounds that contain dithiophosphoric acid or a derivative thereof, with the general formula ROP(S)(=S)OR', (R,R'=H, or organyl group)."@en ;
        skos:inScheme    vlcs:chemische_stof ;
        skos:notation    "CHEMONTID:0003385" ;
        skos:prefLabel   "Organic dithiophosphoric acids and derivatives"@en .

csc:CHEMONTID_0004788
        a                skos:Concept ;
        rdfs:seeAlso     tax_nodes:C0004788 ;
        skos:broader     csc:CHEMONTID_0000002 ;
        skos:definition  "Aromatic heterocyclic chemical compounds containing a naphthalene derivative, where two carbon atoms are replaced by nitrogen atoms. They are subdivided in benzodiazines and naphthyridines."@en ;
        skos:inScheme    vlcs:chemische_stof ;
        skos:notation    "CHEMONTID:0004788" ;
        skos:prefLabel   "Diazanaphthalenes"@en .

csc:CHEMONTID_0000245
        a                skos:Concept ;
        rdfs:seeAlso     tax_nodes:C0000245 ;
        skos:altLabel    "purines"@en ;
        skos:broader     csc:CHEMONTID_0001797 ;
        skos:definition  "Aromatic heterocyclic compounds containing a purine moiety, which is formed a pyrimidine-ring ring fused to an imidazole ring."@en ;
        skos:inScheme    vlcs:chemische_stof ;
        skos:notation    "CHEMONTID:0000245" ;
        skos:prefLabel   "Purines and purine derivatives"@en .

csc:CHEMONTID_0000291
        a                skos:Concept ;
        skos:altLabel    "pyrimidone"@en ;
        skos:broader     csc:CHEMONTID_0000075 ;
        skos:definition  "Compounds that contain a pyrimidine ring, which bears a ketone. Pyrimidine is a 6-membered ring consisting of four carbon atoms and two nitrogen centers at the 1- and 3- ring positions."@en ;
        skos:inScheme    vlcs:chemische_stof ;
        skos:notation    "CHEMONTID:0000291" ;
        skos:prefLabel   "Pyrimidones"@en .

csc:CHEMONTID_0004756
        a                skos:Concept ;
        skos:broader     csc:CHEMONTID_0004755 ;
        skos:definition  "Aromatic heterocyclic compounds contaning a furan ring that is substituted at the 2-position with an anilide."@en ;
        skos:inScheme    vlcs:chemische_stof ;
        skos:notation    "CHEMONTID:0004756" ;
        skos:prefLabel   "2-furanilides"@en .

csc:CHEMONTID_0003100
        a                skos:Concept ;
        skos:altLabel    "carbonyl compound"@en , "organohalogen compound"@en ;
        skos:broader     csc:CHEMONTID_0003096 ;
        skos:definition  "Benzoic acids or derivatives carrying a halogen atom at the 4-position of the benzene ring."@en ;
        skos:inScheme    vlcs:chemische_stof ;
        skos:notation    "CHEMONTID:0003100" ;
        skos:prefLabel   "4-halobenzoic acids and derivatives"@en .

csc:CHEMONTID_0003528
        a                skos:Concept ;
        skos:altLabel    "rotenones"@en ;
        skos:broader     csc:CHEMONTID_0001607 ;
        skos:definition  "Rotenoids with a structure based on a 6a,12a-dihydrochromeno[3,4-b]chromen-12(6H)-one skeleton."@en ;
        skos:inScheme    vlcs:chemische_stof ;
        skos:notation    "CHEMONTID:0003528" ;
        skos:prefLabel   "Rotenones"@en .

csc:CHEMONTID_0002346
        a                skos:Concept ;
        skos:altLabel    "methoxybenzoic acid"@en ;
        skos:broader     csc:CHEMONTID_0002344 ;
        skos:definition  "Benzoic acids in which the hydrogen atom at position 4 of the benzene ring is replaced by a methoxy group."@en ;
        skos:inScheme    vlcs:chemische_stof ;
        skos:notation    "CHEMONTID:0002346" ;
        skos:prefLabel   "P-methoxybenzoic acids and derivatives"@en .

csc:CHEMONTID_0001662
        a                skos:Concept ;
        skos:altLabel    "carboxamide"@en ;
        skos:broader     csc:CHEMONTID_0000475 ;
        skos:definition  "Compounds comprising primary carboxylic acid amide functional group, with the general structure RC(=O)NH2."@en ;
        skos:inScheme    vlcs:chemische_stof ;
        skos:notation    "CHEMONTID:0001662" ;
        skos:prefLabel   "Primary carboxylic acid amides"@en .

csc:CHEMONTID_0000434
        a                skos:Concept ;
        rdfs:seeAlso     tax_nodes:C0000434 ;
        skos:broader     csc:CHEMONTID_0000423 ;
        skos:definition  "Inorganic non-metallic compounds in which the largest atom belongs to the class of 'other nonmetals'."@en , "Inorganic non-metallic compounds in which the largest atom belongs to the class of 'other non-metals'."@en ;
        skos:inScheme    vlcs:chemische_stof ;
        skos:notation    "CHEMONTID:0000434" ;
        skos:prefLabel   "Homogeneous other non-metal compounds"@en .

csc:CHEMONTID_0004479
        a                skos:Concept ;
        skos:altLabel    "Organosilicon Compounds"@en ;
        skos:broader     csc:CHEMONTID_0004445 ;
        skos:definition  "Organoheterosilanes, bearing a silicon atom linked to three alkyl groups and one heteroatom."@en ;
        skos:inScheme    vlcs:chemische_stof ;
        skos:notation    "CHEMONTID:0004479" ;
        skos:prefLabel   "Trialkylheterosilanes"@en .

csc:CHEMONTID_0004770
        a                skos:Concept ;
        skos:broader     csc:CHEMONTID_0000093 ;
        skos:definition  "Aromatic heterocyclic compounds containing a 1,3,4-thiadiazole ring, which is substituted at the 2-position with an organothiophosphate group."@en ;
        skos:inScheme    vlcs:chemische_stof ;
        skos:notation    "CHEMONTID:0004770" ;
        skos:prefLabel   "1,3,4-thiadiazol-3-yl-organothiophosphates"@en .

csc:CHEMONTID_0004226
        a                skos:Concept ;
        skos:broader     csc:CHEMONTID_0004097 ;
        skos:definition  "Aromatic compounds containing a 1,4-benzodiazepine fused to and sharing a nitrogen atom with a 1,2,4-triazole ring."@en ;
        skos:inScheme    vlcs:chemische_stof ;
        skos:notation    "CHEMONTID:0004226" ;
        skos:prefLabel   "1,2,4-triazolo[4,3-a][1,4]benzodiazepines"@en .

csc:CHEMONTID_0000189
        a                skos:Concept ;
        rdfs:seeAlso     tax_nodes:C0000189 ;
        skos:altLabel    "Piperazines"@en ;
        skos:broader     csc:CHEMONTID_0002389 ;
        skos:definition  "Compounds containing a piperazine ring, which is a saturated aliphatic six-member heterocyclic with two nitrogen atoms at positions 1 and 4, as well as four carbon atoms."@en ;
        skos:inScheme    vlcs:chemische_stof ;
        skos:notation    "CHEMONTID:0000189" ;
        skos:prefLabel   "Piperazines"@en .

csc:CHEMONTID_0000480
        a                skos:Concept ;
        rdfs:seeAlso     tax_nodes:C0000480 ;
        skos:altLabel    "pyrimidine nucleoside"@en ;
        skos:broader     csc:CHEMONTID_0000289 ;
        skos:definition  "Compounds comprising a pyrimidine base attached to a ribosyl or deoxyribosyl moiety."@en ;
        skos:inScheme    vlcs:chemische_stof ;
        skos:notation    "CHEMONTID:0000480" ;
        skos:prefLabel   "Pyrimidine nucleosides"@en .

csc:CHEMONTID_0002314
        a                skos:Concept ;
        skos:altLabel    "quinazolines"@en ;
        skos:broader     csc:CHEMONTID_0000485 ;
        skos:definition  "Heterocyclic aromatic compounds containing a quianazoline moiety substituted by one or more amine groups."@en ;
        skos:inScheme    vlcs:chemische_stof ;
        skos:notation    "CHEMONTID:0002314" ;
        skos:prefLabel   "Quinazolinamines"@en .

csc:CHEMONTID_0000402
        a                skos:Concept ;
        rdfs:seeAlso     tax_nodes:C0000402 ;
        skos:altLabel    "phosphoric acid derivative"@en ;
        skos:broader     csc:CHEMONTID_0000264 ;
        skos:definition  "Organic compounds containing phosphoric acid or a derivative thereof."@en ;
        skos:inScheme    vlcs:chemische_stof ;
        skos:notation    "CHEMONTID:0000402" ;
        skos:prefLabel   "Organic phosphoric acids and derivatives"@en .

csc:CHEMONTID_0001851
        a                skos:Concept ;
        rdfs:seeAlso     tax_nodes:C0001851 ;
        skos:altLabel    "pyrenes"@en ;
        skos:broader     csc:CHEMONTID_0002448 ;
        skos:definition  "Compounds containing a pyrene moiety, which consists four fused benzene rings, resulting in a flat aromatic system."@en ;
        skos:inScheme    vlcs:chemische_stof ;
        skos:notation    "CHEMONTID:0001851" ;
        skos:prefLabel   "Pyrenes"@en .

csc:CHEMONTID_0003265
        a                skos:Concept ;
        skos:altLabel    "silyl ether"@en ;
        skos:broader     csc:CHEMONTID_0003194 ;
        skos:definition  "Organosilicon compounds with the general formula RO[Si](OR')(R'')(R''') (R,R' = organyl; R'',R''' = any atom)."@en ;
        skos:inScheme    vlcs:chemische_stof ;
        skos:notation    "CHEMONTID:0003265" ;
        skos:prefLabel   "Alkoxysilanes"@en .

csc:CHEMONTID_0004668
        a                skos:Concept ;
        skos:broader     csc:CHEMONTID_0004001 ;
        skos:definition  "Aromatic compounds containing a 1,3,4-thiadiazole ring, which is substituted at the 2-position with urea."@en ;
        skos:inScheme    vlcs:chemische_stof ;
        skos:notation    "CHEMONTID:0004668" ;
        skos:prefLabel   "1,3,4-thiadiazol-2-ylureas"@en .

csc:CHEMONTID_0002581
        a                skos:Concept ;
        rdfs:seeAlso     tax_nodes:C0002581 ;
        skos:altLabel    "neoflavonoid"@en ;
        skos:broader     csc:CHEMONTID_0001614 ;
        skos:definition  "Neoflavonoids with a structure based on a 3,4-dihydro-4-aryl-2H-1-benzopyran skeleton."@en ;
        skos:inScheme    vlcs:chemische_stof ;
        skos:notation    "CHEMONTID:0002581" ;
        skos:prefLabel   "Neoflavans"@en .

csc:CHEMONTID_0001100
        a                skos:Concept ;
        skos:altLabel    "organofluorine compound"@en ;
        skos:broader     csc:CHEMONTID_0000035 ;
        skos:definition  "Compounds containing one or more fluorine atoms attached to a benzene ring."@en ;
        skos:inScheme    vlcs:chemische_stof ;
        skos:notation    "CHEMONTID:0001100" ;
        skos:prefLabel   "Fluorobenzenes"@en .

csc:CHEMONTID_0003952
        a                skos:Concept ;
        skos:altLabel    "anthraquinone"@en ;
        skos:broader     csc:CHEMONTID_0000151 ;
        skos:definition  "Organic compounds containing an anthraquinone ring system, which is substituted at the 2-position by an amino group."@en ;
        skos:inScheme    vlcs:chemische_stof ;
        skos:notation    "CHEMONTID:0003952" ;
        skos:prefLabel   "2-aminoanthraquinones"@en .

csc:CHEMONTID_0000346
        a                skos:Concept ;
        rdfs:seeAlso     tax_nodes:C0000346 ;
        skos:altLabel    "dicarboxylic acid"@en , "Dicarboxylic acids"@en ;
        skos:broader     csc:CHEMONTID_0000265 ;
        skos:definition  "Organic compounds containing exactly two carboxylic acid groups."@en ;
        skos:inScheme    vlcs:chemische_stof ;
        skos:notation    "CHEMONTID:0000346" ;
        skos:prefLabel   "Dicarboxylic acids and derivatives"@en .

csc:CHEMONTID_0004682
        a                skos:Concept ;
        skos:broader     csc:CHEMONTID_0004681 ;
        skos:definition  "Polycyclic aromatic compounds containing a 1,2,4-triazolo[1,5-a]pyrimidine ring system, which is substituted with a sulfonanilide at the 2-position."@en ;
        skos:inScheme    vlcs:chemische_stof ;
        skos:notation    "CHEMONTID:0004682" ;
        skos:prefLabel   "1,2,4-triazolopyrimidine-2-sulfonanilides"@en .

csc:CHEMONTID_0003454
        a                skos:Concept ;
        skos:altLabel    "thiopurine"@en ;
        skos:broader     csc:CHEMONTID_0002987 ;
        skos:definition  "Compounds that contain an alkylamine group attached at the 6-position of a purine. Purine is a bicyclic aromatic compound made up of a pyrimidine ring fused to an imidazole ring."@en ;
        skos:inScheme    vlcs:chemische_stof ;
        skos:notation    "CHEMONTID:0003454" ;
        skos:prefLabel   "6-alkylaminopurines"@en .

csc:CHEMONTID_0000392
        a                skos:Concept ;
        rdfs:seeAlso     tax_nodes:C0000392 ;
        skos:altLabel    "morpholines"@en , "1,4-Oxazinanes"@en ;
        skos:broader     csc:CHEMONTID_0000107 ;
        skos:definition  "Organic compounds containing a morpholine moiety, which consists of a six-member aliphatic saturated ring with the formula C4H9NO, where the oxygen and nitrogen atoms lie at positions 1 and 4, respectively."@en ;
        skos:inScheme    vlcs:chemische_stof ;
        skos:notation    "CHEMONTID:0000392" ;
        skos:prefLabel   "Morpholines"@en .

csc:CHEMONTID_0002770
        a                skos:Concept ;
        skos:altLabel    "monochlorophenol"@en ;
        skos:broader     csc:CHEMONTID_0002766 ;
        skos:definition  "Chlorophenols carrying a iodine at the C3 position of the benzene ring."@en ;
        skos:inScheme    vlcs:chemische_stof ;
        skos:notation    "CHEMONTID:0002770" ;
        skos:prefLabel   "M-chlorophenols"@en .

csc:CHEMONTID_0004152
        a                skos:Concept ;
        rdfs:seeAlso     tax_nodes:C0004152 ;
        skos:altLabel    "methylpyridines"@en ;
        skos:broader     csc:CHEMONTID_0000089 ;
        skos:definition  "Organic compounds containing a pyridine ring substituted at one or more positions by a methyl group."@en ;
        skos:inScheme    vlcs:chemische_stof ;
        skos:notation    "CHEMONTID:0004152" ;
        skos:prefLabel   "Methylpyridines"@en .

csc:CHEMONTID_0001510
        a                skos:Concept ;
        rdfs:seeAlso     tax_nodes:C0001510 ;
        skos:altLabel    "lignan"@en , "lactone"@en ;
        skos:broader     csc:CHEMONTID_0001392 ;
        skos:definition  "Lignans that contain a lactone moiety. They include 1-aryltetralin lactones, dibenzylbutyrolactone lignans, and podophyllotoxins, among others."@en ;
        skos:inScheme    vlcs:chemische_stof ;
        skos:notation    "CHEMONTID:0001510" ;
        skos:prefLabel   "Lignan lactones"@en .

csc:CHEMONTID_0002913
        a                skos:Concept ;
        skos:altLabel    "beta-hydroxy ketone"@en , "Beta-hydroxyketones"@en ;
        skos:broader     csc:CHEMONTID_0000118 ;
        skos:definition  "Ketones containing a hydroxyl group attached to the beta-carbon atom, relative to the C=O group."@en ;
        skos:inScheme    vlcs:chemische_stof ;
        skos:notation    "CHEMONTID:0002913" ;
        skos:prefLabel   "Beta-hydroxy ketones"@en .

csc:CHEMONTID_0000037
        a                skos:Concept ;
        rdfs:seeAlso     tax_nodes:C0000037 ;
        skos:altLabel    "Styrenes"@en , "styrenes"@en ;
        skos:broader     csc:CHEMONTID_0002279 ;
        skos:definition  "Organic compounds containing an ethenylbenzene moiety."@en ;
        skos:inScheme    vlcs:chemische_stof ;
        skos:notation    "CHEMONTID:0000037" ;
        skos:prefLabel   "Styrenes"@en .

csc:CHEMONTID_0001984
        a                skos:Concept ;
        skos:altLabel    "piperazines"@en , "a phenylpiperazine"@en ;
        skos:broader     csc:CHEMONTID_0000189 ;
        skos:definition  "Compounds containing a phenylpiperazine skeleton, which consists of a piperazine bound to a phenyl group."@en ;
        skos:inScheme    vlcs:chemische_stof ;
        skos:notation    "CHEMONTID:0001984" ;
        skos:prefLabel   "Phenylpiperazines"@en .

csc:CHEMONTID_0000756
        a                skos:Concept ;
        rdfs:seeAlso     tax_nodes:C0000756 ;
        skos:altLabel    "imidazothiazole"@en , "an imidazothiazole"@en ;
        skos:broader     csc:CHEMONTID_0000002 ;
        skos:definition  "Organic polycyclic compounds containing an imidazole ring fused to a thiazole ring. Imidazole is 5-membered ring consisting of three carbon atoms, and two nitrogen centers at the 1- and 3-positions. Thiazole is a 6-membered ring that contains both sulfur and nitrogen."@en ;
        skos:inScheme    vlcs:chemische_stof ;
        skos:notation    "CHEMONTID:0000756" ;
        skos:prefLabel   "Imidazothiazoles"@en .

csc:CHEMONTID_0000503
        a                skos:Concept ;
        rdfs:seeAlso     tax_nodes:C0000503 ;
        skos:altLabel    "Quaternary Ammonium Compounds"@en , "quaternary ammonium salt"@en , "quaternary ammonium compounds"@en ;
        skos:broader     csc:CHEMONTID_0000278 ;
        skos:definition  "Compounds containing positively charged polyatomic ion of the structure NR4+, R being an alkyl group or an aryl group."@en ;
        skos:inScheme    vlcs:chemische_stof ;
        skos:notation    "CHEMONTID:0000503" ;
        skos:prefLabel   "Quaternary ammonium salts"@en .

csc:CHEMONTID_0003864
        a                skos:Concept ;
        skos:broader     csc:CHEMONTID_0004631 ;
        skos:definition  "Organosulfur compounds containing a thioether group that is substituted by two aryl groups."@en ;
        skos:inScheme    vlcs:chemische_stof ;
        skos:notation    "CHEMONTID:0003864" ;
        skos:prefLabel   "Diarylthioethers"@en .

csc:CHEMONTID_0000258
        a                skos:Concept ;
        rdfs:seeAlso     tax_nodes:C0000258 ;
        skos:altLabel    "steroid"@en , "A steroid"@en , "Sterol Lipids"@en , "steroids"@en , "Steroids"@en ;
        skos:broader     csc:CHEMONTID_0000012 ;
        skos:definition  "Compounds based on the cyclopenta[a]phenanthrene carbon skeleton, partially or completely hydrogenated; there are usually methyl groups at C-10 and C-13, and often an alkyl group at C-17. By extension, one or more bond scissions, ring expansions and/or ring contractions of the skeleton may have occurred."@en ;
        skos:inScheme    vlcs:chemische_stof ;
        skos:notation    "CHEMONTID:0000258" ;
        skos:prefLabel   "Steroids and steroid derivatives"@en .

csc:CHEMONTID_0000051
        a                skos:Concept ;
        skos:altLabel    "monoterpenoid"@en ;
        skos:broader     csc:CHEMONTID_0001549 ;
        skos:definition  "Monoterpenoids containing at least one aromatic ring."@en ;
        skos:inScheme    vlcs:chemische_stof ;
        skos:notation    "CHEMONTID:0000051" ;
        skos:prefLabel   "Aromatic monoterpenoids"@en .

csc:CHEMONTID_0000226
        a                skos:Concept ;
        rdfs:seeAlso     tax_nodes:C0000226 ;
        skos:altLabel    "Thiazolidines"@en ;
        skos:broader     csc:CHEMONTID_0002491 ;
        skos:definition  "Heterocyclic compounds containing a five-member saturated aliphatic ring with one nitrogen atom, one sulfur atom, three carbon atoms."@en ;
        skos:inScheme    vlcs:chemische_stof ;
        skos:notation    "CHEMONTID:0000226" ;
        skos:prefLabel   "Thiazolidines"@en .

csc:CHEMONTID_0001920
        a                skos:Concept ;
        rdfs:seeAlso     tax_nodes:C0001920 ;
        skos:altLabel    "triazines"@en ;
        skos:broader     csc:CHEMONTID_0000098 ;
        skos:definition  "Compounds containing a triazine ring which bears a ketone group a carbon atom."@en ;
        skos:inScheme    vlcs:chemische_stof ;
        skos:notation    "CHEMONTID:0001920" ;
        skos:prefLabel   "Triazinones"@en .

csc:CHEMONTID_0002106
        a                skos:Concept ;
        rdfs:seeAlso     tax_nodes:C0002106 ;
        skos:altLabel    "Anthracyclinones"@en , "anthracycline"@en ;
        skos:broader     csc:CHEMONTID_0000261 ;
        skos:definition  "Polyketides containing a tetracenequinone ring structure with a sugar attached by glycosidic linkage."@en ;
        skos:inScheme    vlcs:chemische_stof ;
        skos:notation    "CHEMONTID:0002106" ;
        skos:prefLabel   "Anthracyclines"@en .

csc:CHEMONTID_0002650
        a                skos:Concept ;
        rdfs:seeAlso     tax_nodes:C0002650 ;
        skos:altLabel    "diarylheptanoid"@en ;
        skos:broader     csc:CHEMONTID_0000261 ;
        skos:definition  "Phenylpropanoids with a structure containing two  aromatic rings joined by a seven carbons (a 1,7-diphenylheptane skeleton) and may have various substituents."@en ;
        skos:inScheme    vlcs:chemische_stof ;
        skos:notation    "CHEMONTID:0002650" ;
        skos:prefLabel   "Diarylheptanoids"@en .

csc:CHEMONTID_0001675
        a                skos:Concept ;
        skos:altLabel    "amino cyclitol"@en , "glycoside"@en ;
        skos:broader     csc:CHEMONTID_0000282 ;
        skos:definition  "Organic compounds containing an amicocyclitol moiety glycosidically linked to a carbohydrate moiety. There are two major classes of aminoglycosides containing a 2-streptamine core. They are called 4,5- and 4,6-disubstituted 2-deoxystreptamines."@en ;
        skos:inScheme    vlcs:chemische_stof ;
        skos:notation    "CHEMONTID:0001675" ;
        skos:prefLabel   "Aminocyclitol glycosides"@en .

csc:CHEMONTID_0004239
        a                skos:Concept ;
        skos:altLabel    "Pentaorganosubstituted compounds"@en , "Pentaorganosubstituted arsenic derivatives"@en ;
        skos:broader     csc:CHEMONTID_0004056 ;
        skos:definition  "Organoarsenic compounds containing an arsenic compound that is pentasubstituted by only organic groups."@en ;
        skos:inScheme    vlcs:chemische_stof ;
        skos:notation    "CHEMONTID:0004239" ;
        skos:prefLabel   "Pentaorganoarsanes"@en .

csc:CHEMONTID_0002327
        a                skos:Concept ;
        skos:altLabel    "imidazoles"@en ;
        skos:broader     csc:CHEMONTID_0002310 ;
        skos:definition  "Polycyclic aromatic compounds containing a benzene ring linked to an imidazole ring through a CC or CN bond."@en ;
        skos:inScheme    vlcs:chemische_stof ;
        skos:notation    "CHEMONTID:0002327" ;
        skos:prefLabel   "Phenylimidazoles"@en .

csc:CHEMONTID_0004705
        a                skos:Concept ;
        skos:broader     csc:CHEMONTID_0000490 ;
        skos:definition  "Aromatic heterocyclic compounds containing a pyrimidine ring which is substituted with a sulfonylurea at the ring 2-position."@en ;
        skos:inScheme    vlcs:chemische_stof ;
        skos:notation    "CHEMONTID:0004705" ;
        skos:prefLabel   "Pyrimidinyl-2-sulfonylureas"@en .

csc:CHEMONTID_0000461
        a                skos:Concept ;
        rdfs:seeAlso     tax_nodes:C0000461 ;
        skos:broader     csc:CHEMONTID_0000424 ;
        skos:definition  "Inorganic compounds belonging to either the alkaline earth metal hydrides, alkaline earth metal nitrides, alkaline earth metal oxides, alkaline earth metal sulfides."@en ;
        skos:inScheme    vlcs:chemische_stof ;
        skos:notation    "CHEMONTID:0000461" ;
        skos:prefLabel   "Transition metal organides"@en .

csc:CHEMONTID_0003278
        a                skos:Concept ;
        skos:altLabel    "Tosylates"@en , "benzenesulfonates"@en ;
        skos:broader     csc:CHEMONTID_0000032 ;
        skos:definition  "Benzenesulfonic acids (or derivative thereof) carrying a methyl group at the para- position."@en ;
        skos:inScheme    vlcs:chemische_stof ;
        skos:notation    "CHEMONTID:0003278" ;
        skos:prefLabel   "p-Methylbenzenesulfonates"@en .

csc:CHEMONTID_0002341
        a                skos:Concept ;
        rdfs:seeAlso     tax_nodes:C0002341 ;
        skos:altLabel    "aromatic ether"@en ;
        skos:broader     csc:CHEMONTID_0002448 ;
        skos:definition  "Aromatic compounds containing an ether group substituted with a benzene ring."@en ;
        skos:inScheme    vlcs:chemische_stof ;
        skos:notation    "CHEMONTID:0002341" ;
        skos:prefLabel   "Phenol ethers"@en .

csc:CHEMONTID_0002769
        a                skos:Concept ;
        skos:altLabel    "bromophenol"@en ;
        skos:broader     csc:CHEMONTID_0002764 ;
        skos:definition  "Bromophenols carrying a iodine at the C4 position of the benzene ring."@en ;
        skos:inScheme    vlcs:chemische_stof ;
        skos:notation    "CHEMONTID:0002769" ;
        skos:prefLabel   "P-bromophenols"@en .

csc:CHEMONTID_0000138
        a                skos:Concept ;
        rdfs:seeAlso     tax_nodes:C0000138 ;
        skos:altLabel    "Anisoles"@en ;
        skos:broader     csc:CHEMONTID_0002341 ;
        skos:definition  "Organic compounds containing a methoxybenzene or a derivative thereof."@en ;
        skos:inScheme    vlcs:chemische_stof ;
        skos:notation    "CHEMONTID:0000138" ;
        skos:prefLabel   "Anisoles"@en .

csc:CHEMONTID_0004474
        a                skos:Concept ;
        rdfs:seeAlso     tax_nodes:C0004474 ;
        skos:broader     csc:CHEMONTID_0002837 ;
        skos:definition  "Hydrocarbons that contains only saturated carbon atoms, which are linked to one another through single bonds. These includes alkanes and cycloalkanes."@en ;
        skos:inScheme    vlcs:chemische_stof ;
        skos:notation    "CHEMONTID:0004474" ;
        skos:prefLabel   "Saturated hydrocarbons"@en .

csc:CHEMONTID_0002562
        a                skos:Concept ;
        skos:altLabel    "organosulfur heterocyclic compound"@en , "organonitrogen heterocyclic compound"@en ;
        skos:broader     csc:CHEMONTID_0000093 ;
        skos:definition  "Thiadiazoles with an amino group attached to the thiadiazole ring."@en ;
        skos:inScheme    vlcs:chemische_stof ;
        skos:notation    "CHEMONTID:0002562" ;
        skos:prefLabel   "Aminothiadiazoles"@en .

csc:CHEMONTID_0003965
        a                skos:Concept ;
        skos:altLabel    "aminotoluene"@en ;
        skos:broader     csc:CHEMONTID_0003964 ;
        skos:definition  "Organic aromatic compounds containing a benzene that carries a single methyl group exactly 2 amino groups."@en ;
        skos:inScheme    vlcs:chemische_stof ;
        skos:notation    "CHEMONTID:0003965" ;
        skos:prefLabel   "Diaminotoluenes"@en .

csc:CHEMONTID_0001334
        a                skos:Concept ;
        rdfs:seeAlso     tax_nodes:C0001334 ;
        skos:altLabel    "Fatty alcohols"@en , "Fatty Alcohols"@en , "aliphatic alcohol"@en ;
        skos:broader     csc:CHEMONTID_0003909 ;
        skos:definition  "Aliphatic alcohols consisting of a chain of a least six carbon atoms."@en ;
        skos:inScheme    vlcs:chemische_stof ;
        skos:notation    "CHEMONTID:0001334" ;
        skos:prefLabel   "Fatty alcohols"@en .

csc:CHEMONTID_0000106
        a                skos:Concept ;
        rdfs:seeAlso     tax_nodes:C0000106 ;
        skos:altLabel    "oxathiolane"@en ;
        skos:broader     csc:CHEMONTID_0000002 ;
        skos:definition  "Compounds containing an oxathiolane moiety, which consists of a saturated aliphatic five-member ring with one oxygen atom, a sulfur atom, and three carbon atoms. Isomers  of oxaphospholane include meta-oxathiolane, and ortho-oxathiolane."@en ;
        skos:inScheme    vlcs:chemische_stof ;
        skos:notation    "CHEMONTID:0000106" ;
        skos:prefLabel   "Oxathiolanes"@en .

csc:CHEMONTID_0003467
        a                skos:Concept ;
        rdfs:seeAlso     tax_nodes:C0003467 ;
        skos:altLabel    "1,3-diphenylpropenes"@en , " Diarylpropane flavonoids"@en , "aromatic compound"@en ;
        skos:broader     csc:CHEMONTID_0000261 ;
        skos:definition  "Organic compounds with a structure based on a C6-C3-C6 skeleton, where the two benzene rings are not linked together."@en ;
        skos:inScheme    vlcs:chemische_stof ;
        skos:notation    "CHEMONTID:0003467" ;
        skos:prefLabel   "Linear 1,3-diarylpropanoids"@en .

csc:CHEMONTID_0002239
        a                skos:Concept ;
        skos:altLabel    "a trialkylamine"@en , "tertiary amino compound"@en ;
        skos:broader     csc:CHEMONTID_0002452 ;
        skos:definition  "Organic compounds containing a trialkylamine group, characterized by exactly three alkyl groups bonded to the amino nitrogen."@en ;
        skos:inScheme    vlcs:chemische_stof ;
        skos:notation    "CHEMONTID:0002239" ;
        skos:prefLabel   "Trialkylamines"@en .

csc:CHEMONTID_0001302
        a                skos:Concept ;
        rdfs:seeAlso     tax_nodes:C0001302 ;
        skos:altLabel    "phosphonic acids"@en ;
        skos:broader     csc:CHEMONTID_0000419 ;
        skos:definition  "Organic compounds containing phosphonic acid."@en ;
        skos:inScheme    vlcs:chemische_stof ;
        skos:notation    "CHEMONTID:0001302" ;
        skos:prefLabel   "Organic phosphonic acids"@en .

csc:CHEMONTID_0000327
        a                skos:Concept ;
        rdfs:seeAlso     tax_nodes:C0000327 ;
        skos:altLabel    "1,1-bis(phosphonic acid)"@en ;
        skos:broader     csc:CHEMONTID_0000419 ;
        skos:definition  "Organic compounds containing two phosphonate groups linked together through a carbon atoms."@en ;
        skos:inScheme    vlcs:chemische_stof ;
        skos:notation    "CHEMONTID:0000327" ;
        skos:prefLabel   "Bisphosphonates"@en .

csc:CHEMONTID_0003260
        a                skos:Concept ;
        rdfs:seeAlso     tax_nodes:C0003260 ;
        skos:altLabel    "organosulfur compound"@en , "a sulfenyl compound"@en ;
        skos:broader     csc:CHEMONTID_0000004 ;
        skos:definition  "Organosulfur compounds a sulfenyl group with the general formula RS (R = organyl)."@en ;
        skos:inScheme    vlcs:chemische_stof ;
        skos:notation    "CHEMONTID:0003260" ;
        skos:prefLabel   "Sulfenyl compounds"@en .

csc:CHEMONTID_0002285
        a                skos:Concept ;
        rdfs:seeAlso     tax_nodes:C0002285 ;
        skos:altLabel    "organonitrogen compound"@en ;
        skos:broader     csc:CHEMONTID_0000264 ;
        skos:definition  "Compounds containing a carboximidic group, with the general formula R-C(=NR1)OR2."@en ;
        skos:inScheme    vlcs:chemische_stof ;
        skos:notation    "CHEMONTID:0002285" ;
        skos:prefLabel   "Carboximidic acids and derivatives"@en .

csc:CHEMONTID_0003688
        a                skos:Concept ;
        rdfs:seeAlso     tax_nodes:C0003688 ;
        skos:altLabel    "diazo compound"@en ;
        skos:broader     csc:CHEMONTID_0003633 ;
        skos:definition  "Organic compounds having the divalent diazo group, =N+=N-, attached to a carbon atom."@en ;
        skos:inScheme    vlcs:chemische_stof ;
        skos:notation    "CHEMONTID:0003688" ;
        skos:prefLabel   "Diazo compounds"@en .

csc:CHEMONTID_0001057
        a                skos:Concept ;
        rdfs:seeAlso     tax_nodes:C0001057 ;
        skos:altLabel    "p-block molecular entity"@en ;
        skos:broader     csc:CHEMONTID_0000435 ;
        skos:definition  "Inorganic non-metallic compounds containing a hypochlorite as its largest oxoanion."@en ;
        skos:inScheme    vlcs:chemische_stof ;
        skos:notation    "CHEMONTID:0001057" ;
        skos:prefLabel   "Non-metal hypochlorites"@en .

csc:CHEMONTID_0004410
        a                skos:Concept ;
        skos:broader     csc:CHEMONTID_0000173 ;
        skos:definition  "Cephalosporins that are substituted at the 3'-position by a carbamate group."@en ;
        skos:inScheme    vlcs:chemische_stof ;
        skos:notation    "CHEMONTID:0004410" ;
        skos:prefLabel   "Cephalosporin 3'-carbamates"@en .

csc:CHEMONTID_0001523
        a                skos:Concept ;
        rdfs:seeAlso     tax_nodes:C0001523 ;
        skos:broader     csc:CHEMONTID_0000462 ;
        skos:definition  "Organic compounds containing a post-transition metal atom."@en ;
        skos:inScheme    vlcs:chemische_stof ;
        skos:notation    "CHEMONTID:0001523" ;
        skos:prefLabel   "Organo-post-transition metal compounds"@en .

csc:CHEMONTID_0002207
        a                skos:Concept ;
        skos:altLabel    "glycoside"@en ;
        skos:broader     csc:CHEMONTID_0002105 ;
        skos:definition  "Glycoside in which a sugar group is bonded through one carbon to another group via a O-glycosidic bond."@en ;
        skos:inScheme    vlcs:chemische_stof ;
        skos:notation    "CHEMONTID:0002207" ;
        skos:prefLabel   "O-glycosyl compounds"@en .

csc:CHEMONTID_0000120
        a                skos:Concept ;
        rdfs:seeAlso     tax_nodes:C0000120 ;
        skos:altLabel    "benzophenones"@en , "Benzophenones"@en ;
        skos:broader     csc:CHEMONTID_0002279 ;
        skos:definition  "Organic compounds containing a ketone attached to two phenyl groups."@en ;
        skos:inScheme    vlcs:chemische_stof ;
        skos:notation    "CHEMONTID:0000120" ;
        skos:prefLabel   "Benzophenones"@en .

csc:CHEMONTID_0000548
        a                skos:Concept ;
        rdfs:seeAlso     tax_nodes:C0000548 ;
        skos:altLabel    "hydrogen halide"@en ;
        skos:broader     csc:CHEMONTID_0000454 ;
        skos:definition  "Inorganic compounds in which the heaviest atom bonded to a hydrogen atom is a halogen."@en ;
        skos:inScheme    vlcs:chemische_stof ;
        skos:notation    "CHEMONTID:0000548" ;
        skos:prefLabel   "Halogen hydrides"@en .

csc:CHEMONTID_0003901
        a                skos:Concept ;
        skos:altLabel    "tertiary amino compound"@en , "dialkylarylamine"@en ;
        skos:broader     csc:CHEMONTID_0002454 ;
        skos:definition  "Aliphatic aromatic amines in which the amino group is linked to two aliphatic chains and one aromatic group."@en ;
        skos:inScheme    vlcs:chemische_stof ;
        skos:notation    "CHEMONTID:0003901" ;
        skos:prefLabel   "Dialkylarylamines"@en .

csc:CHEMONTID_0002253
        a                skos:Concept ;
        skos:altLabel    "pyridinecarboxamide"@en ;
        skos:broader     csc:CHEMONTID_0001326 ;
        skos:definition  "Heterocyclic aromatic compounds containing a pyridine ring substituted at position 3 by a carboxamide group."@en ;
        skos:inScheme    vlcs:chemische_stof ;
        skos:notation    "CHEMONTID:0002253" ;
        skos:prefLabel   "Nicotinamides"@en .

csc:CHEMONTID_0004631
        a                skos:Concept ;
        rdfs:seeAlso     tax_nodes:C0004631 ;
        skos:altLabel    "aryl sulfide"@en ;
        skos:broader     csc:CHEMONTID_0001202 ;
        skos:definition  "Organosulfur compounds containing a thioether group that is substituted by an aryl group."@en ;
        skos:inScheme    vlcs:chemische_stof ;
        skos:notation    "CHEMONTID:0004631" ;
        skos:prefLabel   "Aryl thioethers"@en .

csc:CHEMONTID_0000018
        a                skos:Concept ;
        rdfs:seeAlso     tax_nodes:C0000018 ;
        skos:altLabel    "anthracenes"@en , "Anthracenes"@en ;
        skos:broader     csc:CHEMONTID_0002448 ;
        skos:definition  "Organic compounds containing a system of three linearly fused benzene rings."@en ;
        skos:inScheme    vlcs:chemische_stof ;
        skos:notation    "CHEMONTID:0000018" ;
        skos:prefLabel   "Anthracenes"@en .

csc:CHEMONTID_0001467
        a                skos:Concept ;
        skos:altLabel    "3-hydroxy steroid"@en ;
        skos:broader     csc:CHEMONTID_0003568 ;
        skos:definition  "3-hydroxylated C19 steroid hormones. They are known to favor the development of masculine characteristics. They also show profound effects on scalp and body hair in humans."@en ;
        skos:inScheme    vlcs:chemische_stof ;
        skos:notation    "CHEMONTID:0001467" ;
        skos:prefLabel   "Androgens and derivatives"@en .

csc:CHEMONTID_0003670
        a                skos:Concept ;
        skos:altLabel    "aromatic ketone"@en ;
        skos:broader     csc:CHEMONTID_0000118 ;
        skos:definition  "Organic aromatic compounds that contain a ketone group substituted at one C-atom with an aryl group. They have the generic structure RC(=O)R', where R = aryl group and R'=organyl group."@en ;
        skos:inScheme    vlcs:chemische_stof ;
        skos:notation    "CHEMONTID:0003670" ;
        skos:prefLabel   "Aryl ketones"@en .

csc:CHEMONTID_0001292
        a                skos:Concept ;
        skos:altLabel    "organic hydroxy compound"@en ;
        skos:broader     csc:CHEMONTID_0000129 ;
        skos:definition  "Organic compounds containing an aliphatic ring substituted with at least one hydroxyl group."@en ;
        skos:inScheme    vlcs:chemische_stof ;
        skos:notation    "CHEMONTID:0001292" ;
        skos:prefLabel   "Cyclic alcohols and derivatives"@en .

csc:CHEMONTID_0002695
        a                skos:Concept ;
        skos:broader     csc:CHEMONTID_0002334 ;
        skos:definition  "Aromatic heterocyclic compounds with a structure based on a pyrrole ring linked to exactly two phenyl groups."@en ;
        skos:inScheme    vlcs:chemische_stof ;
        skos:notation    "CHEMONTID:0002695" ;
        skos:prefLabel   "Diphenylpyrroles"@en .

csc:CHEMONTID_0000064
        a                skos:Concept ;
        rdfs:seeAlso     tax_nodes:C0000064 ;
        skos:broader     csc:CHEMONTID_0000261 ;
        skos:definition  "Cyclic amides of amino carboxylic acids, having a 1-azacycloalkan-2-one structure, or analogues having unsaturation or heteroatoms replacing one or more carbon atoms of the ring.  They are nitrogen analogues (the a nitrogen atom replacing the o atom of the cyclic carboxylic acid group ) of the naturally occurring macrolides."@en ;
        skos:inScheme    vlcs:chemische_stof ;
        skos:notation    "CHEMONTID:0000064" ;
        skos:prefLabel   "Macrolactams"@en .

csc:CHEMONTID_0002442
        a                skos:Concept ;
        rdfs:seeAlso     tax_nodes:C0002442 ;
        skos:altLabel    "nitroso compound"@en , "piperidines"@en ;
        skos:broader     csc:CHEMONTID_0000195 ;
        skos:definition  "Piperidines with a nitroso functional group attached to the piperidine ring."@en ;
        skos:inScheme    vlcs:chemische_stof ;
        skos:notation    "CHEMONTID:0002442" ;
        skos:prefLabel   "Nitrosopiperidines"@en .

csc:CHEMONTID_0000530
        a                skos:Concept ;
        rdfs:seeAlso     tax_nodes:C0000530 ;
        skos:altLabel    "p-block molecular entity"@en , "inorganic oxide"@en ;
        skos:broader     csc:CHEMONTID_0000458 ;
        skos:definition  "Inorganic compounds containing an oxygen atom of an oxidation state of -2, in which the heaviest atom bonded to the oxygen is a post-transition metal."@en ;
        skos:inScheme    vlcs:chemische_stof ;
        skos:notation    "CHEMONTID:0000530" ;
        skos:prefLabel   "Post-transition metal oxides"@en .

csc:CHEMONTID_0004322
        a                skos:Concept ;
        skos:broader     csc:CHEMONTID_0000060 ;
        skos:definition  "Compounds containing proline or a derivative thereof resulting from reaction of proline at the amino group or the carboxy group, or from the replacement of any hydrogen of glycine by a heteroatom."@en ;
        skos:inScheme    vlcs:chemische_stof ;
        skos:notation    "CHEMONTID:0004322" ;
        skos:prefLabel   "Proline and derivatives"@en .

csc:CHEMONTID_0000285
        a                skos:Concept ;
        rdfs:seeAlso     tax_nodes:C0000285 ;
        skos:altLabel    "anilide"@en , "Carboxanilides"@en , "anilides"@en ;
        skos:broader     csc:CHEMONTID_0002279 ;
        skos:definition  "Organic heterocyclic compounds derived from oxoacids RkE(=O)l(OH)m (l not 0) by replacing an OH group by the NHPh group or derivative formed by ring substitution."@en ;
        skos:inScheme    vlcs:chemische_stof ;
        skos:notation    "CHEMONTID:0000285" ;
        skos:prefLabel   "Anilides"@en .

csc:CHEMONTID_0000032
        a                skos:Concept ;
        rdfs:seeAlso     tax_nodes:C0000032 ;
        skos:altLabel    "Benzenesulfonates"@en ;
        skos:broader     csc:CHEMONTID_0002279 ;
        skos:definition  "Organic compounds containing a sulfonic acid or a derivative thereof that is linked to a benzene ring."@en ;
        skos:inScheme    vlcs:chemische_stof ;
        skos:notation    "CHEMONTID:0000032" ;
        skos:prefLabel   "Benzenesulfonic acids and derivatives"@en .

csc:CHEMONTID_0002838
        a                skos:Concept ;
        rdfs:seeAlso     tax_nodes:C0002838 ;
        skos:altLabel    "olefins"@en , "olefin"@en ;
        skos:broader     csc:CHEMONTID_0004475 ;
        skos:definition  "Acyclic and cyclic hydrocarbons having one or more carbon-carbon double bonds, apart from the formal ones in aromatic compounds. The class of olefins subsumes alkenes and cycloalkenes and the corresponding polyenes."@en ;
        skos:inScheme    vlcs:chemische_stof ;
        skos:notation    "CHEMONTID:0002838" ;
        skos:prefLabel   "Olefins"@en .

csc:CHEMONTID_0000207
        a                skos:Concept ;
        skos:altLabel    "2,3-diazanaphthalenes"@en , "phthalazines"@en ;
        skos:broader     csc:CHEMONTID_0004789 ;
        skos:definition  "Compounds containing a phthalazine moiety, which consists of a benzene ring fused to a pyridazine, forming a 2,3-benzodiazine skeleton."@en ;
        skos:inScheme    vlcs:chemische_stof ;
        skos:notation    "CHEMONTID:0000207" ;
        skos:prefLabel   "Phthalazines"@en .

csc:CHEMONTID_0000428
        a                skos:Concept ;
        rdfs:seeAlso     tax_nodes:C0000428 ;
        skos:broader     csc:CHEMONTID_0000422 ;
        skos:definition  "Inorganic compounds containing only metal atoms,with the largest atom being a alkaline earth metal atom."@en ;
        skos:inScheme    vlcs:chemische_stof ;
        skos:notation    "CHEMONTID:0000428" ;
        skos:prefLabel   "Homogeneous alkaline earth metal compounds"@en .

csc:CHEMONTID_0003568
        a                skos:Concept ;
        rdfs:seeAlso     tax_nodes:C0003568 ;
        skos:altLabel    "C19 steroids (androgens) and derivatives"@en , "androstanoid"@en , "Androstanes"@en ;
        skos:broader     csc:CHEMONTID_0000258 ;
        skos:definition  "Steroids with a structure based on the 19-carbon androstane skeleton."@en ;
        skos:inScheme    vlcs:chemische_stof ;
        skos:notation    "CHEMONTID:0003568" ;
        skos:prefLabel   "Androstane steroids"@en .

csc:CHEMONTID_0001656
        a                skos:Concept ;
        skos:altLabel    "acetal"@en ;
        skos:broader     csc:CHEMONTID_0000254 ;
        skos:definition  "Compounds having the structure R2C(OR')2 ( R' not Hydrogen) and thus diethers of geminal diols. Originally, the term was confined to derivatives of aldehydes (one R = H), but it now applies equally to derivatives of ketones (neither R = H ). Mixed acetals have different R' groups."@en ;
        skos:inScheme    vlcs:chemische_stof ;
        skos:notation    "CHEMONTID:0001656" ;
        skos:prefLabel   "Acetals"@en .

csc:CHEMONTID_0000253
        a                skos:Concept ;
        rdfs:seeAlso     tax_nodes:C0000253 ;
        skos:altLabel    "stilbenoid"@en ;
        skos:broader     csc:CHEMONTID_0000261 ;
        skos:definition  "Organic compounds containing a 1,2-diphenylethylene moiety. Stilbenes (C6-C2-C6 ) are derived from the common phenylpropene (C6-C3) skeleton building block. The introduction of one or more hydroxyl groups  to a phenyl ring lead to stilbenoids."@en ;
        skos:inScheme    vlcs:chemische_stof ;
        skos:notation    "CHEMONTID:0000253" ;
        skos:prefLabel   "Stilbenes"@en .

csc:CHEMONTID_0004718
        a                skos:Concept ;
        skos:altLabel    "2-haloacetanilides"@en ;
        skos:broader     csc:CHEMONTID_0004716 ;
        skos:definition  "Organic compounds containing an acetamide group conjugated to a phenyl group, which is in turn ortho-substituted with a halogen atom."@en ;
        skos:inScheme    vlcs:chemische_stof ;
        skos:notation    "CHEMONTID:0004718" ;
        skos:prefLabel   "O-haloacetanilides"@en .

csc:CHEMONTID_0004298
        a                skos:Concept ;
        skos:broader     csc:CHEMONTID_0004296 ;
        skos:definition  "Aromatic compounds containing a ketone substituted by one alkyl group, and a phenyl group."@en ;
        skos:inScheme    vlcs:chemische_stof ;
        skos:notation    "CHEMONTID:0004298" ;
        skos:prefLabel   "Alkyl-phenylketones"@en .

csc:CHEMONTID_0000000
        a                  skos:Concept ;
        rdfs:seeAlso       tax_nodes:C0000000 ;
        skos:altLabel      "an organic compound"@en , "organic molecule"@en ;
        skos:definition    "Compounds that contain at least carbon atom, excluding isocyanide/cyanide and their non-hydrocarbyl derivatives, thiophosgene, carbon diselenide, carbon monosulfide, carbon disulfide, carbon subsulfide, carbon monoxide, carbon trioxide, Carbon suboxide, and dicarbon monoxide."@en , "Compounds that contain at least one carbon atom, excluding isocyanide/cyanide and their non-hydrocarbyl derivatives, thiophosgene, carbon diselenide, carbon monosulfide, carbon disulfide, carbon subsulfide, carbon monoxide, carbon dioxide, Carbon suboxide, and dicarbon monoxide."@en ;
        skos:inScheme      vlcs:chemische_stof ;
        skos:notation      "CHEMONTID:0000000" ;
        skos:prefLabel     "Organic compounds"@en ;
        skos:topConceptOf  vlcs:chemische_stof .

csc:CHEMONTID_0001403
        a                skos:Concept ;
        skos:altLabel    "ergostanoid"@en ;
        skos:broader     csc:CHEMONTID_0003567 ;
        skos:definition  "Steroids containing ergosta-5,7,22-trien-3beta-ol or a  derivative thereof, which is based on the 3beta-hydroxylated ergostane skeleton."@en ;
        skos:inScheme    vlcs:chemische_stof ;
        skos:notation    "CHEMONTID:0001403" ;
        skos:prefLabel   "Ergosterols and derivatives"@en .

csc:CHEMONTID_0004091
        a                skos:Concept ;
        skos:broader     csc:CHEMONTID_0000395 ;
        skos:definition  "Organic compounds containing a nitrate that is O-linked to an alkyl group."@en ;
        skos:inScheme    vlcs:chemische_stof ;
        skos:notation    "CHEMONTID:0004091" ;
        skos:prefLabel   "Alkyl nitrates"@en .

csc:CHEMONTID_0001158
        a                skos:Concept ;
        rdfs:seeAlso     tax_nodes:C0001158 ;
        skos:altLabel    "pyrrolidinone"@en ;
        skos:broader     csc:CHEMONTID_0000218 ;
        skos:definition  "Compounds containing a pyrrolidine ring which bears a C=O group."@en ;
        skos:inScheme    vlcs:chemische_stof ;
        skos:notation    "CHEMONTID:0001158" ;
        skos:prefLabel   "Pyrrolidones"@en .

csc:CHEMONTID_0004511
        a                skos:Concept ;
        skos:broader     csc:CHEMONTID_0000112 ;
        skos:definition  "Organonitrogen compounds that containing a hydrazine group to which an alkyl group is attached."@en ;
        skos:inScheme    vlcs:chemische_stof ;
        skos:notation    "CHEMONTID:0004511" ;
        skos:prefLabel   "Alkylhydrazines"@en .

csc:CHEMONTID_0000474
        a                skos:Concept ;
        skos:altLabel    "biguanides"@en , "Biguanides"@en ;
        skos:broader     csc:CHEMONTID_0000375 ;
        skos:definition  "Organic compounds containing two N-linked guanidines."@en ;
        skos:inScheme    vlcs:chemische_stof ;
        skos:notation    "CHEMONTID:0000474" ;
        skos:prefLabel   "Biguanides"@en .

csc:CHEMONTID_0002308
        a                skos:Concept ;
        skos:altLabel    "pyrimidines"@en ;
        skos:broader     csc:CHEMONTID_0000075 ;
        skos:definition  "Polycyclic aromatic compounds containing a benzene ring linked to a pyrimidine ring through a CC or CN bond.  Pyrimidine is a 6-membered ring consisting of four carbon atoms and two nitrogen centers at the 1- and 3- ring positions."@en ;
        skos:inScheme    vlcs:chemische_stof ;
        skos:notation    "CHEMONTID:0002308" ;
        skos:prefLabel   "Phenylpyrimidines"@en .

csc:CHEMONTID_0004013
        a                skos:Concept ;
        skos:altLabel    "gibberellin carboxylic acid anion"@en ;
        skos:broader     csc:CHEMONTID_0002998 ;
        skos:definition  "C19-gibberellins with a carboxyl group at the 6-position."@en ;
        skos:inScheme    vlcs:chemische_stof ;
        skos:notation    "CHEMONTID:0004013" ;
        skos:prefLabel   "C19-gibberellin 6-carboxylic acids"@en .

csc:CHEMONTID_0001379
        a                skos:Concept ;
        rdfs:seeAlso     tax_nodes:C0001379 ;
        skos:altLabel    "benzodioxine"@en ;
        skos:broader     csc:CHEMONTID_0002100 ;
        skos:definition  "Organic compounds containing a benzene ring fused to a 1,4-dioxin ring."@en ;
        skos:inScheme    vlcs:chemische_stof ;
        skos:notation    "CHEMONTID:0001379" ;
        skos:prefLabel   "Benzo-p-dioxins"@en .

csc:CHEMONTID_0002354
        a                skos:Concept ;
        skos:altLabel    "ester"@en ;
        skos:broader     csc:CHEMONTID_0001238 ;
        skos:definition  "Ester derivatives of enols. They have the general formula RC=COC(=O)R' where R, R' = H or organyl group."@en ;
        skos:inScheme    vlcs:chemische_stof ;
        skos:notation    "CHEMONTID:0002354" ;
        skos:prefLabel   "Enol esters"@en .

csc:CHEMONTID_0001670
        a                skos:Concept ;
        skos:altLabel    "tertiary alcohols"@en , "tertiary alcohol"@en ;
        skos:broader     csc:CHEMONTID_0000129 ;
        skos:definition  "Compounds in which a hydroxy group, -OH, is attached to a saturated carbon atom R3COH (R not H )."@en ;
        skos:inScheme    vlcs:chemische_stof ;
        skos:notation    "CHEMONTID:0001670" ;
        skos:prefLabel   "Tertiary alcohols"@en .

csc:CHEMONTID_0000442
        a                skos:Concept ;
        rdfs:seeAlso     tax_nodes:C0000442 ;
        skos:altLabel    "Metalloids"@en , "Inorganic Chemicals"@en , "inorganic salt"@en ;
        skos:broader     csc:CHEMONTID_0000424 ;
        skos:definition  "Inorganic halogenic compounds in which the heaviest metal atom is a metalloid."@en ;
        skos:inScheme    vlcs:chemische_stof ;
        skos:notation    "CHEMONTID:0000442" ;
        skos:prefLabel   "Metalloid salts"@en .

csc:CHEMONTID_0001845
        a                skos:Concept ;
        skos:altLabel    "organobromine compound"@en , "aromatic ether"@en ;
        skos:broader     csc:CHEMONTID_0004155 ;
        skos:definition  "Compounds that contain two benzene groups linked to each other via an ether bond, and where at least one ring is substituted with a bromo group."@en ;
        skos:inScheme    vlcs:chemische_stof ;
        skos:notation    "CHEMONTID:0001845" ;
        skos:prefLabel   "Bromodiphenyl ethers"@en .

csc:CHEMONTID_0001891
        a                skos:Concept ;
        rdfs:seeAlso     tax_nodes:C0001891 ;
        skos:altLabel    "benzimidazoles"@en , "sulfoxide"@en ;
        skos:broader     csc:CHEMONTID_0000294 ;
        skos:definition  "Polycyclic aromatic compounds containing a sulfinyl group attached at the position 2 of a benzimidazole moiety."@en ;
        skos:inScheme    vlcs:chemische_stof ;
        skos:notation    "CHEMONTID:0001891" ;
        skos:prefLabel   "Sulfinylbenzimidazoles"@en .

csc:CHEMONTID_0004280
        a                skos:Concept ;
        skos:altLabel    "Oxygen-Containing Organoarsenicals"@en ;
        skos:broader     csc:CHEMONTID_0000405 ;
        skos:definition  "Organoarsenic compounds that containing an oxygen atom."@en ;
        skos:inScheme    vlcs:chemische_stof ;
        skos:notation    "CHEMONTID:0004280" ;
        skos:prefLabel   "Oxygen-containing organoarsenic compounds"@en .

csc:CHEMONTID_0000410
        a                skos:Concept ;
        rdfs:seeAlso     tax_nodes:C0000410 ;
        skos:altLabel    "azo compound"@en , "Azo Compounds"@en ;
        skos:broader     csc:CHEMONTID_0000278 ;
        skos:definition  "Derivatives of diazene(diimide), HN=NH, wherein both hydrogens are substituted by hydrocarbyl groups, e.g. PhN=NPh azobenzene or diphenyldiazene."@en ;
        skos:inScheme    vlcs:chemische_stof ;
        skos:notation    "CHEMONTID:0000410" ;
        skos:prefLabel   "Azo compounds"@en .

csc:CHEMONTID_0001813
        a                skos:Concept ;
        rdfs:seeAlso     tax_nodes:C0001813 ;
        skos:altLabel    "peptidomimetic"@en ;
        skos:broader     csc:CHEMONTID_0000264 ;
        skos:definition  "Compounds containing non-peptidic structural elements that is capable of mimicking or antagonizing the biological action(s) of a natural parent peptide."@en ;
        skos:inScheme    vlcs:chemische_stof ;
        skos:notation    "CHEMONTID:0001813" ;
        skos:prefLabel   "Peptidomimetics"@en .

csc:CHEMONTID_0004676
        a                skos:Concept ;
        rdfs:seeAlso     tax_nodes:C0004676 ;
        skos:broader     csc:CHEMONTID_0002279 ;
        skos:definition  "Aromatic compounds hat contain a phenol ether attached to the C2-atom of a phenylpropionic acid."@en ;
        skos:inScheme    vlcs:chemische_stof ;
        skos:notation    "CHEMONTID:0004676" ;
        skos:prefLabel   "2-phenoxypropionic acids"@en .

csc:CHEMONTID_0002764
        a                skos:Concept ;
        skos:altLabel    "bromophenol"@en ;
        skos:broader     csc:CHEMONTID_0002320 ;
        skos:definition  "Halophenols carrying a bromine on the benzene ring."@en ;
        skos:inScheme    vlcs:chemische_stof ;
        skos:notation    "CHEMONTID:0002764" ;
        skos:prefLabel   "Bromophenols"@en .

csc:CHEMONTID_0000133
        a                skos:Concept ;
        skos:altLabel    "a 1,3-dicarbonyl compound"@en ;
        skos:broader     csc:CHEMONTID_0001831 ;
        skos:definition  "Carbonyl compounds with the generic formula O=C(R)C(H)C(R')=O, where R and R' can be any group."@en ;
        skos:inScheme    vlcs:chemische_stof ;
        skos:notation    "CHEMONTID:0000133" ;
        skos:prefLabel   "1,3-dicarbonyl compounds"@en .

csc:CHEMONTID_0000308
        a                skos:Concept ;
        rdfs:seeAlso     tax_nodes:C0000308 ;
        skos:altLabel    "Benzothiadiazines"@en ;
        skos:broader     csc:CHEMONTID_0000224 ;
        skos:definition  "Organic compounds containing a benzene fused to a thiadiazine ring (a six-member ring with two nitrogen atoms and a sulfur atom)."@en ;
        skos:inScheme    vlcs:chemische_stof ;
        skos:notation    "CHEMONTID:0000308" ;
        skos:prefLabel   "Benzothiadiazines"@en .

csc:CHEMONTID_0003416
        a                skos:Concept ;
        skos:altLabel    "carboxylic ester"@en ;
        skos:broader     csc:CHEMONTID_0001238 ;
        skos:definition  "Organic compounds containing a carboxyl group that is esterified with a methyl group. They have the general structure RC(=O)OR', where R=H or organyl group and R'=methyl group."@en ;
        skos:inScheme    vlcs:chemische_stof ;
        skos:notation    "CHEMONTID:0003416" ;
        skos:prefLabel   "Methyl esters"@en .

csc:CHEMONTID_0003960
        a                skos:Concept ;
        skos:broader     csc:CHEMONTID_0003961 ;
        skos:definition  "Organic compounds containing an octyl chain attached to the sulfur of a sulfonic acid (or a derivative thereof), where all hydrogens of the octyl chain are replaced by fluorine atoms."@en ;
        skos:inScheme    vlcs:chemische_stof ;
        skos:notation    "CHEMONTID:0003960" ;
        skos:prefLabel   "Perfluorooctane sulfonic acid and derivatives"@en .

csc:CHEMONTID_0001550
        a                skos:Concept ;
        rdfs:seeAlso     tax_nodes:C0001550 ;
        skos:altLabel    "C15 isoprenoids (sesquiterpenes)"@en , "sesquiterpenoid"@en ;
        skos:broader     csc:CHEMONTID_0000259 ;
        skos:definition  "Terpenes with three consecutive isoprene units."@en ;
        skos:inScheme    vlcs:chemische_stof ;
        skos:notation    "CHEMONTID:0001550" ;
        skos:prefLabel   "Sesquiterpenoids"@en .

csc:CHEMONTID_0002202
        a                skos:Concept ;
        skos:altLabel    "pyrimidines"@en ;
        skos:broader     csc:CHEMONTID_0000075 ;
        skos:definition  "Compounds containing a hydrogenated pyrimidine ring (i.e. containing less than the maximum number of double bonds.)."@en ;
        skos:inScheme    vlcs:chemische_stof ;
        skos:notation    "CHEMONTID:0002202" ;
        skos:prefLabel   "Hydropyrimidines"@en .

csc:CHEMONTID_0004160
        a                skos:Concept ;
        skos:altLabel    "Trihalomethanes"@en , "a trihalomethane"@en , "haloforms"@en ;
        skos:broader     csc:CHEMONTID_0004157 ;
        skos:definition  "Organic compounds in which exactly three of the four hydrogen atoms of methane (CH4) are replaced by halogen atoms."@en ;
        skos:inScheme    vlcs:chemische_stof ;
        skos:notation    "CHEMONTID:0004160" ;
        skos:prefLabel   "Trihalomethanes"@en .

csc:CHEMONTID_0001273
        a                skos:Concept ;
        skos:altLabel    "hydroxytoluene"@en , "a 1,3-cresol"@en , "m-Cresols"@en , "a m-cresol"@en , "1,3-Cresols"@en ;
        skos:broader     csc:CHEMONTID_0001272 ;
        skos:definition  "Aromatic compounds containing a meta-cresol moiety, which consists of a benzene ring bearing a methyl group and a hydroxyl group at ring positions 1 and 3, respectively."@en ;
        skos:inScheme    vlcs:chemische_stof ;
        skos:notation    "CHEMONTID:0001273" ;
        skos:prefLabel   "Meta cresols"@en .

csc:CHEMONTID_0000298
        a                skos:Concept ;
        rdfs:seeAlso     tax_nodes:C0000298 ;
        skos:altLabel    "fatty aldehyde"@en , "Fatty Aldehydes"@en ;
        skos:broader     csc:CHEMONTID_0003909 ;
        skos:definition  "Long chain aldehydes with a chain of at least 12 carbon atoms."@en ;
        skos:inScheme    vlcs:chemische_stof ;
        skos:notation    "CHEMONTID:0000298" ;
        skos:prefLabel   "Fatty aldehydes"@en .

csc:CHEMONTID_0000045
        a                skos:Concept ;
        rdfs:seeAlso     tax_nodes:C0000045 ;
        skos:broader     csc:CHEMONTID_0002279 ;
        skos:definition  "Compounds containing a phenylpropene moiety, which consists of a propene substituent bound to a phenyl group."@en ;
        skos:inScheme    vlcs:chemische_stof ;
        skos:notation    "CHEMONTID:0000045" ;
        skos:prefLabel   "Phenylpropenes"@en .

csc:CHEMONTID_0000013
        a                skos:Concept ;
        rdfs:seeAlso     tax_nodes:C0000013 ;
        skos:altLabel    "Amino Acids, Peptides, and Proteins"@en ;
        skos:broader     csc:CHEMONTID_0000265 ;
        skos:definition  "Organic compounds containing an amino acid or a peptide backbone, or derivatives thereof."@en ;
        skos:inScheme    vlcs:chemische_stof ;
        skos:notation    "CHEMONTID:0000013" ;
        skos:prefLabel   "Amino acids, peptides, and analogues"@en .

csc:CHEMONTID_0004777
        a                skos:Concept ;
        skos:broader     csc:CHEMONTID_0004776 ;
        skos:definition  "Organic compounds containing a n-nitroso group -NN=O."@en ;
        skos:inScheme    vlcs:chemische_stof ;
        skos:notation    "CHEMONTID:0004777" ;
        skos:prefLabel   "Organic N-nitroso compounds"@en .

csc:CHEMONTID_0004524
        a                skos:Concept ;
        rdfs:seeAlso     tax_nodes:C0004524 ;
        skos:broader     csc:CHEMONTID_0002448 ;
        skos:definition  "Aromatic compounds containing a triphenyl moiety."@en ;
        skos:inScheme    vlcs:chemische_stof ;
        skos:notation    "CHEMONTID:0004524" ;
        skos:prefLabel   "Triphenyl compounds"@en .

csc:CHEMONTID_0000487
        a                skos:Concept ;
        skos:altLabel    "benzenes"@en , "carbonyl compound"@en ;
        skos:broader     csc:CHEMONTID_0001248 ;
        skos:definition  "Compounds containing a 2-hydroxybenzoic acid moiety or a derivative thereof."@en ;
        skos:inScheme    vlcs:chemische_stof ;
        skos:notation    "CHEMONTID:0000487" ;
        skos:prefLabel   "Salicylic acid and derivatives"@en .

csc:CHEMONTID_0002865
        a                skos:Concept ;
        rdfs:seeAlso     tax_nodes:C0002865 ;
        skos:altLabel    "acyl halide"@en ;
        skos:broader     csc:CHEMONTID_0000267 ;
        skos:definition  "Organic compounds with the general structure RC(=O)X, where X is a halogen atom."@en ;
        skos:inScheme    vlcs:chemische_stof ;
        skos:notation    "CHEMONTID:0002865" ;
        skos:prefLabel   "Acyl halides"@en .

csc:CHEMONTID_0003097
        a                skos:Concept ;
        skos:altLabel    "organohalogen compound"@en , "benzoic acids"@en ;
        skos:broader     csc:CHEMONTID_0003096 ;
        skos:definition  "Benzoic acids carrying a halogen atom on the benzene ring."@en ;
        skos:inScheme    vlcs:chemische_stof ;
        skos:notation    "CHEMONTID:0003097" ;
        skos:prefLabel   "Halobenzoic acids"@en .

csc:CHEMONTID_0000455
        a                skos:Concept ;
        rdfs:seeAlso     tax_nodes:C0000455 ;
        skos:altLabel    "actinoid molecular entity"@en ;
        skos:broader     csc:CHEMONTID_0000424 ;
        skos:definition  "Organic compounds belonging to either the actinide hydrides, actinide nitrides, actinide oxides, or actinide sulfides."@en ;
        skos:inScheme    vlcs:chemische_stof ;
        skos:notation    "CHEMONTID:0000455" ;
        skos:prefLabel   "Actinide organides"@en .

csc:CHEMONTID_0001858
        a                skos:Concept ;
        skos:altLabel    "naphthyridine derivative"@en ;
        skos:broader     csc:CHEMONTID_0001857 ;
        skos:definition  "Compounds containing a naphthyridine moiety, where one of the ring atoms bears a carboxylic acid group."@en ;
        skos:inScheme    vlcs:chemische_stof ;
        skos:notation    "CHEMONTID:0001858" ;
        skos:prefLabel   "Naphthyridine carboxylic acids and derivatives"@en .

csc:CHEMONTID_0004072
        a                skos:Concept ;
        skos:altLabel    "Trialkyltin Compounds"@en ;
        skos:broader     csc:CHEMONTID_0004066 ;
        skos:definition  "Triorganotin compounds where the tin atom is linked to exactly three alkyl groups."@en ;
        skos:inScheme    vlcs:chemische_stof ;
        skos:notation    "CHEMONTID:0004072" ;
        skos:prefLabel   "Trialkyltins"@en .

csc:CHEMONTID_0001185
        a                skos:Concept ;
        skos:altLabel    "Sulfuric Acid Esters"@en , "a sulfuric acid monoester"@en , "sulfuric ester"@en ;
        skos:broader     csc:CHEMONTID_0003455 ;
        skos:definition  "Organic compounds containing the sulfuric acid monoester functional group, with the generic structure ROS(O)(=O)=O, (R=organyl group)."@en ;
        skos:inScheme    vlcs:chemische_stof ;
        skos:notation    "CHEMONTID:0001185" ;
        skos:prefLabel   "Sulfuric acid monoesters"@en .

csc:CHEMONTID_0004791
        a                skos:Concept ;
        skos:broader     csc:CHEMONTID_0002452 ;
        skos:definition  "Organic disulfides that have the general structural formula RN(R')C(=S)SSC(=S)N(R\")R\"', where R-R\"'=alkyl groups."@en ;
        skos:inScheme    vlcs:chemische_stof ;
        skos:notation    "CHEMONTID:0004791" ;
        skos:prefLabel   "Thiuram disulfides"@en .

csc:CHEMONTID_0000921
        a                skos:Concept ;
        rdfs:seeAlso     tax_nodes:C0000921 ;
        skos:altLabel    "alkaline earth salt"@en ;
        skos:broader     csc:CHEMONTID_0000446 ;
        skos:definition  "Inorganic compounds in which the largest oxoanion is silicate, and in which the heaviest atom not in an oxoanion is an alkaline earth metal."@en ;
        skos:inScheme    vlcs:chemische_stof ;
        skos:notation    "CHEMONTID:0000921" ;
        skos:prefLabel   "Alkaline earth metal silicates"@en .

csc:CHEMONTID_0003310
        a                skos:Concept ;
        skos:altLabel    "a naphthalene sulfate"@en , "naphthalenesulfonic acid"@en ;
        skos:broader     csc:CHEMONTID_0003597 ;
        skos:definition  "Organic aromatic compounds that contain a naphthalene moiety that carries a sulfonic acid group at one or more positions. Naphthalene is a bicyclic compound that is made up of two fused benzene ring."@en ;
        skos:inScheme    vlcs:chemische_stof ;
        skos:notation    "CHEMONTID:0003310" ;
        skos:prefLabel   "Naphthalene sulfonates"@en .

csc:CHEMONTID_0004713
        a                skos:Concept ;
        skos:altLabel    "N-phenylbenzamides"@en ;
        skos:broader     csc:CHEMONTID_0004712 ;
        skos:definition  "Aromatic compounds containing an anilide group in which the carboxamide group is substituted with a benzene ring. They have the general structure RNC(=O)R', where R,R'= benzene."@en ;
        skos:inScheme    vlcs:chemische_stof ;
        skos:notation    "CHEMONTID:0004713" ;
        skos:prefLabel   "Benzanilides"@en .

csc:CHEMONTID_0000676
        a                skos:Concept ;
        skos:altLabel    "Taxane and Abeotaxane diterpenoids"@en , "taxane diterpenoid"@en ;
        skos:broader     csc:CHEMONTID_0001551 ;
        skos:definition  "Diterpenoids with a structure based either on the taxane skeleton, or a derivative thereof. In term of phytochemistry, several derivatives of the taxane skeleton exist: 2(3->20)-abeotaxane, 3,11-cyclotaxane, 11(15->1),11(10->9)-abeotaxane, 3,8-seco-taxane, and 11(15->1)-abeotaxane, among others. More complex skeletons have been found recently, which include the taxane-derived [3.3.3] propellane ring system."@en ;
        skos:inScheme    vlcs:chemische_stof ;
        skos:notation    "CHEMONTID:0000676" ;
        skos:prefLabel   "Taxanes and derivatives"@en .

csc:CHEMONTID_0000423
        a                skos:Concept ;
        rdfs:seeAlso     tax_nodes:C0000423 ;
        skos:broader     csc:CHEMONTID_0000001 ;
        skos:definition  "Inorganic compounds that contain only non-metal elements."@en , "Inorganic compounds that contain only metal elements."@en ;
        skos:inScheme    vlcs:chemische_stof ;
        skos:notation    "CHEMONTID:0000423" ;
        skos:prefLabel   "Homogeneous non-metal compounds"@en .

csc:CHEMONTID_0004215
        a                skos:Concept ;
        skos:broader     csc:CHEMONTID_0004212 ;
        skos:definition  "Aromatic compounds that contain a p-xylenol moiety, which is a monocyclic benzene carrying exactly two methyl groups at the 1- and 4-positions, and at least one hydroxyl group."@en ;
        skos:inScheme    vlcs:chemische_stof ;
        skos:notation    "CHEMONTID:0004215" ;
        skos:prefLabel   "p-Xylenols"@en .

csc:CHEMONTID_0000178
        a                skos:Concept ;
        skos:altLabel    "benzamides"@en , "Benzamides"@en ;
        skos:broader     csc:CHEMONTID_0000176 ;
        skos:definition  "Organic compounds containing a carboxamido substituent attached to a benzene ring."@en ;
        skos:inScheme    vlcs:chemische_stof ;
        skos:notation    "CHEMONTID:0000178" ;
        skos:prefLabel   "Benzamides"@en .

csc:CHEMONTID_0004436
        a                skos:Concept ;
        rdfs:seeAlso     tax_nodes:C0004436 ;
        skos:altLabel    "Alkyl-metal compounds"@en ;
        skos:broader     csc:CHEMONTID_0000462 ;
        skos:definition  "Organometallic compounds hat containing a metal atom substituted by on or more alkyl groups."@en ;
        skos:inScheme    vlcs:chemische_stof ;
        skos:notation    "CHEMONTID:0004436" ;
        skos:prefLabel   "Metal alkyls"@en .

csc:CHEMONTID_0000399
        a                skos:Concept ;
        rdfs:seeAlso     tax_nodes:C0000399 ;
        skos:altLabel    "azide"@en ;
        skos:broader     csc:CHEMONTID_0002279 ;
        skos:definition  "Compounds containing a phenylazide moiety, which consists of a linear azide substituent attached to a phenyl group."@en ;
        skos:inScheme    vlcs:chemische_stof ;
        skos:notation    "CHEMONTID:0000399" ;
        skos:prefLabel   "Phenylazides"@en .

csc:CHEMONTID_0003752
        a                skos:Concept ;
        skos:altLabel    "cedrane sesquiterpenoid"@en , "Cedrane and isocedrane sesquiterpenoids"@en ;
        skos:broader     csc:CHEMONTID_0001550 ;
        skos:definition  "Sesquiternoids with a structure based on the cedrane or the isocedrane skeleton. Cedrane is a tricyclic molecules a 3,6,8,8-tetramethyl-1H-3a,7-methano-azulene moiety. Isocedrane is a rearranged cedrane arising from the migration of methyl group moved from the 6-position to the 4-position."@en ;
        skos:inScheme    vlcs:chemische_stof ;
        skos:notation    "CHEMONTID:0003752" ;
        skos:prefLabel   "Cedrane and isocedrane sesquiterpenoids"@en .

csc:CHEMONTID_0001549
        a                skos:Concept ;
        rdfs:seeAlso     tax_nodes:C0001549 ;
        skos:altLabel    "C10 isoprenoids (monoterpenes)"@en , "monoterpenoid"@en ;
        skos:broader     csc:CHEMONTID_0000259 ;
        skos:definition  "Compounds containing a chain of two isoprene units."@en ;
        skos:inScheme    vlcs:chemische_stof ;
        skos:notation    "CHEMONTID:0001549" ;
        skos:prefLabel   "Monoterpenoids"@en .

csc:CHEMONTID_0004482
        a                skos:Concept ;
        skos:broader     csc:CHEMONTID_0003893 ;
        skos:definition  "Compounds containing a phosphonic acid that is diesterified with alkyl groups, and the phosphorus atom is also directly attached to an alkyl group."@en ;
        skos:inScheme    vlcs:chemische_stof ;
        skos:notation    "CHEMONTID:0004482" ;
        skos:prefLabel   "Dialkyl alkylphosphonates"@en .

csc:CHEMONTID_0002279
        a                skos:Concept ;
        rdfs:seeAlso     tax_nodes:C0002279 ;
        skos:altLabel    "Benzene compounds"@en , "benzenes"@en ;
        skos:broader     csc:CHEMONTID_0002448 ;
        skos:definition  "Aromatic compounds containing one monocyclic ring system consisting of benzene."@en ;
        skos:inScheme    vlcs:chemische_stof ;
        skos:notation    "CHEMONTID:0002279" ;
        skos:prefLabel   "Benzene and substituted derivatives"@en .

csc:CHEMONTID_0002998
        a                skos:Concept ;
        skos:altLabel    "C19-gibberellin"@en , "20-norgibberellane diterpenoids"@en , "20-norgibberellins"@en ;
        skos:broader     csc:CHEMONTID_0001767 ;
        skos:definition  "Gibberellins containing 19 carbon atoms, with the COOH group in position 7. In nearly all C19-gibberellins, the carboxyl group at C-4 forms a lactone  ring at C-10, a configuration which arises in connection with the loss of the extra C-20 atom."@en ;
        skos:inScheme    vlcs:chemische_stof ;
        skos:notation    "CHEMONTID:0002998" ;
        skos:prefLabel   "C19-gibberellins"@en .

csc:CHEMONTID_0001517
        a                skos:Concept ;
        rdfs:seeAlso     tax_nodes:C0001517 ;
        skos:altLabel    "organofluorine compound"@en , "Fluorocarbons"@en , "an organofluride"@en ;
        skos:broader     csc:CHEMONTID_0000267 ;
        skos:definition  "Compounds containing a chemical bond between a carbon atom and a fluorine atom."@en ;
        skos:inScheme    vlcs:chemische_stof ;
        skos:notation    "CHEMONTID:0001517" ;
        skos:prefLabel   "Organofluorides"@en .

csc:CHEMONTID_0001097
        a                skos:Concept ;
        rdfs:seeAlso     tax_nodes:C0001097 ;
        skos:altLabel    "a benzyloxycarbonyl compound"@en , "Benzyloxycarbonyl compound"@en , "a benzyloxycarbonyl"@en , "carboxylic ester"@en ;
        skos:broader     csc:CHEMONTID_0002279 ;
        skos:definition  "Organic compounds containing a carbonyl group substituted with a benzyloxyl group."@en ;
        skos:inScheme    vlcs:chemische_stof ;
        skos:notation    "CHEMONTID:0001097" ;
        skos:prefLabel   "Benzyloxycarbonyls"@en .

csc:CHEMONTID_0004450
        a                skos:Concept ;
        rdfs:seeAlso     tax_nodes:C0004450 ;
        skos:broader     csc:CHEMONTID_0000265 ;
        skos:definition  "Organic compounds containing acrylic acid CH2=CHCO2H or a derivative thereof."@en ;
        skos:inScheme    vlcs:chemische_stof ;
        skos:notation    "CHEMONTID:0004450" ;
        skos:prefLabel   "Acrylic acids and derivatives"@en .

csc:CHEMONTID_0001563
        a                skos:Concept ;
        skos:altLabel    "monoterpenoid"@en ;
        skos:broader     csc:CHEMONTID_0001549 ;
        skos:definition  "Monoterpenoids containing 1 ring in the isoprene chain."@en ;
        skos:inScheme    vlcs:chemische_stof ;
        skos:notation    "CHEMONTID:0001563" ;
        skos:prefLabel   "Monocyclic monoterpenoids"@en .

csc:CHEMONTID_0000160
        a                skos:Concept ;
        rdfs:seeAlso     tax_nodes:C0000160 ;
        skos:altLabel    "lactam"@en , "Lactams"@en , "lactams"@en ;
        skos:broader     csc:CHEMONTID_0000002 ;
        skos:definition  "Compounds containing a lactam ring, which is a cyclic amide of amino carboxylic acids, having a 1-azacycloalkan-2-one structure (or an analogue having unsaturation or heteroatoms replacing one or more carbon atoms of the ring)."@en ;
        skos:inScheme    vlcs:chemische_stof ;
        skos:notation    "CHEMONTID:0000160" ;
        skos:prefLabel   "Lactams"@en .

csc:CHEMONTID_0001019
        a                skos:Concept ;
        skos:altLabel    "alkadiene"@en ;
        skos:broader     csc:CHEMONTID_0002839 ;
        skos:definition  "Acyclic hydrocarbons that contain exactly two carbon-to-carbon double bonds."@en ;
        skos:inScheme    vlcs:chemische_stof ;
        skos:notation    "CHEMONTID:0001019" ;
        skos:prefLabel   "Alkadienes"@en .

csc:CHEMONTID_0002966
        a                skos:Concept ;
        rdfs:seeAlso     tax_nodes:C0002966 ;
        skos:broader     csc:CHEMONTID_0000265 ;
        skos:definition  "Carboxylic acids containing exactly four carboxyl groups."@en ;
        skos:inScheme    vlcs:chemische_stof ;
        skos:notation    "CHEMONTID:0002966" ;
        skos:prefLabel   "Tetracarboxylic acids and derivatives"@en .

csc:CHEMONTID_0004671
        a                skos:Concept ;
        skos:broader     csc:CHEMONTID_0000036 ;
        skos:definition  "Aromatic compounds containing a nitrobenzene moiety that carries an ether group on the benzene ring."@en ;
        skos:inScheme    vlcs:chemische_stof ;
        skos:notation    "CHEMONTID:0004671" ;
        skos:prefLabel   "Nitrophenyl ethers"@en .

csc:CHEMONTID_0001065
        a                skos:Concept ;
        rdfs:seeAlso     tax_nodes:C0001065 ;
        skos:altLabel    "p-block molecular entity"@en ;
        skos:broader     csc:CHEMONTID_0000435 ;
        skos:definition  "Inorganic non-metallic compounds containing a perchlorate as its largest oxoanion."@en , "Inorganic non-metallic compoundscontaining a perchlorate as its largest oxoanion."@en ;
        skos:inScheme    vlcs:chemische_stof ;
        skos:notation    "CHEMONTID:0001065" ;
        skos:prefLabel   "Non-metal perchlorates"@en .

csc:CHEMONTID_0000303
        a                skos:Concept ;
        rdfs:seeAlso     tax_nodes:C0000303 ;
        skos:broader     csc:CHEMONTID_0000195 ;
        skos:definition  "Compounds containing a phenylpiperidine skeleton, which consists of a piperidine bound to a phenyl group."@en ;
        skos:inScheme    vlcs:chemische_stof ;
        skos:notation    "CHEMONTID:0000303" ;
        skos:prefLabel   "Phenylpiperidines"@en .

csc:CHEMONTID_0004348
        a                skos:Concept ;
        skos:broader     csc:CHEMONTID_0001524 ;
        skos:definition  "Compounds containing a tin compound bonded to exactly four carbon atoms."@en ;
        skos:inScheme    vlcs:chemische_stof ;
        skos:notation    "CHEMONTID:0004348" ;
        skos:prefLabel   "Tetraorganotin compounds"@en .

csc:CHEMONTID_0001286
        a                skos:Concept ;
        rdfs:seeAlso     tax_nodes:C0001286 ;
        skos:altLabel    "benzenediols"@en ;
        skos:broader     csc:CHEMONTID_0000134 ;
        skos:definition  "Organic compounds containing two hydroxyl groups attached to a benzene ring."@en ;
        skos:inScheme    vlcs:chemische_stof ;
        skos:notation    "CHEMONTID:0001286" ;
        skos:prefLabel   "Benzenediols"@en .

csc:CHEMONTID_0002436
        a                skos:Concept ;
        skos:altLabel    "enal"@en ;
        skos:broader     csc:CHEMONTID_0002433 ;
        skos:definition  "An alpha,beta-unsaturated aldehyde of general formula RC=C-CH=O in which the aldehydic C=O function is conjugated to a C=C triple bond at the alpha,beta position."@en ;
        skos:inScheme    vlcs:chemische_stof ;
        skos:notation    "CHEMONTID:0002436" ;
        skos:prefLabel   "Enals"@en .

csc:CHEMONTID_0000058
        a                skos:Concept ;
        rdfs:seeAlso     tax_nodes:C0000058 ;
        skos:altLabel    "Morphinans"@en , "morphinane alkaloid"@en ;
        skos:broader     csc:CHEMONTID_0000279 ;
        skos:definition  "Polycyclic compounds with a four-ring skeleton with three condensed six-member rings forming a partially hydrogenated phenanthrene moiety, one of which is aromatic while the two others are alicyclic."@en ;
        skos:inScheme    vlcs:chemische_stof ;
        skos:notation    "CHEMONTID:0000058" ;
        skos:prefLabel   "Morphinans"@en .

csc:CHEMONTID_0003411
        a                skos:Concept ;
        rdfs:seeAlso     tax_nodes:C0003411 ;
        skos:altLabel    "2-benzopyran"@en , "Isochromenes"@en ;
        skos:broader     csc:CHEMONTID_0000123 ;
        skos:definition  "Organic aromatic compounds that 1-benzopyran, a bicyclic compound made up of a benzene ring fused to a pyran, so that the oxygen atom is at the 2-position."@en ;
        skos:inScheme    vlcs:chemische_stof ;
        skos:notation    "CHEMONTID:0003411" ;
        skos:prefLabel   "2-benzopyrans"@en .

csc:CHEMONTID_0002902
        a                skos:Concept ;
        rdfs:seeAlso     tax_nodes:C0002902 ;
        skos:altLabel    "milbemycin"@en ;
        skos:broader     csc:CHEMONTID_0000147 ;
        skos:definition  "A group of macrolides with a structure containing a 16-membered lactone ring fused to a 1,7-dioxaspiroundecane ring system and to either a benzofuran (or hydrogenated derivative thereof). In some cases (e.g. Milbemycin E), the tetrahydrofuranyl ring is missing. Milbemycins can be o-glycosylated at C13 to form Avermectins. Milbemycins are produced by Streptomyces species."@en ;
        skos:inScheme    vlcs:chemische_stof ;
        skos:notation    "CHEMONTID:0002902" ;
        skos:prefLabel   "Milbemycins"@en .

csc:CHEMONTID_0000279
        a                skos:Concept ;
        rdfs:seeAlso     tax_nodes:C0000279 ;
        skos:altLabel    "alkaloids"@en , "an alkaloid"@en , "alkaloid"@en , "Alkaloids"@en ;
        skos:broader     csc:CHEMONTID_0000000 ;
        skos:definition  "Naturally occurring chemical compounds that contain mostly basic nitrogen atoms. This group also includes some related compounds with neutral and even weakly acidic properties. Also some synthetic compounds of similar structure are attributed to alkaloids. In addition to carbon, hydrogen and nitrogen, alkaloids may also contain oxygen, sulfur and more rarely other elements such as chlorine, bromine, and phosphorus."@en ;
        skos:inScheme    vlcs:chemische_stof ;
        skos:notation    "CHEMONTID:0000279" ;
        skos:prefLabel   "Alkaloids and derivatives"@en .

csc:CHEMONTID_0002404
        a                skos:Concept ;
        skos:altLabel    "alpha-amino acid"@en ;
        skos:broader     csc:CHEMONTID_0000060 ;
        skos:definition  "Amino acids in which the amino group is attached to the carbon atom immediately adjacent to the carboxylate group (alpha carbon)."@en ;
        skos:inScheme    vlcs:chemische_stof ;
        skos:notation    "CHEMONTID:0002404" ;
        skos:prefLabel   "Alpha amino acids"@en .

csc:CHEMONTID_0001973
        a                skos:Concept ;
        rdfs:seeAlso     tax_nodes:C0001973 ;
        skos:altLabel    "benzoxazole"@en ;
        skos:broader     csc:CHEMONTID_0000302 ;
        skos:definition  "Organic compounds containing a benzene fused to an oxazole ring (a five-member aliphatic ring with three carbon atoms, one oxygen atom, and one nitrogen atom) bearing a ketone group."@en ;
        skos:inScheme    vlcs:chemische_stof ;
        skos:notation    "CHEMONTID:0001973" ;
        skos:prefLabel   "Benzoxazolones"@en .

csc:CHEMONTID_0002450
        a                skos:Concept ;
        skos:altLabel    "a primary amine"@en , "primary amine"@en ;
        skos:broader     csc:CHEMONTID_0002449 ;
        skos:definition  "Amines having the nitrogen atom linked to exactly one hydrocarbyl group."@en ;
        skos:inScheme    vlcs:chemische_stof ;
        skos:notation    "CHEMONTID:0002450" ;
        skos:prefLabel   "Primary amines"@en .

csc:CHEMONTID_0004537
        a                skos:Concept ;
        skos:broader     csc:CHEMONTID_0000053 ;
        skos:definition  "Organic compounds containing an amino group attached to the 4-position of a quinoline ring system."@en ;
        skos:inScheme    vlcs:chemische_stof ;
        skos:notation    "CHEMONTID:0004537" ;
        skos:prefLabel   "4-aminoquinolines"@en .

csc:CHEMONTID_0000072
        a                skos:Concept ;
        rdfs:seeAlso     tax_nodes:C0000072 ;
        skos:altLabel    "dibenzodiazepine"@en ;
        skos:broader     csc:CHEMONTID_0000295 ;
        skos:definition  "Compounds containing a dibenzodiazepine moiety, which consists of two benzene connected by diazepine ring."@en ;
        skos:inScheme    vlcs:chemische_stof ;
        skos:notation    "CHEMONTID:0000072" ;
        skos:prefLabel   "Dibenzodiazepines"@en .

csc:CHEMONTID_0001475
        a                skos:Concept ;
        skos:broader     csc:CHEMONTID_0001470 ;
        skos:definition  "Inorganic compounds in which the largest metallic oxoanion is arsenite, to which either no atom or a non metal atom is bonded."@en ;
        skos:inScheme    vlcs:chemische_stof ;
        skos:notation    "CHEMONTID:0001475" ;
        skos:prefLabel   "Miscellaneous arsenites"@en .

csc:CHEMONTID_0000247
        a                skos:Concept ;
        skos:altLabel    "Xanthines"@en , "a xanthine"@en ;
        skos:broader     csc:CHEMONTID_0000245 ;
        skos:definition  "Purine derivatives with a ketone group conjugated at carbons 2 and 6 of the purine moiety."@en ;
        skos:inScheme    vlcs:chemische_stof ;
        skos:notation    "CHEMONTID:0000247" ;
        skos:prefLabel   "Xanthines"@en .

csc:CHEMONTID_0003600
        a                skos:Concept ;
        skos:altLabel    "naphthalenesulfonic acid"@en ;
        skos:broader     csc:CHEMONTID_0003310 ;
        skos:definition  "Organic aromatic compounds that contain a naphthalene moiety that carries a sulfonic acid group at the 1-position. Naphthalene is a bicyclic compound that is made up of two fused benzene ring."@en ;
        skos:inScheme    vlcs:chemische_stof ;
        skos:notation    "CHEMONTID:0003600" ;
        skos:prefLabel   "1-naphthalene sulfonates"@en .

csc:CHEMONTID_0000293
        a                skos:Concept ;
        rdfs:seeAlso     tax_nodes:C0000293 ;
        skos:altLabel    "Benzazepines"@en ;
        skos:broader     csc:CHEMONTID_0000002 ;
        skos:definition  "Organic compounds containing a benzene ring fused to an azepine ring (unsaturated seven-membered heterocycle with one nitrogen atom replacing a carbon atom)."@en ;
        skos:inScheme    vlcs:chemische_stof ;
        skos:notation    "CHEMONTID:0000293" ;
        skos:prefLabel   "Benzazepines"@en .

csc:CHEMONTID_0004758
        a                skos:Concept ;
        rdfs:seeAlso     tax_nodes:C0004758 ;
        skos:broader     csc:CHEMONTID_0000076 ;
        skos:definition  "Aromatic heterocyclic compounds containing a furan ring, which carries a carboxyl group or a derivative thereof."@en ;
        skos:inScheme    vlcs:chemische_stof ;
        skos:notation    "CHEMONTID:0004758" ;
        skos:prefLabel   "Furoic acid and derivatives"@en .

csc:CHEMONTID_0004505
        a                skos:Concept ;
        skos:broader     csc:CHEMONTID_0000141 ;
        skos:definition  "Organic aromatic compounds containing a benzene that carries a single phenol group and exactly two nitro groups."@en ;
        skos:inScheme    vlcs:chemische_stof ;
        skos:notation    "CHEMONTID:0004505" ;
        skos:prefLabel   "Dinitrophenols"@en .

csc:CHEMONTID_0001443
        a                skos:Concept ;
        rdfs:seeAlso     tax_nodes:C0001443 ;
        skos:altLabel    "triazolopyrimidines"@en ;
        skos:broader     csc:CHEMONTID_0000002 ;
        skos:definition  "Polycyclic aromatic compounds containing triazole ring fused to a pyrimidine ring. Triazole is a five-membered ring consisting of two carbon atoms and three nitrogen atoms. Pyrimidine is a 6-membered ring consisting of four carbon atoms and two nitrogen centers at the 1- and 3- ring positions."@en ;
        skos:inScheme    vlcs:chemische_stof ;
        skos:notation    "CHEMONTID:0001443" ;
        skos:prefLabel   "Triazolopyrimidines"@en .

csc:CHEMONTID_0000215
        a                skos:Concept ;
        skos:broader     csc:CHEMONTID_0000011 ;
        skos:definition  "Compounds containing a saccharide unit which bears a carboxylic acid group."@en ;
        skos:inScheme    vlcs:chemische_stof ;
        skos:notation    "CHEMONTID:0000215" ;
        skos:prefLabel   "Sugar acids and derivatives"@en .

csc:CHEMONTID_0001198
        a                skos:Concept ;
        rdfs:seeAlso     tax_nodes:C0001198 ;
        skos:altLabel    "thiocarbonyl compound"@en ;
        skos:broader     csc:CHEMONTID_0000004 ;
        skos:definition  "Organic compounds containing a functional group with the general structure R1C(=S)R2 (R1, R2=H, alkyl, aryl)."@en ;
        skos:inScheme    vlcs:chemische_stof ;
        skos:notation    "CHEMONTID:0001198" ;
        skos:prefLabel   "Thiocarbonyl compounds"@en .

csc:CHEMONTID_0004551
        a                skos:Concept ;
        rdfs:seeAlso     tax_nodes:C0004551 ;
        skos:altLabel    "(trifluoromethyl)benzenes"@en ;
        skos:broader     csc:CHEMONTID_0002279 ;
        skos:definition  "Organofluorine compounds that contain a benzene ring substituted with one or more trifluoromethyl groups."@en ;
        skos:inScheme    vlcs:chemische_stof ;
        skos:notation    "CHEMONTID:0004551" ;
        skos:prefLabel   "Trifluoromethylbenzenes"@en .

csc:CHEMONTID_0002348
        a                skos:Concept ;
        rdfs:seeAlso     tax_nodes:C0002348 ;
        skos:altLabel    "quinolines"@en ;
        skos:broader     csc:CHEMONTID_0001253 ;
        skos:definition  "Heterocyclic compounds containing a quinoline moiety substituted with a phenyl group."@en ;
        skos:inScheme    vlcs:chemische_stof ;
        skos:notation    "CHEMONTID:0002348" ;
        skos:prefLabel   "Phenylquinolines"@en .

csc:CHEMONTID_0000261
        a                skos:Concept ;
        rdfs:seeAlso     tax_nodes:C0000261 ;
        skos:broader     csc:CHEMONTID_0000000 ;
        skos:definition  "Organic compounds that are synthesized either from the amino acid phenylalanine (phenylpropanoids) or the decarboxylative condensation of malonyl-CoA (polyketides). Phenylpropanoids are aromatic compounds based on the phenylpropane skeleton. Polyketides usually consist of alternating carbonyl and methylene groups (beta-polyketones), biogenetically derived from repeated condensation of acetyl coenzyme A (via malonyl coenzyme A), and usually the compounds derived from them by further condensations."@en ;
        skos:inScheme    vlcs:chemische_stof ;
        skos:notation    "CHEMONTID:0000261" ;
        skos:prefLabel   "Phenylpropanoids and polyketides"@en .

csc:CHEMONTID_0001664
        a                skos:Concept ;
        skos:altLabel    "carboxamide"@en ;
        skos:broader     csc:CHEMONTID_0000475 ;
        skos:definition  "Compounds containing an amide derivative of carboxylic acid, with the general structure RN(R1)C(R2)=O (R1-R2 any atom but H)."@en ;
        skos:inScheme    vlcs:chemische_stof ;
        skos:notation    "CHEMONTID:0001664" ;
        skos:prefLabel   "Tertiary carboxylic acid amides"@en .

csc:CHEMONTID_0000436
        a                skos:Concept ;
        rdfs:seeAlso     tax_nodes:C0000436 ;
        skos:altLabel    "Azoles"@en , "azole"@en ;
        skos:broader     csc:CHEMONTID_0000002 ;
        skos:definition  "Organic compounds comprising a five-member nitrogen heterocyclic ring containing at least one other non-carbon atom of either nitrogen, sulfur, or oxygen. The parent compounds are aromatic and have two double bonds; there are successively reduced analogs (azolines and azolidines) with fewer."@en , "Organic compounds comprising a five-member nitrogen heterocyclic ring containing at least one other non-carbon atom of either nitrogen, sulfur, or oxygen."@en ;
        skos:inScheme    vlcs:chemische_stof ;
        skos:notation    "CHEMONTID:0000436" ;
        skos:prefLabel   "Azoles"@en .

csc:CHEMONTID_0003544
        a                skos:Concept ;
        skos:altLabel    "methyl-branched fatty acid"@en ;
        skos:broader     csc:CHEMONTID_0000338 ;
        skos:definition  "Fatty acids with an acyl chain that has a methyl branch. Usually, they are saturated and contain only one or more methyl group. However, branches other than methyl may be present."@en ;
        skos:inScheme    vlcs:chemische_stof ;
        skos:notation    "CHEMONTID:0003544" ;
        skos:prefLabel   "Methyl-branched fatty acids"@en .

csc:CHEMONTID_0002362
        a                skos:Concept ;
        skos:altLabel    "Thienamycins"@en , "carbapenems"@en ;
        skos:broader     csc:CHEMONTID_0000167 ;
        skos:definition  "Beta-lactam antibiotics that differ from penicillins in having the thiazolidine sulfur atom replaced by carbon, the sulfur then becoming the first atom in the side chain."@en ;
        skos:inScheme    vlcs:chemische_stof ;
        skos:notation    "CHEMONTID:0002362" ;
        skos:prefLabel   "Thienamycins"@en .

csc:CHEMONTID_0000159
        a                skos:Concept ;
        rdfs:seeAlso     tax_nodes:C0000159 ;
        skos:altLabel    "Oxiranes"@en , "Epoxy Compounds"@en , "An epoxide"@en ;
        skos:broader     csc:CHEMONTID_0000002 ;
        skos:definition  "Compounds containing a cyclic ether with three ring atoms(one oxygen and two carbon atoms)."@en ;
        skos:inScheme    vlcs:chemische_stof ;
        skos:notation    "CHEMONTID:0000159" ;
        skos:prefLabel   "Epoxides"@en .

csc:CHEMONTID_0001853
        a                skos:Concept ;
        rdfs:seeAlso     tax_nodes:C0001853 ;
        skos:altLabel    "trioxane"@en ;
        skos:broader     csc:CHEMONTID_0000002 ;
        skos:definition  "Compounds containing a six-member aliphatic saturated heterocycle made up of three oxygen atoms and three carbon atoms."@en ;
        skos:inScheme    vlcs:chemische_stof ;
        skos:notation    "CHEMONTID:0001853" ;
        skos:prefLabel   "Trioxanes"@en .

csc:CHEMONTID_0001180
        a                skos:Concept ;
        rdfs:seeAlso     tax_nodes:C0001180 ;
        skos:altLabel    "Sulfuric Acids"@en , "organic sulfate"@en ;
        skos:broader     csc:CHEMONTID_0000403 ;
        skos:definition  "Organic compounds containing the sulfuric acid functional group, with the generic structure HOS(=O)(=O)OH."@en ;
        skos:inScheme    vlcs:chemische_stof ;
        skos:notation    "CHEMONTID:0001180" ;
        skos:prefLabel   "Organic sulfuric acids"@en .

csc:CHEMONTID_0004638
        a                skos:Concept ;
        skos:broader     csc:CHEMONTID_0004105 ;
        skos:definition  "Aromatic compounds containing a 1,3,5-triazine ring that is substituted at the 2-position with an alkoxy group."@en ;
        skos:inScheme    vlcs:chemische_stof ;
        skos:notation    "CHEMONTID:0004638" ;
        skos:prefLabel   "Alkoxy-S-triazines"@en .

csc:CHEMONTID_0004210
        a                skos:Concept ;
        skos:broader     csc:CHEMONTID_0004208 ;
        skos:definition  "Aromatic compounds that contain a o-xylene moiety, which is a monocyclic benzene carrying exactly two methyl groups at the 1- and 2-positions."@en ;
        skos:inScheme    vlcs:chemische_stof ;
        skos:notation    "CHEMONTID:0004210" ;
        skos:prefLabel   "o-Xylenes"@en .

csc:CHEMONTID_0000173
        a                skos:Concept ;
        skos:altLabel    "Cephalosporins"@en , "cephalosporins"@en , "cephalosporin"@en ;
        skos:broader     csc:CHEMONTID_0000168 ;
        skos:definition  "Compounds containing a 1,2-thiazine fused to a 2-azetidinone to for a oxo-5-thia-1-azabicyclo[4.2.0]oct-2-ene-2-carboxylic acid moiety or a derivative thereof."@en ;
        skos:inScheme    vlcs:chemische_stof ;
        skos:notation    "CHEMONTID:0000173" ;
        skos:prefLabel   "Cephalosporins"@en .

csc:CHEMONTID_0002551
        a                skos:Concept ;
        rdfs:seeAlso     tax_nodes:C0002551 ;
        skos:broader     csc:CHEMONTID_0000261 ;
        skos:definition  "Compounds with a structure containing a benzene ring conjugated to a propanoic acid."@en ;
        skos:inScheme    vlcs:chemische_stof ;
        skos:notation    "CHEMONTID:0002551" ;
        skos:prefLabel   "Phenylpropanoic acids"@en .

csc:CHEMONTID_0003954
        a                skos:Concept ;
        skos:altLabel    "organochlorine compound"@en , "a polybrominated biphenyl"@en , "PBBs"@en , "biphenyls"@en ;
        skos:broader     csc:CHEMONTID_0000052 ;
        skos:definition  "Organic aromatic compounds containing a biphenyl moiety, which is substituted at two or more ring positions by a bromine atom."@en ;
        skos:inScheme    vlcs:chemische_stof ;
        skos:notation    "CHEMONTID:0003954" ;
        skos:prefLabel   "Polybrominated biphenyls"@en .

csc:CHEMONTID_0000348
        a                skos:Concept ;
        skos:altLabel    "peptide"@en , "Peptides"@en ;
        skos:broader     csc:CHEMONTID_0000013 ;
        skos:definition  "Compounds containing an amide derived from two or more amino carboxylic acid molecules (the same or different) by formation of a covalent bond from the carbonyl carbon of one to the nitrogen atom of another."@en ;
        skos:inScheme    vlcs:chemische_stof ;
        skos:notation    "CHEMONTID:0000348" ;
        skos:prefLabel   "Peptides"@en .

csc:CHEMONTID_0001797
        a                skos:Concept ;
        rdfs:seeAlso     tax_nodes:C0001797 ;
        skos:altLabel    "imidazopyrimidine"@en ;
        skos:broader     csc:CHEMONTID_0000002 ;
        skos:definition  "Organic polycyclic compounds containing an imidazole ring fused to a pyrimidine ring. Imidazole is 5-membered ring consisting of three carbon atoms, and two nitrogen centers at the 1- and 3-positions. Pyrimidine is a 6-membered ring consisting of four carbon atoms and two nitrogen centers at the 1- and 3- ring positions."@en ;
        skos:inScheme    vlcs:chemische_stof ;
        skos:notation    "CHEMONTID:0001797" ;
        skos:prefLabel   "Imidazopyrimidines"@en .

csc:CHEMONTID_0003203
        a                skos:Concept ;
        skos:altLabel    "maleimides"@en ;
        skos:broader     csc:CHEMONTID_0001158 ;
        skos:definition  "Compounds containing a 2,5-pyrroledione moiety."@en ;
        skos:inScheme    vlcs:chemische_stof ;
        skos:notation    "CHEMONTID:0003203" ;
        skos:prefLabel   "Maleimides"@en .

csc:CHEMONTID_0000394
        a                skos:Concept ;
        skos:altLabel    "alpha-amino acid ester"@en ;
        skos:broader     csc:CHEMONTID_0000060 ;
        skos:definition  "Ester derivatives of alpha amino acids."@en ;
        skos:inScheme    vlcs:chemische_stof ;
        skos:notation    "CHEMONTID:0000394" ;
        skos:prefLabel   "Alpha amino acid esters"@en .

csc:CHEMONTID_0002228
        a                skos:Concept ;
        skos:altLabel    "secondary amino compound"@en ;
        skos:broader     csc:CHEMONTID_0002451 ;
        skos:definition  "Organic compounds containing a dialkylamine group, characterized by two alkyl groups bonded to the amino nitrogen."@en ;
        skos:inScheme    vlcs:chemische_stof ;
        skos:notation    "CHEMONTID:0002228" ;
        skos:prefLabel   "Dialkylamines"@en .

csc:CHEMONTID_0002772
        a                skos:Concept ;
        skos:altLabel    "monochlorophenol"@en ;
        skos:broader     csc:CHEMONTID_0002766 ;
        skos:definition  "Chlorophenols carrying a iodine at the C4 position of the benzene ring."@en ;
        skos:inScheme    vlcs:chemische_stof ;
        skos:notation    "CHEMONTID:0002772" ;
        skos:prefLabel   "P-chlorophenols"@en .

csc:CHEMONTID_0000141
        a                skos:Concept ;
        rdfs:seeAlso     tax_nodes:C0000141 ;
        skos:altLabel    "Nitrophenols"@en ;
        skos:broader     csc:CHEMONTID_0000134 ;
        skos:definition  "Compounds containing a nitrophenol moiety, which consists of a benzene ring bearing both a hydroxyl group and a nitro group on two different ring carbon atoms."@en ;
        skos:inScheme    vlcs:chemische_stof ;
        skos:notation    "CHEMONTID:0000141" ;
        skos:prefLabel   "Nitrophenols"@en .

csc:CHEMONTID_0001544
        a                skos:Concept ;
        rdfs:seeAlso     tax_nodes:C0001544 ;
        skos:altLabel    "purine ribonucleotide"@en ;
        skos:broader     csc:CHEMONTID_0001506 ;
        skos:definition  "Nucleotides consisting of a purine base linked to a ribose to which at least one phosphate group is attached."@en ;
        skos:inScheme    vlcs:chemische_stof ;
        skos:notation    "CHEMONTID:0001544" ;
        skos:prefLabel   "Purine ribonucleotides"@en .

csc:CHEMONTID_0003922
        a                skos:Concept ;
        skos:altLabel    "acetamides"@en ;
        skos:broader     csc:CHEMONTID_0000475 ;
        skos:definition  "Organic compounds with the general formula RNHC(=O)CH3, where R= organyl group."@en ;
        skos:inScheme    vlcs:chemische_stof ;
        skos:notation    "CHEMONTID:0003922" ;
        skos:prefLabel   "Acetamides"@en .

csc:CHEMONTID_0000316
        a                skos:Concept ;
        rdfs:seeAlso     tax_nodes:C0000316 ;
        skos:altLabel    "Benzopyrenes"@en ;
        skos:broader     csc:CHEMONTID_0001851 ;
        skos:definition  "Organic compounds containing a benzene fused to a pyrene(benzo[def]phenanthrene) ring system."@en ;
        skos:inScheme    vlcs:chemische_stof ;
        skos:notation    "CHEMONTID:0000316" ;
        skos:prefLabel   "Benzopyrenes"@en .

csc:CHEMONTID_0004108
        a                skos:Concept ;
        skos:altLabel    "nitrotoluene"@en ;
        skos:broader     csc:CHEMONTID_0001091 ;
        skos:definition  "Organic aromatic compounds containing a benzene that carries a single methyl group and at least 1 nitro group."@en ;
        skos:inScheme    vlcs:chemische_stof ;
        skos:notation    "CHEMONTID:0004108" ;
        skos:prefLabel   "Nitrotoluenes"@en .

csc:CHEMONTID_0002449
        a                skos:Concept ;
        rdfs:seeAlso     tax_nodes:C0002449 ;
        skos:altLabel    "amine"@en , "amines"@en ;
        skos:broader     csc:CHEMONTID_0000278 ;
        skos:definition  "Compounds formally derived from ammonia by replacing one, two or three hydrogen atoms by hydrocarbyl groups, and having the general structures RNH2 (primary amines), R2NH (secondary amines), R3N (tertiary amines)."@en ;
        skos:inScheme    vlcs:chemische_stof ;
        skos:notation    "CHEMONTID:0002449" ;
        skos:prefLabel   "Amines"@en .

csc:CHEMONTID_0000362
        a                skos:Concept ;
        skos:altLabel    "Cyanides"@en , "nitriles"@en , "Nitriles"@en , "nitrile"@en ;
        skos:broader     csc:CHEMONTID_0004504 ;
        skos:definition  "Compounds having the structure RC#N; thus C-substituted derivatives of hydrocyanic acid, HC#N."@en ;
        skos:inScheme    vlcs:chemische_stof ;
        skos:notation    "CHEMONTID:0000362" ;
        skos:prefLabel   "Nitriles"@en .

csc:CHEMONTID_0001092
        a                skos:Concept ;
        skos:altLabel    "hemiacetal"@en ;
        skos:broader     csc:CHEMONTID_0000254 ;
        skos:definition  "Compounds comprising the hemiacetal functional group, with the general formula R2C(OH)OR' ( R' not Hydrogen )."@en ;
        skos:inScheme    vlcs:chemische_stof ;
        skos:notation    "CHEMONTID:0001092" ;
        skos:prefLabel   "Hemiacetals"@en .

csc:CHEMONTID_0002495
        a                skos:Concept ;
        skos:altLabel    "quinone"@en , "a quinone"@en , "quinones"@en ;
        skos:broader     csc:CHEMONTID_0003487 ;
        skos:definition  "Compounds having a fully conjugated cyclic dione structure, such as that of benzoquinones, derived from aromatic compounds by conversion of an even number of number of -CH= groups into -C(=O)- groups with any necessary rearrangement of double bonds (polycyclic and heterocyclic analogues are included)."@en ;
        skos:inScheme    vlcs:chemische_stof ;
        skos:notation    "CHEMONTID:0002495" ;
        skos:prefLabel   "Quinones"@en .

csc:CHEMONTID_0000039
        a                skos:Concept ;
        rdfs:seeAlso     tax_nodes:C0000039 ;
        skos:broader     csc:CHEMONTID_0000264 ;
        skos:definition  "Organic compounds containing a sulfamic acid moiety or a derivative, with the general structure R1N(R2)S(=O)2OR3  (R1,R2,R3=H, alkyl, aryl)."@en ;
        skos:inScheme    vlcs:chemische_stof ;
        skos:notation    "CHEMONTID:0000039" ;
        skos:prefLabel   "Sulfamic acid derivatives"@en .

csc:CHEMONTID_0004620
        a                skos:Concept ;
        skos:broader     csc:CHEMONTID_0002500 ;
        skos:definition  "Acyclic branched hydrocarbons having the general formula CnH2n+2."@en ;
        skos:inScheme    vlcs:chemische_stof ;
        skos:notation    "CHEMONTID:0004620" ;
        skos:prefLabel   "Branched alkanes"@en .

csc:CHEMONTID_0000583
        a                skos:Concept ;
        rdfs:seeAlso     tax_nodes:C0000583 ;
        skos:altLabel    "inorganic chloride"@en , "Inorganic Chemicals"@en , "Metalloids"@en ;
        skos:broader     csc:CHEMONTID_0000442 ;
        skos:definition  "Inorganic compounds in which the largest halogen atom is Chlorine, and the heaviest metal atom is a metalloid."@en ;
        skos:inScheme    vlcs:chemische_stof ;
        skos:notation    "CHEMONTID:0000583" ;
        skos:prefLabel   "Metalloid chlorides"@en .

csc:CHEMONTID_0001986
        a                skos:Concept ;
        rdfs:seeAlso     tax_nodes:C0001986 ;
        skos:altLabel    "carbonyl compound"@en ;
        skos:broader     csc:CHEMONTID_0000265 ;
        skos:definition  "Carboxylic acids containing exactly three carboxyl groups."@en ;
        skos:inScheme    vlcs:chemische_stof ;
        skos:notation    "CHEMONTID:0001986" ;
        skos:prefLabel   "Tricarboxylic acids and derivatives"@en .

csc:CHEMONTID_0000330
        a                skos:Concept ;
        rdfs:seeAlso     tax_nodes:C0000330 ;
        skos:altLabel    "benzimidazoles"@en ;
        skos:broader     csc:CHEMONTID_0000294 ;
        skos:definition  "Compounds containing a phenylbenzimidazole skeleton, which consists of a benzimidazole moiety where its imidazole ring is attached to a phenyl group."@en ;
        skos:inScheme    vlcs:chemische_stof ;
        skos:notation    "CHEMONTID:0000330" ;
        skos:prefLabel   "Phenylbenzimidazoles"@en .

csc:CHEMONTID_0000505
        a                skos:Concept ;
        rdfs:seeAlso     tax_nodes:C0000505 ;
        skos:altLabel    "Sulfones"@en , "sulfones"@en , "sulfone"@en ;
        skos:broader     csc:CHEMONTID_0001157 ;
        skos:definition  "Compounds containing a sulfonyl group( which as the general structure RS(=O)2R' (R,R' =alkyl, aryl)) attached to two carbon atoms."@en ;
        skos:inScheme    vlcs:chemische_stof ;
        skos:notation    "CHEMONTID:0000505" ;
        skos:prefLabel   "Sulfones"@en .

csc:CHEMONTID_0001908
        a                skos:Concept ;
        rdfs:seeAlso     tax_nodes:C0001908 ;
        skos:altLabel    "organonitrogen heterocyclic compound"@en , "organic heterotricyclic compound"@en ;
        skos:broader     csc:CHEMONTID_0001253 ;
        skos:definition  "Organic compounds containing a benzene fused to a quinoline ring system."@en ;
        skos:inScheme    vlcs:chemische_stof ;
        skos:notation    "CHEMONTID:0001908" ;
        skos:prefLabel   "Benzoquinolines"@en .

csc:CHEMONTID_0002463
        a                skos:Concept ;
        skos:altLabel    "aromatic ether"@en ;
        skos:broader     csc:CHEMONTID_0000254 ;
        skos:definition  "Organic compounds containing the dialkyl ether functional group, with the formula ROR', where R and R' are aryl groups."@en ;
        skos:inScheme    vlcs:chemische_stof ;
        skos:notation    "CHEMONTID:0002463" ;
        skos:prefLabel   "Diarylethers"@en .

csc:CHEMONTID_0002210
        a                skos:Concept ;
        skos:altLabel    "alditol"@en ;
        skos:broader     csc:CHEMONTID_0000011 ;
        skos:definition  "Hydrogenated forms of carbohydrate in which the carbonyl group (aldehyde or ketone, reducing sugar) has been reduced to a primary or secondary hydroxyl group."@en ;
        skos:inScheme    vlcs:chemische_stof ;
        skos:notation    "CHEMONTID:0002210" ;
        skos:prefLabel   "Sugar alcohols"@en .

csc:CHEMONTID_0000053
        a                skos:Concept ;
        rdfs:seeAlso     tax_nodes:C0000053 ;
        skos:altLabel    "Aminoquinolines"@en ;
        skos:broader     csc:CHEMONTID_0001253 ;
        skos:definition  "Organic compounds containing an amino group attached to a quinoline ring system."@en ;
        skos:inScheme    vlcs:chemische_stof ;
        skos:notation    "CHEMONTID:0000053" ;
        skos:prefLabel   "Aminoquinolines and derivatives"@en .
